<?xml version="1.0"?>
<rdf:RDF xmlns="http://purl.obolibrary.org/obo/cro.owl#"
     xml:base="http://purl.obolibrary.org/obo/cro.owl"
     xmlns:dc="http://purl.org/dc/elements/1.1/"
     xmlns:obo="http://purl.obolibrary.org/obo/"
     xmlns:owl="http://www.w3.org/2002/07/owl#"
     xmlns:rdf="http://www.w3.org/1999/02/22-rdf-syntax-ns#"
     xmlns:xml="http://www.w3.org/XML/1998/namespace"
     xmlns:xsd="http://www.w3.org/2001/XMLSchema#"
     xmlns:foaf="http://xmlns.com/foaf/0.1/"
     xmlns:rdfs="http://www.w3.org/2000/01/rdf-schema#"
     xmlns:oboInOwl="http://www.geneontology.org/formats/oboInOwl#">
    <owl:Ontology rdf:about="http://purl.obolibrary.org/obo/cro.owl">
        <owl:versionIRI rdf:resource="http://purl.obolibrary.org/obo/cro/releases/2019-12-11/cro.owl"/>
        <owl:imports rdf:resource="http://purl.obolibrary.org/obo/cro/imports/bfo_import.owl"/>
        <owl:imports rdf:resource="http://purl.obolibrary.org/obo/cro/imports/credit_import.owl"/>
        <owl:imports rdf:resource="http://purl.obolibrary.org/obo/cro/imports/iao_import.owl"/>
        <rdfs:comment>Contributor Role Ontology</rdfs:comment>
    </owl:Ontology>
    


    <!-- 
    ///////////////////////////////////////////////////////////////////////////////////////
    //
    // Annotation properties
    //
    ///////////////////////////////////////////////////////////////////////////////////////
     -->

    


    <!-- http://purl.obolibrary.org/obo/IAO_0000234 -->

    <owl:AnnotationProperty rdf:about="http://purl.obolibrary.org/obo/IAO_0000234">
        <rdfs:label>ontology term requester</rdfs:label>
    </owl:AnnotationProperty>
    


    <!-- http://purl.obolibrary.org/obo/IAO_0000412 -->

    <owl:AnnotationProperty rdf:about="http://purl.obolibrary.org/obo/IAO_0000412"/>
    


    <!-- http://purl.obolibrary.org/obo/IAO_0100001 -->

    <owl:AnnotationProperty rdf:about="http://purl.obolibrary.org/obo/IAO_0100001">
        <rdfs:label>term replaced by</rdfs:label>
    </owl:AnnotationProperty>
    


    <!-- http://purl.org/dc/elements/1.1/creator -->

    <owl:AnnotationProperty rdf:about="http://purl.org/dc/elements/1.1/creator"/>
    


    <!-- http://purl.org/dc/elements/1.1/date -->

    <owl:AnnotationProperty rdf:about="http://purl.org/dc/elements/1.1/date"/>
    


    <!-- http://www.geneontology.org/formats/oboInOwl#created_by -->

    <owl:AnnotationProperty rdf:about="http://www.geneontology.org/formats/oboInOwl#created_by"/>
    


    <!-- http://www.geneontology.org/formats/oboInOwl#hasSynonym -->

    <owl:AnnotationProperty rdf:about="http://www.geneontology.org/formats/oboInOwl#hasSynonym"/>
    


    <!-- 
    ///////////////////////////////////////////////////////////////////////////////////////
    //
    // Classes
    //
    ///////////////////////////////////////////////////////////////////////////////////////
     -->

    


    <!-- http://purl.obolibrary.org/obo/BFO_0000001 -->

    <rdf:Description rdf:about="http://purl.obolibrary.org/obo/BFO_0000001">
        <rdfs:subClassOf rdf:resource="http://www.w3.org/2002/07/owl#Thing"/>
    </rdf:Description>
    


    <!-- http://purl.obolibrary.org/obo/BFO_0000002 -->

    <rdf:Description rdf:about="http://purl.obolibrary.org/obo/BFO_0000002">
        <rdfs:subClassOf rdf:resource="http://purl.obolibrary.org/obo/BFO_0000001"/>
    </rdf:Description>
    


    <!-- http://purl.obolibrary.org/obo/BFO_0000020 -->

    <rdf:Description rdf:about="http://purl.obolibrary.org/obo/BFO_0000020">
        <rdfs:subClassOf rdf:resource="http://purl.obolibrary.org/obo/BFO_0000002"/>
    </rdf:Description>
    


    <!-- http://purl.obolibrary.org/obo/BFO_0000031 -->

    <rdf:Description rdf:about="http://purl.obolibrary.org/obo/BFO_0000031">
        <rdfs:subClassOf rdf:resource="http://purl.obolibrary.org/obo/BFO_0000002"/>
    </rdf:Description>
    


    <!-- http://purl.obolibrary.org/obo/CRO_0000000 -->

    <owl:Class rdf:about="http://purl.obolibrary.org/obo/CRO_0000000">
        <rdfs:subClassOf rdf:resource="http://www.w3.org/2002/07/owl#Thing"/>
        <obo:IAO_0000111>contributor role</obo:IAO_0000111>
        <obo:IAO_0000114>http://purl.obolibrary.org/obo/IAO_0000120</obo:IAO_0000114>
        <obo:IAO_0000115>A high-level classification of the diverse roles performed in the work leading to a published research output in the sciences. Its purpose to provide transparency in contributions to scholarly published work, to enable improved systems of attribution, credit, and accountability.</obo:IAO_0000115>
        <obo:IAO_0000117>https://orcid.org/0000-0001-5059-4132</obo:IAO_0000117>
        <obo:IAO_0000119>http://dictionary.casrai.org/Contributor_Roles</obo:IAO_0000119>
        <oboInOwl:hasDbXref>9dbb95f4-55ed-4e43-9301-a9f0e3e17afe</oboInOwl:hasDbXref>
        <oboInOwl:hasSynonym rdf:resource="http://purl.org/credit/ontology#CREDIT_00000000"/>
        <rdfs:label xml:lang="en">contributor role</rdfs:label>
    </owl:Class>
    


    <!-- http://purl.obolibrary.org/obo/CRO_0000001 -->

    <owl:Class rdf:about="http://purl.obolibrary.org/obo/CRO_0000001">
        <rdfs:subClassOf rdf:resource="http://purl.obolibrary.org/obo/CRO_0000000"/>
        <obo:IAO_0000115>Creation and/or presentation of a published research object, such as books, journal articles, and other publications like technical documentation, web sites, code, ontologies, or data models.</obo:IAO_0000115>
        <obo:IAO_0000118>writer role</obo:IAO_0000118>
        <dc:creator rdf:resource="http://orcid.org/0000-0001-5208-3432"/>
        <dc:date rdf:datatype="http://www.w3.org/2001/XMLSchema#dateTime">2018-09-14T19:47:01Z</dc:date>
        <rdfs:label>author role</rdfs:label>
    </owl:Class>
    <owl:Axiom>
        <owl:annotatedSource rdf:resource="http://purl.obolibrary.org/obo/CRO_0000001"/>
        <owl:annotatedProperty rdf:resource="http://purl.obolibrary.org/obo/IAO_0000115"/>
        <owl:annotatedTarget>Creation and/or presentation of a published research object, such as books, journal articles, and other publications like technical documentation, web sites, code, ontologies, or data models.</owl:annotatedTarget>
        <obo:IAO_0000119>https://orcid.org/0000-0002-1048-5019</obo:IAO_0000119>
    </owl:Axiom>
    


    <!-- http://purl.obolibrary.org/obo/CRO_0000003 -->

    <owl:Class rdf:about="http://purl.obolibrary.org/obo/CRO_0000003">
        <rdfs:subClassOf rdf:resource="http://purl.org/credit/ontology#CREDIT_00000012"/>
        <obo:IAO_0000115>Preparation, creation and/or presentation of figures for a manuscript, presentation or other use.</obo:IAO_0000115>
        <dc:creator rdf:resource="http://orcid.org/0000-0001-5208-3432"/>
        <dc:date rdf:datatype="http://www.w3.org/2001/XMLSchema#dateTime">2018-09-14T19:49:22Z</dc:date>
        <rdfs:label>figure development role</rdfs:label>
    </owl:Class>
    <owl:Axiom>
        <owl:annotatedSource rdf:resource="http://purl.obolibrary.org/obo/CRO_0000003"/>
        <owl:annotatedProperty rdf:resource="http://purl.obolibrary.org/obo/IAO_0000115"/>
        <owl:annotatedTarget>Preparation, creation and/or presentation of figures for a manuscript, presentation or other use.</owl:annotatedTarget>
        <obo:IAO_0000119>http://dictionary.casrai.org/Contributor_Roles/Visualization</obo:IAO_0000119>
    </owl:Axiom>
    


    <!-- http://purl.obolibrary.org/obo/CRO_0000004 -->

    <owl:Class rdf:about="http://purl.obolibrary.org/obo/CRO_0000004">
        <rdfs:subClassOf rdf:resource="http://purl.org/credit/ontology#CREDIT_00000008"/>
        <obo:IAO_0000115>Translating words or text from one language to another.</obo:IAO_0000115>
        <dc:creator rdf:resource="http://orcid.org/0000-0001-5208-3432"/>
        <dc:date rdf:datatype="http://www.w3.org/2001/XMLSchema#dateTime">2018-09-14T19:49:51Z</dc:date>
        <rdfs:label>translator role</rdfs:label>
    </owl:Class>
    


    <!-- http://purl.obolibrary.org/obo/CRO_0000006 -->

    <owl:Class rdf:about="http://purl.obolibrary.org/obo/CRO_0000006">
        <rdfs:subClassOf rdf:resource="http://purl.obolibrary.org/obo/CRO_0000111"/>
        <obo:IAO_0000115>Includes literature searches and contributions to review activities (systematic reviews, scoping reviews, etc.)</obo:IAO_0000115>
        <dc:creator rdf:resource="http://orcid.org/0000-0001-5208-3432"/>
        <dc:date rdf:datatype="http://www.w3.org/2001/XMLSchema#dateTime">2018-09-14T19:51:01Z</dc:date>
        <rdfs:label>background and literature search role</rdfs:label>
    </owl:Class>
    


    <!-- http://purl.obolibrary.org/obo/CRO_0000007 -->

    <owl:Class rdf:about="http://purl.obolibrary.org/obo/CRO_0000007">
        <rdfs:subClassOf rdf:resource="http://purl.obolibrary.org/obo/CRO_0000000"/>
        <obo:IAO_0000115>Coordination of research dissemination through popular media and the press, as well as community outreach and liaising of project directly to the community.</obo:IAO_0000115>
        <obo:IAO_0000116>Similar to vivo:OutreachProviderRole?</obo:IAO_0000116>
        <obo:IAO_0000118>communication role</obo:IAO_0000118>
        <obo:IAO_0000118>outreach role</obo:IAO_0000118>
        <dc:creator rdf:resource="http://orcid.org/0000-0001-5208-3432"/>
        <dc:date rdf:datatype="http://www.w3.org/2001/XMLSchema#dateTime">2018-09-14T19:51:26Z</dc:date>
        <rdfs:label>marketing and communication role</rdfs:label>
    </owl:Class>
    


    <!-- http://purl.obolibrary.org/obo/CRO_0000008 -->

    <owl:Class rdf:about="http://purl.obolibrary.org/obo/CRO_0000008">
        <rdfs:subClassOf rdf:resource="http://purl.obolibrary.org/obo/CRO_0000007"/>
        <obo:IAO_0000115>Creation or refinement of a website, a set of related web pages served from a single web domain.</obo:IAO_0000115>
        <obo:IAO_0000118>website development role</obo:IAO_0000118>
        <obo:IAO_0000118>website maintenance role</obo:IAO_0000118>
        <dc:creator rdf:resource="http://orcid.org/0000-0001-5208-3432"/>
        <dc:date rdf:datatype="http://www.w3.org/2001/XMLSchema#dateTime">2018-09-14T19:51:53Z</dc:date>
        <rdfs:label>website role</rdfs:label>
    </owl:Class>
    <owl:Axiom>
        <owl:annotatedSource rdf:resource="http://purl.obolibrary.org/obo/CRO_0000008"/>
        <owl:annotatedProperty rdf:resource="http://purl.obolibrary.org/obo/IAO_0000115"/>
        <owl:annotatedTarget>Creation or refinement of a website, a set of related web pages served from a single web domain.</owl:annotatedTarget>
        <obo:IAO_0000119>https://www.wikidata.org/wiki/Q35127</obo:IAO_0000119>
    </owl:Axiom>
    


    <!-- http://purl.obolibrary.org/obo/CRO_0000009 -->

    <owl:Class rdf:about="http://purl.obolibrary.org/obo/CRO_0000009">
        <rdfs:subClassOf rdf:resource="http://www.w3.org/2002/07/owl#Thing"/>
        <obo:IAO_0000115>A communication role that encompasses facilitate co-operation between people or organizations.</obo:IAO_0000115>
        <dc:creator rdf:resource="http://orcid.org/0000-0001-5208-3432"/>
        <dc:date rdf:datatype="http://www.w3.org/2001/XMLSchema#dateTime">2018-09-14T19:52:02Z</dc:date>
        <rdfs:label>obsolete networking facilitation role</rdfs:label>
        <owl:deprecated rdf:datatype="http://www.w3.org/2001/XMLSchema#boolean">true</owl:deprecated>
    </owl:Class>
    <owl:Axiom>
        <owl:annotatedSource rdf:resource="http://purl.obolibrary.org/obo/CRO_0000009"/>
        <owl:annotatedProperty rdf:resource="http://purl.obolibrary.org/obo/IAO_0000115"/>
        <owl:annotatedTarget>A communication role that encompasses facilitate co-operation between people or organizations.</owl:annotatedTarget>
        <obo:IAO_0000119>(2009) The functions and roles of network facilitators. In: Franz HW., Sarcina R. (eds) Building Leadership in Project and Network Management. Springer, Berlin, Heidelberg</obo:IAO_0000119>
    </owl:Axiom>
    


    <!-- http://purl.obolibrary.org/obo/CRO_0000010 -->

    <owl:Class rdf:about="http://purl.obolibrary.org/obo/CRO_0000010">
        <rdfs:subClassOf rdf:resource="http://www.w3.org/2002/07/owl#Thing"/>
        <obo:IAO_0000115>A communication role that involves the activity, set of institutions, and processes for creating, communicating, delivering, and exchanging offerings that have value for customers, clients, partners, and society at large.</obo:IAO_0000115>
        <dc:creator rdf:resource="http://orcid.org/0000-0001-5208-3432"/>
        <dc:date rdf:datatype="http://www.w3.org/2001/XMLSchema#dateTime">2018-09-14T19:52:12Z</dc:date>
        <rdfs:label>obsolete marketing role</rdfs:label>
        <owl:deprecated rdf:datatype="http://www.w3.org/2001/XMLSchema#boolean">true</owl:deprecated>
    </owl:Class>
    <owl:Axiom>
        <owl:annotatedSource rdf:resource="http://purl.obolibrary.org/obo/CRO_0000010"/>
        <owl:annotatedProperty rdf:resource="http://purl.obolibrary.org/obo/IAO_0000115"/>
        <owl:annotatedTarget>A communication role that involves the activity, set of institutions, and processes for creating, communicating, delivering, and exchanging offerings that have value for customers, clients, partners, and society at large.</owl:annotatedTarget>
        <obo:IAO_0000119>https://www.ama.org/the-definition-of-marketing/</obo:IAO_0000119>
    </owl:Axiom>
    


    <!-- http://purl.obolibrary.org/obo/CRO_0000011 -->

    <owl:Class rdf:about="http://purl.obolibrary.org/obo/CRO_0000011">
        <rdfs:subClassOf rdf:resource="http://purl.obolibrary.org/obo/CRO_0000007"/>
        <obo:IAO_0000115>A communication role in which one records the details of an event, a process, a workflow, etc.</obo:IAO_0000115>
        <dc:creator rdf:resource="http://orcid.org/0000-0001-5208-3432"/>
        <dc:date rdf:datatype="http://www.w3.org/2001/XMLSchema#dateTime">2018-09-14T19:52:17Z</dc:date>
        <rdfs:label>documentation role</rdfs:label>
    </owl:Class>
    <owl:Axiom>
        <owl:annotatedSource rdf:resource="http://purl.obolibrary.org/obo/CRO_0000011"/>
        <owl:annotatedProperty rdf:resource="http://purl.obolibrary.org/obo/IAO_0000115"/>
        <owl:annotatedTarget>A communication role in which one records the details of an event, a process, a workflow, etc.</owl:annotatedTarget>
        <obo:IAO_0000119>https://dictionary.cambridge.org/us/dictionary/english/document</obo:IAO_0000119>
    </owl:Axiom>
    


    <!-- http://purl.obolibrary.org/obo/CRO_0000012 -->

    <owl:Class rdf:about="http://purl.obolibrary.org/obo/CRO_0000012">
        <rdfs:subClassOf rdf:resource="http://purl.org/credit/ontology#CREDIT_00000012"/>
        <obo:IAO_0000115>A communication role that utilizes the art or profession of using design elements (such as typography and images) to convey information, create visualizations, or create an effect.</obo:IAO_0000115>
        <dc:creator rdf:resource="http://orcid.org/0000-0001-5208-3432"/>
        <dc:date rdf:datatype="http://www.w3.org/2001/XMLSchema#dateTime">2018-09-14T19:52:27Z</dc:date>
        <rdfs:label>graphic design role</rdfs:label>
    </owl:Class>
    <owl:Axiom>
        <owl:annotatedSource rdf:resource="http://purl.obolibrary.org/obo/CRO_0000012"/>
        <owl:annotatedProperty rdf:resource="http://purl.obolibrary.org/obo/IAO_0000115"/>
        <owl:annotatedTarget>A communication role that utilizes the art or profession of using design elements (such as typography and images) to convey information, create visualizations, or create an effect.</owl:annotatedTarget>
        <obo:IAO_0000119>https://www.merriam-webster.com/dictionary/graphic%20design</obo:IAO_0000119>
    </owl:Axiom>
    


    <!-- http://purl.obolibrary.org/obo/CRO_0000014 -->

    <owl:Class rdf:about="http://purl.obolibrary.org/obo/CRO_0000014">
        <rdfs:subClassOf rdf:resource="http://purl.obolibrary.org/obo/CRO_0000001"/>
        <obo:IAO_0000115>Creation of software documentation.</obo:IAO_0000115>
        <obo:IAO_0000118>software documentation role</obo:IAO_0000118>
        <dc:creator rdf:resource="http://orcid.org/0000-0001-5208-3432"/>
        <dc:date rdf:datatype="http://www.w3.org/2001/XMLSchema#dateTime">2018-09-14T20:26:05Z</dc:date>
        <rdfs:label>technical documentation role</rdfs:label>
    </owl:Class>
    


    <!-- http://purl.obolibrary.org/obo/CRO_0000015 -->

    <owl:Class rdf:about="http://purl.obolibrary.org/obo/CRO_0000015">
        <rdfs:subClassOf rdf:resource="http://purl.obolibrary.org/obo/CRO_0000000"/>
        <obo:IAO_0000115>A role that encompasses effective and efficient operation and usage of data, including, but not limited to management, handling, or manipulation.</obo:IAO_0000115>
        <dc:creator rdf:resource="http://orcid.org/0000-0001-5208-3432"/>
        <dc:date rdf:datatype="http://www.w3.org/2001/XMLSchema#dateTime">2018-09-14T19:55:34Z</dc:date>
        <rdfs:label>data role</rdfs:label>
    </owl:Class>
    


    <!-- http://purl.obolibrary.org/obo/CRO_0000016 -->

    <owl:Class rdf:about="http://purl.obolibrary.org/obo/CRO_0000016">
        <rdfs:subClassOf rdf:resource="http://purl.obolibrary.org/obo/CRO_0000000"/>
        <obo:IAO_0000115>A role in which a person participates in the transfer of knowledge and skills, through teaching, development of educational materials or curriculum, through program development or other means.</obo:IAO_0000115>
        <obo:IAO_0000118>educational role</obo:IAO_0000118>
        <dc:creator rdf:resource="http://orcid.org/0000-0001-5208-3432"/>
        <dc:date rdf:datatype="http://www.w3.org/2001/XMLSchema#dateTime">2018-09-14T19:55:45Z</dc:date>
        <rdfs:label>education and training role</rdfs:label>
    </owl:Class>
    


    <!-- http://purl.obolibrary.org/obo/CRO_0000018 -->

    <owl:Class rdf:about="http://purl.obolibrary.org/obo/CRO_0000018">
        <rdfs:subClassOf rdf:resource="http://www.w3.org/2002/07/owl#Thing"/>
        <obo:IAO_0000115>A role that involves the development, management, and use of computer-based information systems.</obo:IAO_0000115>
        <dc:creator rdf:resource="http://orcid.org/0000-0001-5208-3432"/>
        <dc:date rdf:datatype="http://www.w3.org/2001/XMLSchema#dateTime">2018-09-14T19:56:05Z</dc:date>
        <rdfs:label>obsolete information technology systems role</rdfs:label>
        <owl:deprecated rdf:datatype="http://www.w3.org/2001/XMLSchema#boolean">true</owl:deprecated>
    </owl:Class>
    <owl:Axiom>
        <owl:annotatedSource rdf:resource="http://purl.obolibrary.org/obo/CRO_0000018"/>
        <owl:annotatedProperty rdf:resource="http://purl.obolibrary.org/obo/IAO_0000115"/>
        <owl:annotatedTarget>A role that involves the development, management, and use of computer-based information systems.</owl:annotatedTarget>
        <obo:IAO_0000119>https://www.wikidata.org/wiki/Q11661</obo:IAO_0000119>
    </owl:Axiom>
    


    <!-- http://purl.obolibrary.org/obo/CRO_0000019 -->

    <owl:Class rdf:about="http://purl.obolibrary.org/obo/CRO_0000019">
        <rdfs:subClassOf rdf:resource="http://purl.org/credit/ontology#CREDIT_00000009"/>
        <obo:IAO_0000115>Verification that software meets requirements; validation that software meets users&apos; needs, identification of software bugs, assessment of software performance and usability.</obo:IAO_0000115>
        <obo:IAO_0000118>Software Quality Assurance Role</obo:IAO_0000118>
        <dc:creator rdf:resource="http://orcid.org/0000-0001-5208-3432"/>
        <dc:date rdf:datatype="http://www.w3.org/2001/XMLSchema#dateTime">2018-09-14T20:26:00Z</dc:date>
        <rdfs:label>software testing role</rdfs:label>
    </owl:Class>
    


    <!-- http://purl.obolibrary.org/obo/CRO_0000020 -->

    <owl:Class rdf:about="http://purl.obolibrary.org/obo/CRO_0000020">
        <rdfs:subClassOf rdf:resource="http://purl.obolibrary.org/obo/CRO_0000078"/>
        <obo:IAO_0000115>A role related to creations of the mind, such as inventions; literary and artistic works; designs; and symbols, names and images used in commerce. from.</obo:IAO_0000115>
        <dc:creator rdf:resource="http://orcid.org/0000-0001-5208-3432"/>
        <dc:date rdf:datatype="http://www.w3.org/2001/XMLSchema#dateTime">2018-09-14T19:56:34Z</dc:date>
        <rdfs:label>intellectual property role</rdfs:label>
    </owl:Class>
    <owl:Axiom>
        <owl:annotatedSource rdf:resource="http://purl.obolibrary.org/obo/CRO_0000020"/>
        <owl:annotatedProperty rdf:resource="http://purl.obolibrary.org/obo/IAO_0000115"/>
        <owl:annotatedTarget>A role related to creations of the mind, such as inventions; literary and artistic works; designs; and symbols, names and images used in commerce. from.</owl:annotatedTarget>
        <obo:IAO_0000119>https://www.wipo.int/about-ip/en/</obo:IAO_0000119>
    </owl:Axiom>
    


    <!-- http://purl.obolibrary.org/obo/CRO_0000022 -->

    <owl:Class rdf:about="http://purl.obolibrary.org/obo/CRO_0000022">
        <rdfs:subClassOf rdf:resource="http://purl.obolibrary.org/obo/CRO_0000000"/>
        <obo:IAO_0000115>Policy development generally involves research, analysis, consultation and synthesis of information to produce recommendations for action by an individual or an organization. It should also involve an evaluation of options against a set of criteria used to assess each option.</obo:IAO_0000115>
        <dc:creator rdf:resource="http://orcid.org/0000-0001-5208-3432"/>
        <dc:date rdf:datatype="http://www.w3.org/2001/XMLSchema#dateTime">2018-09-14T20:04:29Z</dc:date>
        <rdfs:label>policy development role</rdfs:label>
    </owl:Class>
    


    <!-- http://purl.obolibrary.org/obo/CRO_0000023 -->

    <owl:Class rdf:about="http://purl.obolibrary.org/obo/CRO_0000023">
        <rdfs:subClassOf rdf:resource="http://purl.obolibrary.org/obo/CRO_0000000"/>
        <obo:IAO_0000115>Set of activities aimed at prolonging the life of a record.</obo:IAO_0000115>
        <dc:creator rdf:resource="http://orcid.org/0000-0001-5208-3432"/>
        <dc:date rdf:datatype="http://www.w3.org/2001/XMLSchema#dateTime">2018-09-14T20:04:39Z</dc:date>
        <rdfs:label>preservation role</rdfs:label>
    </owl:Class>
    <owl:Axiom>
        <owl:annotatedSource rdf:resource="http://purl.obolibrary.org/obo/CRO_0000023"/>
        <owl:annotatedProperty rdf:resource="http://purl.obolibrary.org/obo/IAO_0000115"/>
        <owl:annotatedTarget>Set of activities aimed at prolonging the life of a record.</owl:annotatedTarget>
        <obo:IAO_0000119>https://www.wikidata.org/wiki/Q830393</obo:IAO_0000119>
    </owl:Axiom>
    


    <!-- http://purl.obolibrary.org/obo/CRO_0000025 -->

    <owl:Class rdf:about="http://purl.obolibrary.org/obo/CRO_0000025">
        <rdfs:subClassOf rdf:resource="http://purl.obolibrary.org/obo/CRO_0000078"/>
        <obo:IAO_0000115>Manage regulatory and compliance issues for the research project.</obo:IAO_0000115>
        <obo:IAO_0000118>regulatory administration role</obo:IAO_0000118>
        <dc:creator rdf:resource="http://orcid.org/0000-0001-5208-3432"/>
        <dc:date rdf:datatype="http://www.w3.org/2001/XMLSchema#dateTime">2018-09-14T20:05:56Z</dc:date>
        <rdfs:label>regulatory and compliance role</rdfs:label>
    </owl:Class>
    


    <!-- http://purl.obolibrary.org/obo/CRO_0000026 -->

    <owl:Class rdf:about="http://purl.obolibrary.org/obo/CRO_0000026">
        <rdfs:subClassOf rdf:resource="http://purl.obolibrary.org/obo/CRO_0000000"/>
        <obo:IAO_0000115>A person that is responsible for usage of instrumentation, such as equipment or devices, or instruments like a survey or questionnaire.</obo:IAO_0000115>
        <dc:creator rdf:resource="http://orcid.org/0000-0001-5208-3432"/>
        <dc:date rdf:datatype="http://www.w3.org/2001/XMLSchema#dateTime">2018-09-14T20:06:00Z</dc:date>
        <rdfs:label>instrumentation role</rdfs:label>
    </owl:Class>
    


    <!-- http://purl.obolibrary.org/obo/CRO_0000027 -->

    <owl:Class rdf:about="http://purl.obolibrary.org/obo/CRO_0000027">
        <rdfs:subClassOf rdf:resource="http://purl.obolibrary.org/obo/CRO_0000023"/>
        <obo:IAO_0000115>Management activities to annotate, maintain, research, and preserve physical objects to maximize their use for research and education now and into the future.</obo:IAO_0000115>
        <obo:IAO_0000234>https://orcid.org/0000-0002-2908-3327</obo:IAO_0000234>
        <dc:creator rdf:resource="http://orcid.org/0000-0001-5208-3432"/>
        <rdfs:label>curator role</rdfs:label>
    </owl:Class>
    


    <!-- http://purl.obolibrary.org/obo/CRO_0000028 -->

    <owl:Class rdf:about="http://purl.obolibrary.org/obo/CRO_0000028">
        <rdfs:subClassOf rdf:resource="http://purl.obolibrary.org/obo/CRO_0000000"/>
        <obo:IAO_0000115>Activities to obtain physical objects for research or scholarly purposes or to add to a collection.</obo:IAO_0000115>
        <obo:IAO_0000234>https://orcid.org/0000-0002-2908-3327</obo:IAO_0000234>
        <dc:creator rdf:resource="http://orcid.org/0000-0001-5208-3432"/>
        <rdfs:label>collection role</rdfs:label>
    </owl:Class>
    


    <!-- http://purl.obolibrary.org/obo/CRO_0000031 -->

    <owl:Class rdf:about="http://purl.obolibrary.org/obo/CRO_0000031">
        <rdfs:subClassOf rdf:resource="http://purl.obolibrary.org/obo/CRO_0000078"/>
        <obo:IAO_0000115>Coordination of diverse team members, often across different disciplines and locations.</obo:IAO_0000115>
        <dc:creator rdf:resource="http://orcid.org/0000-0001-5208-3432"/>
        <dc:date rdf:datatype="http://www.w3.org/2001/XMLSchema#dateTime">2018-09-14T20:06:26Z</dc:date>
        <rdfs:label>team management role</rdfs:label>
    </owl:Class>
    


    <!-- http://purl.obolibrary.org/obo/CRO_0000033 -->

    <owl:Class rdf:about="http://purl.obolibrary.org/obo/CRO_0000033">
        <rdfs:subClassOf rdf:resource="http://www.w3.org/2002/07/owl#Thing"/>
        <obo:IAO_0000115>The compiling of information with intent to prepare combined datasets for data processing.</obo:IAO_0000115>
        <obo:IAO_0100001 rdf:resource="http://purl.obolibrary.org/obo/CRO_0000036"/>
        <dc:creator rdf:resource="http://orcid.org/0000-0001-5208-3432"/>
        <dc:date rdf:datatype="http://www.w3.org/2001/XMLSchema#dateTime">2018-09-14T20:11:23Z</dc:date>
        <rdfs:label>obsolete data aggregation role</rdfs:label>
        <owl:deprecated rdf:datatype="http://www.w3.org/2001/XMLSchema#boolean">true</owl:deprecated>
    </owl:Class>
    <owl:Axiom>
        <owl:annotatedSource rdf:resource="http://purl.obolibrary.org/obo/CRO_0000033"/>
        <owl:annotatedProperty rdf:resource="http://purl.obolibrary.org/obo/IAO_0000115"/>
        <owl:annotatedTarget>The compiling of information with intent to prepare combined datasets for data processing.</owl:annotatedTarget>
        <obo:IAO_0000119>Stanley, Jay; Steinhardt, Barry (January 2003). &quot;Bigger Monster, Weaker Chains: The Growth of an American Surveillance Society&quot;. American Civil Liberties Union.</obo:IAO_0000119>
    </owl:Axiom>
    


    <!-- http://purl.obolibrary.org/obo/CRO_0000035 -->

    <owl:Class rdf:about="http://purl.obolibrary.org/obo/CRO_0000035">
        <rdfs:subClassOf rdf:resource="http://purl.org/credit/ontology#CREDIT_00000003"/>
        <obo:IAO_0000115>Statistical aspects of research, including data collection, organization, analysis, interpretation and presentation of data from surveys and experiments</obo:IAO_0000115>
        <obo:IAO_0000118>statistical data analysis role</obo:IAO_0000118>
        <dc:creator rdf:resource="http://orcid.org/0000-0001-5208-3432"/>
        <dc:date rdf:datatype="http://www.w3.org/2001/XMLSchema#dateTime">2018-09-14T20:11:35Z</dc:date>
        <rdfs:label>statistical analysis role</rdfs:label>
    </owl:Class>
    <owl:Axiom>
        <owl:annotatedSource rdf:resource="http://purl.obolibrary.org/obo/CRO_0000035"/>
        <owl:annotatedProperty rdf:resource="http://purl.obolibrary.org/obo/IAO_0000115"/>
        <owl:annotatedTarget>Statistical aspects of research, including data collection, organization, analysis, interpretation and presentation of data from surveys and experiments</owl:annotatedTarget>
        <obo:IAO_0000119>https://en.wikipedia.org/wiki/Statistics</obo:IAO_0000119>
    </owl:Axiom>
    


    <!-- http://purl.obolibrary.org/obo/CRO_0000036 -->

    <owl:Class rdf:about="http://purl.obolibrary.org/obo/CRO_0000036">
        <rdfs:subClassOf rdf:resource="http://purl.obolibrary.org/obo/CRO_0000015"/>
        <obo:IAO_0000115>The process of gathering and measuring data, information or any variables of interest in a standardized and established manner that enables the collector to answer or test hypothesis and evaluate outcomes of the particular collection.</obo:IAO_0000115>
        <obo:IAO_0000118>data aggregation role</obo:IAO_0000118>
        <dc:creator rdf:resource="http://orcid.org/0000-0001-5208-3432"/>
        <dc:date rdf:datatype="http://www.w3.org/2001/XMLSchema#dateTime">2018-09-14T20:11:40Z</dc:date>
        <rdfs:label>data collection role</rdfs:label>
    </owl:Class>
    <owl:Axiom>
        <owl:annotatedSource rdf:resource="http://purl.obolibrary.org/obo/CRO_0000036"/>
        <owl:annotatedProperty rdf:resource="http://purl.obolibrary.org/obo/IAO_0000115"/>
        <owl:annotatedTarget>The process of gathering and measuring data, information or any variables of interest in a standardized and established manner that enables the collector to answer or test hypothesis and evaluate outcomes of the particular collection.</owl:annotatedTarget>
        <obo:IAO_0000119>https://www.techopedia.com/definition/30318/data-collection</obo:IAO_0000119>
    </owl:Axiom>
    


    <!-- http://purl.obolibrary.org/obo/CRO_0000038 -->

    <owl:Class rdf:about="http://purl.obolibrary.org/obo/CRO_0000038">
        <rdfs:subClassOf rdf:resource="http://purl.obolibrary.org/obo/CRO_0000015"/>
        <obo:IAO_0000115>The annotation of data with descriptive information that describes the data (metadata), with the goal of making the data more usuable or reusable for future use.</obo:IAO_0000115>
        <obo:IAO_0000118>metadata application role</obo:IAO_0000118>
        <dc:creator rdf:resource="http://orcid.org/0000-0001-5208-3432"/>
        <dc:date rdf:datatype="http://www.w3.org/2001/XMLSchema#dateTime">2018-09-14T20:11:50Z</dc:date>
        <rdfs:label>metadata role</rdfs:label>
    </owl:Class>
    <owl:Axiom>
        <owl:annotatedSource rdf:resource="http://purl.obolibrary.org/obo/CRO_0000038"/>
        <owl:annotatedProperty rdf:resource="http://purl.obolibrary.org/obo/IAO_0000115"/>
        <owl:annotatedTarget>The annotation of data with descriptive information that describes the data (metadata), with the goal of making the data more usuable or reusable for future use.</owl:annotatedTarget>
        <obo:IAO_0000119>https://whatis.techtarget.com/definition/metadata-management</obo:IAO_0000119>
    </owl:Axiom>
    


    <!-- http://purl.obolibrary.org/obo/CRO_0000039 -->

    <owl:Class rdf:about="http://purl.obolibrary.org/obo/CRO_0000039">
        <rdfs:subClassOf rdf:resource="http://purl.obolibrary.org/obo/CRO_0000015"/>
        <obo:IAO_0000115>The process of inputting data into a computerized form.</obo:IAO_0000115>
        <dc:creator rdf:resource="http://orcid.org/0000-0001-5208-3432"/>
        <dc:date rdf:datatype="http://www.w3.org/2001/XMLSchema#dateTime">2018-09-14T20:11:54Z</dc:date>
        <rdfs:label>data entry role</rdfs:label>
    </owl:Class>
    <owl:Axiom>
        <owl:annotatedSource rdf:resource="http://purl.obolibrary.org/obo/CRO_0000039"/>
        <owl:annotatedProperty rdf:resource="http://purl.obolibrary.org/obo/IAO_0000115"/>
        <owl:annotatedTarget>The process of inputting data into a computerized form.</owl:annotatedTarget>
        <obo:IAO_0000119>https://www.dictionary.com/browse/data-entry</obo:IAO_0000119>
    </owl:Axiom>
    


    <!-- http://purl.obolibrary.org/obo/CRO_0000040 -->

    <owl:Class rdf:about="http://purl.obolibrary.org/obo/CRO_0000040">
        <rdfs:subClassOf rdf:resource="http://purl.obolibrary.org/obo/CRO_0000015"/>
        <obo:IAO_0000115>The process of combining data from different sources to provide a standardized or unified view.</obo:IAO_0000115>
        <dc:creator rdf:resource="http://orcid.org/0000-0001-5208-3432"/>
        <dc:date rdf:datatype="http://www.w3.org/2001/XMLSchema#dateTime">2018-09-14T20:12:00Z</dc:date>
        <rdfs:label>data integration role</rdfs:label>
    </owl:Class>
    <owl:Axiom>
        <owl:annotatedSource rdf:resource="http://purl.obolibrary.org/obo/CRO_0000040"/>
        <owl:annotatedProperty rdf:resource="http://purl.obolibrary.org/obo/IAO_0000115"/>
        <owl:annotatedTarget>The process of combining data from different sources to provide a standardized or unified view.</owl:annotatedTarget>
        <obo:IAO_0000119>https://www.wikidata.org/wiki/Q386824</obo:IAO_0000119>
    </owl:Axiom>
    


    <!-- http://purl.obolibrary.org/obo/CRO_0000041 -->

    <owl:Class rdf:about="http://purl.obolibrary.org/obo/CRO_0000041">
        <rdfs:subClassOf rdf:resource="http://purl.obolibrary.org/obo/CRO_0000015"/>
        <obo:IAO_0000115>The process of creating a data model for an information system by applying certain formal techniques.</obo:IAO_0000115>
        <dc:creator rdf:resource="http://orcid.org/0000-0001-5208-3432"/>
        <dc:date rdf:datatype="http://www.w3.org/2001/XMLSchema#dateTime">2018-09-14T20:12:07Z</dc:date>
        <rdfs:label>data modeling role</rdfs:label>
    </owl:Class>
    <owl:Axiom>
        <owl:annotatedSource rdf:resource="http://purl.obolibrary.org/obo/CRO_0000041"/>
        <owl:annotatedProperty rdf:resource="http://purl.obolibrary.org/obo/IAO_0000115"/>
        <owl:annotatedTarget>The process of creating a data model for an information system by applying certain formal techniques.</owl:annotatedTarget>
        <obo:IAO_0000119>https://www.wikidata.org/wiki/Q367664</obo:IAO_0000119>
    </owl:Axiom>
    


    <!-- http://purl.obolibrary.org/obo/CRO_0000042 -->

    <owl:Class rdf:about="http://purl.obolibrary.org/obo/CRO_0000042">
        <rdfs:subClassOf rdf:resource="http://purl.obolibrary.org/obo/CRO_0000015"/>
        <obo:IAO_0000115>A procedure intended to verify the efficiency and reliability of data.</obo:IAO_0000115>
        <obo:IAO_0000118>Data Scrubbing Role</obo:IAO_0000118>
        <dc:creator rdf:resource="http://orcid.org/0000-0001-5208-3432"/>
        <dc:date rdf:datatype="http://www.w3.org/2001/XMLSchema#dateTime">2018-09-14T20:12:14Z</dc:date>
        <rdfs:label>data quality assurance role</rdfs:label>
    </owl:Class>
    <owl:Axiom>
        <owl:annotatedSource rdf:resource="http://purl.obolibrary.org/obo/CRO_0000042"/>
        <owl:annotatedProperty rdf:resource="http://purl.obolibrary.org/obo/IAO_0000115"/>
        <owl:annotatedTarget>A procedure intended to verify the efficiency and reliability of data.</owl:annotatedTarget>
        <obo:IAO_0000119>https://www.techopedia.com/definition/14653/data-quality</obo:IAO_0000119>
    </owl:Axiom>
    


    <!-- http://purl.obolibrary.org/obo/CRO_0000043 -->

    <owl:Class rdf:about="http://purl.obolibrary.org/obo/CRO_0000043">
        <rdfs:subClassOf rdf:resource="http://www.w3.org/2002/07/owl#Thing"/>
        <obo:IAO_0000115>The process of creating data standards, which are the rules by which data are described and recorded in order to share, exchange, and understand data. Examples include development of an ontology, terminology, code lists, etc.</obo:IAO_0000115>
        <dc:creator rdf:resource="http://orcid.org/0000-0001-5208-3432"/>
        <dc:date rdf:datatype="http://www.w3.org/2001/XMLSchema#dateTime">2018-09-14T20:12:25Z</dc:date>
        <rdfs:label>obsolete data standards developer role</rdfs:label>
        <owl:deprecated rdf:datatype="http://www.w3.org/2001/XMLSchema#boolean">true</owl:deprecated>
    </owl:Class>
    <owl:Axiom>
        <owl:annotatedSource rdf:resource="http://purl.obolibrary.org/obo/CRO_0000043"/>
        <owl:annotatedProperty rdf:resource="http://purl.obolibrary.org/obo/IAO_0000115"/>
        <owl:annotatedTarget>The process of creating data standards, which are the rules by which data are described and recorded in order to share, exchange, and understand data. Examples include development of an ontology, terminology, code lists, etc.</owl:annotatedTarget>
        <obo:IAO_0000119>https://www.usgs.gov/products/data-and-tools/data-management/data-standards</obo:IAO_0000119>
    </owl:Axiom>
    


    <!-- http://purl.obolibrary.org/obo/CRO_0000045 -->

    <owl:Class rdf:about="http://purl.obolibrary.org/obo/CRO_0000045">
        <rdfs:subClassOf rdf:resource="http://purl.obolibrary.org/obo/CRO_0000016"/>
        <obo:IAO_0000115>An educational role in which a person develops educational or training materials that are intended to transfer knowledge, for use in a classroom, indpendent learning or other settings.</obo:IAO_0000115>
        <obo:IAO_0000118>educational material development role</obo:IAO_0000118>
        <dc:creator rdf:resource="http://orcid.org/0000-0001-5208-3432"/>
        <dc:date rdf:datatype="http://www.w3.org/2001/XMLSchema#dateTime">2018-09-14T20:15:18Z</dc:date>
        <rdfs:label>training material role</rdfs:label>
    </owl:Class>
    


    <!-- http://purl.obolibrary.org/obo/CRO_0000046 -->

    <owl:Class rdf:about="http://purl.obolibrary.org/obo/CRO_0000046">
        <rdfs:subClassOf rdf:resource="http://purl.obolibrary.org/obo/CRO_0000016"/>
        <obo:IAO_0000115>An educational role in which a person participates in the development of an educational program, designed for learners to achieve a set of compentencies around a given topic or area of focus.</obo:IAO_0000115>
        <obo:IAO_0000118>educational program development role</obo:IAO_0000118>
        <dc:creator rdf:resource="http://orcid.org/0000-0001-5208-3432"/>
        <dc:date rdf:datatype="http://www.w3.org/2001/XMLSchema#dateTime">2018-09-14T20:15:23Z</dc:date>
        <rdfs:label>training program development role</rdfs:label>
    </owl:Class>
    


    <!-- http://purl.obolibrary.org/obo/CRO_0000047 -->

    <owl:Class rdf:about="http://purl.obolibrary.org/obo/CRO_0000047">
        <rdfs:subClassOf rdf:resource="http://purl.obolibrary.org/obo/CRO_0000016"/>
        <obo:IAO_0000115>An educational role in which knowledge and skills are transferred through teaching.</obo:IAO_0000115>
        <obo:IAO_0000116>This may be equivalent to vivo:Teacher Role.</obo:IAO_0000116>
        <obo:IAO_0000118>educational instruction role</obo:IAO_0000118>
        <obo:IAO_0000118>educational training role</obo:IAO_0000118>
        <obo:IAO_0000118>teaching role</obo:IAO_0000118>
        <dc:creator rdf:resource="http://orcid.org/0000-0001-5208-3432"/>
        <dc:date rdf:datatype="http://www.w3.org/2001/XMLSchema#dateTime">2018-09-14T20:15:29Z</dc:date>
        <rdfs:label>instruction role</rdfs:label>
    </owl:Class>
    <owl:Axiom>
        <owl:annotatedSource rdf:resource="http://purl.obolibrary.org/obo/CRO_0000047"/>
        <owl:annotatedProperty rdf:resource="http://purl.obolibrary.org/obo/IAO_0000115"/>
        <owl:annotatedTarget>An educational role in which knowledge and skills are transferred through teaching.</owl:annotatedTarget>
        <obo:IAO_0000119>https://www.wikidata.org/wiki/Q8434</obo:IAO_0000119>
    </owl:Axiom>
    


    <!-- http://purl.obolibrary.org/obo/CRO_0000048 -->

    <owl:Class rdf:about="http://purl.obolibrary.org/obo/CRO_0000048">
        <rdfs:subClassOf rdf:resource="http://purl.obolibrary.org/obo/CRO_0000000"/>
        <obo:IAO_0000115>An information technology systems role that specifically focuses on the computer hardware, the physical components of a computer system.</obo:IAO_0000115>
        <obo:IAO_0000118>hardware systems role</obo:IAO_0000118>
        <dc:creator rdf:resource="http://orcid.org/0000-0001-5208-3432"/>
        <dc:date rdf:datatype="http://www.w3.org/2001/XMLSchema#dateTime">2018-09-14T20:17:16Z</dc:date>
        <rdfs:label>hardware role</rdfs:label>
    </owl:Class>
    <owl:Axiom>
        <owl:annotatedSource rdf:resource="http://purl.obolibrary.org/obo/CRO_0000048"/>
        <owl:annotatedProperty rdf:resource="http://purl.obolibrary.org/obo/IAO_0000115"/>
        <owl:annotatedTarget>An information technology systems role that specifically focuses on the computer hardware, the physical components of a computer system.</owl:annotatedTarget>
        <obo:IAO_0000119>https://www.wikidata.org/wiki/Q3966</obo:IAO_0000119>
    </owl:Axiom>
    


    <!-- http://purl.obolibrary.org/obo/CRO_0000049 -->

    <owl:Class rdf:about="http://purl.obolibrary.org/obo/CRO_0000049">
        <rdfs:subClassOf rdf:resource="http://www.w3.org/2002/07/owl#Thing"/>
        <obo:IAO_0000115>An information technology systems role that specifically focuses on the computer software, the non-tangible executable component of a computer.</obo:IAO_0000115>
        <obo:IAO_0100001 rdf:resource="http://purl.org/credit/ontology#CREDIT_00000009"/>
        <dc:creator rdf:resource="http://orcid.org/0000-0001-5208-3432"/>
        <dc:date rdf:datatype="http://www.w3.org/2001/XMLSchema#dateTime">2018-09-14T20:17:20Z</dc:date>
        <rdfs:label>obsolete software systems role</rdfs:label>
        <owl:deprecated rdf:datatype="http://www.w3.org/2001/XMLSchema#boolean">true</owl:deprecated>
    </owl:Class>
    <owl:Axiom>
        <owl:annotatedSource rdf:resource="http://purl.obolibrary.org/obo/CRO_0000049"/>
        <owl:annotatedProperty rdf:resource="http://purl.obolibrary.org/obo/IAO_0000115"/>
        <owl:annotatedTarget>An information technology systems role that specifically focuses on the computer software, the non-tangible executable component of a computer.</owl:annotatedTarget>
        <obo:IAO_0000119>https://www.wikidata.org/wiki/Q7397</obo:IAO_0000119>
    </owl:Axiom>
    


    <!-- http://purl.obolibrary.org/obo/CRO_0000050 -->

    <owl:Class rdf:about="http://purl.obolibrary.org/obo/CRO_0000050">
        <rdfs:subClassOf rdf:resource="http://purl.obolibrary.org/obo/CRO_0000108"/>
        <obo:IAO_0000115>A role usually within the Information Technology department, charged with the creation, maintenance, backups, querying, tuning, user rights assignment and security of an organization&apos;s databases.</obo:IAO_0000115>
        <obo:IAO_0000118>database administration role</obo:IAO_0000118>
        <dc:creator rdf:resource="http://orcid.org/0000-0001-5208-3432"/>
        <dc:date rdf:datatype="http://www.w3.org/2001/XMLSchema#dateTime">2018-09-14T20:17:25Z</dc:date>
        <rdfs:label>database administrator role</rdfs:label>
    </owl:Class>
    <owl:Axiom>
        <owl:annotatedSource rdf:resource="http://purl.obolibrary.org/obo/CRO_0000050"/>
        <owl:annotatedProperty rdf:resource="http://purl.obolibrary.org/obo/IAO_0000115"/>
        <owl:annotatedTarget>A role usually within the Information Technology department, charged with the creation, maintenance, backups, querying, tuning, user rights assignment and security of an organization&apos;s databases.</owl:annotatedTarget>
        <obo:IAO_0000119>https://www.techopedia.com/definition/1187/database-administrator-dba</obo:IAO_0000119>
    </owl:Axiom>
    


    <!-- http://purl.obolibrary.org/obo/CRO_0000051 -->

    <owl:Class rdf:about="http://purl.obolibrary.org/obo/CRO_0000051">
        <rdfs:subClassOf rdf:resource="http://purl.org/credit/ontology#CREDIT_00000009"/>
        <obo:IAO_0000115>A software systems role that involves maintenance and operation of a computer system and/or network.</obo:IAO_0000115>
        <obo:IAO_0000118>sysadmin role</obo:IAO_0000118>
        <obo:IAO_0000118>systems administration role</obo:IAO_0000118>
        <dc:creator rdf:resource="http://orcid.org/0000-0001-5208-3432"/>
        <dc:date rdf:datatype="http://www.w3.org/2001/XMLSchema#dateTime">2018-09-14T20:17:32Z</dc:date>
        <rdfs:label>system administrator role</rdfs:label>
    </owl:Class>
    <owl:Axiom>
        <owl:annotatedSource rdf:resource="http://purl.obolibrary.org/obo/CRO_0000051"/>
        <owl:annotatedProperty rdf:resource="http://purl.obolibrary.org/obo/IAO_0000115"/>
        <owl:annotatedTarget>A software systems role that involves maintenance and operation of a computer system and/or network.</owl:annotatedTarget>
        <obo:IAO_0000119>https://www.wikidata.org/wiki/Q327353</obo:IAO_0000119>
    </owl:Axiom>
    


    <!-- http://purl.obolibrary.org/obo/CRO_0000052 -->

    <owl:Class rdf:about="http://purl.obolibrary.org/obo/CRO_0000052">
        <rdfs:subClassOf rdf:resource="http://purl.org/credit/ontology#CREDIT_00000006"/>
        <obo:IAO_0000115>A methodology role that involves development of information that suggests how something should be done.</obo:IAO_0000115>
        <obo:IAO_0000118>Best Practices Role</obo:IAO_0000118>
        <obo:IAO_0000118>guideline development role</obo:IAO_0000118>
        <obo:IAO_0000118>standard operating procedure development role</obo:IAO_0000118>
        <dc:creator rdf:resource="http://orcid.org/0000-0001-5208-3432"/>
        <dc:date rdf:datatype="http://www.w3.org/2001/XMLSchema#dateTime">2018-09-14T20:19:52Z</dc:date>
        <rdfs:label>standards role</rdfs:label>
    </owl:Class>
    <owl:Axiom>
        <owl:annotatedSource rdf:resource="http://purl.obolibrary.org/obo/CRO_0000052"/>
        <owl:annotatedProperty rdf:resource="http://purl.obolibrary.org/obo/IAO_0000115"/>
        <owl:annotatedTarget>A methodology role that involves development of information that suggests how something should be done.</owl:annotatedTarget>
        <obo:IAO_0000119>https://dictionary.cambridge.org/us/dictionary/english/guideline</obo:IAO_0000119>
    </owl:Axiom>
    


    <!-- http://purl.obolibrary.org/obo/CRO_0000053 -->

    <owl:Class rdf:about="http://purl.obolibrary.org/obo/CRO_0000053">
        <rdfs:subClassOf rdf:resource="http://purl.org/credit/ontology#CREDIT_00000006"/>
        <obo:IAO_0000115>A methodology role that involves creation of a detailed plan of a scientific or medical experiment, treatment, or procedure.</obo:IAO_0000115>
        <obo:IAO_0000118>protocol development role</obo:IAO_0000118>
        <dc:creator rdf:resource="http://orcid.org/0000-0001-5208-3432"/>
        <dc:date rdf:datatype="http://www.w3.org/2001/XMLSchema#dateTime">2018-09-14T20:19:56Z</dc:date>
        <rdfs:label>protocol creation role</rdfs:label>
    </owl:Class>
    <owl:Axiom>
        <owl:annotatedSource rdf:resource="http://purl.obolibrary.org/obo/CRO_0000053"/>
        <owl:annotatedProperty rdf:resource="http://purl.obolibrary.org/obo/IAO_0000115"/>
        <owl:annotatedTarget>A methodology role that involves creation of a detailed plan of a scientific or medical experiment, treatment, or procedure.</owl:annotatedTarget>
        <obo:IAO_0000119>https://www.merriam-webster.com/dictionary/protocol</obo:IAO_0000119>
    </owl:Axiom>
    


    <!-- http://purl.obolibrary.org/obo/CRO_0000054 -->

    <owl:Class rdf:about="http://purl.obolibrary.org/obo/CRO_0000054">
        <rdfs:subClassOf rdf:resource="http://www.w3.org/2002/07/owl#Thing"/>
        <obo:IAO_0000115>A methodology role that involves the development or creation of an established or prescribed methods to be followed routinely for the performance of designated operations or in designated situations.</obo:IAO_0000115>
        <obo:IAO_0100001 rdf:resource="http://purl.obolibrary.org/obo/CRO_0000052"/>
        <dc:creator rdf:resource="http://orcid.org/0000-0001-5208-3432"/>
        <dc:date rdf:datatype="http://www.w3.org/2001/XMLSchema#dateTime">2018-09-14T20:20:02Z</dc:date>
        <rdfs:label>obsolete standard operating procedure development role</rdfs:label>
        <owl:deprecated rdf:datatype="http://www.w3.org/2001/XMLSchema#boolean">true</owl:deprecated>
    </owl:Class>
    <owl:Axiom>
        <owl:annotatedSource rdf:resource="http://purl.obolibrary.org/obo/CRO_0000054"/>
        <owl:annotatedProperty rdf:resource="http://purl.obolibrary.org/obo/IAO_0000115"/>
        <owl:annotatedTarget>A methodology role that involves the development or creation of an established or prescribed methods to be followed routinely for the performance of designated operations or in designated situations.</owl:annotatedTarget>
        <obo:IAO_0000119>https://www.merriam-webster.com/dictionary/standard%20operating%20procedure</obo:IAO_0000119>
    </owl:Axiom>
    


    <!-- http://purl.obolibrary.org/obo/CRO_0000055 -->

    <owl:Class rdf:about="http://purl.obolibrary.org/obo/CRO_0000055">
        <rdfs:subClassOf rdf:resource="http://purl.org/credit/ontology#CREDIT_00000006"/>
        <obo:IAO_0000115>Detailed design of study components including data collection, analysis, and dissemination.</obo:IAO_0000115>
        <dc:creator rdf:resource="http://orcid.org/0000-0001-5208-3432"/>
        <dc:date rdf:datatype="http://www.w3.org/2001/XMLSchema#dateTime">2018-09-14T20:20:06Z</dc:date>
        <rdfs:label>study design role</rdfs:label>
    </owl:Class>
    


    <!-- http://purl.obolibrary.org/obo/CRO_0000056 -->

    <owl:Class rdf:about="http://purl.obolibrary.org/obo/CRO_0000056">
        <rdfs:subClassOf rdf:resource="http://purl.org/credit/ontology#CREDIT_00000006"/>
        <obo:IAO_0000115>A methodology role that involves the creation or refinement of a manner or method by which an activity is performed.</obo:IAO_0000115>
        <dc:creator rdf:resource="http://orcid.org/0000-0001-5208-3432"/>
        <dc:date rdf:datatype="http://www.w3.org/2001/XMLSchema#dateTime">2018-09-14T20:20:11Z</dc:date>
        <rdfs:label>technique development role</rdfs:label>
    </owl:Class>
    <owl:Axiom>
        <owl:annotatedSource rdf:resource="http://purl.obolibrary.org/obo/CRO_0000056"/>
        <owl:annotatedProperty rdf:resource="http://purl.obolibrary.org/obo/IAO_0000115"/>
        <owl:annotatedTarget>A methodology role that involves the creation or refinement of a manner or method by which an activity is performed.</owl:annotatedTarget>
        <obo:IAO_0000119>https://www.wikidata.org/wiki/Q2695280</obo:IAO_0000119>
    </owl:Axiom>
    


    <!-- http://purl.obolibrary.org/obo/CRO_0000057 -->

    <owl:Class rdf:about="http://purl.obolibrary.org/obo/CRO_0000057">
        <rdfs:subClassOf rdf:resource="http://purl.obolibrary.org/obo/CRO_0000026"/>
        <obo:IAO_0000115>A role charged with conceptualization, design, development and marketing of complex equipment.</obo:IAO_0000115>
        <obo:IAO_0000118>instrument development role</obo:IAO_0000118>
        <dc:creator rdf:resource="http://orcid.org/0000-0001-5208-3432"/>
        <dc:date rdf:datatype="http://www.w3.org/2001/XMLSchema#dateTime">2018-09-14T20:23:39Z</dc:date>
        <rdfs:label>device development role</rdfs:label>
    </owl:Class>
    <owl:Axiom>
        <owl:annotatedSource rdf:resource="http://purl.obolibrary.org/obo/CRO_0000057"/>
        <owl:annotatedProperty rdf:resource="http://purl.obolibrary.org/obo/IAO_0000115"/>
        <owl:annotatedTarget>A role charged with conceptualization, design, development and marketing of complex equipment.</owl:annotatedTarget>
        <obo:IAO_0000119>https://searchcio.techtarget.com/definition/product-development-or-new-product-development-NPD</obo:IAO_0000119>
    </owl:Axiom>
    


    <!-- http://purl.obolibrary.org/obo/CRO_0000058 -->

    <owl:Class rdf:about="http://purl.obolibrary.org/obo/CRO_0000058">
        <rdfs:subClassOf rdf:resource="http://purl.obolibrary.org/obo/CRO_0000026"/>
        <obo:IAO_0000115>A person that is responsible for operating equipment or instrumentation and/or that ensures equipment is well-maintained, properly configured, and safely functional.</obo:IAO_0000115>
        <obo:IAO_0000118>instrument technician role</obo:IAO_0000118>
        <dc:creator rdf:resource="http://orcid.org/0000-0001-5208-3432"/>
        <dc:date rdf:datatype="http://www.w3.org/2001/XMLSchema#dateTime">2018-09-14T20:23:44Z</dc:date>
        <rdfs:label>equipment technician role</rdfs:label>
    </owl:Class>
    <owl:Axiom>
        <owl:annotatedSource rdf:resource="http://purl.obolibrary.org/obo/CRO_0000058"/>
        <owl:annotatedProperty rdf:resource="http://purl.obolibrary.org/obo/IAO_0000115"/>
        <owl:annotatedTarget>A person that is responsible for operating equipment or instrumentation and/or that ensures equipment is well-maintained, properly configured, and safely functional.</owl:annotatedTarget>
        <obo:IAO_0000119>https://en.wikipedia.org/wiki/Biomedical_equipment_technician</obo:IAO_0000119>
    </owl:Axiom>
    


    <!-- http://purl.obolibrary.org/obo/CRO_0000059 -->

    <owl:Class rdf:about="http://purl.obolibrary.org/obo/CRO_0000059">
        <rdfs:subClassOf rdf:resource="http://purl.obolibrary.org/obo/CRO_0000106"/>
        <obo:IAO_0000115>Creation or refinement of a survey or questionnaire, a list of questions aimed at extracting specific data from a particular group of people.</obo:IAO_0000115>
        <dc:creator rdf:resource="http://orcid.org/0000-0001-5208-3432"/>
        <dc:date rdf:datatype="http://www.w3.org/2001/XMLSchema#dateTime">2018-09-14T20:23:49Z</dc:date>
        <rdfs:label>survey and questionnaire development role</rdfs:label>
    </owl:Class>
    <owl:Axiom>
        <owl:annotatedSource rdf:resource="http://purl.obolibrary.org/obo/CRO_0000059"/>
        <owl:annotatedProperty rdf:resource="http://purl.obolibrary.org/obo/IAO_0000115"/>
        <owl:annotatedTarget>Creation or refinement of a survey or questionnaire, a list of questions aimed at extracting specific data from a particular group of people.</owl:annotatedTarget>
        <obo:IAO_0000119>https://www.wikidata.org/wiki/Q7257997</obo:IAO_0000119>
    </owl:Axiom>
    


    <!-- http://purl.obolibrary.org/obo/CRO_0000060 -->

    <owl:Class rdf:about="http://purl.obolibrary.org/obo/CRO_0000060">
        <rdfs:subClassOf rdf:resource="http://purl.obolibrary.org/obo/CRO_0000101"/>
        <rdfs:subClassOf rdf:resource="http://purl.org/credit/ontology#CREDIT_00000009"/>
        <obo:IAO_0000115>Examination of software code to identify build-breaking changes prior to acceptance into a codebase.</obo:IAO_0000115>
        <obo:IAO_0000118>software code review role</obo:IAO_0000118>
        <dc:creator rdf:resource="http://orcid.org/0000-0001-5208-3432"/>
        <dc:date rdf:datatype="http://www.w3.org/2001/XMLSchema#dateTime">2018-09-14T20:25:30Z</dc:date>
        <rdfs:label>code review role</rdfs:label>
    </owl:Class>
    


    <!-- http://purl.obolibrary.org/obo/CRO_0000061 -->

    <owl:Class rdf:about="http://purl.obolibrary.org/obo/CRO_0000061">
        <rdfs:subClassOf rdf:resource="http://www.w3.org/2002/07/owl#Thing"/>
        <obo:IAO_0000115>Algorithm development and implementation of software in a computer programming language.</obo:IAO_0000115>
        <obo:IAO_0100001 rdf:resource="http://purl.obolibrary.org/obo/CRO_0000064"/>
        <dc:creator rdf:resource="http://orcid.org/0000-0001-5208-3432"/>
        <dc:date rdf:datatype="http://www.w3.org/2001/XMLSchema#dateTime">2018-09-14T20:25:35Z</dc:date>
        <rdfs:label>obsolete computer programming role</rdfs:label>
        <owl:deprecated rdf:datatype="http://www.w3.org/2001/XMLSchema#boolean">true</owl:deprecated>
    </owl:Class>
    


    <!-- http://purl.obolibrary.org/obo/CRO_0000062 -->

    <owl:Class rdf:about="http://purl.obolibrary.org/obo/CRO_0000062">
        <rdfs:subClassOf rdf:resource="http://purl.org/credit/ontology#CREDIT_00000009"/>
        <obo:IAO_0000115>Creation of high-level structures of a software system.</obo:IAO_0000115>
        <dc:creator rdf:resource="http://orcid.org/0000-0001-5208-3432"/>
        <dc:date rdf:datatype="http://www.w3.org/2001/XMLSchema#dateTime">2018-09-14T20:25:40Z</dc:date>
        <rdfs:label>software architecture role</rdfs:label>
    </owl:Class>
    


    <!-- http://purl.obolibrary.org/obo/CRO_0000063 -->

    <owl:Class rdf:about="http://purl.obolibrary.org/obo/CRO_0000063">
        <rdfs:subClassOf rdf:resource="http://purl.org/credit/ontology#CREDIT_00000009"/>
        <obo:IAO_0000115>Creation of low-level software component and algorithm design.</obo:IAO_0000115>
        <dc:creator rdf:resource="http://orcid.org/0000-0001-5208-3432"/>
        <dc:date rdf:datatype="http://www.w3.org/2001/XMLSchema#dateTime">2018-09-14T20:25:45Z</dc:date>
        <rdfs:label>software design role</rdfs:label>
    </owl:Class>
    <owl:Axiom>
        <owl:annotatedSource rdf:resource="http://purl.obolibrary.org/obo/CRO_0000063"/>
        <owl:annotatedProperty rdf:resource="http://purl.obolibrary.org/obo/IAO_0000115"/>
        <owl:annotatedTarget>Creation of low-level software component and algorithm design.</owl:annotatedTarget>
        <obo:IAO_0000119>https://en.wikipedia.org/wiki/Low-level_design</obo:IAO_0000119>
    </owl:Axiom>
    


    <!-- http://purl.obolibrary.org/obo/CRO_0000064 -->

    <owl:Class rdf:about="http://purl.obolibrary.org/obo/CRO_0000064">
        <rdfs:subClassOf rdf:resource="http://purl.org/credit/ontology#CREDIT_00000009"/>
        <obo:IAO_0000115>Systematic application of scientific and technological knowledge, methods, and experience to the design, implementation, testing, and documentation of software.</obo:IAO_0000115>
        <obo:IAO_0000118>computer programming role</obo:IAO_0000118>
        <dc:creator rdf:resource="http://orcid.org/0000-0001-5208-3432"/>
        <dc:date rdf:datatype="http://www.w3.org/2001/XMLSchema#dateTime">2018-09-14T20:25:49Z</dc:date>
        <rdfs:label>software engineering role</rdfs:label>
    </owl:Class>
    


    <!-- http://purl.obolibrary.org/obo/CRO_0000065 -->

    <owl:Class rdf:about="http://purl.obolibrary.org/obo/CRO_0000065">
        <rdfs:subClassOf rdf:resource="http://purl.obolibrary.org/obo/CRO_0000078"/>
        <obo:IAO_0000115>Planning, management, and monitoring of projects.</obo:IAO_0000115>
        <dc:creator rdf:resource="http://orcid.org/0000-0001-5208-3432"/>
        <dc:date rdf:datatype="http://www.w3.org/2001/XMLSchema#dateTime">2018-09-14T20:25:55Z</dc:date>
        <rdfs:label>project management role</rdfs:label>
    </owl:Class>
    


    <!-- http://purl.obolibrary.org/obo/CRO_0000067 -->

    <owl:Class rdf:about="http://purl.obolibrary.org/obo/CRO_0000067">
        <rdfs:subClassOf rdf:resource="http://purl.obolibrary.org/obo/CRO_0000023"/>
        <obo:IAO_0000115>A professional who assesses, collects, organizes, preserves, maintains control over, and provides access to information determined to have long-term value.</obo:IAO_0000115>
        <dc:creator rdf:resource="http://orcid.org/0000-0001-5208-3432"/>
        <dc:date rdf:datatype="http://www.w3.org/2001/XMLSchema#dateTime">2018-09-15T16:25:54Z</dc:date>
        <rdfs:label>archivist role</rdfs:label>
    </owl:Class>
    <owl:Axiom>
        <owl:annotatedSource rdf:resource="http://purl.obolibrary.org/obo/CRO_0000067"/>
        <owl:annotatedProperty rdf:resource="http://purl.obolibrary.org/obo/IAO_0000115"/>
        <owl:annotatedTarget>A professional who assesses, collects, organizes, preserves, maintains control over, and provides access to information determined to have long-term value.</owl:annotatedTarget>
        <obo:IAO_0000119>https://www.wikidata.org/wiki/Q635734</obo:IAO_0000119>
    </owl:Axiom>
    


    <!-- http://purl.obolibrary.org/obo/CRO_0000068 -->

    <owl:Class rdf:about="http://purl.obolibrary.org/obo/CRO_0000068">
        <rdfs:subClassOf rdf:resource="http://purl.obolibrary.org/obo/CRO_0000023"/>
        <obo:IAO_0000115>A person responsible for the preservation of artistic and cultural artifacts.</obo:IAO_0000115>
        <dc:creator rdf:resource="http://orcid.org/0000-0001-5208-3432"/>
        <dc:date rdf:datatype="http://www.w3.org/2001/XMLSchema#dateTime">2018-09-15T16:26:00Z</dc:date>
        <rdfs:label>conservator role</rdfs:label>
    </owl:Class>
    <owl:Axiom>
        <owl:annotatedSource rdf:resource="http://purl.obolibrary.org/obo/CRO_0000068"/>
        <owl:annotatedProperty rdf:resource="http://purl.obolibrary.org/obo/IAO_0000115"/>
        <owl:annotatedTarget>A person responsible for the preservation of artistic and cultural artifacts.</owl:annotatedTarget>
        <obo:IAO_0000119>https://www.wikidata.org/wiki/Q446966</obo:IAO_0000119>
    </owl:Axiom>
    


    <!-- http://purl.obolibrary.org/obo/CRO_0000069 -->

    <owl:Class rdf:about="http://purl.obolibrary.org/obo/CRO_0000069">
        <rdfs:subClassOf rdf:resource="http://purl.obolibrary.org/obo/CRO_0000023"/>
        <obo:IAO_0000115>A role that includes the formal endeavor to ensure that digital information of continuing value remains accessible, trustworthy, and usable.</obo:IAO_0000115>
        <dc:creator rdf:resource="http://orcid.org/0000-0001-5208-3432"/>
        <dc:date rdf:datatype="http://www.w3.org/2001/XMLSchema#dateTime">2018-09-15T16:26:05Z</dc:date>
        <rdfs:label>digital preservation role</rdfs:label>
    </owl:Class>
    <owl:Axiom>
        <owl:annotatedSource rdf:resource="http://purl.obolibrary.org/obo/CRO_0000069"/>
        <owl:annotatedProperty rdf:resource="http://purl.obolibrary.org/obo/IAO_0000115"/>
        <owl:annotatedTarget>A role that includes the formal endeavor to ensure that digital information of continuing value remains accessible, trustworthy, and usable.</owl:annotatedTarget>
        <obo:IAO_0000119>https://www.wikidata.org/wiki/Q632897</obo:IAO_0000119>
    </owl:Axiom>
    


    <!-- http://purl.obolibrary.org/obo/CRO_0000070 -->

    <owl:Class rdf:about="http://purl.obolibrary.org/obo/CRO_0000070">
        <rdfs:subClassOf rdf:resource="http://www.w3.org/2002/07/owl#Thing"/>
        <dc:creator rdf:resource="http://orcid.org/0000-0001-5208-3432"/>
        <dc:date rdf:datatype="http://www.w3.org/2001/XMLSchema#dateTime">2018-09-15T16:29:29Z</dc:date>
        <rdfs:label>relationship</rdfs:label>
    </owl:Class>
    


    <!-- http://purl.obolibrary.org/obo/CRO_0000071 -->

    <owl:Class rdf:about="http://purl.obolibrary.org/obo/CRO_0000071">
        <rdfs:subClassOf rdf:resource="http://purl.obolibrary.org/obo/CRO_0000070"/>
        <dc:creator rdf:resource="http://orcid.org/0000-0001-5208-3432"/>
        <dc:date rdf:datatype="http://www.w3.org/2001/XMLSchema#dateTime">2018-09-15T16:29:43Z</dc:date>
        <rdfs:label>contributorship</rdfs:label>
    </owl:Class>
    


    <!-- http://purl.obolibrary.org/obo/CRO_0000072 -->

    <owl:Class rdf:about="http://purl.obolibrary.org/obo/CRO_0000072">
        <rdfs:subClassOf rdf:resource="http://purl.obolibrary.org/obo/CRO_0000015"/>
        <obo:IAO_0000115>Aggregation, integration, manipulation of data.</obo:IAO_0000115>
        <obo:IAO_0000118>data manipulation role</obo:IAO_0000118>
        <dc:creator rdf:resource="http://orcid.org/0000-0001-5208-3432"/>
        <dc:date rdf:datatype="http://www.w3.org/2001/XMLSchema#dateTime">2018-10-01T20:32:37Z</dc:date>
        <rdfs:label>data transformation role</rdfs:label>
    </owl:Class>
    


    <!-- http://purl.obolibrary.org/obo/CRO_0000073 -->

    <owl:Class rdf:about="http://purl.obolibrary.org/obo/CRO_0000073">
        <rdfs:subClassOf rdf:resource="http://purl.obolibrary.org/obo/CRO_0000000"/>
        <obo:IAO_0000115>The process of creating standards, which aare an established norm or requirement in regard to technical systems. It is usually a formal document that establishes uniform engineering or technical criteria, methods, processes, and practices.</obo:IAO_0000115>
        <obo:IAO_0000118>standard development role</obo:IAO_0000118>
        <dc:creator rdf:resource="http://orcid.org/0000-0001-5208-3432"/>
        <dc:date rdf:datatype="http://www.w3.org/2001/XMLSchema#dateTime">2018-10-01T20:33:58Z</dc:date>
        <rdfs:label>standards development role</rdfs:label>
    </owl:Class>
    <owl:Axiom>
        <owl:annotatedSource rdf:resource="http://purl.obolibrary.org/obo/CRO_0000073"/>
        <owl:annotatedProperty rdf:resource="http://purl.obolibrary.org/obo/IAO_0000115"/>
        <owl:annotatedTarget>The process of creating standards, which aare an established norm or requirement in regard to technical systems. It is usually a formal document that establishes uniform engineering or technical criteria, methods, processes, and practices.</owl:annotatedTarget>
        <obo:IAO_0000119>https://en.wikipedia.org/wiki/Technical_standard</obo:IAO_0000119>
    </owl:Axiom>
    


    <!-- http://purl.obolibrary.org/obo/CRO_0000074 -->

    <owl:Class rdf:about="http://purl.obolibrary.org/obo/CRO_0000074">
        <rdfs:subClassOf rdf:resource="http://purl.obolibrary.org/obo/CRO_0000015"/>
        <obo:IAO_0000115>Verification, whether as a part of the activity or separate, of the overall replication/reproducibility of results/experiments and other research outputs.</obo:IAO_0000115>
        <dc:creator rdf:resource="http://orcid.org/0000-0001-5208-3432"/>
        <dc:date rdf:datatype="http://www.w3.org/2001/XMLSchema#dateTime">2018-10-01T20:35:43Z</dc:date>
        <rdfs:label>data validation role</rdfs:label>
    </owl:Class>
    


    <!-- http://purl.obolibrary.org/obo/CRO_0000075 -->

    <owl:Class rdf:about="http://purl.obolibrary.org/obo/CRO_0000075">
        <rdfs:subClassOf rdf:resource="http://www.w3.org/2002/07/owl#Thing"/>
        <obo:IAO_0000118>formal training role</obo:IAO_0000118>
        <obo:IAO_0100001 rdf:resource="http://purl.obolibrary.org/obo/CRO_0000047"/>
        <dc:creator rdf:resource="http://orcid.org/0000-0001-5208-3432"/>
        <dc:date rdf:datatype="http://www.w3.org/2001/XMLSchema#dateTime">2018-10-01T20:42:52Z</dc:date>
        <rdfs:label>educational training role</rdfs:label>
        <owl:deprecated rdf:datatype="http://www.w3.org/2001/XMLSchema#boolean">true</owl:deprecated>
    </owl:Class>
    


    <!-- http://purl.obolibrary.org/obo/CRO_0000076 -->

    <owl:Class rdf:about="http://purl.obolibrary.org/obo/CRO_0000076">
        <rdfs:subClassOf rdf:resource="http://www.w3.org/2002/07/owl#Thing"/>
        <obo:IAO_0000115>A role that includes the design and implementation of the physical components of a computer system.</obo:IAO_0000115>
        <obo:IAO_0000118>information technology hardware systems design and implementation role</obo:IAO_0000118>
        <dc:creator rdf:resource="http://orcid.org/0000-0001-5208-3432"/>
        <dc:date rdf:datatype="http://www.w3.org/2001/XMLSchema#dateTime">2018-10-01T20:43:37Z</dc:date>
        <rdfs:label>obsolete IT hardware systems design and implementation role</rdfs:label>
        <owl:deprecated rdf:datatype="http://www.w3.org/2001/XMLSchema#boolean">true</owl:deprecated>
    </owl:Class>
    <owl:Axiom>
        <owl:annotatedSource rdf:resource="http://purl.obolibrary.org/obo/CRO_0000076"/>
        <owl:annotatedProperty rdf:resource="http://purl.obolibrary.org/obo/IAO_0000115"/>
        <owl:annotatedTarget>A role that includes the design and implementation of the physical components of a computer system.</owl:annotatedTarget>
        <obo:IAO_0000119>https://www.wikidata.org/wiki/Q3966</obo:IAO_0000119>
    </owl:Axiom>
    


    <!-- http://purl.obolibrary.org/obo/CRO_0000077 -->

    <owl:Class rdf:about="http://purl.obolibrary.org/obo/CRO_0000077">
        <rdfs:subClassOf rdf:resource="http://www.w3.org/2002/07/owl#Thing"/>
        <obo:IAO_0100001 rdf:resource="http://purl.obolibrary.org/obo/CRO_0000051"/>
        <dc:creator rdf:resource="http://orcid.org/0000-0001-5208-3432"/>
        <dc:date rdf:datatype="http://www.w3.org/2001/XMLSchema#dateTime">2018-10-01T20:44:21Z</dc:date>
        <rdfs:label>systems administration role</rdfs:label>
        <owl:deprecated rdf:datatype="http://www.w3.org/2001/XMLSchema#boolean">true</owl:deprecated>
    </owl:Class>
    


    <!-- http://purl.obolibrary.org/obo/CRO_0000078 -->

    <owl:Class rdf:about="http://purl.obolibrary.org/obo/CRO_0000078">
        <rdfs:subClassOf rdf:resource="http://purl.obolibrary.org/obo/CRO_0000000"/>
        <obo:IAO_0000115>Contribution to the basic, underlying framework or features of a system or organization.</obo:IAO_0000115>
        <dc:creator rdf:resource="http://orcid.org/0000-0001-5208-3432"/>
        <dc:date rdf:datatype="http://www.w3.org/2001/XMLSchema#dateTime">2018-10-01T20:48:11Z</dc:date>
        <rdfs:label>infrastructure role</rdfs:label>
    </owl:Class>
    <owl:Axiom>
        <owl:annotatedSource rdf:resource="http://purl.obolibrary.org/obo/CRO_0000078"/>
        <owl:annotatedProperty rdf:resource="http://purl.obolibrary.org/obo/IAO_0000115"/>
        <owl:annotatedTarget>Contribution to the basic, underlying framework or features of a system or organization.</owl:annotatedTarget>
        <obo:IAO_0000119>https://www.dictionary.com/browse/infrastructure</obo:IAO_0000119>
    </owl:Axiom>
    


    <!-- http://purl.obolibrary.org/obo/CRO_0000079 -->

    <owl:Class rdf:about="http://purl.obolibrary.org/obo/CRO_0000079">
        <rdfs:subClassOf rdf:resource="http://purl.obolibrary.org/obo/CRO_0000078"/>
        <obo:IAO_0000115>Evaluation is a systematic method for collecting, analyzing, and using information to answer questions about projects, policies and programs, particularly about their effectiveness and efficiency.</obo:IAO_0000115>
        <dc:creator rdf:resource="http://orcid.org/0000-0001-5208-3432"/>
        <dc:date rdf:datatype="http://www.w3.org/2001/XMLSchema#dateTime">2018-10-01T20:48:24Z</dc:date>
        <rdfs:label>project, policy or program evaluation role</rdfs:label>
    </owl:Class>
    <owl:Axiom>
        <owl:annotatedSource rdf:resource="http://purl.obolibrary.org/obo/CRO_0000079"/>
        <owl:annotatedProperty rdf:resource="http://purl.obolibrary.org/obo/IAO_0000115"/>
        <owl:annotatedTarget>Evaluation is a systematic method for collecting, analyzing, and using information to answer questions about projects, policies and programs, particularly about their effectiveness and efficiency.</owl:annotatedTarget>
        <obo:IAO_0000119>https://en.wikipedia.org/wiki/Program_evaluation</obo:IAO_0000119>
    </owl:Axiom>
    


    <!-- http://purl.obolibrary.org/obo/CRO_0000080 -->

    <owl:Class rdf:about="http://purl.obolibrary.org/obo/CRO_0000080">
        <rdfs:subClassOf rdf:resource="http://www.w3.org/2002/07/owl#Thing"/>
        <obo:IAO_0000115>An infrastructure role that is accountable for management and coordination of a program, to help achieve the program goals.</obo:IAO_0000115>
        <obo:IAO_0100001 rdf:resource="http://purl.org/credit/ontology#CREDIT_00000007"/>
        <dc:creator rdf:resource="http://orcid.org/0000-0001-5208-3432"/>
        <dc:date rdf:datatype="http://www.w3.org/2001/XMLSchema#dateTime">2018-10-01T20:48:37Z</dc:date>
        <rdfs:label>obsolete program administration role</rdfs:label>
        <owl:deprecated rdf:datatype="http://www.w3.org/2001/XMLSchema#boolean">true</owl:deprecated>
    </owl:Class>
    


    <!-- http://purl.obolibrary.org/obo/CRO_0000081 -->

    <owl:Class rdf:about="http://purl.obolibrary.org/obo/CRO_0000081">
        <rdfs:subClassOf rdf:resource="http://purl.obolibrary.org/obo/CRO_0000078"/>
        <obo:IAO_0000115>The organization of the different elements needed to implement a study.</obo:IAO_0000115>
        <dc:creator rdf:resource="http://orcid.org/0000-0001-5208-3432"/>
        <dc:date rdf:datatype="http://www.w3.org/2001/XMLSchema#dateTime">2018-10-01T20:49:10Z</dc:date>
        <rdfs:label>coordination role</rdfs:label>
    </owl:Class>
    <owl:Axiom>
        <owl:annotatedSource rdf:resource="http://purl.obolibrary.org/obo/CRO_0000081"/>
        <owl:annotatedProperty rdf:resource="http://purl.obolibrary.org/obo/IAO_0000115"/>
        <owl:annotatedTarget>The organization of the different elements needed to implement a study.</owl:annotatedTarget>
        <obo:IAO_0000119>https://learn.nursing.jhu.edu/face-to-face/courses/research-coordinator/index.html</obo:IAO_0000119>
    </owl:Axiom>
    


    <!-- http://purl.obolibrary.org/obo/CRO_0000082 -->

    <owl:Class rdf:about="http://purl.obolibrary.org/obo/CRO_0000082">
        <rdfs:subClassOf rdf:resource="http://www.w3.org/2002/07/owl#Thing"/>
        <obo:IAO_0000115>Oversight and leadership responsibility for the research activity planning and execution, including mentorship external to the core team.</obo:IAO_0000115>
        <obo:IAO_0100001 rdf:resource="http://purl.org/credit/ontology#CREDIT_00000010"/>
        <dc:creator rdf:resource="http://orcid.org/0000-0001-5208-3432"/>
        <dc:date rdf:datatype="http://www.w3.org/2001/XMLSchema#dateTime">2018-10-01T20:49:54Z</dc:date>
        <rdfs:label>supervisory role</rdfs:label>
        <owl:deprecated rdf:datatype="http://www.w3.org/2001/XMLSchema#boolean">true</owl:deprecated>
    </owl:Class>
    


    <!-- http://purl.obolibrary.org/obo/CRO_0000083 -->

    <owl:Class rdf:about="http://purl.obolibrary.org/obo/CRO_0000083">
        <rdfs:subClassOf rdf:resource="http://purl.obolibrary.org/obo/CRO_0000007"/>
        <obo:IAO_0000115>A communication role which involves the dynamic relational process that facilitates communication, interaction, involvement, and exchange between an organization and a community for a range of social and organizational outcomes.</obo:IAO_0000115>
        <dc:creator rdf:resource="http://orcid.org/0000-0001-5208-3432"/>
        <dc:date rdf:datatype="http://www.w3.org/2001/XMLSchema#dateTime">2018-10-01T20:55:22Z</dc:date>
        <rdfs:label>community engagement role</rdfs:label>
    </owl:Class>
    <owl:Axiom>
        <owl:annotatedSource rdf:resource="http://purl.obolibrary.org/obo/CRO_0000083"/>
        <owl:annotatedProperty rdf:resource="http://purl.obolibrary.org/obo/IAO_0000115"/>
        <owl:annotatedTarget>A communication role which involves the dynamic relational process that facilitates communication, interaction, involvement, and exchange between an organization and a community for a range of social and organizational outcomes.</owl:annotatedTarget>
        <obo:IAO_0000119>Johnston, K. A. (2018). Toward a theory of social engagement. In K. A. Johnston &amp; M. Taylor (Eds.), The Handbook of Communication Engagement (pp. 19-32). Hoboken, NJ: Wiley.</obo:IAO_0000119>
    </owl:Axiom>
    


    <!-- http://purl.obolibrary.org/obo/CRO_0000084 -->

    <owl:Class rdf:about="http://purl.obolibrary.org/obo/CRO_0000084">
        <rdfs:subClassOf rdf:resource="http://purl.obolibrary.org/obo/CRO_0000007"/>
        <obo:IAO_0000115>A communication role that involves development or production of materials, such as brochures, websites, flyers, presentations, etc., for the purposes of promotion of a entity, like a project, group or organization.</obo:IAO_0000115>
        <dc:creator rdf:resource="http://orcid.org/0000-0001-5208-3432"/>
        <dc:date rdf:datatype="http://www.w3.org/2001/XMLSchema#dateTime">2018-10-01T20:56:18Z</dc:date>
        <rdfs:label>outreach materials development role</rdfs:label>
    </owl:Class>
    


    <!-- http://purl.obolibrary.org/obo/CRO_0000085 -->

    <owl:Class rdf:about="http://purl.obolibrary.org/obo/CRO_0000085">
        <rdfs:subClassOf rdf:resource="http://www.w3.org/2002/07/owl#Thing"/>
        <obo:IAO_0000115>Role that involves identifying eligible participants, explaining the study to potential participants, recruiting an adequate sample based on study goals and design, obtaining informed consent/maintaining ethical standards, and retaining participants until study completion.</obo:IAO_0000115>
        <dc:creator rdf:resource="http://orcid.org/0000-0001-5208-3432"/>
        <dc:date rdf:datatype="http://www.w3.org/2001/XMLSchema#dateTime">2018-10-01T20:57:17Z</dc:date>
        <rdfs:label>obsolete participant recruitment role</rdfs:label>
        <owl:deprecated rdf:datatype="http://www.w3.org/2001/XMLSchema#boolean">true</owl:deprecated>
    </owl:Class>
    <owl:Axiom>
        <owl:annotatedSource rdf:resource="http://purl.obolibrary.org/obo/CRO_0000085"/>
        <owl:annotatedProperty rdf:resource="http://purl.obolibrary.org/obo/IAO_0000115"/>
        <owl:annotatedTarget>Role that involves identifying eligible participants, explaining the study to potential participants, recruiting an adequate sample based on study goals and design, obtaining informed consent/maintaining ethical standards, and retaining participants until study completion.</owl:annotatedTarget>
        <obo:IAO_0000119>https://healthit.ahrq.gov/ahrq-funded-projects/emerging-lessons/participant-recruitment-research</obo:IAO_0000119>
    </owl:Axiom>
    


    <!-- http://purl.obolibrary.org/obo/CRO_0000086 -->

    <owl:Class rdf:about="http://purl.obolibrary.org/obo/CRO_0000086">
        <rdfs:subClassOf rdf:resource="http://www.w3.org/2002/07/owl#Thing"/>
        <obo:IAO_0000118>Ideas; formulation or evolution of overarching research goals and aims.</obo:IAO_0000118>
        <obo:IAO_0100001 rdf:resource="http://purl.org/credit/ontology#CREDIT_00000001"/>
        <dc:creator rdf:resource="http://orcid.org/0000-0001-5208-3432"/>
        <dc:date rdf:datatype="http://www.w3.org/2001/XMLSchema#dateTime">2018-10-01T20:57:53Z</dc:date>
        <rdfs:label>research conceptualization role</rdfs:label>
        <owl:deprecated rdf:datatype="http://www.w3.org/2001/XMLSchema#boolean">true</owl:deprecated>
    </owl:Class>
    


    <!-- http://purl.obolibrary.org/obo/CRO_0000087 -->

    <owl:Class rdf:about="http://purl.obolibrary.org/obo/CRO_0000087">
        <rdfs:subClassOf rdf:resource="http://purl.org/credit/ontology#CREDIT_00000005"/>
        <obo:IAO_0000115>One who is proficient in the relevant skill and technique, with a relatively practical understanding of the theoretical principles.</obo:IAO_0000115>
        <dc:creator rdf:resource="http://orcid.org/0000-0001-5208-3432"/>
        <dc:date rdf:datatype="http://www.w3.org/2001/XMLSchema#dateTime">2018-10-01T20:58:59Z</dc:date>
        <rdfs:label>technician role</rdfs:label>
    </owl:Class>
    <owl:Axiom>
        <owl:annotatedSource rdf:resource="http://purl.obolibrary.org/obo/CRO_0000087"/>
        <owl:annotatedProperty rdf:resource="http://purl.obolibrary.org/obo/IAO_0000115"/>
        <owl:annotatedTarget>One who is proficient in the relevant skill and technique, with a relatively practical understanding of the theoretical principles.</owl:annotatedTarget>
        <obo:IAO_0000119>https://en.wikipedia.org/wiki/Technician</obo:IAO_0000119>
    </owl:Axiom>
    


    <!-- http://purl.obolibrary.org/obo/CRO_0000088 -->

    <owl:Class rdf:about="http://purl.obolibrary.org/obo/CRO_0000088">
        <rdfs:subClassOf rdf:resource="http://www.w3.org/2002/07/owl#Thing"/>
        <obo:IAO_0000115>Creation and/or presentation of the published work, specifically writing the initial draft (including substantive translation).</obo:IAO_0000115>
        <obo:IAO_0100001 rdf:resource="http://purl.org/credit/ontology#CREDIT_00000013"/>
        <dc:creator rdf:resource="http://orcid.org/0000-0001-5208-3432"/>
        <dc:date rdf:datatype="http://www.w3.org/2001/XMLSchema#dateTime">2018-10-01T21:03:36Z</dc:date>
        <rdfs:label>original draft preparation role</rdfs:label>
        <owl:deprecated rdf:datatype="http://www.w3.org/2001/XMLSchema#boolean">true</owl:deprecated>
    </owl:Class>
    


    <!-- http://purl.obolibrary.org/obo/CRO_0000089 -->

    <owl:Class rdf:about="http://purl.obolibrary.org/obo/CRO_0000089">
        <rdfs:subClassOf rdf:resource="http://purl.obolibrary.org/obo/CRO_0000001"/>
        <obo:IAO_0000115>A role in which one provides a summary of a research output, such as a journal article, that is understandable by a lay person or non-expert audience.</obo:IAO_0000115>
        <obo:IAO_0000118>lay synthesis of research output role</obo:IAO_0000118>
        <dc:creator rdf:resource="http://orcid.org/0000-0001-5208-3432"/>
        <dc:date rdf:datatype="http://www.w3.org/2001/XMLSchema#dateTime">2018-10-01T21:04:14Z</dc:date>
        <rdfs:label>lay summary role</rdfs:label>
    </owl:Class>
    


    <!-- http://purl.obolibrary.org/obo/CRO_0000090 -->

    <owl:Class rdf:about="http://purl.obolibrary.org/obo/CRO_0000090">
        <rdfs:subClassOf rdf:resource="http://www.w3.org/2002/07/owl#Thing"/>
        <obo:IAO_0000115>A method or steps that maintain, update content, clean up, or repair a website.</obo:IAO_0000115>
        <obo:IAO_0100001 rdf:resource="http://purl.obolibrary.org/obo/CRO_0000008"/>
        <dc:creator rdf:resource="http://orcid.org/0000-0001-5208-3432"/>
        <dc:date rdf:datatype="http://www.w3.org/2001/XMLSchema#dateTime">2018-10-01T21:13:13Z</dc:date>
        <rdfs:label>obsolete website maintenance role</rdfs:label>
        <owl:deprecated rdf:datatype="http://www.w3.org/2001/XMLSchema#boolean">true</owl:deprecated>
    </owl:Class>
    <owl:Axiom>
        <owl:annotatedSource rdf:resource="http://purl.obolibrary.org/obo/CRO_0000090"/>
        <owl:annotatedProperty rdf:resource="http://purl.obolibrary.org/obo/IAO_0000115"/>
        <owl:annotatedTarget>A method or steps that maintain, update content, clean up, or repair a website.</owl:annotatedTarget>
        <obo:IAO_0000119>https://www.wikidata.org/wiki/Q17634596</obo:IAO_0000119>
    </owl:Axiom>
    


    <!-- http://purl.obolibrary.org/obo/CRO_0000091 -->

    <owl:Class rdf:about="http://purl.obolibrary.org/obo/CRO_0000091">
        <rdfs:subClassOf rdf:resource="http://purl.obolibrary.org/obo/CRO_0000011"/>
        <obo:IAO_0000115>A documentation role that involves preparation of instruction manuals, journal articles, and other supporting documents to communicate complex and technical information more easily.</obo:IAO_0000115>
        <oboInOwl:created_by rdf:resource="http://orcid.org/0000-0001-5208-3432"/>
        <rdfs:label>technical writing role</rdfs:label>
    </owl:Class>
    <owl:Axiom>
        <owl:annotatedSource rdf:resource="http://purl.obolibrary.org/obo/CRO_0000091"/>
        <owl:annotatedProperty rdf:resource="http://purl.obolibrary.org/obo/IAO_0000115"/>
        <owl:annotatedTarget>A documentation role that involves preparation of instruction manuals, journal articles, and other supporting documents to communicate complex and technical information more easily.</owl:annotatedTarget>
        <obo:IAO_0000119>https://www.truity.com/career-profile/technical-writer</obo:IAO_0000119>
    </owl:Axiom>
    


    <!-- http://purl.obolibrary.org/obo/CRO_0000092 -->

    <owl:Class rdf:about="http://purl.obolibrary.org/obo/CRO_0000092">
        <rdfs:subClassOf rdf:resource="http://purl.org/credit/ontology#CREDIT_00000009"/>
        <obo:IAO_0000115>The tasks that go into determining the needs or conditions to meet for a new or altered software product or project, taking account of the possibly conflicting requirements of the various stakeholders, analyzing, documenting, validating and managing software or system requirements.</obo:IAO_0000115>
        <oboInOwl:created_by rdf:resource="http://orcid.org/0000-0001-5208-3432"/>
        <rdfs:label>requirements analysis role</rdfs:label>
    </owl:Class>
    <owl:Axiom>
        <owl:annotatedSource rdf:resource="http://purl.obolibrary.org/obo/CRO_0000092"/>
        <owl:annotatedProperty rdf:resource="http://purl.obolibrary.org/obo/IAO_0000115"/>
        <owl:annotatedTarget>The tasks that go into determining the needs or conditions to meet for a new or altered software product or project, taking account of the possibly conflicting requirements of the various stakeholders, analyzing, documenting, validating and managing software or system requirements.</owl:annotatedTarget>
        <obo:IAO_0000119>Kotonya, G. and Sommerville, I. 1998. Requirements Engineering: Processes and Techniques Chichester, UK: John Wiley and Sons.</obo:IAO_0000119>
    </owl:Axiom>
    


    <!-- http://purl.obolibrary.org/obo/CRO_0000093 -->

    <owl:Class rdf:about="http://purl.obolibrary.org/obo/CRO_0000093">
        <rdfs:subClassOf rdf:resource="http://purl.obolibrary.org/obo/CRO_0000028"/>
        <obo:IAO_0000115>Obtaining a material entity for potential use as an input during an investigation.</obo:IAO_0000115>
        <obo:IAO_0000234>https://orcid.org/0000-0002-2908-3327</obo:IAO_0000234>
        <oboInOwl:created_by rdf:resource="http://orcid.org/0000-0001-5208-3432"/>
        <rdfs:label>specimen collection role</rdfs:label>
    </owl:Class>
    


    <!-- http://purl.obolibrary.org/obo/CRO_0000094 -->

    <owl:Class rdf:about="http://purl.obolibrary.org/obo/CRO_0000094">
        <rdfs:subClassOf rdf:resource="http://purl.obolibrary.org/obo/CRO_0000093"/>
        <obo:IAO_0000115>In botany, this is the collector listed first for a particular specimen. Each specimen has one primary collector. The primary collector assigns a number to that specimen from his/her own number series.</obo:IAO_0000115>
        <obo:IAO_0000234>http://orcid.org/0000-0002-2908-3327</obo:IAO_0000234>
        <oboInOwl:created_by rdf:resource="http://orcid.org/0000-0001-5208-3432"/>
        <rdfs:label>primary collector role</rdfs:label>
    </owl:Class>
    


    <!-- http://purl.obolibrary.org/obo/CRO_0000095 -->

    <owl:Class rdf:about="http://purl.obolibrary.org/obo/CRO_0000095">
        <rdfs:subClassOf rdf:resource="http://purl.obolibrary.org/obo/CRO_0000101"/>
        <obo:IAO_0000115>Evaluation of grant applications by others working in the same field.</obo:IAO_0000115>
        <obo:IAO_0000234>https://orcid.org/0000-0001-9114-8737</obo:IAO_0000234>
        <oboInOwl:created_by rdf:resource="http://orcid.org/0000-0001-5208-3432"/>
        <rdfs:label>grant peer review role</rdfs:label>
    </owl:Class>
    


    <!-- http://purl.obolibrary.org/obo/CRO_0000096 -->

    <owl:Class rdf:about="http://purl.obolibrary.org/obo/CRO_0000096">
        <rdfs:subClassOf rdf:resource="http://purl.obolibrary.org/obo/CRO_0000028"/>
        <obo:IAO_0000115>Selecting, ordering, and receiving materials or physical objects for research, scholarly, library or archival collections.</obo:IAO_0000115>
        <obo:IAO_0000234>https://orcid.org/0000-0002-2908-3327</obo:IAO_0000234>
        <oboInOwl:created_by rdf:resource="http://orcid.org/0000-0001-5208-3432"/>
        <rdfs:label>acquisition role</rdfs:label>
    </owl:Class>
    


    <!-- http://purl.obolibrary.org/obo/CRO_0000097 -->

    <owl:Class rdf:about="http://purl.obolibrary.org/obo/CRO_0000097">
        <rdfs:subClassOf rdf:resource="http://purl.obolibrary.org/obo/CRO_0000000"/>
        <obo:IAO_0000115>The person or organization that provides money for a particular purpose, such as a grant to perform research.</obo:IAO_0000115>
        <obo:IAO_0000118>funder role</obo:IAO_0000118>
        <oboInOwl:created_by rdf:resource="http://orcid.org/0000-0001-5208-3432"/>
        <rdfs:label>funding source role</rdfs:label>
    </owl:Class>
    <owl:Axiom>
        <owl:annotatedSource rdf:resource="http://purl.obolibrary.org/obo/CRO_0000097"/>
        <owl:annotatedProperty rdf:resource="http://purl.obolibrary.org/obo/IAO_0000115"/>
        <owl:annotatedTarget>The person or organization that provides money for a particular purpose, such as a grant to perform research.</owl:annotatedTarget>
        <obo:IAO_0000119>https://www.lexico.com/en/definition/funder</obo:IAO_0000119>
    </owl:Axiom>
    


    <!-- http://purl.obolibrary.org/obo/CRO_0000098 -->

    <owl:Class rdf:about="http://purl.obolibrary.org/obo/CRO_0000098">
        <rdfs:subClassOf rdf:resource="http://purl.obolibrary.org/obo/CRO_0000000"/>
        <obo:IAO_0000115>The person or organization that is responsible for a new or novel discovery, i.e., the process of finding information, a place, or an object, especially for the first time, or the thing that is found. For example, a researcher discovering a new gene mutation that contributes to a disease.</obo:IAO_0000115>
        <oboInOwl:created_by rdf:resource="http://orcid.org/0000-0001-5208-3432"/>
        <rdfs:label>discovery role</rdfs:label>
    </owl:Class>
    <owl:Axiom>
        <owl:annotatedSource rdf:resource="http://purl.obolibrary.org/obo/CRO_0000098"/>
        <owl:annotatedProperty rdf:resource="http://purl.obolibrary.org/obo/IAO_0000115"/>
        <owl:annotatedTarget>The person or organization that is responsible for a new or novel discovery, i.e., the process of finding information, a place, or an object, especially for the first time, or the thing that is found. For example, a researcher discovering a new gene mutation that contributes to a disease.</owl:annotatedTarget>
        <obo:IAO_0000119>https://dictionary.cambridge.org/us/dictionary/english/discovery</obo:IAO_0000119>
    </owl:Axiom>
    


    <!-- http://purl.obolibrary.org/obo/CRO_0000099 -->

    <owl:Class rdf:about="http://purl.obolibrary.org/obo/CRO_0000099">
        <rdfs:subClassOf rdf:resource="http://purl.obolibrary.org/obo/CRO_0000000"/>
        <obo:IAO_0000115>A person or organization who helps guide a patient through the healthcare system. This includes help going through the screening, diagnosis, treatment (including clinical trials), and follow-up of a medical condition, such as cancer.</obo:IAO_0000115>
        <oboInOwl:created_by rdf:resource="http://orcid.org/0000-0001-5208-3432"/>
        <rdfs:label>patient advocate role</rdfs:label>
    </owl:Class>
    <owl:Axiom>
        <owl:annotatedSource rdf:resource="http://purl.obolibrary.org/obo/CRO_0000099"/>
        <owl:annotatedProperty rdf:resource="http://purl.obolibrary.org/obo/IAO_0000115"/>
        <owl:annotatedTarget>A person or organization who helps guide a patient through the healthcare system. This includes help going through the screening, diagnosis, treatment (including clinical trials), and follow-up of a medical condition, such as cancer.</owl:annotatedTarget>
        <obo:IAO_0000119>https://www.cancer.gov/publications/dictionaries/cancer-terms/def/patient-advocate</obo:IAO_0000119>
    </owl:Axiom>
    


    <!-- http://purl.obolibrary.org/obo/CRO_0000100 -->

    <owl:Class rdf:about="http://purl.obolibrary.org/obo/CRO_0000100">
        <rdfs:subClassOf rdf:resource="http://purl.obolibrary.org/obo/CRO_0000000"/>
        <obo:IAO_0000115>Oral presentation intended to present information or teach people about a particular subject, such as a talk or poster presentation at a conference.</obo:IAO_0000115>
        <obo:IAO_0000118>lecture role</obo:IAO_0000118>
        <obo:IAO_0000118>lecturer role</obo:IAO_0000118>
        <obo:IAO_0000118>presentation role</obo:IAO_0000118>
        <obo:IAO_0000118>speaker role</obo:IAO_0000118>
        <oboInOwl:created_by rdf:resource="http://orcid.org/0000-0001-5208-3432"/>
        <rdfs:label>presenter role</rdfs:label>
    </owl:Class>
    <owl:Axiom>
        <owl:annotatedSource rdf:resource="http://purl.obolibrary.org/obo/CRO_0000100"/>
        <owl:annotatedProperty rdf:resource="http://purl.obolibrary.org/obo/IAO_0000115"/>
        <owl:annotatedTarget>Oral presentation intended to present information or teach people about a particular subject, such as a talk or poster presentation at a conference.</owl:annotatedTarget>
        <obo:IAO_0000119>https://www.wikidata.org/wiki/Q603773</obo:IAO_0000119>
    </owl:Axiom>
    


    <!-- http://purl.obolibrary.org/obo/CRO_0000101 -->

    <owl:Class rdf:about="http://purl.obolibrary.org/obo/CRO_0000101">
        <rdfs:subClassOf rdf:resource="http://purl.obolibrary.org/obo/CRO_0000000"/>
        <obo:IAO_0000115>Evaluation of scientific, academic, or professional work, such as manuscripts or grants by others working in the same field.</obo:IAO_0000115>
        <obo:IAO_0000118>manuscript review role</obo:IAO_0000118>
        <oboInOwl:created_by rdf:resource="http://orcid.org/0000-0001-5208-3432"/>
        <rdfs:label>peer review role</rdfs:label>
    </owl:Class>
    <owl:Axiom>
        <owl:annotatedSource rdf:resource="http://purl.obolibrary.org/obo/CRO_0000101"/>
        <owl:annotatedProperty rdf:resource="http://purl.obolibrary.org/obo/IAO_0000115"/>
        <owl:annotatedTarget>Evaluation of scientific, academic, or professional work, such as manuscripts or grants by others working in the same field.</owl:annotatedTarget>
        <obo:IAO_0000119>https://www.lexico.com/en/definition/peer_review</obo:IAO_0000119>
    </owl:Axiom>
    


    <!-- http://purl.obolibrary.org/obo/CRO_0000102 -->

    <owl:Class rdf:about="http://purl.obolibrary.org/obo/CRO_0000102">
        <rdfs:subClassOf rdf:resource="http://purl.obolibrary.org/obo/CRO_0000000"/>
        <obo:IAO_0000115>A role that involves giving advice in a particular field.</obo:IAO_0000115>
        <obo:IAO_0000234>https://orcid.org/0000-0001-8420-5254</obo:IAO_0000234>
        <oboInOwl:created_by rdf:resource="http://orcid.org/0000-0001-5208-3432"/>
        <rdfs:label>advisory role</rdfs:label>
    </owl:Class>
    <owl:Axiom>
        <owl:annotatedSource rdf:resource="http://purl.obolibrary.org/obo/CRO_0000102"/>
        <owl:annotatedProperty rdf:resource="http://www.w3.org/2000/01/rdf-schema#label"/>
        <owl:annotatedTarget>advisory role</owl:annotatedTarget>
        <obo:IAO_0000119>https://www.lexico.com/en/definition/adviser</obo:IAO_0000119>
    </owl:Axiom>
    


    <!-- http://purl.obolibrary.org/obo/CRO_0000103 -->

    <owl:Class rdf:about="http://purl.obolibrary.org/obo/CRO_0000103">
        <rdfs:subClassOf rdf:resource="http://purl.obolibrary.org/obo/CRO_0000000"/>
        <obo:IAO_0000115>A role that is realized through the modification of an existing artifact (e.g. adding or removing content to/from a document, updating information in a data record, fixing errors in a manuscript, etc.)</obo:IAO_0000115>
        <obo:IAO_0000118>updater role</obo:IAO_0000118>
        <obo:IAO_0000234>https://orcid.org/0000-0002-1048-5019</obo:IAO_0000234>
        <oboInOwl:created_by rdf:resource="http://orcid.org/0000-0001-5208-3432"/>
        <rdfs:comment>The nature of a modification will vary depending on the type of artifact being modified, and more specific terms may exist in the CRO to describe certain types of modification.</rdfs:comment>
        <rdfs:label>modifier role</rdfs:label>
    </owl:Class>
    <owl:Axiom>
        <owl:annotatedSource rdf:resource="http://purl.obolibrary.org/obo/CRO_0000103"/>
        <owl:annotatedProperty rdf:resource="http://purl.obolibrary.org/obo/IAO_0000115"/>
        <owl:annotatedTarget>A role that is realized through the modification of an existing artifact (e.g. adding or removing content to/from a document, updating information in a data record, fixing errors in a manuscript, etc.)</owl:annotatedTarget>
        <obo:IAO_0000119>https://orcid.org/0000-0002-1048-5019</obo:IAO_0000119>
    </owl:Axiom>
    


    <!-- http://purl.obolibrary.org/obo/CRO_0000104 -->

    <owl:Class rdf:about="http://purl.obolibrary.org/obo/CRO_0000104">
        <rdfs:subClassOf rdf:resource="http://purl.obolibrary.org/obo/CRO_0000000"/>
        <obo:IAO_0000115>A role that is realized through the act of formally accepting an artifact for inclusion in some larger resource (e.g. database, registry, collection, etc.)</obo:IAO_0000115>
        <obo:IAO_0000234>https://orcid.org/0000-0002-1048-5019</obo:IAO_0000234>
        <oboInOwl:created_by rdf:resource="http://orcid.org/0000-0001-5208-3432"/>
        <rdfs:comment>An agent accepting an artifact possesses the authority to decide if it belongs in a particular resource or collection. This agent may or may not also have directly evaluated it themselves - but if they did, an &apos;evaluator role&apos; could additionally be captured.</rdfs:comment>
        <rdfs:label>acceptor role</rdfs:label>
    </owl:Class>
    <owl:Axiom>
        <owl:annotatedSource rdf:resource="http://purl.obolibrary.org/obo/CRO_0000104"/>
        <owl:annotatedProperty rdf:resource="http://purl.obolibrary.org/obo/IAO_0000115"/>
        <owl:annotatedTarget>A role that is realized through the act of formally accepting an artifact for inclusion in some larger resource (e.g. database, registry, collection, etc.)</owl:annotatedTarget>
        <obo:IAO_0000119>https://orcid.org/0000-0002-1048-5019</obo:IAO_0000119>
    </owl:Axiom>
    


    <!-- http://purl.obolibrary.org/obo/CRO_0000105 -->

    <owl:Class rdf:about="http://purl.obolibrary.org/obo/CRO_0000105">
        <rdfs:subClassOf rdf:resource="http://purl.obolibrary.org/obo/CRO_0000000"/>
        <obo:IAO_0000115>A role that is realized through the act of formally submitting or depositing an artifact to be included in some larger resource (e.g. database, registry, collection, etc.)</obo:IAO_0000115>
        <obo:IAO_0000118>depositor role</obo:IAO_0000118>
        <obo:IAO_0000234>https://orcid.org/0000-0002-1048-5019</obo:IAO_0000234>
        <oboInOwl:created_by rdf:resource="http://orcid.org/0000-0001-5208-3432"/>
        <rdfs:comment>An agent submitting an artifact may or may not also have contributed to its creation. If they did, and additional ‘creator role’ can be applied.</rdfs:comment>
        <rdfs:label>submitter role</rdfs:label>
    </owl:Class>
    <owl:Axiom>
        <owl:annotatedSource rdf:resource="http://purl.obolibrary.org/obo/CRO_0000105"/>
        <owl:annotatedProperty rdf:resource="http://purl.obolibrary.org/obo/IAO_0000115"/>
        <owl:annotatedTarget>A role that is realized through the act of formally submitting or depositing an artifact to be included in some larger resource (e.g. database, registry, collection, etc.)</owl:annotatedTarget>
        <obo:IAO_0000119>https://orcid.org/0000-0002-1048-5019</obo:IAO_0000119>
    </owl:Axiom>
    


    <!-- http://purl.obolibrary.org/obo/CRO_0000106 -->

    <owl:Class rdf:about="http://purl.obolibrary.org/obo/CRO_0000106">
        <rdfs:subClassOf rdf:resource="http://purl.obolibrary.org/obo/CRO_0000078"/>
        <obo:IAO_0000115>A role that is realized through the review and evaluation of an artifact - generally to assess its quality, completeness, relevance, or other characteristics.</obo:IAO_0000115>
        <obo:IAO_0000118>assessor role</obo:IAO_0000118>
        <obo:IAO_0000118>reviewer role</obo:IAO_0000118>
        <obo:IAO_0000234>https://orcid.org/0000-0002-1048-5019</obo:IAO_0000234>
        <oboInOwl:created_by rdf:resource="http://orcid.org/0000-0001-5208-3432"/>
        <rdfs:comment>Evaluating an artifact does not involve modification of the assessed artifact - however the suggestion of alterations can be a separate outcome of an evaluation. If the artifact is modified by the agent during or subsequent to the evaluation, a &apos;modifier role&apos; should additionally be applied.</rdfs:comment>
        <rdfs:label>evaluator role</rdfs:label>
    </owl:Class>
    <owl:Axiom>
        <owl:annotatedSource rdf:resource="http://purl.obolibrary.org/obo/CRO_0000106"/>
        <owl:annotatedProperty rdf:resource="http://purl.obolibrary.org/obo/IAO_0000115"/>
        <owl:annotatedTarget>A role that is realized through the review and evaluation of an artifact - generally to assess its quality, completeness, relevance, or other characteristics.</owl:annotatedTarget>
        <obo:IAO_0000119>https://orcid.org/0000-0002-1048-5019</obo:IAO_0000119>
    </owl:Axiom>
    


    <!-- http://purl.obolibrary.org/obo/CRO_0000107 -->

    <owl:Class rdf:about="http://purl.obolibrary.org/obo/CRO_0000107">
        <rdfs:subClassOf rdf:resource="http://purl.obolibrary.org/obo/CRO_0000023"/>
        <obo:IAO_0000115>A role used to indicate that an agent was the creator of an artifact (i.e. had significant or sole responsibility for its initial generation).</obo:IAO_0000115>
        <obo:IAO_0000234>https://orcid.org/0000-0002-1048-5019</obo:IAO_0000234>
        <oboInOwl:created_by rdf:resource="http://orcid.org/0000-0001-5208-3432"/>
        <rdfs:comment>This is a generic role to be used when a more specific term suitable for the contribution scenario is not available or warranted. For example, the &apos;author role&apos; term describes creator roles for published works, and should be used to describe creation of things like books or journal articles.</rdfs:comment>
        <rdfs:label>creator role</rdfs:label>
    </owl:Class>
    <owl:Axiom>
        <owl:annotatedSource rdf:resource="http://purl.obolibrary.org/obo/CRO_0000107"/>
        <owl:annotatedProperty rdf:resource="http://purl.obolibrary.org/obo/IAO_0000115"/>
        <owl:annotatedTarget>A role used to indicate that an agent was the creator of an artifact (i.e. had significant or sole responsibility for its initial generation).</owl:annotatedTarget>
        <obo:IAO_0000119>https://orcid.org/0000-0002-1048-5019</obo:IAO_0000119>
    </owl:Axiom>
    


    <!-- http://purl.obolibrary.org/obo/CRO_0000108 -->

    <owl:Class rdf:about="http://purl.obolibrary.org/obo/CRO_0000108">
        <rdfs:subClassOf rdf:resource="http://purl.obolibrary.org/obo/CRO_0000015"/>
        <obo:IAO_0000115>A role that involves creation, maintenance or administration of a database.</obo:IAO_0000115>
        <obo:IAO_0000234>https://orcid.org/0000-0001-8420-5254</obo:IAO_0000234>
        <oboInOwl:created_by rdf:resource="http://orcid.org/0000-0001-5208-3432"/>
        <rdfs:label>database role</rdfs:label>
    </owl:Class>
    


    <!-- http://purl.obolibrary.org/obo/CRO_0000110 -->

    <owl:Class rdf:about="http://purl.obolibrary.org/obo/CRO_0000110">
        <rdfs:subClassOf rdf:resource="http://purl.org/credit/ontology#CREDIT_00000005"/>
        <obo:IAO_0000234>https://orcid.org/0000-0001-8420-5254</obo:IAO_0000234>
        <oboInOwl:created_by rdf:resource="http://orcid.org/0000-0001-5208-3432"/>
        <rdfs:label>community research partner</rdfs:label>
    </owl:Class>
    


    <!-- http://purl.obolibrary.org/obo/CRO_0000111 -->

    <owl:Class rdf:about="http://purl.obolibrary.org/obo/CRO_0000111">
        <rdfs:subClassOf rdf:resource="http://purl.obolibrary.org/obo/CRO_0000000"/>
        <obo:IAO_0000115>A person who deals with provision and maintenance of information in many formats, including: books; electronic resources; magazines; newspapers; audio and video recordings; maps; manuscripts; photographs and other graphic material; bibliographic databases; and web-based and digital resources. A librarian may also provide other information services, including: information literacy instruction; computer provision and training; coordination with community groups to host public programs; assistive technology for people with disabilities; and assistance locating community resources. Librarians often work in a library, but can also work in other physical settings or virtual environments.</obo:IAO_0000115>
        <obo:IAO_0000234>https://orcid.org/0000-0001-8420-5254</obo:IAO_0000234>
        <oboInOwl:created_by rdf:resource="http://orcid.org/0000-0001-5208-3432"/>
        <rdfs:label>librarian role</rdfs:label>
    </owl:Class>
    <owl:Axiom>
        <owl:annotatedSource rdf:resource="http://purl.obolibrary.org/obo/CRO_0000111"/>
        <owl:annotatedProperty rdf:resource="http://purl.obolibrary.org/obo/IAO_0000115"/>
        <owl:annotatedTarget>A person who deals with provision and maintenance of information in many formats, including: books; electronic resources; magazines; newspapers; audio and video recordings; maps; manuscripts; photographs and other graphic material; bibliographic databases; and web-based and digital resources. A librarian may also provide other information services, including: information literacy instruction; computer provision and training; coordination with community groups to host public programs; assistive technology for people with disabilities; and assistance locating community resources. Librarians often work in a library, but can also work in other physical settings or virtual environments.</owl:annotatedTarget>
        <obo:IAO_0000119>https://en.wikipedia.org/wiki/Librarian</obo:IAO_0000119>
    </owl:Axiom>
    


    <!-- http://purl.obolibrary.org/obo/IAO_0000027 -->

    <rdf:Description rdf:about="http://purl.obolibrary.org/obo/IAO_0000027">
        <rdfs:subClassOf rdf:resource="http://purl.obolibrary.org/obo/IAO_0000030"/>
    </rdf:Description>
    


    <!-- http://purl.obolibrary.org/obo/IAO_0000030 -->

    <rdf:Description rdf:about="http://purl.obolibrary.org/obo/IAO_0000030">
        <rdfs:subClassOf rdf:resource="http://purl.obolibrary.org/obo/BFO_0000031"/>
    </rdf:Description>
    


    <!-- http://purl.obolibrary.org/obo/IAO_0000078 -->

    <rdf:Description rdf:about="http://purl.obolibrary.org/obo/IAO_0000078">
        <rdfs:subClassOf rdf:resource="http://purl.obolibrary.org/obo/IAO_0000102"/>
    </rdf:Description>
    


    <!-- http://purl.obolibrary.org/obo/IAO_0000102 -->

    <rdf:Description rdf:about="http://purl.obolibrary.org/obo/IAO_0000102">
        <rdfs:subClassOf rdf:resource="http://purl.obolibrary.org/obo/IAO_0000027"/>
    </rdf:Description>
    


    <!-- http://purl.obolibrary.org/obo/IAO_0000225 -->

    <rdf:Description rdf:about="http://purl.obolibrary.org/obo/IAO_0000225">
        <rdfs:subClassOf rdf:resource="http://purl.obolibrary.org/obo/IAO_0000102"/>
    </rdf:Description>
    


    <!-- http://purl.obolibrary.org/obo/IAO_0000409 -->

    <rdf:Description rdf:about="http://purl.obolibrary.org/obo/IAO_0000409">
        <rdfs:subClassOf rdf:resource="http://purl.obolibrary.org/obo/IAO_0000102"/>
    </rdf:Description>
    


    <!-- http://purl.org/credit/ontology#CREDIT_00000001 -->

    <owl:Class rdf:about="http://purl.org/credit/ontology#CREDIT_00000001">
        <rdfs:subClassOf rdf:resource="http://purl.obolibrary.org/obo/CRO_0000000"/>
        <obo:IAO_0000118>research conceptualization role</obo:IAO_0000118>
        <obo:IAO_0000412>http://purl.org/credit/ontology</obo:IAO_0000412>
    </owl:Class>
    


    <!-- http://purl.org/credit/ontology#CREDIT_00000002 -->

    <owl:Class rdf:about="http://purl.org/credit/ontology#CREDIT_00000002">
        <rdfs:subClassOf rdf:resource="http://purl.obolibrary.org/obo/CRO_0000015"/>
        <obo:IAO_0000412>http://purl.org/credit/ontology</obo:IAO_0000412>
    </owl:Class>
    


    <!-- http://purl.org/credit/ontology#CREDIT_00000003 -->

    <owl:Class rdf:about="http://purl.org/credit/ontology#CREDIT_00000003">
        <rdfs:subClassOf rdf:resource="http://purl.obolibrary.org/obo/CRO_0000000"/>
        <obo:IAO_0000118>data analysis role</obo:IAO_0000118>
        <obo:IAO_0000412>http://purl.org/credit/ontology</obo:IAO_0000412>
    </owl:Class>
    


    <!-- http://purl.org/credit/ontology#CREDIT_00000004 -->

    <rdf:Description rdf:about="http://purl.org/credit/ontology#CREDIT_00000004">
        <rdfs:subClassOf rdf:resource="http://purl.obolibrary.org/obo/CRO_0000000"/>
        <obo:IAO_0000118>grant acquisition role</obo:IAO_0000118>
        <obo:IAO_0000412>http://purl.org/credit/ontology</obo:IAO_0000412>
    </rdf:Description>
    


    <!-- http://purl.org/credit/ontology#CREDIT_00000005 -->

    <owl:Class rdf:about="http://purl.org/credit/ontology#CREDIT_00000005">
        <rdfs:subClassOf rdf:resource="http://purl.obolibrary.org/obo/CRO_0000000"/>
        <obo:IAO_0000412>http://purl.org/credit/ontology</obo:IAO_0000412>
    </owl:Class>
    


    <!-- http://purl.org/credit/ontology#CREDIT_00000006 -->

    <owl:Class rdf:about="http://purl.org/credit/ontology#CREDIT_00000006">
        <rdfs:subClassOf rdf:resource="http://purl.obolibrary.org/obo/CRO_0000000"/>
        <obo:IAO_0000412>http://purl.org/credit/ontology</obo:IAO_0000412>
    </owl:Class>
    


    <!-- http://purl.org/credit/ontology#CREDIT_00000007 -->

    <rdf:Description rdf:about="http://purl.org/credit/ontology#CREDIT_00000007">
        <rdfs:subClassOf rdf:resource="http://purl.obolibrary.org/obo/CRO_0000000"/>
        <obo:IAO_0000118>program administration role</obo:IAO_0000118>
        <obo:IAO_0000412>http://purl.org/credit/ontology</obo:IAO_0000412>
    </rdf:Description>
    


    <!-- http://purl.org/credit/ontology#CREDIT_00000008 -->

    <rdf:Description rdf:about="http://purl.org/credit/ontology#CREDIT_00000008">
        <rdfs:subClassOf rdf:resource="http://purl.obolibrary.org/obo/CRO_0000000"/>
        <obo:IAO_0000118>resource provision role</obo:IAO_0000118>
        <obo:IAO_0000412>http://purl.org/credit/ontology</obo:IAO_0000412>
    </rdf:Description>
    


    <!-- http://purl.org/credit/ontology#CREDIT_00000009 -->

    <owl:Class rdf:about="http://purl.org/credit/ontology#CREDIT_00000009">
        <rdfs:subClassOf rdf:resource="http://purl.obolibrary.org/obo/CRO_0000000"/>
        <obo:IAO_0000118>software systems role</obo:IAO_0000118>
        <obo:IAO_0000412>http://purl.org/credit/ontology</obo:IAO_0000412>
    </owl:Class>
    


    <!-- http://purl.org/credit/ontology#CREDIT_00000010 -->

    <rdf:Description rdf:about="http://purl.org/credit/ontology#CREDIT_00000010">
        <rdfs:subClassOf rdf:resource="http://purl.obolibrary.org/obo/CRO_0000000"/>
        <obo:IAO_0000118>supervisory role</obo:IAO_0000118>
        <obo:IAO_0000412>http://purl.org/credit/ontology</obo:IAO_0000412>
    </rdf:Description>
    


    <!-- http://purl.org/credit/ontology#CREDIT_00000011 -->

    <rdf:Description rdf:about="http://purl.org/credit/ontology#CREDIT_00000011">
        <rdfs:subClassOf rdf:resource="http://purl.obolibrary.org/obo/CRO_0000000"/>
        <obo:IAO_0000412>http://purl.org/credit/ontology</obo:IAO_0000412>
    </rdf:Description>
    


    <!-- http://purl.org/credit/ontology#CREDIT_00000012 -->

    <rdf:Description rdf:about="http://purl.org/credit/ontology#CREDIT_00000012">
        <rdfs:subClassOf rdf:resource="http://purl.obolibrary.org/obo/CRO_0000000"/>
        <obo:IAO_0000412>http://purl.org/credit/ontology</obo:IAO_0000412>
    </rdf:Description>
    


    <!-- http://purl.org/credit/ontology#CREDIT_00000013 -->

    <owl:Class rdf:about="http://purl.org/credit/ontology#CREDIT_00000013">
        <rdfs:subClassOf rdf:resource="http://purl.obolibrary.org/obo/CRO_0000001"/>
        <obo:IAO_0000118>original draft preparation role</obo:IAO_0000118>
        <obo:IAO_0000412>http://purl.org/credit/ontology</obo:IAO_0000412>
    </owl:Class>
    


    <!-- http://purl.org/credit/ontology#CREDIT_00000014 -->

    <rdf:Description rdf:about="http://purl.org/credit/ontology#CREDIT_00000014">
        <rdfs:subClassOf rdf:resource="http://purl.obolibrary.org/obo/CRO_0000001"/>
        <obo:IAO_0000412>http://purl.org/credit/ontology</obo:IAO_0000412>
    </rdf:Description>
    


    <!-- http://www.geneontology.org/formats/oboInOwl#Subset -->

    <rdf:Description rdf:about="http://www.geneontology.org/formats/oboInOwl#Subset">
        <rdfs:subClassOf rdf:resource="http://purl.obolibrary.org/obo/IAO_0000102"/>
    </rdf:Description>
</rdf:RDF>



<!-- Generated by the OWL API (version 4.5.6) https://github.com/owlcs/owlapi -->

