<?xml version="1.0"?>
<rdf:RDF xmlns="http://opendata.aragon.es/def/ei2a#"
     xml:base="http://opendata.aragon.es/def/ei2a"
     xmlns:schema="http://schema.org/"
     xmlns:owl="http://www.w3.org/2002/07/owl#"
     xmlns:ns="http://creativecommons.org/ns#"
     xmlns:org="http://www.w3.org/ns/org#"
     xmlns:powder-s="http://www.w3.org/2007/05/powder-s#"
     xmlns:xsd="http://www.w3.org/2001/XMLSchema#"
     xmlns:voaf="http://purl.org/vocommons/voaf#"
     xmlns:skos="http://www.w3.org/2004/02/skos/core#"
     xmlns:gtfs="http://vocab.gtfs.org/terms#"
     xmlns:rdfs="http://www.w3.org/2000/01/rdf-schema#"
     xmlns:rdf="http://www.w3.org/1999/02/22-rdf-syntax-ns#"
     xmlns:terms="http://purl.org/dc/terms/"
     xmlns:xml="http://www.w3.org/XML/1998/namespace"
     xmlns:wgs84_pos="http://www.w3.org/2003/01/geo/wgs84_pos#"
     xmlns:rec54="http://www.w3.org/2001/02pd/rec54#"
     xmlns:locn="http://www.w3.org/ns/locn#"
     xmlns:dcat="http://www.w3.org/ns/dcat#"
     xmlns:vann="http://purl.org/vocab/vann/"
     xmlns:ei2a="http://opendata.aragon.es/def/ei2a#"
     xmlns:foaf="http://xmlns.com/foaf/0.1/"
     xmlns:status="http://www.w3.org/2003/06/sw-vocab-status/ns#"
     xmlns:dc="http://purl.org/dc/elements/1.1/">
    <owl:Ontology rdf:about="http://opendata.aragon.es/def/ei2a">
        <owl:imports rdf:resource="http://www.w3.org/ns/locn"/>
        <owl:imports rdf:resource="http://purl.org/NET/c4dm/event.owl"/>
        <owl:imports rdf:resource="http://www.w3.org/ns/person"/>
        <owl:imports rdf:resource="http://www.w3.org/ns/org#"/>
        <owl:imports rdf:resource="http://opendata.aragon.es/def/ei2a/categorization"/>
        <terms:contributor xml:lang="es">DEPARTAMENTO DE EDUCACIÓN, CULTURA Y DEPORTE (Gobierno de Aragón): V, Coronas, R. Perales</terms:contributor>
        <terms:contributor xml:lang="es">DEPARTAMENTO DE INNOVACIÓN, INVESTIGACIÓN Y UNIVERSIDAD (AST, Government of Aragon): N. Porta, O. A. Torrero</terms:contributor>
        <terms:contributor xml:lang="es">DEPARTAMENTO DE SANIDAD (Gobierno de Aragón): F. J. Martón</terms:contributor>
        <terms:rights xml:lang="es">Trabajo bajo licencia Creative Commons Attribution-ShareAlike 4.0 International.</terms:rights>
        <terms:contributor xml:lang="en">DEPARTMENT OF RURAL DEVELOPMENT AND SUSTAINABILITY (Government of Aragon): J. Borque</terms:contributor>
        <terms:creator xml:lang="en">V. Rodrigálvarez (Technological Institute of Aragon, ITAINNOVA)</terms:creator>
        <terms:contributor xml:lang="es">DEPARTAMENTO DE ECONOMÍA, INDUSTRIA Y EMPLEO (INAEM, Gobierno de Aragón): J. Masa</terms:contributor>
        <terms:creator xml:lang="en">I. Alonso (Electronic Administration and Information Society, Government of Aragon)</terms:creator>
        <terms:contributor xml:lang="en">E. Meléndez (Technological Institute of Aragon, ITAINNOVA)</terms:contributor>
        <terms:creator xml:lang="en">J.M. Subero (Electronic Administration and Information Society, Government of Aragon)</terms:creator>
        <terms:contributor xml:lang="es">DEPARTMENTO DE HACIENDA Y ADMINISTRACIÓN PÚBLICA (Gobierno de Aragón): M. J.  Segura, T. Royo, J. Moyano</terms:contributor>
        <terms:creator xml:lang="es">J.M. Subero (Administración electrónica y Sociedad de la Información, Gobierno de Aragón)</terms:creator>
        <terms:contributor xml:lang="en">DEPARTMENT OF VERTEBRATION OF THE TERRITORY, MOBILITY AND HOUSING (IGEAR, Government of Aragon): F. López, S. Monteagudo, R. Martínez</terms:contributor>
        <terms:creator xml:lang="es">I. Alonso (Administración electrónica y Sociedad de la Información, Gobierno de Aragón)</terms:creator>
        <terms:contributor xml:lang="en">DEPARTAMENT OF INNOVATION, RESEARCH AND UNIVERSITY (AST, Government of Aragon): N. Porta, O. A. Torrero</terms:contributor>
        <terms:creator xml:lang="es">V. Rodrigálvarez (Instituto Tecnológico de Aragón, ITAINNOVA)</terms:creator>
        <owl:versionInfo xml:lang="en">1.2.0</owl:versionInfo>
        <terms:contributor xml:lang="en">DEPARTMENT OF CITIZENSHIP AND SOCIAL RIGHTS (IASS, Government of Aragon): S. Sánchez, J. A. Ramiro</terms:contributor>
        <rdfs:label xml:lang="es">Ontología Estructura de Información Interoperable de Aragón
EI2A</rdfs:label>
        <owl:versionInfo xml:lang="es">1.2.0</owl:versionInfo>
        <terms:contributor xml:lang="es">DEPARTAMENTO DE DESARROLLO RURAL Y SOSTENIBILIDAD (Gobierno de Aragón): J. Borque</terms:contributor>
        <terms:contributor xml:lang="en">DEPARTMENT OF HEALTH (Government of Aragon): F. J. Martón</terms:contributor>
        <terms:contributor xml:lang="es">INSTITUTO ARAGONÉS DE GESTIÓN AMBIENTAL (INAGA, Gobierno de Aragón): M. Zapata, R. Doñate</terms:contributor>
	 <terms:contributor xml:lang="es">GNOSS: E. Sota, J. Valer, S. López</terms:contributor>
 	 <terms:contributor xml:lang="en">GNOSS: E. Sota, J. Valer, S. López</terms:contributor>

        <rdfs:comment xml:lang="es">La iniciativa Aragón Open Data se inició por Acuerdo de 17 de julio de 2012 del Gobierno de Aragón. En virtud del mismo se ordenó el inicio del proyecto de apertura de datos públicos y el 6 de febrero de 2013 se implantó a través del Portal &lt;a href=&quot;http://opendata.aragon.es/&quot;&gt;opendata.aragon.es&lt;/a&gt;.

A lo largo de este tiempo se han realizado numerosos trabajos para conseguir la automatización en la publicación de la información para asegurar que terceros puedan reutilizarla de la mejor manera. Dado el volumen de datos que empieza a existir, dentro de la línea de trabajo de la automatización en la gestión de la información, están empezando a tener una especial relevancia todos aquellos elementos que ayuden en la mejora de la &lt;b&gt;estructuración de la información&lt;/b&gt; y en la &lt;b&gt;estandarización de los datos &lt;/b&gt;que contienen las bases de datos.

En base a esto, dentro de la Dirección General de Administración Electrónica y Sociedad de la Información, surge la idea de generar un conjunto de reglas técnicas y legales que permitan profundizar en esa estandarización y que llevan a pensar en la creación del Esquema de Información Interoperable de Aragón (E2IA). El E2IA surge así como el marco en el que los datos abiertos y en general la información del Gobierno de Aragón pueden comenzar a automatizarse de una manera mucho más profunda. El E2IA ha de contar con una serie de elementos técnicos, organizativos y legales que es necesario desarrollar. 

Por ello, se ha encomendado al Instituto Tecnológico de Aragón (ITAINNOVA) llevar a cabo actuaciones consistentes en identificar, estudiar y analizar las tendencias de investigación actuales y desarrollo tecnológico en relación a ontologías y diccionarios de interoperabilidad de datos, definir la propuesta ontológica, realizar las pruebas necesarias para validar la propuesta ontológica y generar las versiones texto y web de la ontología.</rdfs:comment>
        <terms:contributor xml:lang="en">DEPARTMENT OF INNOVATION, RESEARCH AND UNIVERSITY (Electronic Administration and Information Society, Government of Aragon): M. A. Lozano, E. Nuez</terms:contributor>
        <terms:contributor xml:lang="en">DEPARTMENT OF HACIENDA AND PUBLIC ADMINISTRATION (Government of Aragon): M. J. Segura, T. Royo, J. Moyano</terms:contributor>
        <terms:rights xml:lang="en">This work is licensed under a Creative Commons Attribution-ShareAlike 4.0 International.</terms:rights>
        <terms:contributor xml:lang="en">ARAGONÉS INSTITUTE OF ENVIRONMENTAL MANAGEMENT (INAGA, Government of Aragon): M. Zapata, R. Doñate</terms:contributor>
        <rdfs:comment xml:lang="en">The initiative Aragón Open Data was initiated by agreement of 17 of July of 2012 of the Government of Aragon. Under the same was ordered the start of the project to open public data and on February 6, 2013 was implemented through the Portal &lt;a href=&quot;http://opendata.aragon.es/&quot;&gt; opendata.aragon.es &lt;/a&gt;.

Throughout this time there have been numerous works to achieve automation in the publication of information to ensure that third parties can reuse it in the best way. Given the volume of data that begins to exist, within the line of work of automation in information management, all those elements that help in the improvement of the &lt;b&gt; structuring of information &lt;/b&gt;  and the &lt;b&gt; standardization of the data &lt;/b&gt; contained in the databases are beginning to have a special relevance.

Based on this, within the General Directorate of Electronic Administration and Information Society, the idea arises of generating a set of technical and legal rules that allow to deepen in that standardization and that lead to think in the creation of the Interoperable Information Scheme Of Aragon (E2IA). The E2IA thus emerges as the framework in which the open data and in general the information of the Government of Aragon can begin to be automated in a much more profound way. The E2IA has to have a number of technical, organizational and legal elements that need to be developed.

For this reason, the Technological Institute of Aragon (ITAINNOVA) has been entrusted with carrying out actions consisting in identifying, studying and analyzing current research trends and technological development in relation to ontologies and dictionaries of data interoperability, defining the ontological proposal, performing The necessary tests to validate the ontological proposal and generate the text and web versions of the ontology.</rdfs:comment>
        <terms:creator xml:lang="es">P. Peña (Instituto Tecnológico de Aragón, ITAINNOVA)</terms:creator>
        <rdfs:label xml:lang="en">Aragon Interoperable Information Structure Ontology
EI2A</rdfs:label>
        <terms:contributor xml:lang="es">E. Meléndez (Instituto Tecnológico de Aragón, ITAINNOVA)</terms:contributor>
        <terms:creator xml:lang="en">P. Peña (Technological Institute of Aragon, ITAINNOVA)</terms:creator>
        <terms:contributor xml:lang="es">DEPARTAMENTO DE CIUDADANÍA Y DERECHOS SOCIALES (IASS, Gobierno de Aragón): S.  Sánchez , J. A. Ramiro</terms:contributor>
        <terms:contributor xml:lang="es">DEPARTAMENTO DE VERTEBRACIÓN DEL TERRITORIO, MOVILIDAD Y VIVIENDA  (IGEAR, Gobierno de Aragón): F. López ,S.  Monteagudo, R. Martínez</terms:contributor>
        <terms:contributor xml:lang="en">DEPARTMENT OF ECONOMY, INDUSTRY AND EMPLOYMENT (INAEM, Government of Aragon): J. Masa</terms:contributor>
        <terms:contributor xml:lang="en">DEPARTMENT OF EDUCATION, CULTURE AND SPORTS (Government of Aragon): V, Coronas, R. Perales</terms:contributor>
        <terms:contributor xml:lang="es">DEPARTAMENTO DE INNOVACIÓN, INVESTIGACIÓN Y UNIVERSIDAD (Administración electrónica y Sociedad de la Información, Gobierno de Aragón):  M. A.  Lozano, E. Nuez</terms:contributor>
    </owl:Ontology>
    


    <!-- 
    ///////////////////////////////////////////////////////////////////////////////////////
    //
    // Annotation properties
    //
    ///////////////////////////////////////////////////////////////////////////////////////
     -->

    


    <!-- http://opendata.aragon.es/def/ei2a#alignedWithIFC -->

    <owl:AnnotationProperty rdf:about="http://opendata.aragon.es/def/ei2a#alignedWithIFC"/>
    


    <!-- http://opendata.aragon.es/def/ei2a#alignedWithInspire -->

    <owl:AnnotationProperty rdf:about="http://opendata.aragon.es/def/ei2a#alignedWithInspire"/>
    


    <!-- http://opendata.aragon.es/def/ei2a#alignedWithSaref -->

    <owl:AnnotationProperty rdf:about="http://opendata.aragon.es/def/ei2a#alignedWithSaref"/>
    


    <!-- http://opendata.aragon.es/def/ei2a#alignedWithWatERP -->

    <owl:AnnotationProperty rdf:about="http://opendata.aragon.es/def/ei2a#alignedWithWatERP"/>
    


    <!-- http://opendata.aragon.es/def/ei2a#comment -->

    <owl:AnnotationProperty rdf:about="http://opendata.aragon.es/def/ei2a#comment"/>
    


    <!-- http://opendata.aragon.es/def/ei2a#X -->

    <owl:AnnotationProperty rdf:about="http://opendata.aragon.es/def/ei2a#X">
        <rdfs:comment xml:lang="es">Coordenada X. Propiedad que debe seguir la especificación de datos del sistema de referencia.</rdfs:comment>
        <rdfs:comment xml:lang="en">Coordinate X. Property that must follow the data specification of the reference system.</rdfs:comment>
        <rdfs:label>X</rdfs:label>
        <rdfs:range rdf:resource="http://www.w3.org/2001/XMLSchema#float"/>
        <rdfs:domain rdf:resource="http://www.w3.org/2003/01/geo/wgs84_pos#SpatialThing"/>
    </owl:AnnotationProperty>
    


    <!-- http://opendata.aragon.es/def/ei2a#Y -->

    <owl:AnnotationProperty rdf:about="http://opendata.aragon.es/def/ei2a#Y">
        <rdfs:comment xml:lang="es">Coordenada Y. Propiedad que debe seguir la especificación de datos del sistema de referencia.</rdfs:comment>
        <rdfs:comment xml:lang="en">Coordinate Y. Property that must follow the data specification of the reference system.</rdfs:comment>
        <rdfs:label>Y</rdfs:label>
        <rdfs:range rdf:resource="http://www.w3.org/2001/XMLSchema#float"/>
        <rdfs:domain rdf:resource="http://www.w3.org/2003/01/geo/wgs84_pos#SpatialThing"/>
    </owl:AnnotationProperty>
    


    <!-- http://opendata.aragon.es/def/ei2a#Z -->

    <owl:AnnotationProperty rdf:about="http://opendata.aragon.es/def/ei2a#Z">
        <rdfs:comment xml:lang="es">Coordenada Z. Propiedad que debe seguir la especificación de datos del sistema de referencia.</rdfs:comment>
        <rdfs:comment xml:lang="en">Coordinate Z. Property that must follow the data specification of the reference system.</rdfs:comment>
        <rdfs:label>Z</rdfs:label>
        <rdfs:range rdf:resource="http://www.w3.org/2001/XMLSchema#float"/>
        <rdfs:domain rdf:resource="http://www.w3.org/2003/01/geo/wgs84_pos#SpatialThing"/>
    </owl:AnnotationProperty>
    


    <!-- http://purl.org/dc/elements/1.1/source -->

    <owl:AnnotationProperty rdf:about="http://purl.org/dc/elements/1.1/source"/>
    


    <!-- http://purl.org/dc/terms/comment -->

    <owl:AnnotationProperty rdf:about="http://purl.org/dc/terms/comment"/>
    


    <!-- http://purl.org/dc/terms/description -->

    <owl:AnnotationProperty rdf:about="http://purl.org/dc/terms/description"/>
    


    <!-- http://purl.org/dc/terms/source -->

    <owl:AnnotationProperty rdf:about="http://purl.org/dc/terms/source">
        <rdfs:comment xml:lang="en">A related resource from which the described resource is derived</rdfs:comment>
        <rdfs:comment xml:lang="es">Recurso relacionado del cual se deriva el recurso descrito</rdfs:comment>
    </owl:AnnotationProperty>
    


    <!-- http://vocab.gtfs.org/terms#longName -->

    <owl:AnnotationProperty rdf:about="http://vocab.gtfs.org/terms#longName">
        <rdfs:comment xml:lang="en">Long name given to a route</rdfs:comment>
        <rdfs:comment xml:lang="es">Nombre completo de una ruta</rdfs:comment>
        <rdfs:label xml:lang="en">Long name</rdfs:label>
        <rdfs:label xml:lang="es">nombre completo</rdfs:label>
        <rdfs:seeAlso rdf:resource="https://developers.google.com/transit/gtfs/examples/display-to-users#RouteLongName"/>
        <status:term_status xml:lang="es">inestable</status:term_status>
        <status:term_status xml:lang="en">unstable</status:term_status>
        <rdfs:subPropertyOf rdf:resource="http://purl.org/dc/terms/title"/>
        <rdfs:domain rdf:resource="http://vocab.gtfs.org/terms#Route"/>
    </owl:AnnotationProperty>
    


    <!-- http://vocab.gtfs.org/terms#shortName -->

    <owl:AnnotationProperty rdf:about="http://vocab.gtfs.org/terms#shortName">
        <rdfs:comment xml:lang="es">Nombre corto dado a una ruta o viaje</rdfs:comment>
        <rdfs:comment xml:lang="en">Short name given to a route or a trip</rdfs:comment>
        <rdfs:label xml:lang="en">Short name</rdfs:label>
        <rdfs:label xml:lang="es">nombre corto</rdfs:label>
        <rdfs:seeAlso rdf:resource="https://developers.google.com/transit/gtfs/examples/display-to-users#RouteShortName"/>
        <status:term_status xml:lang="es">inestable</status:term_status>
        <status:term_status xml:lang="en">unstable</status:term_status>
        <rdfs:subPropertyOf rdf:resource="http://purl.org/dc/terms/title"/>
        <rdfs:domain rdf:resource="http://vocab.gtfs.org/terms#Route"/>
        <rdfs:domain rdf:resource="http://vocab.gtfs.org/terms#Trip"/>
    </owl:AnnotationProperty>
    


    <!-- http://www.w3.org/2003/01/geo/wgs84_pos#alt -->

    <owl:AnnotationProperty rdf:about="http://www.w3.org/2003/01/geo/wgs84_pos#alt">
        <rdfs:comment>The WGS84 altitude of a SpatialThing (decimal meters 
above the local reference ellipsoid).</rdfs:comment>
        <rdfs:label>altitude</rdfs:label>
        <rdfs:range rdf:resource="http://www.w3.org/2001/XMLSchema#float"/>
        <rdfs:domain rdf:resource="http://www.w3.org/2003/01/geo/wgs84_pos#SpatialThing"/>
    </owl:AnnotationProperty>
    


    <!-- http://www.w3.org/2003/01/geo/wgs84_pos#lat -->

    <owl:AnnotationProperty rdf:about="http://www.w3.org/2003/01/geo/wgs84_pos#lat">
        <rdfs:comment>The WGS84 latitude of a SpatialThing (decimal degrees).</rdfs:comment>
        <rdfs:label>latitude</rdfs:label>
        <rdfs:range rdf:resource="http://www.w3.org/2001/XMLSchema#float"/>
        <rdfs:domain rdf:resource="http://www.w3.org/2003/01/geo/wgs84_pos#SpatialThing"/>
    </owl:AnnotationProperty>
    


    <!-- http://www.w3.org/2003/01/geo/wgs84_pos#long -->

    <owl:AnnotationProperty rdf:about="http://www.w3.org/2003/01/geo/wgs84_pos#long">
        <rdfs:comment>The WGS84 longitude of a SpatialThing (decimal degrees).</rdfs:comment>
        <rdfs:label>longitude</rdfs:label>
        <rdfs:range rdf:resource="http://www.w3.org/2001/XMLSchema#float"/>
        <rdfs:domain rdf:resource="http://www.w3.org/2003/01/geo/wgs84_pos#SpatialThing"/>
    </owl:AnnotationProperty>
    


    <!-- http://www.w3.org/ns/dcat#theme -->

    <owl:AnnotationProperty rdf:about="http://www.w3.org/ns/dcat#theme"/>
    


    <!-- http://xmlns.com/foaf/0.1/based_near -->

    <owl:AnnotationProperty rdf:about="http://xmlns.com/foaf/0.1/based_near"/>
    


    <!-- 
    ///////////////////////////////////////////////////////////////////////////////////////
    //
    // Object Properties
    //
    ///////////////////////////////////////////////////////////////////////////////////////
     -->

    


    <!-- http://harmonet.org/harmonise.rdfs#accommodationType -->

    <owl:ObjectProperty rdf:about="http://harmonet.org/harmonise.rdfs#accommodationType">
        <rdfs:domain rdf:resource="http://harmonet.org/harmonise.rdfs#Accommodation"/>
        <rdfs:range rdf:resource="http://harmonet.org/harmonise.rdfs#ListValue"/>
    </owl:ObjectProperty>
    


    <!-- http://harmonet.org/harmonise.rdfs#award -->

    <owl:ObjectProperty rdf:about="http://harmonet.org/harmonise.rdfs#award">
        <rdfs:domain rdf:resource="http://harmonet.org/harmonise.rdfs#Accommodation"/>
        <rdfs:domain rdf:resource="http://harmonet.org/harmonise.rdfs#Attraction"/>
        <rdfs:domain rdf:resource="http://harmonet.org/harmonise.rdfs#Gastro"/>
        <rdfs:range rdf:resource="http://harmonet.org/harmonise.rdfs#Award"/>
    </owl:ObjectProperty>
    


    <!-- http://harmonet.org/harmonise.rdfs#changed -->

    <owl:ObjectProperty rdf:about="http://harmonet.org/harmonise.rdfs#changed">
        <rdfs:domain rdf:resource="http://harmonet.org/harmonise.rdfs#Accommodation"/>
        <rdfs:domain rdf:resource="http://harmonet.org/harmonise.rdfs#Attraction"/>
        <rdfs:domain rdf:resource="http://harmonet.org/harmonise.rdfs#Gastro"/>
        <rdfs:range rdf:resource="http://harmonet.org/harmonise.rdfs#PointOfTime"/>
        <rdfs:label>changed</rdfs:label>
    </owl:ObjectProperty>
    


    <!-- http://harmonet.org/harmonise.rdfs#date -->

    <owl:ObjectProperty rdf:about="http://harmonet.org/harmonise.rdfs#date">
        <rdfs:domain rdf:resource="http://harmonet.org/harmonise.rdfs#PointOfTime"/>
        <rdfs:range rdf:resource="http://harmonet.org/harmonise.rdfs#Date"/>
        <rdfs:label>date</rdfs:label>
    </owl:ObjectProperty>
    


    <!-- http://harmonet.org/harmonise.rdfs#dateRange -->

    <owl:ObjectProperty rdf:about="http://harmonet.org/harmonise.rdfs#dateRange">
        <rdfs:domain rdf:resource="http://harmonet.org/harmonise.rdfs#Timeline"/>
        <rdfs:range rdf:resource="http://harmonet.org/harmonise.rdfs#DateRange"/>
        <rdfs:label>dateRange</rdfs:label>
    </owl:ObjectProperty>
    


    <!-- http://harmonet.org/harmonise.rdfs#endDate -->

    <owl:ObjectProperty rdf:about="http://harmonet.org/harmonise.rdfs#endDate">
        <rdfs:domain rdf:resource="http://harmonet.org/harmonise.rdfs#DateRange"/>
        <rdfs:range rdf:resource="http://harmonet.org/harmonise.rdfs#Date"/>
        <rdfs:label>endDate</rdfs:label>
    </owl:ObjectProperty>
    


    <!-- http://harmonet.org/harmonise.rdfs#facility -->

    <owl:ObjectProperty rdf:about="http://harmonet.org/harmonise.rdfs#facility">
        <rdfs:domain rdf:resource="http://harmonet.org/harmonise.rdfs#Accommodation"/>
        <rdfs:domain rdf:resource="http://harmonet.org/harmonise.rdfs#Attraction"/>
        <rdfs:domain rdf:resource="http://harmonet.org/harmonise.rdfs#Gastro"/>
        <rdfs:range rdf:resource="http://harmonet.org/harmonise.rdfs#Facility"/>
    </owl:ObjectProperty>
    


    <!-- http://harmonet.org/harmonise.rdfs#facilityName -->

    <owl:ObjectProperty rdf:about="http://harmonet.org/harmonise.rdfs#facilityName">
        <rdfs:domain rdf:resource="http://harmonet.org/harmonise.rdfs#Facility"/>
        <rdfs:range rdf:resource="http://harmonet.org/harmonise.rdfs#ListValue"/>
        <rdfs:label>facilityName</rdfs:label>
    </owl:ObjectProperty>
    


    <!-- http://harmonet.org/harmonise.rdfs#gastroType -->

    <owl:ObjectProperty rdf:about="http://harmonet.org/harmonise.rdfs#gastroType">
        <rdfs:domain rdf:resource="http://harmonet.org/harmonise.rdfs#Gastro"/>
        <rdfs:range rdf:resource="http://harmonet.org/harmonise.rdfs#ListValue"/>
    </owl:ObjectProperty>
    


    <!-- http://harmonet.org/harmonise.rdfs#organiser -->

    <owl:ObjectProperty rdf:about="http://harmonet.org/harmonise.rdfs#organiser">
        <rdfs:domain rdf:resource="http://harmonet.org/harmonise.rdfs#Accommodation"/>
        <rdfs:domain rdf:resource="http://harmonet.org/harmonise.rdfs#Attraction"/>
        <rdfs:domain rdf:resource="http://harmonet.org/harmonise.rdfs#Gastro"/>
        <rdfs:range rdf:resource="http://www.w3.org/ns/org#Organization"/>
    </owl:ObjectProperty>
    


    <!-- http://harmonet.org/harmonise.rdfs#profile -->

    <owl:ObjectProperty rdf:about="http://harmonet.org/harmonise.rdfs#profile">
        <rdfs:domain rdf:resource="http://harmonet.org/harmonise.rdfs#Accommodation"/>
        <rdfs:domain rdf:resource="http://harmonet.org/harmonise.rdfs#Attraction"/>
        <rdfs:domain rdf:resource="http://harmonet.org/harmonise.rdfs#Gastro"/>
        <rdfs:range rdf:resource="http://harmonet.org/harmonise.rdfs#Profile"/>
    </owl:ObjectProperty>
    


    <!-- http://harmonet.org/harmonise.rdfs#profileField -->

    <owl:ObjectProperty rdf:about="http://harmonet.org/harmonise.rdfs#profileField">
        <rdfs:domain rdf:resource="http://harmonet.org/harmonise.rdfs#Profile"/>
        <rdfs:range rdf:resource="http://harmonet.org/harmonise.rdfs#ProfileField"/>
    </owl:ObjectProperty>
    


    <!-- http://harmonet.org/harmonise.rdfs#referencedValue -->

    <owl:ObjectProperty rdf:about="http://harmonet.org/harmonise.rdfs#referencedValue">
        <rdfs:domain rdf:resource="http://harmonet.org/harmonise.rdfs#ListValue"/>
        <rdfs:range rdf:resource="http://harmonet.org/harmonise.rdfs#ReferencedValue"/>
        <rdfs:label>referencedValue</rdfs:label>
    </owl:ObjectProperty>
    


    <!-- http://harmonet.org/harmonise.rdfs#schedule -->

    <owl:ObjectProperty rdf:about="http://harmonet.org/harmonise.rdfs#schedule">
        <rdfs:domain rdf:resource="http://harmonet.org/harmonise.rdfs#Accommodation"/>
        <rdfs:domain rdf:resource="http://harmonet.org/harmonise.rdfs#Attraction"/>
        <rdfs:domain rdf:resource="http://harmonet.org/harmonise.rdfs#Gastro"/>
        <rdfs:range rdf:resource="http://harmonet.org/harmonise.rdfs#Timeline"/>
        <rdfs:comment>The opening time for site</rdfs:comment>
        <rdfs:label>schedule</rdfs:label>
    </owl:ObjectProperty>
    


    <!-- http://harmonet.org/harmonise.rdfs#season -->

    <owl:ObjectProperty rdf:about="http://harmonet.org/harmonise.rdfs#season">
        <rdfs:domain rdf:resource="http://harmonet.org/harmonise.rdfs#Timeline"/>
        <rdfs:range rdf:resource="http://harmonet.org/harmonise.rdfs#ListValue"/>
        <rdfs:comment>optional, one of high season, middle season, low season, holy week, summer months, public holiday, Christmas/New Year, Local festival</rdfs:comment>
        <rdfs:label>season</rdfs:label>
    </owl:ObjectProperty>
    


    <!-- http://harmonet.org/harmonise.rdfs#serviceName -->

    <owl:ObjectProperty rdf:about="http://harmonet.org/harmonise.rdfs#serviceName">
        <rdfs:domain rdf:resource="http://harmonet.org/harmonise.rdfs#Service"/>
        <rdfs:range rdf:resource="http://harmonet.org/harmonise.rdfs#ListValue"/>
        <rdfs:label>serviceName</rdfs:label>
    </owl:ObjectProperty>
    


    <!-- http://harmonet.org/harmonise.rdfs#startDate -->

    <owl:ObjectProperty rdf:about="http://harmonet.org/harmonise.rdfs#startDate">
        <rdfs:domain rdf:resource="http://harmonet.org/harmonise.rdfs#DateRange"/>
        <rdfs:range rdf:resource="http://harmonet.org/harmonise.rdfs#Date"/>
        <rdfs:label>startDate</rdfs:label>
    </owl:ObjectProperty>
    


    <!-- http://harmonet.org/harmonise.rdfs#type -->

    <owl:ObjectProperty rdf:about="http://harmonet.org/harmonise.rdfs#type">
        <rdfs:domain rdf:resource="http://harmonet.org/harmonise.rdfs#Attraction"/>
        <rdfs:range rdf:resource="http://harmonet.org/harmonise.rdfs#ListValue"/>
    </owl:ObjectProperty>
    


    <!-- http://opendata.aragon.es/def/ei2a#administrativeLevel -->

    <owl:ObjectProperty rdf:about="http://opendata.aragon.es/def/ei2a#administrativeLevel">
        <rdfs:domain rdf:resource="http://www.w3.org/ns/org#Organization"/>
        <rdfs:range rdf:resource="http://opendata.aragon.es/def/ei2a#AdministrativeLevel"/>
        <rdfs:comment xml:lang="es">Nivel territorial de administración al que pertenece la unidad orgánica, según el artículo 2.1 de la Ley 30/1992</rdfs:comment>
    </owl:ObjectProperty>
    


    <!-- http://opendata.aragon.es/def/ei2a#administrativeRecordStatus -->

    <owl:ObjectProperty rdf:about="http://opendata.aragon.es/def/ei2a#administrativeRecordStatus">
        <rdfs:domain rdf:resource="http://opendata.aragon.es/def/ei2a#AdministrativeRecord"/>
        <rdfs:range rdf:resource="http://opendata.aragon.es/def/ei2a#AdministrativeRecordStatus"/>
        <rdfs:comment xml:lang="en">Links a state of the administrative record at the time of exchange (electronic)</rdfs:comment>
        <rdfs:comment xml:lang="es">Vincula un estado del expediente en el momento de intercambio (electrónico)</rdfs:comment>
    </owl:ObjectProperty>
    


    <!-- http://opendata.aragon.es/def/ei2a#aidsAssociatedToCrop -->

    <owl:ObjectProperty rdf:about="http://opendata.aragon.es/def/ei2a#aidsAssociatedToCrop">
        <rdfs:domain rdf:resource="http://opendata.aragon.es/def/ei2a#PACAidsRequest"/>
        <rdfs:range rdf:resource="http://opendata.aragon.es/def/ei2a#Crop"/>
        <rdfs:comment xml:lang="en">Aids associated to the crop</rdfs:comment>
        <rdfs:comment xml:lang="es">Ayudas asociadas al cultivo</rdfs:comment>
    </owl:ObjectProperty>
    


    <!-- http://opendata.aragon.es/def/ei2a#applyFor -->

    <owl:ObjectProperty rdf:about="http://opendata.aragon.es/def/ei2a#applyFor">
        <owl:inverseOf rdf:resource="http://opendata.aragon.es/def/ei2a#isOfInterestTo"/>
        <rdfs:domain>
            <owl:Class>
                <owl:unionOf rdf:parseType="Collection">
                    <rdf:Description rdf:about="http://www.w3.org/ns/org#Organization"/>
                    <rdf:Description rdf:about="http://www.w3.org/ns/person#Person"/>
                </owl:unionOf>
            </owl:Class>
        </rdfs:domain>
        <rdfs:range rdf:resource="http://opendata.aragon.es/def/ei2a#Document"/>
        <rdfs:comment xml:lang="en">A person, legal entity or organization may request the opening of a administrative record.</rdfs:comment>
        <rdfs:comment xml:lang="es">Una persona, persona jurídica u organización puede solicitar la apertura de un expediente</rdfs:comment>
    </owl:ObjectProperty>
    


    <!-- http://opendata.aragon.es/def/ei2a#bankAccountOf -->

    <owl:ObjectProperty rdf:about="http://opendata.aragon.es/def/ei2a#bankAccountOf">
        <owl:inverseOf rdf:resource="http://opendata.aragon.es/def/ei2a#hasBankAccount"/>
        <rdfs:domain rdf:resource="http://opendata.aragon.es/def/ei2a#BankAccount"/>
        <rdfs:range>
            <owl:Class>
                <owl:unionOf rdf:parseType="Collection">
                    <rdf:Description rdf:about="http://www.w3.org/ns/org#Organization"/>
                    <rdf:Description rdf:about="http://www.w3.org/ns/person#Person"/>
                </owl:unionOf>
            </owl:Class>
        </rdfs:range>
        <rdfs:comment xml:lang="en">Bank account of a person or organization</rdfs:comment>
        <rdfs:comment xml:lang="es">Cuenta bancaria de una persona u organización</rdfs:comment>
    </owl:ObjectProperty>
    


    <!-- http://opendata.aragon.es/def/ei2a#belongToSocialMediaSource -->

    <owl:ObjectProperty rdf:about="http://opendata.aragon.es/def/ei2a#belongToSocialMediaSource">
        <rdfs:domain rdf:resource="http://opendata.aragon.es/def/ei2a#SocialMedia"/>
        <rdfs:range rdf:resource="http://opendata.aragon.es/def/ei2a#SocialMediaSources"/>
        <rdfs:comment xml:lang="es">Indica la fuente de comunicación social: Twitter, Facebook, etc.</rdfs:comment>
        <rdfs:comment xml:lang="en">Indicates the source of social communication: Twitter, Facebook, etc.</rdfs:comment>
    </owl:ObjectProperty>
    


    <!-- http://opendata.aragon.es/def/ei2a#belongsTo -->

    <owl:ObjectProperty rdf:about="http://opendata.aragon.es/def/ei2a#belongsTo">
        <rdfs:domain rdf:resource="http://opendata.aragon.es/def/ei2a#Procedure"/>
        <rdfs:range rdf:resource="http://opendata.aragon.es/def/ei2a#Series"/>
        <rdfs:comment xml:lang="es">Relación de pertenencia de un procedimiento a una serie.</rdfs:comment>
        <rdfs:comment xml:lang="en">Relationship of membership of a procedure to a series</rdfs:comment>
    </owl:ObjectProperty>
    


    <!-- http://opendata.aragon.es/def/ei2a#captureOn -->

    <owl:ObjectProperty rdf:about="http://opendata.aragon.es/def/ei2a#captureOn">
        <rdfs:domain rdf:resource="http://opendata.aragon.es/def/ei2a#SocialMedia"/>
        <rdfs:range rdf:resource="http://www.w3.org/2006/time#Instant"/>
        <rdfs:comment xml:lang="en">Date of capture of the social communication</rdfs:comment>
        <rdfs:comment xml:lang="es">Fecha de captura de la comunicación social</rdfs:comment>
    </owl:ObjectProperty>
    


    <!-- http://opendata.aragon.es/def/ei2a#citationOnEntity -->

    <owl:ObjectProperty rdf:about="http://opendata.aragon.es/def/ei2a#citationOnEntity">
        <owl:inverseOf rdf:resource="http://opendata.aragon.es/def/ei2a#isCited"/>
        <rdf:type rdf:resource="http://www.w3.org/2002/07/owl#FunctionalProperty"/>
        <rdfs:domain rdf:resource="http://opendata.aragon.es/def/ei2a#Citation"/>
        <rdfs:range>
            <owl:Class>
                <owl:unionOf rdf:parseType="Collection">
                    <rdf:Description rdf:about="http://purl.org/dc/terms/Location"/>
                    <rdf:Description rdf:about="http://www.w3.org/ns/org#Organization"/>
                    <rdf:Description rdf:about="http://www.w3.org/ns/person#Person"/>
                </owl:unionOf>
            </owl:Class>
        </rdfs:range>
        <rdfs:comment xml:lang="es">Entidad (persona, organización o localización) que participa en la relación de citación. Es la relación inversa de &apos;ei2a:isCited&apos;</rdfs:comment>
        <rdfs:comment xml:lang="en">Entity (person, organization or location) that participates in the citation relation. It is the inverse relationship of &apos;ei2a: isCited&apos;</rdfs:comment>
    </owl:ObjectProperty>
    


    <!-- http://opendata.aragon.es/def/ei2a#citationOnWebPage -->

    <owl:ObjectProperty rdf:about="http://opendata.aragon.es/def/ei2a#citationOnWebPage">
        <rdf:type rdf:resource="http://www.w3.org/2002/07/owl#FunctionalProperty"/>
        <rdfs:domain rdf:resource="http://opendata.aragon.es/def/ei2a#Citation"/>
        <rdfs:range rdf:resource="http://opendata.aragon.es/def/ei2a#WebPage"/>
        <rdfs:comment xml:lang="en">Web, subdomain or web portal of the Government of Aragon in which an entity (person, organization or locality) is cited</rdfs:comment>
        <rdfs:comment xml:lang="es">Web, subdominio o portal web del Gobierno de Aragón  en la que una entidad (persona, organización o localidad) es citada</rdfs:comment>
    </owl:ObjectProperty>
    


    <!-- http://opendata.aragon.es/def/ei2a#contains -->

    <owl:ObjectProperty rdf:about="http://opendata.aragon.es/def/ei2a#contains">
        <rdfs:domain rdf:resource="http://opendata.aragon.es/def/ei2a#Series"/>
        <rdfs:range rdf:resource="http://opendata.aragon.es/def/ei2a#Procedure"/>
        <rdfs:comment xml:lang="en">Link to the procedures contained in a series</rdfs:comment>
        <rdfs:comment xml:lang="es">Vínculo con los procedimientos que contiene una serie</rdfs:comment>
    </owl:ObjectProperty>
    


    <!-- http://opendata.aragon.es/def/ei2a#creditCardOf -->

    <owl:ObjectProperty rdf:about="http://opendata.aragon.es/def/ei2a#creditCardOf">
        <owl:inverseOf rdf:resource="http://opendata.aragon.es/def/ei2a#hasCreditCard"/>
        <rdfs:domain rdf:resource="http://opendata.aragon.es/def/ei2a#CreditCard"/>
        <rdfs:range>
            <owl:Class>
                <owl:unionOf rdf:parseType="Collection">
                    <rdf:Description rdf:about="http://www.w3.org/ns/org#Organization"/>
                    <rdf:Description rdf:about="http://www.w3.org/ns/person#Person"/>
                </owl:unionOf>
            </owl:Class>
        </rdfs:range>
        <rdfs:comment xml:lang="en">Credit card of a person or organization</rdfs:comment>
        <rdfs:comment xml:lang="es">Tarjeta de crédito de una persona u organización</rdfs:comment>
    </owl:ObjectProperty>
    


    <!-- http://opendata.aragon.es/def/ei2a#documentCategory -->

    <owl:ObjectProperty rdf:about="http://opendata.aragon.es/def/ei2a#documentCategory">
        <rdfs:domain rdf:resource="http://opendata.aragon.es/def/ei2a#Document"/>
        <rdfs:range rdf:resource="http://opendata.aragon.es/def/ei2a#DocumentCategory"/>
        <rdfs:comment xml:lang="es">Determina el valor del tipo de la entidad documento.</rdfs:comment>
        <rdfs:comment xml:lang="en">Determines the value of the type of Document entity.</rdfs:comment>
    </owl:ObjectProperty>
    


    <!-- http://opendata.aragon.es/def/ei2a#documentLocation -->

    <owl:ObjectProperty rdf:about="http://opendata.aragon.es/def/ei2a#documentLocation">
        <rdfs:domain rdf:resource="http://opendata.aragon.es/def/ei2a#Document"/>
        <rdfs:range rdf:resource="http://purl.org/dc/terms/Location"/>
        <rdfs:comment xml:lang="es">Asocia un documento con una determinada ubicación. 

Nombre normalizado de la localización de la actuación objeto del documento (expediente) en base al callejero normalizado</rdfs:comment>
        <rdfs:comment xml:lang="en">Associates a document with a specific location.

Standardized name of the location of the action object of the document (administrative record) on the basis of the normalized street</rdfs:comment>
    </owl:ObjectProperty>
    


    <!-- http://opendata.aragon.es/def/ei2a#documentOrigin -->

    <owl:ObjectProperty rdf:about="http://opendata.aragon.es/def/ei2a#documentOrigin">
        <rdfs:domain rdf:resource="http://opendata.aragon.es/def/ei2a#Document"/>
        <rdfs:range rdf:resource="http://opendata.aragon.es/def/ei2a#DocumentOrigin"/>
        <rdfs:comment xml:lang="en">Origin of a particular document</rdfs:comment>
        <rdfs:comment xml:lang="es">Procedencia de un determinado documento</rdfs:comment>
    </owl:ObjectProperty>
    


    <!-- http://opendata.aragon.es/def/ei2a#documentStatus -->

    <owl:ObjectProperty rdf:about="http://opendata.aragon.es/def/ei2a#documentStatus">
        <rdfs:domain rdf:resource="http://opendata.aragon.es/def/ei2a#Document"/>
        <rdfs:range rdf:resource="http://opendata.aragon.es/def/ei2a#DocumentStatus"/>
        <rdfs:comment xml:lang="en">Document status (original or copy)</rdfs:comment>
        <rdfs:comment xml:lang="es">Estado del documento (original o copia)</rdfs:comment>
    </owl:ObjectProperty>
    


    <!-- http://opendata.aragon.es/def/ei2a#functionalOrganizationStatus -->

    <owl:ObjectProperty rdf:about="http://opendata.aragon.es/def/ei2a#functionalOrganizationStatus">
        <rdfs:domain rdf:resource="http://www.w3.org/ns/org#Organization"/>
        <rdfs:range rdf:resource="http://opendata.aragon.es/def/ei2a#FunctionalOrganizationStatus"/>
        <rdfs:comment xml:lang="es">Estatus o situación jurídico/funcional de la unidad (C_ID_ESTADO)</rdfs:comment>
        <rdfs:comment xml:lang="en">Status or legal/functional state of the unit (C_ID_ESTADO)</rdfs:comment>
    </owl:ObjectProperty>
    


    <!-- http://opendata.aragon.es/def/ei2a#hasBankAccount -->

    <owl:ObjectProperty rdf:about="http://opendata.aragon.es/def/ei2a#hasBankAccount">
        <rdfs:domain>
            <owl:Class>
                <owl:unionOf rdf:parseType="Collection">
                    <rdf:Description rdf:about="http://www.w3.org/ns/org#Organization"/>
                    <rdf:Description rdf:about="http://www.w3.org/ns/person#Person"/>
                </owl:unionOf>
            </owl:Class>
        </rdfs:domain>
        <rdfs:range rdf:resource="http://opendata.aragon.es/def/ei2a#BankAccount"/>
        <rdfs:comment xml:lang="en">An organization or person owns one or several bank accounts</rdfs:comment>
        <rdfs:comment xml:lang="es">Una organización o persona es propietaria de una o varias tarjetas de crédito</rdfs:comment>
    </owl:ObjectProperty>
    


    <!-- http://opendata.aragon.es/def/ei2a#hasCadastralReference -->

    <owl:ObjectProperty rdf:about="http://opendata.aragon.es/def/ei2a#hasCadastralReference">
        <rdfs:domain rdf:resource="http://www.w3.org/ns/org#Organization"/>
        <rdfs:range rdf:resource="http://opendata.aragon.es/def/ei2a#CadastralParcel"/>
        <rdfs:comment xml:lang="en">Cadastral reference of an organization</rdfs:comment>
        <rdfs:comment xml:lang="es">Referencia catastral de una organización</rdfs:comment>
    </owl:ObjectProperty>
    


    <!-- http://opendata.aragon.es/def/ei2a#hasCompound -->

    <owl:ObjectProperty rdf:about="http://opendata.aragon.es/def/ei2a#hasCompound">
        <rdfs:domain rdf:resource="http://opendata.aragon.es/def/ei2a#CadastralRuralParcel"/>
        <rdfs:range rdf:resource="http://opendata.aragon.es/def/ei2a#Compound"/>
        <rdfs:comment xml:lang="es">Indica los recintos que puede tener una parcela rural</rdfs:comment>
        <rdfs:comment xml:lang="en">Indicate the compounds or enclosures that a rural parcel can have</rdfs:comment>
    </owl:ObjectProperty>
    


    <!-- http://opendata.aragon.es/def/ei2a#hasCreditCard -->

    <owl:ObjectProperty rdf:about="http://opendata.aragon.es/def/ei2a#hasCreditCard">
        <rdfs:domain>
            <owl:Class>
                <owl:unionOf rdf:parseType="Collection">
                    <rdf:Description rdf:about="http://www.w3.org/ns/org#Organization"/>
                    <rdf:Description rdf:about="http://www.w3.org/ns/person#Person"/>
                </owl:unionOf>
            </owl:Class>
        </rdfs:domain>
        <rdfs:range rdf:resource="http://opendata.aragon.es/def/ei2a#CreditCard"/>
        <rdfs:comment xml:lang="en">An organization or person owns one or several credit cards</rdfs:comment>
        <rdfs:comment xml:lang="es">Una organización o persona es propietaria de una o varias tarjetas de crédito</rdfs:comment>
    </owl:ObjectProperty>
    


    <!-- http://opendata.aragon.es/def/ei2a#hasHashtags -->

    <owl:ObjectProperty rdf:about="http://opendata.aragon.es/def/ei2a#hasHashtags">
        <rdfs:domain rdf:resource="http://opendata.aragon.es/def/ei2a#SocialMedia"/>
        <rdfs:range rdf:resource="http://opendata.aragon.es/def/ei2a#SocialMediaHashtag"/>
        <rdfs:comment xml:lang="es">Indica los hashtags de una comunicación social</rdfs:comment>
        <rdfs:comment xml:lang="en">Indicates the hashtags of a social communication</rdfs:comment>
    </owl:ObjectProperty>
    


    <!-- http://opendata.aragon.es/def/ei2a#hasLegalPublicEntityAffiliated -->

    <owl:ObjectProperty rdf:about="http://opendata.aragon.es/def/ei2a#hasLegalPublicEntityAffiliated">
        <rdfs:domain rdf:resource="http://www.w3.org/ns/org#Organization"/>
        <rdfs:range rdf:resource="http://www.w3.org/ns/org#Organization"/>
        <rdfs:comment xml:lang="en">Code of the Public Law Entity associated with the unit. If the unit represents the entity itself, it will refer to itself.</rdfs:comment>
        <rdfs:comment xml:lang="es">Código de la Entidad de Derecho Público asociada a la unidad. Si la unidad representa a la propia entidad, hará referencia a ella misma.</rdfs:comment>
    </owl:ObjectProperty>
    


    <!-- http://opendata.aragon.es/def/ei2a#hasLegalRepresentative -->

    <owl:ObjectProperty rdf:about="http://opendata.aragon.es/def/ei2a#hasLegalRepresentative">
        <rdfs:domain>
            <owl:Class>
                <owl:unionOf rdf:parseType="Collection">
                    <rdf:Description rdf:about="http://www.w3.org/ns/org#Organization"/>
                    <rdf:Description rdf:about="http://www.w3.org/ns/person#Person"/>
                </owl:unionOf>
            </owl:Class>
        </rdfs:domain>
        <rdfs:range>
            <owl:Class>
                <owl:unionOf rdf:parseType="Collection">
                    <rdf:Description rdf:about="http://www.w3.org/ns/org#Organization"/>
                    <rdf:Description rdf:about="http://www.w3.org/ns/person#Person"/>
                </owl:unionOf>
            </owl:Class>
        </rdfs:range>
        <rdfs:comment xml:lang="en">A person has as legal representation a person or an organization</rdfs:comment>
        <rdfs:comment xml:lang="es">Representante legal de una organización. El representate puede ser una persona u otra organización</rdfs:comment>
    </owl:ObjectProperty>
    


    <!-- http://opendata.aragon.es/def/ei2a#hasMentions -->

    <owl:ObjectProperty rdf:about="http://opendata.aragon.es/def/ei2a#hasMentions">
        <rdfs:domain rdf:resource="http://opendata.aragon.es/def/ei2a#SocialMedia"/>
        <rdfs:range rdf:resource="http://opendata.aragon.es/def/ei2a#SocialMediaMention"/>
        <rdfs:comment xml:lang="es">Indica las menciones de una comunicación social</rdfs:comment>
        <rdfs:comment xml:lang="en">Indicates the mentions of a social communication</rdfs:comment>
    </owl:ObjectProperty>
    


    <!-- http://opendata.aragon.es/def/ei2a#hasProcedure -->

    <owl:ObjectProperty rdf:about="http://opendata.aragon.es/def/ei2a#hasProcedure">
        <rdfs:domain rdf:resource="http://opendata.aragon.es/def/ei2a#Document"/>
        <rdfs:range rdf:resource="http://opendata.aragon.es/def/ei2a#Procedure"/>
        <rdfs:comment xml:lang="es">Procedimiento dentro del cual se incluye el documento.</rdfs:comment>
        <rdfs:comment xml:lang="en">Procedure within which the document is included.</rdfs:comment>
    </owl:ObjectProperty>
    


    <!-- http://opendata.aragon.es/def/ei2a#hasProperty -->

    <owl:ObjectProperty rdf:about="http://opendata.aragon.es/def/ei2a#hasProperty">
        <owl:inverseOf rdf:resource="http://opendata.aragon.es/def/ei2a#isProperty"/>
        <rdfs:domain rdf:resource="http://www.w3.org/ns/person#Person"/>
        <rdfs:range rdf:resource="http://opendata.aragon.es/def/ei2a#CadastralParcel"/>
        <rdfs:comment xml:lang="en">A person owns a cadastral parcel</rdfs:comment>
        <rdfs:comment xml:lang="es">Una persona es propietaria de una parcela catastral</rdfs:comment>
    </owl:ObjectProperty>
    


    <!-- http://opendata.aragon.es/def/ei2a#hasSeries -->

    <owl:ObjectProperty rdf:about="http://opendata.aragon.es/def/ei2a#hasSeries">
        <rdfs:domain rdf:resource="http://opendata.aragon.es/def/ei2a#Document"/>
        <rdfs:range rdf:resource="http://opendata.aragon.es/def/ei2a#Series"/>
        <rdfs:comment xml:lang="es">Serie bajo la cual se encuentra un documento</rdfs:comment>
        <rdfs:comment xml:lang="en">Series under which is a document</rdfs:comment>
    </owl:ObjectProperty>
    


    <!-- http://opendata.aragon.es/def/ei2a#hasSimilarity -->

    <owl:ObjectProperty rdf:about="http://opendata.aragon.es/def/ei2a#hasSimilarity">
        <owl:inverseOf rdf:resource="http://opendata.aragon.es/def/ei2a#similarityOnWebPages"/>
        <rdfs:domain rdf:resource="http://opendata.aragon.es/def/ei2a#WebPage"/>
        <rdfs:range rdf:resource="http://opendata.aragon.es/def/ei2a#Similarity"/>
        <rdfs:comment xml:lang="es">Página web que participa en la medida de similitud con otra página web</rdfs:comment>
        <rdfs:comment xml:lang="en">Website that participates in the measure of similarity with another web page</rdfs:comment>
    </owl:ObjectProperty>
    


    <!-- http://opendata.aragon.es/def/ei2a#hasSocialMedia -->

    <owl:ObjectProperty rdf:about="http://opendata.aragon.es/def/ei2a#hasSocialMedia">
        <owl:inverseOf rdf:resource="http://opendata.aragon.es/def/ei2a#isSocialMediaOf"/>
        <rdfs:domain rdf:resource="http://www.w3.org/ns/org#Organization"/>
        <rdfs:range rdf:resource="http://opendata.aragon.es/def/ei2a#SocialMedia"/>
        <rdfs:comment xml:lang="es">Organización que tiene una cuenta de comunicación social</rdfs:comment>
        <rdfs:comment xml:lang="en">Organization that has a social communication account</rdfs:comment>
    </owl:ObjectProperty>
    


    <!-- http://opendata.aragon.es/def/ei2a#hasWebPage -->

    <owl:ObjectProperty rdf:about="http://opendata.aragon.es/def/ei2a#hasWebPage">
        <owl:inverseOf rdf:resource="http://opendata.aragon.es/def/ei2a#isWebPageOf"/>
        <rdfs:domain rdf:resource="http://www.w3.org/ns/org#Organization"/>
        <rdfs:range rdf:resource="http://opendata.aragon.es/def/ei2a#WebPage"/>
        <rdfs:comment xml:lang="es">Organización que tiene una web, subdominio o portal web</rdfs:comment>
        <rdfs:comment xml:lang="en">Organization that has a web, subdomain or web portal</rdfs:comment>
    </owl:ObjectProperty>
    


    <!-- http://opendata.aragon.es/def/ei2a#isAuxiliarOf -->

    <owl:ObjectProperty rdf:about="http://opendata.aragon.es/def/ei2a#isAuxiliarOf">
        <rdfs:domain rdf:resource="http://www.w3.org/ns/org#Organization"/>
        <rdfs:range rdf:resource="http://www.w3.org/ns/org#Organization"/>
        <rdfs:comment xml:lang="en">Code of the responsible office. Only applies to those offices whose type is AUXILIARY</rdfs:comment>
        <rdfs:comment xml:lang="es">Código de la oficina responsable. Solo aplica a aquellas oficinas cuyo tipo es AUXILIAR</rdfs:comment>
    </owl:ObjectProperty>
    


    <!-- http://opendata.aragon.es/def/ei2a#isCited -->

    <owl:ObjectProperty rdf:about="http://opendata.aragon.es/def/ei2a#isCited">
        <rdfs:domain>
            <owl:Class>
                <owl:unionOf rdf:parseType="Collection">
                    <rdf:Description rdf:about="http://purl.org/dc/terms/Location"/>
                    <rdf:Description rdf:about="http://www.w3.org/ns/org#Organization"/>
                    <rdf:Description rdf:about="http://www.w3.org/ns/person#Person"/>
                </owl:unionOf>
            </owl:Class>
        </rdfs:domain>
        <rdfs:range rdf:resource="http://opendata.aragon.es/def/ei2a#Citation"/>
        <rdfs:comment xml:lang="es">Entidad (persona, organización o localización) que es citada en una web, subdominio o portal web del Gobierno de Aragón. Es relación inversa de &apos;ei2a:citationOnEntity&apos;</rdfs:comment>
        <rdfs:comment xml:lang="en">Entity (person, organization or location) that is cited in a web, subdomain or web portal of the Government of Aragon. It is inverse relationship of &apos;ei2a: citationOnEntity&apos;</rdfs:comment>
    </owl:ObjectProperty>
    


    <!-- http://opendata.aragon.es/def/ei2a#isLineMemberOf -->

    <owl:ObjectProperty rdf:about="http://opendata.aragon.es/def/ei2a#isLineMemberOf">
        <rdfs:domain rdf:resource="http://opendata.aragon.es/def/ei2a#MultiLine"/>
        <rdfs:range rdf:resource="http://opendata.aragon.es/def/ei2a#Line"/>
        <rdfs:comment xml:lang="en">Links a Line simple geometry to a MultiLine composite geometry.</rdfs:comment>
        <rdfs:comment xml:lang="es">Vincula una geometría Línea simple a una geometría compuesta MultiLine.</rdfs:comment>
    </owl:ObjectProperty>
    


    <!-- http://opendata.aragon.es/def/ei2a#isLinkedTo -->

    <owl:ObjectProperty rdf:about="http://opendata.aragon.es/def/ei2a#isLinkedTo">
        <rdfs:domain rdf:resource="http://opendata.aragon.es/def/ei2a#Document"/>
        <rdfs:range rdf:resource="http://opendata.aragon.es/def/ei2a#Document"/>
        <rdfs:comment xml:lang="es">Relación existente entre varios documentos.</rdfs:comment>
        <rdfs:comment xml:lang="en">Relationship between several documents.</rdfs:comment>
    </owl:ObjectProperty>
    


    <!-- http://opendata.aragon.es/def/ei2a#isOfInterestTo -->

    <owl:ObjectProperty rdf:about="http://opendata.aragon.es/def/ei2a#isOfInterestTo">
        <rdfs:domain rdf:resource="http://opendata.aragon.es/def/ei2a#Document"/>
        <rdfs:range>
            <owl:Class>
                <owl:unionOf rdf:parseType="Collection">
                    <rdf:Description rdf:about="http://www.w3.org/ns/org#Organization"/>
                    <rdf:Description rdf:about="http://www.w3.org/ns/person#Person"/>
                </owl:unionOf>
            </owl:Class>
        </rdfs:range>
        <rdfs:comment xml:lang="en">Document of interest to a citizen or legal entity, or the administration</rdfs:comment>
        <rdfs:comment xml:lang="es">Documento de interés para un ciudadano o persona jurídica, o la adminsitración</rdfs:comment>
    </owl:ObjectProperty>
    


    <!-- http://opendata.aragon.es/def/ei2a#isPointMemberOf -->

    <owl:ObjectProperty rdf:about="http://opendata.aragon.es/def/ei2a#isPointMemberOf">
        <rdfs:domain rdf:resource="http://opendata.aragon.es/def/ei2a#MultiPoint"/>
        <rdfs:range rdf:resource="http://opendata.aragon.es/def/ei2a#Point"/>
        <rdfs:comment xml:lang="en">Links a Point simple geometry to a MultiPoint composite Geometry.</rdfs:comment>
        <rdfs:comment xml:lang="es">Vincula una geometría simple de Punto a una geometría compuesta Multipunto.</rdfs:comment>
    </owl:ObjectProperty>
    


    <!-- http://opendata.aragon.es/def/ei2a#isPolygonMemberOf -->

    <owl:ObjectProperty rdf:about="http://opendata.aragon.es/def/ei2a#isPolygonMemberOf">
        <rdfs:domain rdf:resource="http://opendata.aragon.es/def/ei2a#MultiPolygon"/>
        <rdfs:range rdf:resource="http://opendata.aragon.es/def/ei2a#Polygon"/>
        <rdfs:comment xml:lang="es">Enlaza una geometría simple de polígono a una geometría compuesta MultiPolygon.</rdfs:comment>
        <rdfs:comment xml:lang="en">Links a Polygon simple geometry to a MultiPolygon composite geometry.</rdfs:comment>
    </owl:ObjectProperty>
    


    <!-- http://opendata.aragon.es/def/ei2a#isProperty -->

    <owl:ObjectProperty rdf:about="http://opendata.aragon.es/def/ei2a#isProperty">
        <rdfs:domain rdf:resource="http://opendata.aragon.es/def/ei2a#CadastralParcel"/>
        <rdfs:range rdf:resource="http://www.w3.org/ns/person#Person"/>
        <rdfs:comment xml:lang="es">Es propiedad de</rdfs:comment>
        <rdfs:comment xml:lang="en">Is property of.</rdfs:comment>
    </owl:ObjectProperty>
    


    <!-- http://opendata.aragon.es/def/ei2a#isRuralParcel -->

    <owl:ObjectProperty rdf:about="http://opendata.aragon.es/def/ei2a#isRuralParcel">
        <rdfs:domain rdf:resource="http://opendata.aragon.es/def/ei2a#CadastralParcel"/>
        <rdfs:range rdf:resource="http://opendata.aragon.es/def/ei2a#RuralParcel"/>
        <rdfs:comment xml:lang="es">Indicador de que es una propiedad rústica</rdfs:comment>
        <rdfs:comment xml:lang="en">Indicator that is a rustic property</rdfs:comment>
    </owl:ObjectProperty>
    


    <!-- http://opendata.aragon.es/def/ei2a#isSocialMediaOf -->

    <owl:ObjectProperty rdf:about="http://opendata.aragon.es/def/ei2a#isSocialMediaOf">
        <rdfs:domain rdf:resource="http://opendata.aragon.es/def/ei2a#SocialMedia"/>
        <rdfs:range rdf:resource="http://www.w3.org/ns/org#Organization"/>
        <rdfs:comment xml:lang="es">Cuenta de comunicación social de una organización</rdfs:comment>
        <rdfs:comment xml:lang="en">Social communication account of an organization</rdfs:comment>
    </owl:ObjectProperty>
    


    <!-- http://opendata.aragon.es/def/ei2a#isUrbanParcel -->

    <owl:ObjectProperty rdf:about="http://opendata.aragon.es/def/ei2a#isUrbanParcel">
        <rdfs:domain rdf:resource="http://opendata.aragon.es/def/ei2a#CadastralParcel"/>
        <rdfs:range rdf:resource="http://opendata.aragon.es/def/ei2a#UrbanParcel"/>
        <rdfs:comment xml:lang="es">Indicador de que es una parcela urbana</rdfs:comment>
        <rdfs:comment xml:lang="en">Indicator that is a urban property</rdfs:comment>
    </owl:ObjectProperty>
    


    <!-- http://opendata.aragon.es/def/ei2a#isWebPageOf -->

    <owl:ObjectProperty rdf:about="http://opendata.aragon.es/def/ei2a#isWebPageOf">
        <rdfs:domain rdf:resource="http://opendata.aragon.es/def/ei2a#WebPage"/>
        <rdfs:range rdf:resource="http://www.w3.org/ns/org#Organization"/>
        <rdfs:comment xml:lang="en">Web, subdomain or web portal that belongs to an organization</rdfs:comment>
        <rdfs:comment xml:lang="es">Web, subdominio o portal web que pertenece a una organización</rdfs:comment>
    </owl:ObjectProperty>
    


    <!-- http://opendata.aragon.es/def/ei2a#linePartOfPolygon -->

    <owl:ObjectProperty rdf:about="http://opendata.aragon.es/def/ei2a#linePartOfPolygon">
        <rdfs:domain rdf:resource="http://opendata.aragon.es/def/ei2a#Line"/>
        <rdfs:range rdf:resource="http://opendata.aragon.es/def/ei2a#Polygon"/>
        <rdfs:comment xml:lang="en">Line that is part of a polygon</rdfs:comment>
        <rdfs:comment xml:lang="es">Línea que es parte de un polígono</rdfs:comment>
    </owl:ObjectProperty>
    


    <!-- http://opendata.aragon.es/def/ei2a#linePositionList -->

    <owl:ObjectProperty rdf:about="http://opendata.aragon.es/def/ei2a#linePositionList">
        <rdfs:domain rdf:resource="http://opendata.aragon.es/def/ei2a#Polygon"/>
        <rdfs:range rdf:resource="http://opendata.aragon.es/def/ei2a#Line"/>
        <rdfs:comment xml:lang="es">Posición de una línea dentro en un polígono</rdfs:comment>
        <rdfs:comment xml:lang="en">Position of a line inside a polygon</rdfs:comment>
    </owl:ObjectProperty>
    


    <!-- http://opendata.aragon.es/def/ei2a#lopdLevel -->

    <owl:ObjectProperty rdf:about="http://opendata.aragon.es/def/ei2a#lopdLevel">
        <rdfs:domain rdf:resource="http://opendata.aragon.es/def/ei2a#Document"/>
        <rdfs:range rdf:resource="http://opendata.aragon.es/def/ei2a#LOPDLevel"/>
        <rdfs:comment xml:lang="en">Data protection level (LOPD).</rdfs:comment>
        <rdfs:comment xml:lang="es">Nivel de protección de datos (LOPD).</rdfs:comment>
    </owl:ObjectProperty>
    


    <!-- http://opendata.aragon.es/def/ei2a#organizationType -->

    <owl:ObjectProperty rdf:about="http://opendata.aragon.es/def/ei2a#organizationType">
        <rdfs:domain rdf:resource="http://www.w3.org/ns/org#Organization"/>
        <rdfs:range rdf:resource="http://opendata.aragon.es/def/ei2a#OrganizationType"/>
        <rdfs:comment xml:lang="es">Indica si la organización es una empresa privada o una administración pública.</rdfs:comment>
        <rdfs:comment xml:lang="en">Indicates whether the organization is a private company or a public administration.</rdfs:comment>
    </owl:ObjectProperty>
    


    <!-- http://opendata.aragon.es/def/ei2a#partOf -->

    <owl:ObjectProperty rdf:about="http://opendata.aragon.es/def/ei2a#partOf">
        <rdfs:domain rdf:resource="http://opendata.aragon.es/def/ei2a#Point"/>
        <rdfs:range rdf:resource="http://opendata.aragon.es/def/ei2a#Line"/>
        <rdfs:comment xml:lang="es">Relaciona un punto con un contorno de forma geométrica.</rdfs:comment>
        <rdfs:comment xml:lang="en">Relates a point to a geometric shape&apos;s boundary.</rdfs:comment>
    </owl:ObjectProperty>
    


    <!-- http://opendata.aragon.es/def/ei2a#personGender -->

    <owl:ObjectProperty rdf:about="http://opendata.aragon.es/def/ei2a#personGender">
        <rdfs:domain rdf:resource="http://www.w3.org/ns/person#Person"/>
        <rdfs:range rdf:resource="http://opendata.aragon.es/def/ei2a#PersonGender"/>
        <rdfs:comment xml:lang="en">Gender or sex associated to a person.

It is always associated the sex that appears in the document proving the identity of the person (male or female)</rdfs:comment>
        <rdfs:comment xml:lang="es">Género o sexo asociada a una persona.

Se asocia siempre el sexo que conste en el documento acreditativo de la identidad de la persona (Masculino o Femenino)</rdfs:comment>
    </owl:ObjectProperty>
    


    <!-- http://opendata.aragon.es/def/ei2a#pesonalIdentifierSystemLinkedTo -->

    <owl:ObjectProperty rdf:about="http://opendata.aragon.es/def/ei2a#pesonalIdentifierSystemLinkedTo">
        <rdfs:domain rdf:resource="http://opendata.aragon.es/def/ei2a#PersonalIdentifierSystem"/>
        <rdfs:range rdf:resource="http://www.w3.org/ns/person#Person"/>
        <rdfs:comment xml:lang="en">It binds the information and identification that is made in a system of a person  with the unique identifier of person (org: identifier).</rdfs:comment>
        <rdfs:comment xml:lang="es">Vincula la información e identificación que se realiza en un sistema de una persona (ei2a: identifierPersonSystem) con el identificador unívoco de persona (org:identifier).</rdfs:comment>
    </owl:ObjectProperty>
    


    <!-- http://opendata.aragon.es/def/ei2a#positionList -->

    <owl:ObjectProperty rdf:about="http://opendata.aragon.es/def/ei2a#positionList">
        <rdfs:domain rdf:resource="http://opendata.aragon.es/def/ei2a#Line"/>
        <rdfs:range rdf:resource="http://opendata.aragon.es/def/ei2a#Point"/>
        <rdfs:comment xml:lang="es">Relaciona una Línea con los puntos que los definen.</rdfs:comment>
        <rdfs:comment xml:lang="en">Relates a Line to the points that define them.</rdfs:comment>
    </owl:ObjectProperty>
    


    <!-- http://opendata.aragon.es/def/ei2a#propertyType -->

    <owl:ObjectProperty rdf:about="http://opendata.aragon.es/def/ei2a#propertyType">
        <rdfs:domain rdf:resource="http://opendata.aragon.es/def/ei2a#CadastralParcel"/>
        <rdfs:range rdf:resource="http://opendata.aragon.es/def/ei2a#PropertyType"/>
        <rdfs:comment xml:lang="es">Indica el tipo de propiedad: urbana o rústica.</rdfs:comment>
        <rdfs:comment xml:lang="en">Indicates the type of property: urban or rustic.</rdfs:comment>
    </owl:ObjectProperty>
    


    <!-- http://opendata.aragon.es/def/ei2a#publicEntityType -->

    <owl:ObjectProperty rdf:about="http://opendata.aragon.es/def/ei2a#publicEntityType">
        <rdfs:domain rdf:resource="http://www.w3.org/ns/org#Organization"/>
        <rdfs:range rdf:resource="http://opendata.aragon.es/def/ei2a#PublicEntityType"/>
        <rdfs:comment xml:lang="es">Clasificación de los distintos tipos de entidades que constituyen la Administración Pública. Por lo general, representa una estructura de unidades orgánicas que constituye una entidad (órgano/organismo) de la Administración Pública.</rdfs:comment>
        <rdfs:comment xml:lang="en">Classification of the different types of entities that constitute the Public Administration. Generally, it represents a structure of organic units that constitutes an entity (organ / organism) of the Public Administration.</rdfs:comment>
    </owl:ObjectProperty>
    


    <!-- http://opendata.aragon.es/def/ei2a#publishedOn -->

    <owl:ObjectProperty rdf:about="http://opendata.aragon.es/def/ei2a#publishedOn">
        <rdfs:domain rdf:resource="http://opendata.aragon.es/def/ei2a#SocialMedia"/>
        <rdfs:range rdf:resource="http://www.w3.org/2006/time#Instant"/>
        <rdfs:comment xml:lang="en">Date of publication of the social communication</rdfs:comment>
        <rdfs:comment xml:lang="es">Fecha de publicación de la comunicación social</rdfs:comment>
    </owl:ObjectProperty>
    


    <!-- http://opendata.aragon.es/def/ei2a#referenceSystem -->

    <owl:ObjectProperty rdf:about="http://opendata.aragon.es/def/ei2a#referenceSystem">
        <rdfs:domain rdf:resource="http://www.w3.org/ns/locn#Geometry"/>
        <rdfs:range rdf:resource="http://opendata.aragon.es/def/ei2a#ReferenceSystem"/>
        <rdfs:comment xml:lang="en">A reference system allows you to express the position of certain elements using their coordinates.

There are different terrestrial reference systems and the coordinates of the same element are different depending on the one used. Consequently, it is imperative that some coordinates are always accompanied by the metadata that indicates their reference system.</rdfs:comment>
        <rdfs:comment xml:lang="es">Un sistema de referencia permite expresar la posición de determinados elementos utilizando sus coordenadas.

Hay distintos sistemas de referencia terrestres y las coordenadas de un mismo elemento son diferentes en función del que se use. Consiguientemente, es imprescindible que unas coordenadas vayan siempre acompañadas del metadato que indica su sistema de referencia.</rdfs:comment>
    </owl:ObjectProperty>
    


    <!-- http://opendata.aragon.es/def/ei2a#requestAids -->

    <owl:ObjectProperty rdf:about="http://opendata.aragon.es/def/ei2a#requestAids">
        <rdfs:domain>
            <owl:Class>
                <owl:unionOf rdf:parseType="Collection">
                    <rdf:Description rdf:about="http://www.w3.org/ns/org#Organization"/>
                    <rdf:Description rdf:about="http://www.w3.org/ns/person#Person"/>
                </owl:unionOf>
            </owl:Class>
        </rdfs:domain>
        <rdfs:range rdf:resource="http://opendata.aragon.es/def/ei2a#PACAidsRequest"/>
        <rdfs:comment xml:lang="es">Indica que una organización o persona solicita una petición de ayuda de la PAC</rdfs:comment>
        <rdfs:comment xml:lang="en">Indicates that an organization or person requests PAC aids</rdfs:comment>
    </owl:ObjectProperty>
    


    <!-- http://opendata.aragon.es/def/ei2a#ruralParcelOrigin -->

    <owl:ObjectProperty rdf:about="http://opendata.aragon.es/def/ei2a#ruralParcelOrigin">
        <rdfs:domain rdf:resource="http://opendata.aragon.es/def/ei2a#RuralParcel"/>
        <rdfs:range rdf:resource="http://opendata.aragon.es/def/ei2a#RuralParcelOrigin"/>
        <rdfs:comment xml:lang="en">Origin of a rural parcel</rdfs:comment>
        <rdfs:comment xml:lang="es">Procedencia de una parcela rural</rdfs:comment>
    </owl:ObjectProperty>
    


    <!-- http://opendata.aragon.es/def/ei2a#similarityOnCategory -->

    <owl:ObjectProperty rdf:about="http://opendata.aragon.es/def/ei2a#similarityOnCategory">
        <rdf:type rdf:resource="http://www.w3.org/2002/07/owl#FunctionalProperty"/>
        <rdfs:domain rdf:resource="http://opendata.aragon.es/def/ei2a#Similarity"/>
        <rdfs:range rdf:resource="http://opendata.aragon.es/def/ei2a/categorization#GeneralCategorization"/>
        <rdfs:comment xml:lang="en">Category to which the similarity between two web pages belongs</rdfs:comment>
        <rdfs:comment xml:lang="es">Categoría a la que pertenece la similitud que hay entre dos página web</rdfs:comment>
    </owl:ObjectProperty>
    


    <!-- http://opendata.aragon.es/def/ei2a#similarityOnWebPages -->

    <owl:ObjectProperty rdf:about="http://opendata.aragon.es/def/ei2a#similarityOnWebPages">
        <rdfs:domain rdf:resource="http://opendata.aragon.es/def/ei2a#Similarity"/>
        <rdfs:range rdf:resource="http://opendata.aragon.es/def/ei2a#WebPage"/>
        <rdfs:comment xml:lang="en">Similarity between two web pages on a category. It is the inverse relationship of &apos;hasSimilarity&apos;</rdfs:comment>
        <rdfs:comment xml:lang="es">Similitud que hay entre dos páginas web sobre una categoría. Es la relación inversa de &apos;hasSimilarity&apos;</rdfs:comment>
    </owl:ObjectProperty>
    


    <!-- http://opendata.aragon.es/def/ei2a#typeGeometryModel -->

    <owl:ObjectProperty rdf:about="http://opendata.aragon.es/def/ei2a#typeGeometryModel">
        <rdfs:domain rdf:resource="http://www.w3.org/ns/locn#Geometry"/>
        <rdfs:range rdf:resource="http://opendata.aragon.es/def/ei2a#TypeGeometryModel"/>
        <rdfs:comment xml:lang="es">Tipos de modelos lógicos que hacen referencia a cómo se muestran y organizan las variables y objetos para lograr una representación lo más adecuada posible y que dan lugar a tipos de capas de información espacial</rdfs:comment>
        <rdfs:comment xml:lang="en">Types of logical models that refer to how variables and objects are displayed and organized to achieve the most appropriate representation possible and which give rise to types of spatial information layers</rdfs:comment>
    </owl:ObjectProperty>
    


    <!-- http://opendata.aragon.es/def/ei2a#varietyOfCrop -->

    <owl:ObjectProperty rdf:about="http://opendata.aragon.es/def/ei2a#varietyOfCrop">
        <rdfs:domain rdf:resource="http://opendata.aragon.es/def/ei2a#Crop"/>
        <rdfs:range rdf:resource="http://opendata.aragon.es/def/ei2a#CropVariety"/>
        <rdfs:comment xml:lang="es">Indica la variedad del cultivo</rdfs:comment>
        <rdfs:comment xml:lang="en">Indicates the variety of the crop</rdfs:comment>
    </owl:ObjectProperty>
    


    <!-- http://opendata.aragon.es/def/ei2a#webPageCategorization -->

    <owl:ObjectProperty rdf:about="http://opendata.aragon.es/def/ei2a#webPageCategorization">
        <rdfs:domain rdf:resource="http://opendata.aragon.es/def/ei2a#WebPage"/>
        <rdfs:range rdf:resource="http://opendata.aragon.es/def/ei2a/categorization#GeneralCategorization"/>
        <rdfs:comment xml:lang="es">Relación que permite categorizar una web, sudominio o portal del Gobierno de Aragón</rdfs:comment>
        <rdfs:comment xml:lang="en">Relation that allows to categorize a web, subdomain or portal of the Government of Aragon</rdfs:comment>
    </owl:ObjectProperty>
    


    <!-- http://purl.oclc.org/NET/ssnx/ssn#forProperty -->

    <owl:ObjectProperty rdf:about="http://purl.oclc.org/NET/ssnx/ssn#forProperty">
        <owl:equivalentProperty rdf:resource="http://www.semanticwater.com/WISDOM#forProperty"/>
        <rdfs:range rdf:resource="http://purl.oclc.org/NET/ssnx/ssn#Property"/>
        <rdfs:comment>A relation between some aspect of a sensing entity and a property.  For example, from a sensor to the properties it can observe, or from a deployment to the properties it was installed to observe.  Also from a measurement capability to the property the capability is described for.  (Used in conjunction with ofFeature).</rdfs:comment>
        <rdfs:isDefinedBy>http://purl.oclc.org/NET/ssnx/ssn</rdfs:isDefinedBy>
        <rdfs:label>for property</rdfs:label>
        <rdfs:seeAlso>http://www.w3.org/2005/Incubator/ssn/wiki/SSN_Skeleton#Skeleton</rdfs:seeAlso>
    </owl:ObjectProperty>
    


    <!-- http://purl.oclc.org/NET/ssnx/ssn#hasMeasurementCapability -->

    <owl:ObjectProperty rdf:about="http://purl.oclc.org/NET/ssnx/ssn#hasMeasurementCapability">
        <owl:equivalentProperty rdf:resource="http://www.semanticwater.com/WISDOM#hasMeasurementCapability"/>
        <rdfs:subPropertyOf rdf:resource="http://purl.oclc.org/NET/ssnx/ssn#hasProperty"/>
        <rdf:type rdf:resource="http://www.w3.org/2002/07/owl#FunctionalProperty"/>
        <rdf:type rdf:resource="http://www.w3.org/2002/07/owl#AsymmetricProperty"/>
        <rdf:type rdf:resource="http://www.w3.org/2002/07/owl#IrreflexiveProperty"/>
        <rdfs:domain rdf:resource="http://purl.oclc.org/NET/ssnx/ssn#Sensor"/>
        <rdfs:range rdf:resource="http://purl.oclc.org/NET/ssnx/ssn#MeasurementCapability"/>
        <rdfs:comment>Relation from a Sensor to a MeasurementCapability describing the measurement properties of the sensor.</rdfs:comment>
        <rdfs:isDefinedBy>http://purl.oclc.org/NET/ssnx/ssn</rdfs:isDefinedBy>
        <rdfs:label>has measurement  capability</rdfs:label>
        <rdfs:seeAlso>http://www.w3.org/2005/Incubator/ssn/wiki/SSN_Sensor#MeasuringCapability</rdfs:seeAlso>
    </owl:ObjectProperty>
    


    <!-- http://purl.oclc.org/NET/ssnx/ssn#hasMeasurementProperty -->

    <owl:ObjectProperty rdf:about="http://purl.oclc.org/NET/ssnx/ssn#hasMeasurementProperty"/>
    


    <!-- http://purl.oclc.org/NET/ssnx/ssn#hasProperty -->

    <owl:ObjectProperty rdf:about="http://purl.oclc.org/NET/ssnx/ssn#hasProperty">
        <rdfs:subPropertyOf rdf:resource="http://www.ontologydesignpatterns.org/ont/dul/DUL.owl#hasQuality"/>
        <owl:inverseOf rdf:resource="http://purl.oclc.org/NET/ssnx/ssn#isPropertyOf"/>
        <rdfs:comment>A relation between a FeatureOfInterest and a Property of that feature.</rdfs:comment>
        <rdfs:isDefinedBy>http://purl.oclc.org/NET/ssnx/ssn</rdfs:isDefinedBy>
        <rdfs:label>has property</rdfs:label>
        <rdfs:seeAlso>http://www.w3.org/2005/Incubator/ssn/wiki/SSN_Skeleton#Skeleton</rdfs:seeAlso>
    </owl:ObjectProperty>
    


    <!-- http://purl.oclc.org/NET/ssnx/ssn#isPropertyOf -->

    <owl:ObjectProperty rdf:about="http://purl.oclc.org/NET/ssnx/ssn#isPropertyOf">
        <rdfs:subPropertyOf rdf:resource="http://www.ontologydesignpatterns.org/ont/dul/DUL.owl#isQualityOf"/>
        <rdfs:comment>Relation between a FeatureOfInterest and a Property (a Quality observable by a sensor) of that feature.</rdfs:comment>
        <rdfs:isDefinedBy>http://purl.oclc.org/NET/ssnx/ssn</rdfs:isDefinedBy>
        <rdfs:label>is property of</rdfs:label>
        <rdfs:seeAlso>http://www.w3.org/2005/Incubator/ssn/wiki/SSN_Skeleton#Skeleton</rdfs:seeAlso>
    </owl:ObjectProperty>
    


    <!-- http://purl.oclc.org/NET/ssnx/ssn#observes -->

    <owl:ObjectProperty rdf:about="http://purl.oclc.org/NET/ssnx/ssn#observes">
        <rdfs:domain rdf:resource="http://purl.oclc.org/NET/ssnx/ssn#Sensor"/>
        <rdfs:range rdf:resource="http://purl.oclc.org/NET/ssnx/ssn#Property"/>
        <owl:propertyChainAxiom rdf:parseType="Collection">
            <rdf:Description rdf:about="http://purl.oclc.org/NET/ssnx/ssn#hasMeasurementCapability"/>
            <rdf:Description rdf:about="http://purl.oclc.org/NET/ssnx/ssn#forProperty"/>
        </owl:propertyChainAxiom>
        <rdfs:comment>Relation between a Sensor and a Property that the sensor can observe.

Note that, given the DUL modelling of Qualities, a sensor defined with &apos;observes only Windspeed&apos; technically links the sensor to particular instances of Windspeed, not to the concept itself - OWL can&apos;t express concept-concept relations, only individual-individual.  The property composition ensures that if an observation is made of a particular quality then one can infer that the sensor observes that quality.</rdfs:comment>
        <rdfs:isDefinedBy>http://purl.oclc.org/NET/ssnx/ssn</rdfs:isDefinedBy>
        <rdfs:label>observes</rdfs:label>
        <rdfs:seeAlso>http://www.w3.org/2005/Incubator/ssn/wiki/SSN_Sensor#Measuring</rdfs:seeAlso>
    </owl:ObjectProperty>
    


    <!-- http://vocab.gtfs.org/terms#agency -->

    <owl:ObjectProperty rdf:about="http://vocab.gtfs.org/terms#agency">
        <rdfs:range rdf:resource="http://www.w3.org/ns/org#Organization"/>
        <rdfs:comment xml:lang="es">Enlaza a una organización (agencia) de la que este concepto es parte.</rdfs:comment>
        <rdfs:comment xml:lang="en">links to an organization (agency) that this is part of.</rdfs:comment>
        <rdfs:label xml:lang="en">agency</rdfs:label>
        <rdfs:label xml:lang="es">empresa</rdfs:label>
        <status:term_status xml:lang="es">inestable</status:term_status>
        <status:term_status xml:lang="en">unstable</status:term_status>
    </owl:ObjectProperty>
    


    <!-- http://vocab.gtfs.org/terms#destinationStop -->

    <owl:ObjectProperty rdf:about="http://vocab.gtfs.org/terms#destinationStop">
        <rdfs:range rdf:resource="http://vocab.gtfs.org/terms#Stop"/>
        <comment xml:lang="es">Conectado a to_stop_id en transfers.txt</comment>
        <comment xml:lang="en">Map from to_stop_id in transfers.txt</comment>
        <rdfs:comment xml:lang="es">Enlace al gtfs:Stop hacia el que va el viaje</rdfs:comment>
        <rdfs:comment xml:lang="en">Link to gtfs:Stop to go to</rdfs:comment>
        <rdfs:label xml:lang="en">Destination Stop</rdfs:label>
        <rdfs:label xml:lang="es">parada de destino</rdfs:label>
        <status:term_status xml:lang="es">inestable</status:term_status>
        <status:term_status xml:lang="en">unstable</status:term_status>
    </owl:ObjectProperty>
    


    <!-- http://vocab.gtfs.org/terms#originStop -->

    <owl:ObjectProperty rdf:about="http://vocab.gtfs.org/terms#originStop">
        <rdfs:range rdf:resource="http://vocab.gtfs.org/terms#Stop"/>
        <comment xml:lang="es">Conectado a from_stop_id en transfers.txt</comment>
        <comment xml:lang="en">Map from from_stop_id in transfers.txt</comment>
        <rdfs:comment xml:lang="es">Enlace al gtfs:Stop desde el que empieza el viaje</rdfs:comment>
        <rdfs:comment xml:lang="en">Link to gtfs:Stop to start from</rdfs:comment>
        <rdfs:label xml:lang="en">Origin Stop</rdfs:label>
        <rdfs:label xml:lang="es">parada de origen</rdfs:label>
        <status:term_status xml:lang="es">inestable</status:term_status>
        <status:term_status xml:lang="en">unstable</status:term_status>
    </owl:ObjectProperty>
    


    <!-- http://vocab.gtfs.org/terms#route -->

    <owl:ObjectProperty rdf:about="http://vocab.gtfs.org/terms#route">
        <rdfs:domain rdf:resource="http://vocab.gtfs.org/terms#Trip"/>
        <rdfs:range rdf:resource="http://vocab.gtfs.org/terms#Route"/>
        <rdfs:comment xml:lang="es">Este viaje forma parte de esta gtfs:Route</rdfs:comment>
        <rdfs:comment xml:lang="en">This thing is applicable to this gtfs:Route</rdfs:comment>
        <rdfs:label xml:lang="en">Route</rdfs:label>
        <rdfs:label xml:lang="es">ruta</rdfs:label>
        <status:term_status xml:lang="es">inestable</status:term_status>
        <status:term_status xml:lang="en">unstable</status:term_status>
    </owl:ObjectProperty>
    


    <!-- http://vocab.gtfs.org/terms#routeType -->

    <owl:ObjectProperty rdf:about="http://vocab.gtfs.org/terms#routeType">
        <rdfs:domain rdf:resource="http://vocab.gtfs.org/terms#Route"/>
        <rdfs:range rdf:resource="http://vocab.gtfs.org/terms#RouteType"/>
        <rdfs:comment xml:lang="es">Enlaza al tipo de vehículo que opera en esta ruta</rdfs:comment>
        <rdfs:comment xml:lang="en">Links to the type of vehicle operating on this route</rdfs:comment>
        <rdfs:label xml:lang="en">Route type</rdfs:label>
        <rdfs:label xml:lang="es">tipo de ruta</rdfs:label>
        <rdfs:seeAlso rdf:resource="https://developers.google.com/transit/gtfs/examples/display-to-users#RouteType"/>
        <status:term_status xml:lang="es">inestable</status:term_status>
        <status:term_status xml:lang="en">unstable</status:term_status>
    </owl:ObjectProperty>
    


    <!-- http://vocab.gtfs.org/terms#service -->

    <owl:ObjectProperty rdf:about="http://vocab.gtfs.org/terms#service">
        <rdfs:range rdf:resource="http://vocab.gtfs.org/terms#Service"/>
        <rdfs:comment xml:lang="es">Cumple este gtfs:Service.</rdfs:comment>
        <rdfs:comment xml:lang="en">Follows this gtfs:Service.</rdfs:comment>
        <rdfs:label xml:lang="en">Service</rdfs:label>
        <rdfs:label xml:lang="es">Servicio</rdfs:label>
        <status:term_status xml:lang="es">inestable</status:term_status>
        <status:term_status xml:lang="en">unstable</status:term_status>
    </owl:ObjectProperty>
    


    <!-- http://vocab.gtfs.org/terms#serviceRule -->

    <owl:ObjectProperty rdf:about="http://vocab.gtfs.org/terms#serviceRule">
        <rdfs:domain rdf:resource="http://vocab.gtfs.org/terms#Service"/>
        <rdfs:range rdf:resource="http://vocab.gtfs.org/terms#ServiceRule"/>
        <rdfs:comment xml:lang="es">Reglas de servicio que definen un conjunto de fechas</rdfs:comment>
        <rdfs:comment xml:lang="en">Service rules which define together a set of dates</rdfs:comment>
        <rdfs:label xml:lang="en">Service rule</rdfs:label>
        <rdfs:label xml:lang="es">regla de servicio</rdfs:label>
        <status:term_status xml:lang="es">inestable</status:term_status>
        <status:term_status xml:lang="en">unstable</status:term_status>
    </owl:ObjectProperty>
    


    <!-- http://vocab.gtfs.org/terms#stop -->

    <owl:ObjectProperty rdf:about="http://vocab.gtfs.org/terms#stop">
        <rdfs:range rdf:resource="http://vocab.gtfs.org/terms#Stop"/>
        <rdfs:comment xml:lang="es">Indica que este concepto tiene cierta parada.</rdfs:comment>
        <rdfs:comment xml:lang="en">Indicates that this has a certain stop.</rdfs:comment>
        <rdfs:label xml:lang="en">Stop</rdfs:label>
        <rdfs:label xml:lang="es">parada</rdfs:label>
        <status:term_status xml:lang="es">inestable</status:term_status>
        <status:term_status xml:lang="en">unstable</status:term_status>
    </owl:ObjectProperty>
    


    <!-- http://vocab.gtfs.org/terms#trip -->

    <owl:ObjectProperty rdf:about="http://vocab.gtfs.org/terms#trip">
        <rdfs:range rdf:resource="http://vocab.gtfs.org/terms#Trip"/>
        <rdfs:comment xml:lang="es">Indica que este concepto es parte de cierto gtfs:Trip</rdfs:comment>
        <rdfs:comment xml:lang="en">Indicates that this is part of a certain gtfs:Trip</rdfs:comment>
        <rdfs:label xml:lang="en">Trip</rdfs:label>
        <rdfs:label xml:lang="es">viaje</rdfs:label>
        <status:term_status xml:lang="es">inestable</status:term_status>
        <status:term_status xml:lang="en">unstable</status:term_status>
    </owl:ObjectProperty>
    


    <!-- http://www.ontologydesignpatterns.org/ont/dul/DUL.owl#hasCommonBoundary -->

    <owl:ObjectProperty rdf:about="http://www.ontologydesignpatterns.org/ont/dul/DUL.owl#hasCommonBoundary">
        <owl:inverseOf rdf:resource="http://www.ontologydesignpatterns.org/ont/dul/DUL.owl#hasCommonBoundary"/>
        <rdf:type rdf:resource="http://www.w3.org/2002/07/owl#SymmetricProperty"/>
        <rdfs:domain rdf:resource="http://www.ontologydesignpatterns.org/ont/dul/DUL.owl#Entity"/>
        <rdfs:range rdf:resource="http://www.ontologydesignpatterns.org/ont/dul/DUL.owl#Entity"/>
        <rdfs:comment>A relation to encode either formal or informal characterizations of &apos;boundaries&apos; common to two different entities: an Event that ends when another begins, two abstract regions that have a common topological boundary, two objects that are said to be &apos;in contact&apos; from a commonsense perspective, etc.</rdfs:comment>
        <rdfs:label xml:lang="en">has common boundary</rdfs:label>
    </owl:ObjectProperty>
    


    <!-- http://www.ontologydesignpatterns.org/ont/dul/DUL.owl#hasConstituent -->

    <owl:ObjectProperty rdf:about="http://www.ontologydesignpatterns.org/ont/dul/DUL.owl#hasConstituent">
        <owl:inverseOf rdf:resource="http://www.ontologydesignpatterns.org/ont/dul/DUL.owl#isConstituentOf"/>
        <rdfs:domain rdf:resource="http://www.ontologydesignpatterns.org/ont/dul/DUL.owl#Entity"/>
        <rdfs:range rdf:resource="http://www.ontologydesignpatterns.org/ont/dul/DUL.owl#Entity"/>
        <rdfs:comment>&apos;Constituency&apos; depends on some layering of  the world described by the ontology. For example, scientific granularities (e.g. body-organ-tissue-cell) or ontological &apos;strata&apos; (e.g. social-mental-biological-physical) are  typical layerings. 
Intuitively, a constituent is a part belonging to a lower layer. Since layering is actually a partition of the world described by the ontology, constituents are not properly classified as parts, although this kinship can be intuitive for common sense.
A desirable advantage of this distinction is that we are able to talk e.g. of physical constituents of non-physical objects (e.g. systems), while this is not possible in terms of parts.
Example of are the persons constituting a social system, the molecules constituting a person, the atoms constituting a river, etc. 
In all these examples, we notice a typical discontinuity between the constituted and the constituent object: e.g. a social system is conceptualized at a different layer from the persons that constitute it, a person is conceptualized at a different layer from the molecules that constitute them, and a river is conceptualized at a different layer from the atoms that constitute it.</rdfs:comment>
        <rdfs:label xml:lang="it">ha costituente</rdfs:label>
        <rdfs:label xml:lang="en">has constituent</rdfs:label>
    </owl:ObjectProperty>
    


    <!-- http://www.ontologydesignpatterns.org/ont/dul/DUL.owl#hasLocation -->

    <owl:ObjectProperty rdf:about="http://www.ontologydesignpatterns.org/ont/dul/DUL.owl#hasLocation">
        <owl:inverseOf rdf:resource="http://www.ontologydesignpatterns.org/ont/dul/DUL.owl#isLocationOf"/>
        <rdfs:domain rdf:resource="http://www.ontologydesignpatterns.org/ont/dul/DUL.owl#Entity"/>
        <rdfs:range rdf:resource="http://www.ontologydesignpatterns.org/ont/dul/DUL.owl#Entity"/>
        <alignedWithIFC>IfcPlacement</alignedWithIFC>
        <rdfs:comment>A generic, relative localization, holding between any entities. E.g. &apos;the cat is on the mat&apos;, &apos;Omar is in Samarcanda&apos;, &apos;the wound is close to the femural artery&apos;.
For &apos;absolute&apos; locations, see SpaceRegion</rdfs:comment>
        <rdfs:label xml:lang="it">ha localizzazione</rdfs:label>
        <rdfs:label xml:lang="en">has location</rdfs:label>
    </owl:ObjectProperty>
    


    <!-- http://www.ontologydesignpatterns.org/ont/dul/DUL.owl#hasQuality -->

    <owl:ObjectProperty rdf:about="http://www.ontologydesignpatterns.org/ont/dul/DUL.owl#hasQuality">
        <owl:inverseOf rdf:resource="http://www.ontologydesignpatterns.org/ont/dul/DUL.owl#isQualityOf"/>
        <rdfs:domain rdf:resource="http://www.ontologydesignpatterns.org/ont/dul/DUL.owl#Entity"/>
        <rdfs:range rdf:resource="http://www.ontologydesignpatterns.org/ont/dul/DUL.owl#Quality"/>
        <rdfs:comment>A relation between entities and qualities, e.g. &apos;Dmitri&apos;s skin is yellowish&apos;.</rdfs:comment>
        <rdfs:label xml:lang="it">ha qualità</rdfs:label>
        <rdfs:label xml:lang="en">has quality</rdfs:label>
    </owl:ObjectProperty>
    


    <!-- http://www.ontologydesignpatterns.org/ont/dul/DUL.owl#isComponentOf -->

    <owl:ObjectProperty rdf:about="http://www.ontologydesignpatterns.org/ont/dul/DUL.owl#isComponentOf">
        <rdfs:subPropertyOf rdf:resource="http://www.ontologydesignpatterns.org/ont/dul/DUL.owl#isPartOf"/>
        <rdfs:domain rdf:resource="http://www.ontologydesignpatterns.org/ont/dul/DUL.owl#Object"/>
        <rdfs:range rdf:resource="http://www.ontologydesignpatterns.org/ont/dul/DUL.owl#Object"/>
        <rdfs:comment>The hasPart relation without transitivity, holding between an Object (the system) and another (the component), and assuming a Design that structures the Object.</rdfs:comment>
        <rdfs:label xml:lang="en">is component of</rdfs:label>
        <rdfs:label xml:lang="it">è componente di</rdfs:label>
    </owl:ObjectProperty>
    


    <!-- http://www.ontologydesignpatterns.org/ont/dul/DUL.owl#isConstituentOf -->

    <owl:ObjectProperty rdf:about="http://www.ontologydesignpatterns.org/ont/dul/DUL.owl#isConstituentOf">
        <rdfs:domain rdf:resource="http://www.ontologydesignpatterns.org/ont/dul/DUL.owl#Entity"/>
        <rdfs:range rdf:resource="http://www.ontologydesignpatterns.org/ont/dul/DUL.owl#Entity"/>
        <rdfs:comment>&apos;Constituency&apos; depends on some layering of  the world described by the ontology. For example, scientific granularities (e.g. body-organ-tissue-cell) or ontological &apos;strata&apos; (e.g. social-mental-biological-physical) are  typical layerings. 
Intuitively, a constituent is a part belonging to a lower layer. Since layering is actually a partition of the world described by the ontology, constituents are not properly classified as parts, although this kinship can be intuitive for common sense.
A desirable advantage of this distinction is that we are able to talk e.g. of physical constituents of non-physical objects (e.g. systems), while this is not possible in terms of parts.
Example of are the persons constituting a social system, the molecules constituting a person, the atoms constituting a river, etc. 
In all these examples, we notice a typical discontinuity between the constituted and the constituent object: e.g. a social system is conceptualized at a different layer from the persons that constitute it, a person is conceptualized at a different layer from the molecules that constitute them, and a river is conceptualized at a different layer from the atoms that constitute it.</rdfs:comment>
        <rdfs:label xml:lang="en">is constituent of</rdfs:label>
        <rdfs:label xml:lang="it">è costituente di</rdfs:label>
    </owl:ObjectProperty>
    


    <!-- http://www.ontologydesignpatterns.org/ont/dul/DUL.owl#isLocationOf -->

    <owl:ObjectProperty rdf:about="http://www.ontologydesignpatterns.org/ont/dul/DUL.owl#isLocationOf">
        <rdfs:domain rdf:resource="http://www.ontologydesignpatterns.org/ont/dul/DUL.owl#Entity"/>
        <rdfs:range rdf:resource="http://www.ontologydesignpatterns.org/ont/dul/DUL.owl#Entity"/>
        <rdfs:comment>A generic, relative localization, holding between any entities. E.g. &apos;Rome is the seat of the Pope&apos;, &apos;the liver is the location of the tumor&apos;.
For &apos;absolute&apos; locations, see SpaceRegion</rdfs:comment>
        <rdfs:label xml:lang="en">is location of</rdfs:label>
        <rdfs:label xml:lang="it">è una localizzazione di</rdfs:label>
    </owl:ObjectProperty>
    


    <!-- http://www.ontologydesignpatterns.org/ont/dul/DUL.owl#isPartOf -->

    <owl:ObjectProperty rdf:about="http://www.ontologydesignpatterns.org/ont/dul/DUL.owl#isPartOf">
        <rdf:type rdf:resource="http://www.w3.org/2002/07/owl#TransitiveProperty"/>
        <rdfs:domain rdf:resource="http://www.ontologydesignpatterns.org/ont/dul/DUL.owl#Entity"/>
        <rdfs:range rdf:resource="http://www.ontologydesignpatterns.org/ont/dul/DUL.owl#Entity"/>
        <rdfs:comment rdf:datatype="http://www.w3.org/2001/XMLSchema#string">A relation between any entities, e.g.&apos;brain is a part of the human body&apos;.</rdfs:comment>
        <rdfs:label xml:lang="en">is part of</rdfs:label>
        <rdfs:label xml:lang="it">è parte di</rdfs:label>
    </owl:ObjectProperty>
    


    <!-- http://www.ontologydesignpatterns.org/ont/dul/DUL.owl#isQualityOf -->

    <owl:ObjectProperty rdf:about="http://www.ontologydesignpatterns.org/ont/dul/DUL.owl#isQualityOf">
        <rdfs:domain rdf:resource="http://www.ontologydesignpatterns.org/ont/dul/DUL.owl#Quality"/>
        <rdfs:range rdf:resource="http://www.ontologydesignpatterns.org/ont/dul/DUL.owl#Entity"/>
        <rdfs:comment>A relation between entities and qualities, e.g. &apos;Dmitri&apos;s skin is yellowish&apos;.</rdfs:comment>
        <rdfs:label xml:lang="en">is quality of</rdfs:label>
        <rdfs:label xml:lang="it">è una qualità di</rdfs:label>
    </owl:ObjectProperty>
    


    <!-- http://www.semanticwater.com/WISDOM#affectedByProblem -->

    <owl:ObjectProperty rdf:about="http://www.semanticwater.com/WISDOM#affectedByProblem">
        <owl:inverseOf rdf:resource="http://www.semanticwater.com/WISDOM#affectsEntity"/>
        <rdfs:domain rdf:resource="http://www.semanticwater.com/WISDOM#PhysicalTopologicalEntity"/>
    </owl:ObjectProperty>
    


    <!-- http://www.semanticwater.com/WISDOM#affectsEntity -->

    <owl:ObjectProperty rdf:about="http://www.semanticwater.com/WISDOM#affectsEntity">
        <rdfs:range rdf:resource="http://www.semanticwater.com/WISDOM#PhysicalTopologicalEntity"/>
    </owl:ObjectProperty>
    


    <!-- http://www.semanticwater.com/WISDOM#atAsset -->

    <owl:ObjectProperty rdf:about="http://www.semanticwater.com/WISDOM#atAsset">
        <rdfs:subPropertyOf rdf:resource="http://www.ontologydesignpatterns.org/ont/dul/DUL.owl#hasLocation"/>
    </owl:ObjectProperty>
    


    <!-- http://www.semanticwater.com/WISDOM#containsDevice -->

    <owl:ObjectProperty rdf:about="http://www.semanticwater.com/WISDOM#containsDevice">
        <owl:inverseOf rdf:resource="http://www.semanticwater.com/WISDOM#isSituatedAtEntity"/>
        <rdf:type rdf:resource="http://www.w3.org/2002/07/owl#InverseFunctionalProperty"/>
        <rdf:type rdf:resource="http://www.w3.org/2002/07/owl#AsymmetricProperty"/>
        <rdf:type rdf:resource="http://www.w3.org/2002/07/owl#IrreflexiveProperty"/>
        <rdfs:domain rdf:resource="http://www.ontologydesignpatterns.org/ont/dul/DUL.owl#Entity"/>
        <rdfs:range rdf:resource="http://purl.oclc.org/NET/ssnx/ssn#Device"/>
    </owl:ObjectProperty>
    


    <!-- http://www.semanticwater.com/WISDOM#controlsArtefact -->

    <owl:ObjectProperty rdf:about="http://www.semanticwater.com/WISDOM#controlsArtefact">
        <owl:inverseOf rdf:resource="http://www.semanticwater.com/WISDOM#isControledBy"/>
        <rdf:type rdf:resource="http://www.w3.org/2002/07/owl#AsymmetricProperty"/>
        <rdf:type rdf:resource="http://www.w3.org/2002/07/owl#IrreflexiveProperty"/>
        <rdfs:range rdf:resource="http://www.semanticwater.com/WISDOM#PhysicalArc"/>
        <rdfs:range rdf:resource="http://www.semanticwater.com/WISDOM#PhysicalNode"/>
    </owl:ObjectProperty>
    


    <!-- http://www.semanticwater.com/WISDOM#deployedAtEntity -->

    <owl:ObjectProperty rdf:about="http://www.semanticwater.com/WISDOM#deployedAtEntity">
        <owl:inverseOf rdf:resource="http://www.semanticwater.com/WISDOM#hasDeployedSensor"/>
        <rdfs:domain rdf:resource="http://www.semanticwater.com/WISDOM#WaterSensor"/>
        <rdfs:range>
            <owl:Class>
                <owl:unionOf rdf:parseType="Collection">
                    <rdf:Description rdf:about="http://www.semanticwater.com/WISDOM#PhysicalArc"/>
                    <rdf:Description rdf:about="http://www.semanticwater.com/WISDOM#PhysicalNode"/>
                </owl:unionOf>
            </owl:Class>
        </rdfs:range>
    </owl:ObjectProperty>
    


    <!-- http://www.semanticwater.com/WISDOM#forProperty -->

    <owl:ObjectProperty rdf:about="http://www.semanticwater.com/WISDOM#forProperty"/>
    


    <!-- http://www.semanticwater.com/WISDOM#hasArcProperty -->

    <owl:ObjectProperty rdf:about="http://www.semanticwater.com/WISDOM#hasArcProperty">
        <rdfs:subPropertyOf rdf:resource="http://www.semanticwater.com/WISDOM#hasNetworkProperty"/>
    </owl:ObjectProperty>
    


    <!-- http://www.semanticwater.com/WISDOM#hasDeployedSensor -->

    <owl:ObjectProperty rdf:about="http://www.semanticwater.com/WISDOM#hasDeployedSensor">
        <rdf:type rdf:resource="http://www.w3.org/2002/07/owl#InverseFunctionalProperty"/>
        <rdf:type rdf:resource="http://www.w3.org/2002/07/owl#AsymmetricProperty"/>
        <rdf:type rdf:resource="http://www.w3.org/2002/07/owl#IrreflexiveProperty"/>
        <rdfs:range rdf:resource="http://purl.oclc.org/NET/ssnx/ssn#Sensor"/>
    </owl:ObjectProperty>
    


    <!-- http://www.semanticwater.com/WISDOM#hasDownstreamEntity -->

    <owl:ObjectProperty rdf:about="http://www.semanticwater.com/WISDOM#hasDownstreamEntity">
        <rdfs:subPropertyOf rdf:resource="http://www.semanticwater.com/WISDOM#hasPhysicalNetworkRelationship"/>
        <owl:inverseOf rdf:resource="http://www.semanticwater.com/WISDOM#hasUpstreamEntity"/>
        <rdf:type rdf:resource="http://www.w3.org/2002/07/owl#TransitiveProperty"/>
        <rdfs:domain rdf:resource="http://www.semanticwater.com/WISDOM#PhysicalTopologicalEntity"/>
        <rdfs:range rdf:resource="http://www.semanticwater.com/WISDOM#PhysicalTopologicalEntity"/>
    </owl:ObjectProperty>
    


    <!-- http://www.semanticwater.com/WISDOM#hasFeatureOfInterest -->

    <owl:ObjectProperty rdf:about="http://www.semanticwater.com/WISDOM#hasFeatureOfInterest"/>
    


    <!-- http://www.semanticwater.com/WISDOM#hasMaterial -->

    <owl:ObjectProperty rdf:about="http://www.semanticwater.com/WISDOM#hasMaterial">
        <rdf:type rdf:resource="http://www.w3.org/2002/07/owl#FunctionalProperty"/>
        <rdf:type rdf:resource="http://www.w3.org/2002/07/owl#AsymmetricProperty"/>
        <rdf:type rdf:resource="http://www.w3.org/2002/07/owl#IrreflexiveProperty"/>
        <rdfs:range rdf:resource="http://www.semanticwater.com/WISDOM#Material"/>
        <rdfs:label xml:lang="en">hasMaterial</rdfs:label>
    </owl:ObjectProperty>
    


    <!-- http://www.semanticwater.com/WISDOM#hasMeasurementCapability -->

    <owl:ObjectProperty rdf:about="http://www.semanticwater.com/WISDOM#hasMeasurementCapability">
        <rdfs:subPropertyOf rdf:resource="http://purl.oclc.org/NET/ssnx/ssn#hasProperty"/>
    </owl:ObjectProperty>
    


    <!-- http://www.semanticwater.com/WISDOM#hasNetworkProperty -->

    <owl:ObjectProperty rdf:about="http://www.semanticwater.com/WISDOM#hasNetworkProperty">
        <rdfs:domain rdf:resource="http://www.semanticwater.com/WISDOM#PhysicalTopologicalEntity"/>
        <rdfs:range rdf:resource="http://www.semanticwater.com/WISDOM#WaterNetworkProperty"/>
    </owl:ObjectProperty>
    


    <!-- http://www.semanticwater.com/WISDOM#hasNetworkRelationship -->

    <owl:ObjectProperty rdf:about="http://www.semanticwater.com/WISDOM#hasNetworkRelationship">
        <rdfs:subPropertyOf rdf:resource="http://www.w3.org/2002/07/owl#topObjectProperty"/>
    </owl:ObjectProperty>
    


    <!-- http://www.semanticwater.com/WISDOM#hasPhysicalNetworkRelationship -->

    <owl:ObjectProperty rdf:about="http://www.semanticwater.com/WISDOM#hasPhysicalNetworkRelationship">
        <rdfs:subPropertyOf rdf:resource="http://www.semanticwater.com/WISDOM#hasNetworkRelationship"/>
        <rdfs:domain rdf:resource="http://www.semanticwater.com/WISDOM#PhysicalTopologicalEntity"/>
        <rdfs:range rdf:resource="http://www.semanticwater.com/WISDOM#PhysicalTopologicalEntity"/>
    </owl:ObjectProperty>
    


    <!-- http://www.semanticwater.com/WISDOM#hasPipeShape -->

    <owl:ObjectProperty rdf:about="http://www.semanticwater.com/WISDOM#hasPipeShape">
        <rdfs:subPropertyOf rdf:resource="http://www.semanticwater.com/WISDOM#hasArcProperty"/>
        <rdf:type rdf:resource="http://www.w3.org/2002/07/owl#FunctionalProperty"/>
        <rdf:type rdf:resource="http://www.w3.org/2002/07/owl#AsymmetricProperty"/>
        <rdf:type rdf:resource="http://www.w3.org/2002/07/owl#IrreflexiveProperty"/>
        <rdfs:domain rdf:resource="http://www.semanticwater.com/WISDOM#Arc"/>
        <rdfs:range rdf:resource="http://www.semanticwater.com/WISDOM#PipeShape"/>
    </owl:ObjectProperty>
    


    <!-- http://www.semanticwater.com/WISDOM#hasProblem -->

    <owl:ObjectProperty rdf:about="http://www.semanticwater.com/WISDOM#hasProblem">
        <rdfs:subPropertyOf rdf:resource="http://www.semanticwater.com/WISDOM#affectedByProblem"/>
        <owl:inverseOf rdf:resource="http://www.semanticwater.com/WISDOM#isAtEntity"/>
        <rdfs:domain>
            <owl:Class>
                <owl:unionOf rdf:parseType="Collection">
                    <rdf:Description rdf:about="http://purl.oclc.org/NET/ssnx/ssn#Device"/>
                    <rdf:Description rdf:about="http://www.semanticwater.com/WISDOM#DesignedAsset"/>
                    <rdf:Description rdf:about="http://www.semanticwater.com/WISDOM#PhysicalTopologicalEntity"/>
                </owl:unionOf>
            </owl:Class>
        </rdfs:domain>
    </owl:ObjectProperty>
    


    <!-- http://www.semanticwater.com/WISDOM#hasSensedNetworkProperty -->

    <owl:ObjectProperty rdf:about="http://www.semanticwater.com/WISDOM#hasSensedNetworkProperty">
        <rdfs:subPropertyOf rdf:resource="http://www.semanticwater.com/WISDOM#hasNetworkProperty"/>
    </owl:ObjectProperty>
    


    <!-- http://www.semanticwater.com/WISDOM#hasUpstreamEntity -->

    <owl:ObjectProperty rdf:about="http://www.semanticwater.com/WISDOM#hasUpstreamEntity">
        <rdfs:subPropertyOf rdf:resource="http://www.semanticwater.com/WISDOM#hasPhysicalNetworkRelationship"/>
        <rdf:type rdf:resource="http://www.w3.org/2002/07/owl#TransitiveProperty"/>
        <rdfs:domain rdf:resource="http://www.semanticwater.com/WISDOM#PhysicalTopologicalEntity"/>
        <rdfs:range rdf:resource="http://www.semanticwater.com/WISDOM#PhysicalTopologicalEntity"/>
    </owl:ObjectProperty>
    


    <!-- http://www.semanticwater.com/WISDOM#isAtEntity -->

    <owl:ObjectProperty rdf:about="http://www.semanticwater.com/WISDOM#isAtEntity">
        <rdfs:subPropertyOf rdf:resource="http://www.semanticwater.com/WISDOM#affectsEntity"/>
    </owl:ObjectProperty>
    


    <!-- http://www.semanticwater.com/WISDOM#isControledBy -->

    <owl:ObjectProperty rdf:about="http://www.semanticwater.com/WISDOM#isControledBy">
        <rdf:type rdf:resource="http://www.w3.org/2002/07/owl#AsymmetricProperty"/>
        <rdf:type rdf:resource="http://www.w3.org/2002/07/owl#IrreflexiveProperty"/>
        <rdfs:domain rdf:resource="http://www.ontologydesignpatterns.org/ont/dul/DUL.owl#DesignedArtifact"/>
    </owl:ObjectProperty>
    


    <!-- http://www.semanticwater.com/WISDOM#isSituatedAtEntity -->

    <owl:ObjectProperty rdf:about="http://www.semanticwater.com/WISDOM#isSituatedAtEntity">
        <rdf:type rdf:resource="http://www.w3.org/2002/07/owl#FunctionalProperty"/>
        <rdf:type rdf:resource="http://www.w3.org/2002/07/owl#AsymmetricProperty"/>
        <rdf:type rdf:resource="http://www.w3.org/2002/07/owl#IrreflexiveProperty"/>
        <rdfs:domain rdf:resource="http://purl.oclc.org/NET/ssnx/ssn#Device"/>
        <rdfs:range rdf:resource="http://www.semanticwater.com/WISDOM#PhysicalArc"/>
        <rdfs:range rdf:resource="http://www.semanticwater.com/WISDOM#PhysicalNode"/>
    </owl:ObjectProperty>
    


    <!-- http://www.semanticwater.com/WISDOM#observesWaterProperty -->

    <owl:ObjectProperty rdf:about="http://www.semanticwater.com/WISDOM#observesWaterProperty">
        <rdfs:subPropertyOf rdf:resource="http://purl.oclc.org/NET/ssnx/ssn#observes"/>
        <rdf:type rdf:resource="http://www.w3.org/2002/07/owl#FunctionalProperty"/>
        <rdf:type rdf:resource="http://www.w3.org/2002/07/owl#AsymmetricProperty"/>
        <rdf:type rdf:resource="http://www.w3.org/2002/07/owl#IrreflexiveProperty"/>
        <rdfs:domain rdf:resource="http://www.semanticwater.com/WISDOM#WaterSensor"/>
        <rdfs:range rdf:resource="http://www.semanticwater.com/WISDOM#WaterNetworkProperty"/>
    </owl:ObjectProperty>
    


    <!-- http://www.w3.org/2003/01/geo/wgs84_pos#location -->

    <owl:ObjectProperty rdf:about="http://www.w3.org/2003/01/geo/wgs84_pos#location">
        <rdfs:range rdf:resource="http://www.w3.org/2003/01/geo/wgs84_pos#SpatialThing"/>
    </owl:ObjectProperty>
    


    <!-- http://www.w3.org/ns/org#siteAddress -->

    <rdf:Description rdf:about="http://www.w3.org/ns/org#siteAddress">
        <rdfs:range rdf:resource="http://www.w3.org/ns/locn#Address"/>
    </rdf:Description>
    


    <!-- 
    ///////////////////////////////////////////////////////////////////////////////////////
    //
    // Data properties
    //
    ///////////////////////////////////////////////////////////////////////////////////////
     -->

    


    <!-- http://harmonet.org/harmonise.rdfs#awardAchieved -->

    <owl:DatatypeProperty rdf:about="http://harmonet.org/harmonise.rdfs#awardAchieved">
        <rdfs:domain rdf:resource="http://harmonet.org/harmonise.rdfs#Award"/>
        <rdfs:range rdf:resource="http://www.w3.org/2000/01/rdf-schema#Literal"/>
    </owl:DatatypeProperty>
    


    <!-- http://harmonet.org/harmonise.rdfs#awardingBody -->

    <owl:DatatypeProperty rdf:about="http://harmonet.org/harmonise.rdfs#awardingBody">
        <rdfs:domain rdf:resource="http://harmonet.org/harmonise.rdfs#Award"/>
        <rdfs:range rdf:resource="http://www.w3.org/2000/01/rdf-schema#Literal"/>
    </owl:DatatypeProperty>
    


    <!-- http://harmonet.org/harmonise.rdfs#domainValue -->

    <owl:DatatypeProperty rdf:about="http://harmonet.org/harmonise.rdfs#domainValue">
        <rdfs:domain rdf:resource="http://harmonet.org/harmonise.rdfs#ReferencedValue"/>
        <rdfs:range rdf:resource="http://www.w3.org/2000/01/rdf-schema#Literal"/>
        <rdfs:label>domainValue</rdfs:label>
    </owl:DatatypeProperty>
    


    <!-- http://harmonet.org/harmonise.rdfs#fieldName -->

    <owl:DatatypeProperty rdf:about="http://harmonet.org/harmonise.rdfs#fieldName">
        <rdfs:domain rdf:resource="http://harmonet.org/harmonise.rdfs#ProfileField"/>
        <rdfs:range rdf:resource="http://www.w3.org/2000/01/rdf-schema#Literal"/>
    </owl:DatatypeProperty>
    


    <!-- http://harmonet.org/harmonise.rdfs#fieldValue -->

    <owl:DatatypeProperty rdf:about="http://harmonet.org/harmonise.rdfs#fieldValue">
        <rdfs:domain rdf:resource="http://harmonet.org/harmonise.rdfs#ProfileField"/>
        <rdfs:range rdf:resource="http://www.w3.org/2000/01/rdf-schema#Literal"/>
    </owl:DatatypeProperty>
    


    <!-- http://harmonet.org/harmonise.rdfs#year -->

    <owl:DatatypeProperty rdf:about="http://harmonet.org/harmonise.rdfs#year">
        <rdfs:domain rdf:resource="http://harmonet.org/harmonise.rdfs#Date"/>
        <rdfs:range rdf:resource="http://www.w3.org/2000/01/rdf-schema#Literal"/>
        <rdfs:label>year</rdfs:label>
    </owl:DatatypeProperty>
    


    <!-- http://opendata.aragon.es/def/ei2a#CIA -->

    <owl:DatatypeProperty rdf:about="http://opendata.aragon.es/def/ei2a#CIA">
        <rdfs:domain rdf:resource="http://www.w3.org/ns/person#Person"/>
        <rdfs:range rdf:resource="http://www.w3.org/2000/01/rdf-schema#Literal"/>
        <rdfs:comment xml:lang="es">Código de Identificación Autonómico</rdfs:comment>
        <rdfs:comment xml:lang="en">Regional Identification Code</rdfs:comment>
    </owl:DatatypeProperty>
    


    <!-- http://opendata.aragon.es/def/ei2a#CIF -->

    <owl:DatatypeProperty rdf:about="http://opendata.aragon.es/def/ei2a#CIF">
        <rdfs:domain>
            <owl:Class>
                <owl:unionOf rdf:parseType="Collection">
                    <rdf:Description rdf:about="http://www.w3.org/ns/org#Organization"/>
                    <rdf:Description rdf:about="http://www.w3.org/ns/org#Site"/>
                </owl:unionOf>
            </owl:Class>
        </rdfs:domain>
        <rdfs:range rdf:resource="http://www.w3.org/2000/01/rdf-schema#Literal"/>
        <rdfs:comment xml:lang="es">Código de Identificación Fiscal</rdfs:comment>
        <rdfs:comment xml:lang="en">Fiscal Identification Code</rdfs:comment>
    </owl:DatatypeProperty>
    


    <!-- http://opendata.aragon.es/def/ei2a#CNAE -->

    <owl:DatatypeProperty rdf:about="http://opendata.aragon.es/def/ei2a#CNAE">
        <rdfs:domain rdf:resource="http://www.w3.org/ns/org#Organization"/>
        <rdfs:range rdf:resource="http://www.w3.org/2000/01/rdf-schema#Literal"/>
        <rdfs:comment xml:lang="es">Código Nacional de Actividades Económicas</rdfs:comment>
        <rdfs:comment xml:lang="en">National Code of Economic Activities</rdfs:comment>
    </owl:DatatypeProperty>
    


    <!-- http://opendata.aragon.es/def/ei2a#CSV -->

    <owl:DatatypeProperty rdf:about="http://opendata.aragon.es/def/ei2a#CSV">
        <rdfs:domain rdf:resource="http://opendata.aragon.es/def/ei2a#Document"/>
        <rdfs:range rdf:resource="http://www.w3.org/2000/01/rdf-schema#Literal"/>
        <rdfs:comment xml:lang="en">Electronic signature value of electronic document in CSV format.</rdfs:comment>
        <rdfs:comment xml:lang="es">Valor de la firma electrónica del documento electrónico en formato CSV</rdfs:comment>
    </owl:DatatypeProperty>
    


    <!-- http://opendata.aragon.es/def/ei2a#CSVScheme -->

    <owl:DatatypeProperty rdf:about="http://opendata.aragon.es/def/ei2a#CSVScheme">
        <rdfs:domain rdf:resource="http://opendata.aragon.es/def/ei2a#Document"/>
        <rdfs:range rdf:resource="http://www.w3.org/2000/01/rdf-schema#Literal"/>
        <rdfs:comment xml:lang="en">Document which defines CSV signature&apos;s creation.</rdfs:comment>
        <rdfs:comment xml:lang="es">Resolución o documento que define la creación del CSV correspondiente.</rdfs:comment>
    </owl:DatatypeProperty>
    


    <!-- http://opendata.aragon.es/def/ei2a#DIR3Code -->

    <owl:DatatypeProperty rdf:about="http://opendata.aragon.es/def/ei2a#DIR3Code">
        <rdfs:domain rdf:resource="http://www.w3.org/ns/org#Organization"/>
        <rdfs:range rdf:resource="http://www.w3.org/2000/01/rdf-schema#Literal"/>
        <rdfs:comment xml:lang="en">An alphanumeric code that uniquely identifies a unit or office within the public administration.

The code of organic units and offices is formed by a alphanumeric literal of 9 positions, of which the first letter is used to identify the administration to which it belongs according to Law 39/2015.</rdfs:comment>
        <rdfs:comment xml:lang="es">Código alfanumérico que identifica de forma unívoca una unidad u oficina dentro de la administración pública.

El código de unidades orgánicas y oficinas está formado por un literal alfanumérico de 9 posiciones, de los cuales, la primera letra se utilizar para identificar la administración a la que pertenece según la Ley 39/2015.</rdfs:comment>
    </owl:DatatypeProperty>
    


    <!-- http://opendata.aragon.es/def/ei2a#NASS -->

    <owl:DatatypeProperty rdf:about="http://opendata.aragon.es/def/ei2a#NASS">
        <rdfs:domain rdf:resource="http://www.w3.org/ns/person#Person"/>
        <rdfs:range rdf:resource="http://www.w3.org/2000/01/rdf-schema#Literal"/>
        <rdfs:comment xml:lang="es">Número de Afiliación a la Seguridad Social</rdfs:comment>
        <rdfs:comment xml:lang="en">Social Security Membership Number</rdfs:comment>
    </owl:DatatypeProperty>
    


    <!-- http://opendata.aragon.es/def/ei2a#NIE -->

    <owl:DatatypeProperty rdf:about="http://opendata.aragon.es/def/ei2a#NIE">
        <rdfs:domain rdf:resource="http://www.w3.org/ns/person#Person"/>
        <rdfs:range rdf:resource="http://www.w3.org/2000/01/rdf-schema#Literal"/>
        <rdfs:comment xml:lang="en">Foreign Identity Number (NIE)</rdfs:comment>
        <rdfs:comment xml:lang="es">Número de Identidad de Extranjero (NIE)</rdfs:comment>
    </owl:DatatypeProperty>
    


    <!-- http://opendata.aragon.es/def/ei2a#NIF -->

    <owl:DatatypeProperty rdf:about="http://opendata.aragon.es/def/ei2a#NIF">
        <rdfs:domain rdf:resource="http://www.w3.org/ns/person#Person"/>
        <rdfs:range rdf:resource="http://www.w3.org/2000/01/rdf-schema#Literal"/>
        <rdfs:comment xml:lang="es">Número de Identificación Fiscal (NIF) que permite la identificación tributaria utilizada en España para las personas físicas, con documento nacional de identidad (DNI) o número de identificación de extranjero (NIE) asignados por el Ministerio del Interior, y las personas jurídicas. El antecedente del NIF es el CIF, utilizado en personas jurídicas</rdfs:comment>
        <rdfs:comment xml:lang="en">Tax identification number (NIF) that allows the tax identification used in Spain for natural persons, with a national identity card (DNI) or foreign identification number (NIE) assigned by the Ministry of the Interior, and legal entities. The antecedent of the NIF is the CIF, used in legal entities</rdfs:comment>
    </owl:DatatypeProperty>
    


    <!-- http://opendata.aragon.es/def/ei2a#NIRI -->

    <owl:DatatypeProperty rdf:about="http://opendata.aragon.es/def/ei2a#NIRI">
        <rdfs:domain rdf:resource="http://www.w3.org/ns/org#Organization"/>
        <rdfs:range rdf:resource="http://www.w3.org/2000/01/rdf-schema#Literal"/>
        <rdfs:comment xml:lang="es">Número de Inscripción en el Registro Industrial</rdfs:comment>
        <rdfs:comment xml:lang="en">Registration Number in the Industrial Registry</rdfs:comment>
    </owl:DatatypeProperty>
    


    <!-- http://opendata.aragon.es/def/ei2a#NTIVersion -->

    <owl:DatatypeProperty rdf:about="http://opendata.aragon.es/def/ei2a#NTIVersion">
        <rdfs:domain rdf:resource="http://opendata.aragon.es/def/ei2a#Document"/>
        <rdfs:range rdf:resource="http://www.w3.org/2001/XMLSchema#anyURI"/>
        <rdfs:comment xml:lang="es">Identificador normalizado de la versión de la Norma Técnica de Interoperabilidad (NTI) de Expediente electrónico conforme a la cual se estructura el expediente

http://administracionelectronica.gob.es/ENI/XSD/v1.0/expediente-e</rdfs:comment>
        <rdfs:comment xml:lang="en">Standardized identifier of the version of the

Identificador normalizado de la versión de la Norma Técnica de Interoperabilidad (NTI) de Expediente electrónico conforme a la cual se estructura el expediente

http://administracionelectronica.gob.es/ENI/XSD/v1.0/expediente-e</rdfs:comment>
    </owl:DatatypeProperty>
    


    <!-- http://opendata.aragon.es/def/ei2a#SIUCode -->

    <owl:DatatypeProperty rdf:about="http://opendata.aragon.es/def/ei2a#SIUCode">
        <rdfs:domain rdf:resource="http://www.w3.org/ns/org#Organization"/>
        <rdfs:range rdf:resource="http://www.w3.org/2000/01/rdf-schema#Literal"/>
        <rdfs:comment xml:lang="en">Code of an organism within the User Identification System of Aragon (SIU)</rdfs:comment>
        <rdfs:comment xml:lang="es">Código de un organismo dentro del Sistema de Identificación de Usuarios de Aragón (SIU)</rdfs:comment>
    </owl:DatatypeProperty>
    


    <!-- http://opendata.aragon.es/def/ei2a#URIDocument -->

    <owl:DatatypeProperty rdf:about="http://opendata.aragon.es/def/ei2a#URIDocument">
        <rdfs:domain rdf:resource="http://opendata.aragon.es/def/ei2a#Document"/>
        <rdfs:range rdf:resource="http://www.w3.org/2001/XMLSchema#anyURI"/>
        <rdfs:comment xml:lang="en">Document URI</rdfs:comment>
        <rdfs:comment xml:lang="es">URI del documento</rdfs:comment>
    </owl:DatatypeProperty>
    


    <!-- http://opendata.aragon.es/def/ei2a#URL -->

    <owl:DatatypeProperty rdf:about="http://opendata.aragon.es/def/ei2a#URL">
        <rdfs:domain>
            <owl:Class>
                <owl:unionOf rdf:parseType="Collection">
                    <rdf:Description rdf:about="http://opendata.aragon.es/def/ei2a#SocialMedia"/>
                    <rdf:Description rdf:about="http://opendata.aragon.es/def/ei2a#WebPage"/>
                </owl:unionOf>
            </owl:Class>
        </rdfs:domain>
        <rdfs:range rdf:resource="http://www.w3.org/2000/01/rdf-schema#Literal"/>
        <rdfs:comment xml:lang="en">Address that serves to accurately locate a web, subdomain or portal</rdfs:comment>
        <rdfs:comment xml:lang="es">Ruta o dirección que sirve para ubicar de manera precisa una web, subdominio o portal</rdfs:comment>
    </owl:DatatypeProperty>
    


    <!-- http://opendata.aragon.es/def/ei2a#URLVerification -->

    <owl:DatatypeProperty rdf:about="http://opendata.aragon.es/def/ei2a#URLVerification">
        <rdfs:domain rdf:resource="http://opendata.aragon.es/def/ei2a#Document"/>
        <rdfs:range rdf:resource="http://www.w3.org/2001/XMLSchema#anyURI"/>
        <rdfs:comment xml:lang="en">Document verification url</rdfs:comment>
        <rdfs:comment xml:lang="es">URL de verificación de documentos</rdfs:comment>
    </owl:DatatypeProperty>
    


    <!-- http://opendata.aragon.es/def/ei2a#accuracy -->

    <owl:DatatypeProperty rdf:about="http://opendata.aragon.es/def/ei2a#accuracy">
        <rdfs:domain rdf:resource="http://opendata.aragon.es/def/ei2a#SocialMedia"/>
        <rdfs:range rdf:resource="http://www.w3.org/2000/01/rdf-schema#Literal"/>
        <rdfs:comment xml:lang="en">Accuracy of social communication</rdfs:comment>
        <rdfs:comment xml:lang="es">Precisión de la comunicación social</rdfs:comment>
    </owl:DatatypeProperty>
    


    <!-- http://opendata.aragon.es/def/ei2a#addressName -->

    <owl:DatatypeProperty rdf:about="http://opendata.aragon.es/def/ei2a#addressName">
        <rdfs:domain rdf:resource="http://www.w3.org/ns/locn#Address"/>
        <rdfs:range rdf:resource="http://www.w3.org/2000/01/rdf-schema#Literal"/>
        <rdfs:comment xml:lang="en">Address name.</rdfs:comment>
        <rdfs:comment xml:lang="es">Nombre de la dirección. Nombre de la calle, vía, paseo...</rdfs:comment>
    </owl:DatatypeProperty>
    


    <!-- http://opendata.aragon.es/def/ei2a#addressNumber -->

    <owl:DatatypeProperty rdf:about="http://opendata.aragon.es/def/ei2a#addressNumber">
        <rdfs:domain rdf:resource="http://www.w3.org/ns/locn#Address"/>
        <rdfs:range rdf:resource="http://www.w3.org/2000/01/rdf-schema#Literal"/>
        <rdfs:comment xml:lang="en">Address number.</rdfs:comment>
        <rdfs:comment xml:lang="es">Número de la dirección</rdfs:comment>
    </owl:DatatypeProperty>
    


    <!-- http://opendata.aragon.es/def/ei2a#addressType -->

    <owl:DatatypeProperty rdf:about="http://opendata.aragon.es/def/ei2a#addressType">
        <rdfs:domain rdf:resource="http://www.w3.org/ns/locn#Address"/>
        <rdfs:range rdf:resource="http://www.w3.org/2000/01/rdf-schema#Literal"/>
        <rdfs:comment xml:lang="en">Address Type (street, square, avenue, ...)</rdfs:comment>
        <rdfs:comment xml:lang="es">Tipo de vía (calle, plaza, avenida, etc.)</rdfs:comment>
    </owl:DatatypeProperty>
    


    <!-- http://opendata.aragon.es/def/ei2a#adminUnitL1 -->

    <owl:DatatypeProperty rdf:about="http://opendata.aragon.es/def/ei2a#adminUnitL1">
        <rdfs:domain rdf:resource="http://www.w3.org/ns/locn#Address"/>
        <rdfs:range rdf:resource="http://www.w3.org/2000/01/rdf-schema#Literal"/>
        <rdfs:comment xml:lang="en">Administrative Unit Level 1.
Country.</rdfs:comment>
        <rdfs:comment xml:lang="es">Unidad administrativa de nivel 1.
País</rdfs:comment>
    </owl:DatatypeProperty>
    


    <!-- http://opendata.aragon.es/def/ei2a#adminUnitL2 -->

    <owl:DatatypeProperty rdf:about="http://opendata.aragon.es/def/ei2a#adminUnitL2">
        <rdfs:domain rdf:resource="http://www.w3.org/ns/locn#Address"/>
        <rdfs:range rdf:resource="http://www.w3.org/2000/01/rdf-schema#Literal"/>
        <rdfs:comment xml:lang="en">Administrative unit level 2.
Region</rdfs:comment>
        <rdfs:comment xml:lang="es">Unidad Administrativa de nivel 2.
Comunidad Autónoma</rdfs:comment>
    </owl:DatatypeProperty>
    


    <!-- http://opendata.aragon.es/def/ei2a#adminUnitL3 -->

    <owl:DatatypeProperty rdf:about="http://opendata.aragon.es/def/ei2a#adminUnitL3">
        <rdfs:domain rdf:resource="http://www.w3.org/ns/locn#Address"/>
        <rdfs:range rdf:resource="http://www.w3.org/2000/01/rdf-schema#Literal"/>
        <rdfs:comment xml:lang="en">Administrative unit level 3.
County.</rdfs:comment>
        <rdfs:comment xml:lang="es">Unidad administrativa de nivel 3.
Provincia.</rdfs:comment>
    </owl:DatatypeProperty>
    


    <!-- http://opendata.aragon.es/def/ei2a#adminUnitL4 -->

    <owl:DatatypeProperty rdf:about="http://opendata.aragon.es/def/ei2a#adminUnitL4">
        <rdfs:domain rdf:resource="http://www.w3.org/ns/locn#Address"/>
        <rdfs:range rdf:resource="http://www.w3.org/2000/01/rdf-schema#Literal"/>
        <rdfs:comment xml:lang="en">Administrative unit level 4.
Group os municipalities (especially in Aragón)</rdfs:comment>
        <rdfs:comment xml:lang="es">Unidad administrativa de nivel 4.
Comarca.</rdfs:comment>
    </owl:DatatypeProperty>
    


    <!-- http://opendata.aragon.es/def/ei2a#adminUnitL5 -->

    <owl:DatatypeProperty rdf:about="http://opendata.aragon.es/def/ei2a#adminUnitL5">
        <rdfs:domain rdf:resource="http://www.w3.org/ns/locn#Address"/>
        <rdfs:range rdf:resource="http://www.w3.org/2000/01/rdf-schema#Literal"/>
        <rdfs:comment xml:lang="en">Administrative unit level 5.
Municipality.</rdfs:comment>
        <rdfs:comment xml:lang="es">Unidad administrativa de nivel 5.
Municipio.</rdfs:comment>
    </owl:DatatypeProperty>
    


    <!-- http://opendata.aragon.es/def/ei2a#adminUnitL6 -->

    <owl:DatatypeProperty rdf:about="http://opendata.aragon.es/def/ei2a#adminUnitL6">
        <rdfs:domain rdf:resource="http://www.w3.org/ns/locn#Address"/>
        <rdfs:range rdf:resource="http://www.w3.org/2000/01/rdf-schema#Literal"/>
        <rdfs:comment xml:lang="en">Administrative unit level 6.
Town.</rdfs:comment>
        <rdfs:comment xml:lang="es">Unidad administrativa de nivel 6.
Localidad.</rdfs:comment>
    </owl:DatatypeProperty>
    


    <!-- http://opendata.aragon.es/def/ei2a#aggregate -->

    <owl:DatatypeProperty rdf:about="http://opendata.aragon.es/def/ei2a#aggregate">
        <rdfs:domain rdf:resource="http://opendata.aragon.es/def/ei2a#Compound"/>
        <rdfs:range rdf:resource="http://www.w3.org/2000/01/rdf-schema#Literal"/>
        <rdfs:comment xml:lang="en">Aggregate of the compound or enclosure</rdfs:comment>
        <rdfs:comment xml:lang="es">Agregado del recinto</rdfs:comment>
    </owl:DatatypeProperty>
    


    <!-- http://opendata.aragon.es/def/ei2a#areaValue -->

    <owl:DatatypeProperty rdf:about="http://opendata.aragon.es/def/ei2a#areaValue">
        <rdfs:domain rdf:resource="http://opendata.aragon.es/def/ei2a#CadastralParcel"/>
        <rdfs:range rdf:resource="http://www.w3.org/2001/XMLSchema#float"/>
        <rdfs:comment xml:lang="en">Land surface in square meters.</rdfs:comment>
        <rdfs:comment xml:lang="es">Superficie de un terreno o una parcela en metros cuadrados</rdfs:comment>
    </owl:DatatypeProperty>
    


    <!-- http://opendata.aragon.es/def/ei2a#bankAccountIdentifier -->

    <owl:DatatypeProperty rdf:about="http://opendata.aragon.es/def/ei2a#bankAccountIdentifier">
        <rdfs:subPropertyOf rdf:resource="http://www.w3.org/2004/02/skos/core#notation"/>
        <rdfs:domain rdf:resource="http://opendata.aragon.es/def/ei2a#BankAccount"/>
        <rdfs:range rdf:resource="http://www.w3.org/2000/01/rdf-schema#Literal"/>
    </owl:DatatypeProperty>
    


    <!-- http://opendata.aragon.es/def/ei2a#birthDate -->

    <owl:DatatypeProperty rdf:about="http://opendata.aragon.es/def/ei2a#birthDate">
        <rdfs:domain rdf:resource="http://www.w3.org/ns/person#Person"/>
        <rdfs:range rdf:resource="http://www.w3.org/2001/XMLSchema#dateTime"/>
        <rdfs:comment xml:lang="en">Date of birth that appears in the document proving the identity of the person.

In the event that the exact date of birth is not recorded or unknown, the one indicated by the person or, failing that, the first day of the year corresponding to the physical appearance of the person (01/01/year corresponding to the physical appearance of the person).</rdfs:comment>
        <rdfs:comment xml:lang="es">Fecha de nacimiento que conste en el documento acreditativo de la identidad de la persona. 

En el caso de que no conste o se desconozca la fecha exacta de nacimiento, se registrará la indicada por la persona o, en su defecto, la del primer día del año correspondiente a la apariencia física del mismo (01/01/año correspondiente al a apariencia física de la persona).</rdfs:comment>
    </owl:DatatypeProperty>
    


    <!-- http://opendata.aragon.es/def/ei2a#buildingIdentifier -->

    <owl:DatatypeProperty rdf:about="http://opendata.aragon.es/def/ei2a#buildingIdentifier">
        <rdfs:domain rdf:resource="http://www.w3.org/ns/locn#Address"/>
        <rdfs:range rdf:resource="http://www.w3.org/2000/01/rdf-schema#Literal"/>
        <rdfs:comment xml:lang="en">Building identifier.</rdfs:comment>
        <rdfs:comment xml:lang="es">Identificador del bloque o edificio.</rdfs:comment>
    </owl:DatatypeProperty>
    


    <!-- http://opendata.aragon.es/def/ei2a#cadastralParcelIdentifier -->

    <owl:DatatypeProperty rdf:about="http://opendata.aragon.es/def/ei2a#cadastralParcelIdentifier">
        <rdfs:subPropertyOf rdf:resource="http://www.w3.org/2004/02/skos/core#notation"/>
        <rdfs:domain rdf:resource="http://opendata.aragon.es/def/ei2a#CadastralParcel"/>
        <rdfs:range rdf:resource="http://www.w3.org/2000/01/rdf-schema#Literal"/>
    </owl:DatatypeProperty>
    


    <!-- http://opendata.aragon.es/def/ei2a#cadastralReference -->

    <owl:DatatypeProperty rdf:about="http://opendata.aragon.es/def/ei2a#cadastralReference">
        <rdfs:domain rdf:resource="http://opendata.aragon.es/def/ei2a#CadastralParcel"/>
        <rdfs:range rdf:resource="http://www.w3.org/2000/01/rdf-schema#Literal"/>
        <rdfs:comment xml:lang="en">Cadastral reference.</rdfs:comment>
        <rdfs:comment xml:lang="es">Referencia catastral</rdfs:comment>
    </owl:DatatypeProperty>
    


    <!-- http://opendata.aragon.es/def/ei2a#cadastralRuralParcelBuildingIdentifier -->

    <owl:DatatypeProperty rdf:about="http://opendata.aragon.es/def/ei2a#cadastralRuralParcelBuildingIdentifier">
        <rdfs:domain rdf:resource="http://opendata.aragon.es/def/ei2a#CadastralRuralParcel"/>
        <rdfs:range rdf:resource="http://www.w3.org/2000/01/rdf-schema#Literal"/>
        <rdfs:comment xml:lang="en">Building identifier of a cadastral rural parcel</rdfs:comment>
        <rdfs:comment xml:lang="es">Identificador del edificio de una parcel rural catastral</rdfs:comment>
    </owl:DatatypeProperty>
    


    <!-- http://opendata.aragon.es/def/ei2a#citationDate -->

    <owl:DatatypeProperty rdf:about="http://opendata.aragon.es/def/ei2a#citationDate">
        <rdfs:domain rdf:resource="http://opendata.aragon.es/def/ei2a#Citation"/>
        <rdfs:range rdf:resource="http://www.w3.org/2001/XMLSchema#dateTimeStamp"/>
    </owl:DatatypeProperty>
    


    <!-- http://opendata.aragon.es/def/ei2a#citationPhrase -->

    <owl:DatatypeProperty rdf:about="http://opendata.aragon.es/def/ei2a#citationPhrase">
        <rdfs:domain rdf:resource="http://opendata.aragon.es/def/ei2a#Citation"/>
        <rdfs:range rdf:resource="http://www.w3.org/2000/01/rdf-schema#Literal"/>
        <rdfs:comment xml:lang="es">Frase de una web, subdominio o portal web del Gobierno de Aragón en la que una entidad (persona, organización o localización) es citada</rdfs:comment>
        <rdfs:comment xml:lang="en">Phrase of a web, subdomain or web portal of the Government of Aragon in which an entity (person, organization or location) is cited</rdfs:comment>
    </owl:DatatypeProperty>
    


    <!-- http://opendata.aragon.es/def/ei2a#civilStatus -->

    <owl:DatatypeProperty rdf:about="http://opendata.aragon.es/def/ei2a#civilStatus">
        <rdfs:domain rdf:resource="http://www.w3.org/ns/person#Person"/>
        <rdfs:range rdf:resource="http://www.w3.org/2000/01/rdf-schema#Literal"/>
        <rdfs:comment xml:lang="es">Situación de una persona determinada por sus relaciones de familia, provenientes del matrimonio o del parentesco, que establece ciertos derechos y deberes.</rdfs:comment>
        <rdfs:comment xml:lang="en">Situation of a person determined by his family relations, coming from marriage or kinship, which establishes certain rights and duties.</rdfs:comment>
    </owl:DatatypeProperty>
    


    <!-- http://opendata.aragon.es/def/ei2a#cosineDistance -->

    <owl:DatatypeProperty rdf:about="http://opendata.aragon.es/def/ei2a#cosineDistance">
        <rdfs:domain rdf:resource="http://opendata.aragon.es/def/ei2a#Similarity"/>
        <rdfs:range rdf:resource="http://www.w3.org/2001/XMLSchema#float"/>
        <rdfs:comment xml:lang="en">Measurement of similarity between two documents based on the cosine distance</rdfs:comment>
        <rdfs:comment xml:lang="es">Medida de similitud entre dos documentos basada en la distancia coseno</rdfs:comment>
    </owl:DatatypeProperty>
    


    <!-- http://opendata.aragon.es/def/ei2a#creditCardIdentifier -->

    <owl:DatatypeProperty rdf:about="http://opendata.aragon.es/def/ei2a#creditCardIdentifier">
        <rdfs:subPropertyOf rdf:resource="http://www.w3.org/2004/02/skos/core#notation"/>
        <rdfs:domain rdf:resource="http://opendata.aragon.es/def/ei2a#CreditCard"/>
        <rdfs:range rdf:resource="http://www.w3.org/2000/01/rdf-schema#Literal"/>
    </owl:DatatypeProperty>
    


    <!-- http://opendata.aragon.es/def/ei2a#cropIdentifier -->

    <owl:DatatypeProperty rdf:about="http://opendata.aragon.es/def/ei2a#cropIdentifier">
        <rdfs:domain rdf:resource="http://opendata.aragon.es/def/ei2a#Crop"/>
        <rdfs:range rdf:resource="http://www.w3.org/2000/01/rdf-schema#Literal"/>
        <rdfs:comment xml:lang="en">Crop identifier</rdfs:comment>
        <rdfs:comment xml:lang="es">Identificador del cultivo</rdfs:comment>
    </owl:DatatypeProperty>
    


    <!-- http://opendata.aragon.es/def/ei2a#cropVarietyIdentifier -->

    <owl:DatatypeProperty rdf:about="http://opendata.aragon.es/def/ei2a#cropVarietyIdentifier">
        <rdfs:domain rdf:resource="http://opendata.aragon.es/def/ei2a#CropVariety"/>
        <rdfs:range rdf:resource="http://www.w3.org/2000/01/rdf-schema#Literal"/>
        <rdfs:comment xml:lang="en">Crop variety identifier</rdfs:comment>
        <rdfs:comment xml:lang="es">Identificador de la variedad del cultivo</rdfs:comment>
    </owl:DatatypeProperty>
    


    <!-- http://opendata.aragon.es/def/ei2a#deadlineDate -->

    <owl:DatatypeProperty rdf:about="http://opendata.aragon.es/def/ei2a#deadlineDate">
        <rdfs:domain rdf:resource="http://opendata.aragon.es/def/ei2a#Document"/>
        <rdfs:range rdf:resource="http://www.w3.org/2001/XMLSchema#dateTime"/>
        <rdfs:comment xml:lang="es">Fecha límite de fin del documento</rdfs:comment>
        <rdfs:comment xml:lang="en">Limit date to finish a document.</rdfs:comment>
    </owl:DatatypeProperty>
    


    <!-- http://opendata.aragon.es/def/ei2a#deathDate -->

    <owl:DatatypeProperty rdf:about="http://opendata.aragon.es/def/ei2a#deathDate">
        <rdfs:domain rdf:resource="http://www.w3.org/ns/person#Person"/>
        <rdfs:range rdf:resource="http://www.w3.org/2000/01/rdf-schema#Literal"/>
        <rdfs:comment xml:lang="en">Date of death of a person</rdfs:comment>
        <rdfs:comment xml:lang="es">Fecha de fallecimiento de una persona</rdfs:comment>
    </owl:DatatypeProperty>
    


    <!-- http://opendata.aragon.es/def/ei2a#documentIdentifier -->

    <owl:DatatypeProperty rdf:about="http://opendata.aragon.es/def/ei2a#documentIdentifier">
        <rdfs:subPropertyOf rdf:resource="http://www.w3.org/2004/02/skos/core#notation"/>
        <rdfs:domain rdf:resource="http://opendata.aragon.es/def/ei2a#Document"/>
        <rdfs:range rdf:resource="http://www.w3.org/2000/01/rdf-schema#Literal"/>
    </owl:DatatypeProperty>
    


    <!-- http://opendata.aragon.es/def/ei2a#documentType -->

    <owl:DatatypeProperty rdf:about="http://opendata.aragon.es/def/ei2a#documentType">
        <rdfs:domain rdf:resource="http://opendata.aragon.es/def/ei2a#Document"/>
        <rdfs:range rdf:resource="http://www.w3.org/2000/01/rdf-schema#Literal"/>
        <rdfs:comment xml:lang="es">Categoría del documento: expediente, documento,...  La categoría es equivalente al tipo de documento</rdfs:comment>
        <rdfs:comment xml:lang="en">Document category: administrative record, document,... Category is equal to document type.</rdfs:comment>
    </owl:DatatypeProperty>
    


    <!-- http://opendata.aragon.es/def/ei2a#drawingSheet -->

    <owl:DatatypeProperty rdf:about="http://opendata.aragon.es/def/ei2a#drawingSheet">
        <rdfs:domain rdf:resource="http://opendata.aragon.es/def/ei2a#UrbanParcel"/>
        <rdfs:range rdf:resource="http://www.w3.org/2000/01/rdf-schema#Literal"/>
        <rdfs:comment xml:lang="es">Hoja del plano donde se ubica el inmueble</rdfs:comment>
        <rdfs:comment xml:lang="en">Sheet where the property is located</rdfs:comment>
    </owl:DatatypeProperty>
    


    <!-- http://opendata.aragon.es/def/ei2a#dryOrIrrigated -->

    <owl:DatatypeProperty rdf:about="http://opendata.aragon.es/def/ei2a#dryOrIrrigated">
        <rdfs:domain rdf:resource="http://opendata.aragon.es/def/ei2a#Compound"/>
        <rdfs:range rdf:resource="http://www.w3.org/2000/01/rdf-schema#Literal"/>
        <rdfs:comment xml:lang="en">Dry or irrigated system</rdfs:comment>
        <rdfs:comment xml:lang="es">Régimen de secano o regadío</rdfs:comment>
    </owl:DatatypeProperty>
    


    <!-- http://opendata.aragon.es/def/ei2a#email -->

    <owl:DatatypeProperty rdf:about="http://opendata.aragon.es/def/ei2a#email">
        <rdfs:domain>
            <owl:Class>
                <owl:unionOf rdf:parseType="Collection">
                    <rdf:Description rdf:about="http://www.w3.org/ns/org#Organization"/>
                    <rdf:Description rdf:about="http://www.w3.org/ns/org#Site"/>
                    <rdf:Description rdf:about="http://www.w3.org/ns/person#Person"/>
                </owl:unionOf>
            </owl:Class>
        </rdfs:domain>
        <rdfs:range rdf:resource="http://www.w3.org/2000/01/rdf-schema#Literal"/>
        <rdfs:comment xml:lang="en">An e-mail address that identifies an e-mail account (virtual mailbox) that is required to send or receive e-mails. Each address is composed of a local part, the separator symbol @ and a part that identifies a domain</rdfs:comment>
        <rdfs:comment xml:lang="es">Dirección de correo electrónico que identifica una cuenta de correo (buzón virtual) y que es necesaria para poder enviar o recibir correos electrónicos. Cada dirección se compone de una parte local, el símbolo separador @ y una parte que identifica un dominio</rdfs:comment>
    </owl:DatatypeProperty>
    


    <!-- http://opendata.aragon.es/def/ei2a#employeeID -->

    <owl:DatatypeProperty rdf:about="http://opendata.aragon.es/def/ei2a#employeeID">
        <rdfs:domain rdf:resource="http://www.w3.org/ns/person#Person"/>
        <rdfs:range rdf:resource="http://www.w3.org/2000/01/rdf-schema#Literal"/>
        <rdfs:comment xml:lang="en">Employee Identification Number</rdfs:comment>
        <rdfs:comment xml:lang="es">Número de identificación como empleado</rdfs:comment>
    </owl:DatatypeProperty>
    


    <!-- http://opendata.aragon.es/def/ei2a#endDate -->

    <owl:DatatypeProperty rdf:about="http://opendata.aragon.es/def/ei2a#endDate">
        <rdfs:domain rdf:resource="http://opendata.aragon.es/def/ei2a#Document"/>
        <rdfs:range rdf:resource="http://www.w3.org/2001/XMLSchema#dateTime"/>
        <rdfs:comment xml:lang="es">Fecha de fin real de tramitación del documento</rdfs:comment>
        <rdfs:comment xml:lang="en">real end date for a document application.</rdfs:comment>
    </owl:DatatypeProperty>
    


    <!-- http://opendata.aragon.es/def/ei2a#endDateResolution -->

    <owl:DatatypeProperty rdf:about="http://opendata.aragon.es/def/ei2a#endDateResolution">
        <rdfs:domain rdf:resource="http://opendata.aragon.es/def/ei2a#AdministrativeRecord"/>
        <rdfs:range rdf:resource="http://www.w3.org/2001/XMLSchema#dateTime"/>
        <rdfs:comment xml:lang="en">End date of resolution of a file (when acknowledgment is received)</rdfs:comment>
        <rdfs:comment xml:lang="es">Fecha fin de resolución de un expediente (cuando se recibe acuse de notificación)</rdfs:comment>
    </owl:DatatypeProperty>
    


    <!-- http://opendata.aragon.es/def/ei2a#entranceDoorIdentifier -->

    <owl:DatatypeProperty rdf:about="http://opendata.aragon.es/def/ei2a#entranceDoorIdentifier">
        <rdfs:domain rdf:resource="http://www.w3.org/ns/locn#Address"/>
        <rdfs:range rdf:resource="http://www.w3.org/2000/01/rdf-schema#Literal"/>
        <rdfs:comment xml:lang="en">Front door</rdfs:comment>
        <rdfs:comment xml:lang="es">Portal</rdfs:comment>
    </owl:DatatypeProperty>
    


    <!-- http://opendata.aragon.es/def/ei2a#expurgatedDate -->

    <owl:DatatypeProperty rdf:about="http://opendata.aragon.es/def/ei2a#expurgatedDate">
        <rdfs:domain rdf:resource="http://opendata.aragon.es/def/ei2a#Document"/>
        <rdfs:range rdf:resource="http://www.w3.org/2001/XMLSchema#dateTime"/>
        <rdfs:comment xml:lang="es">Fecha a partIr de la cual yo no puede ser recuperado un documento y por lo tanto podría ser eliminado (FechaFinDoc)</rdfs:comment>
        <rdfs:comment xml:lang="en">Fecha sinde a document could not be recovered and it could be deleted.</rdfs:comment>
    </owl:DatatypeProperty>
    


    <!-- http://opendata.aragon.es/def/ei2a#floorIdentifier -->

    <owl:DatatypeProperty rdf:about="http://opendata.aragon.es/def/ei2a#floorIdentifier">
        <rdfs:domain rdf:resource="http://www.w3.org/ns/locn#Address"/>
        <rdfs:range rdf:resource="http://www.w3.org/2000/01/rdf-schema#Literal"/>
        <rdfs:comment xml:lang="en">Floor identifier.</rdfs:comment>
        <rdfs:comment xml:lang="es">Planta</rdfs:comment>
    </owl:DatatypeProperty>
    


    <!-- http://opendata.aragon.es/def/ei2a#format -->

    <owl:DatatypeProperty rdf:about="http://opendata.aragon.es/def/ei2a#format">
        <rdfs:domain rdf:resource="http://opendata.aragon.es/def/ei2a#Document"/>
        <rdfs:range rdf:resource="http://www.w3.org/2000/01/rdf-schema#Literal"/>
        <rdfs:comment xml:lang="en">Document format (pdf, csv, doc, ...)</rdfs:comment>
        <rdfs:comment xml:lang="es">Formato del documento (pdf, csv, doc,...)</rdfs:comment>
    </owl:DatatypeProperty>
    


    <!-- http://opendata.aragon.es/def/ei2a#fullName -->

    <owl:DatatypeProperty rdf:about="http://opendata.aragon.es/def/ei2a#fullName">
        <rdfs:domain rdf:resource="http://www.w3.org/ns/person#Person"/>
        <rdfs:range rdf:resource="http://www.w3.org/2000/01/rdf-schema#Literal"/>
        <rdfs:comment xml:lang="en">Full name of a person (name o birthName, surname1 and surname2)</rdfs:comment>
        <rdfs:comment xml:lang="es">Nombre completo de una persona (nombre más apellidos)</rdfs:comment>
    </owl:DatatypeProperty>
    


    <!-- http://opendata.aragon.es/def/ei2a#functionalExpiryDate -->

    <owl:DatatypeProperty rdf:about="http://opendata.aragon.es/def/ei2a#functionalExpiryDate">
        <rdfs:domain rdf:resource="http://www.w3.org/ns/org#Organization"/>
        <rdfs:range rdf:resource="http://www.w3.org/2001/XMLSchema#dateTime"/>
        <rdfs:comment xml:lang="es">Fecha de extinción funcional
Fecha en la que se extingue una unidad u oficina, según una disposición legal.</rdfs:comment>
        <rdfs:comment xml:lang="en">Functional extinction date.
Date in which an unit or a office is dissapeared, depending a legal regulation.</rdfs:comment>
    </owl:DatatypeProperty>
    


    <!-- http://opendata.aragon.es/def/ei2a#geographicName -->

    <owl:DatatypeProperty rdf:about="http://opendata.aragon.es/def/ei2a#geographicName">
        <rdfs:domain rdf:resource="http://purl.org/dc/terms/Location"/>
        <rdfs:range rdf:resource="http://www.w3.org/2000/01/rdf-schema#Literal"/>
        <rdfs:comment xml:lang="es">Nombre geográfico o nombre propio de una localización</rdfs:comment>
    </owl:DatatypeProperty>
    


    <!-- http://opendata.aragon.es/def/ei2a#geoweight -->

    <owl:DatatypeProperty rdf:about="http://opendata.aragon.es/def/ei2a#geoweight">
        <rdfs:domain rdf:resource="http://opendata.aragon.es/def/ei2a#SocialMedia"/>
        <rdfs:range rdf:resource="http://www.w3.org/2001/XMLSchema#float"/>
        <rdfs:comment xml:lang="en">Geographical weight of social communication</rdfs:comment>
        <rdfs:comment xml:lang="es">Peso geográfico de la comunicación social</rdfs:comment>
    </owl:DatatypeProperty>
    


    <!-- http://opendata.aragon.es/def/ei2a#graphicSurface -->

    <owl:DatatypeProperty rdf:about="http://opendata.aragon.es/def/ei2a#graphicSurface">
        <rdfs:domain rdf:resource="http://opendata.aragon.es/def/ei2a#CadastralParcel"/>
        <rdfs:range rdf:resource="http://www.w3.org/2000/01/rdf-schema#Literal"/>
        <rdfs:comment xml:lang="en">Graphic surface of a plot of land</rdfs:comment>
        <rdfs:comment xml:lang="es">Superficie gráfica de un terreno o una parcela</rdfs:comment>
    </owl:DatatypeProperty>
    


    <!-- http://opendata.aragon.es/def/ei2a#hashtag -->

    <owl:DatatypeProperty rdf:about="http://opendata.aragon.es/def/ei2a#hashtag">
        <rdfs:domain rdf:resource="http://opendata.aragon.es/def/ei2a#SocialMediaHashtag"/>
        <rdfs:range rdf:resource="http://www.w3.org/2000/01/rdf-schema#Literal"/>
        <rdfs:comment xml:lang="es">Valor del hashtag de la comunicación social</rdfs:comment>
        <rdfs:comment xml:lang="en">Value of social communication hashtag</rdfs:comment>
    </owl:DatatypeProperty>
    


    <!-- http://opendata.aragon.es/def/ei2a#idEnclosure -->

    <owl:DatatypeProperty rdf:about="http://opendata.aragon.es/def/ei2a#idEnclosure">
        <rdfs:domain rdf:resource="http://opendata.aragon.es/def/ei2a#Compound"/>
        <rdfs:range rdf:resource="http://www.w3.org/2000/01/rdf-schema#Literal"/>
        <rdfs:comment xml:lang="en">Enclosure or compound identifier</rdfs:comment>
        <rdfs:comment xml:lang="es">Identificador del recinto</rdfs:comment>
    </owl:DatatypeProperty>
    


    <!-- http://opendata.aragon.es/def/ei2a#identifierPersonSystem -->

    <owl:DatatypeProperty rdf:about="http://opendata.aragon.es/def/ei2a#identifierPersonSystem">
        <rdfs:domain rdf:resource="http://opendata.aragon.es/def/ei2a#PersonalIdentifierSystem"/>
        <rdfs:range rdf:resource="http://www.w3.org/2000/01/rdf-schema#Literal"/>
        <rdfs:comment xml:lang="en">Link the unique identifier of a Person with the identifier of that person in other systems.</rdfs:comment>
        <rdfs:comment xml:lang="es">Víncula el identificador unívoco de una Persona con el identificador de esa persona  en otros sistemas.</rdfs:comment>
    </owl:DatatypeProperty>
    


    <!-- http://opendata.aragon.es/def/ei2a#isElectronicRegistrationOffice -->

    <owl:DatatypeProperty rdf:about="http://opendata.aragon.es/def/ei2a#isElectronicRegistrationOffice">
        <rdfs:domain rdf:resource="http://www.w3.org/ns/org#Organization"/>
        <rdfs:range rdf:resource="http://www.w3.org/2001/XMLSchema#boolean"/>
        <rdfs:comment xml:lang="es">Dentro de la administración pública, indica si una oficina es una oficina de registro electrónico (DIR3)</rdfs:comment>
        <rdfs:comment xml:lang="en">It indicates whether an office is an electronic registry in the public administration (DIR3).</rdfs:comment>
    </owl:DatatypeProperty>
    


    <!-- http://opendata.aragon.es/def/ei2a#isInformationOffice -->

    <owl:DatatypeProperty rdf:about="http://opendata.aragon.es/def/ei2a#isInformationOffice">
        <rdfs:domain rdf:resource="http://www.w3.org/ns/org#Organization"/>
        <rdfs:range rdf:resource="http://www.w3.org/2001/XMLSchema#boolean"/>
        <rdfs:comment xml:lang="es">Dentro de la Administración pública, indica si una oficina es una oficina de información.</rdfs:comment>
        <rdfs:comment xml:lang="en">It indicates whether an office is an information office in the public administration (DIR3).</rdfs:comment>
    </owl:DatatypeProperty>
    


    <!-- http://opendata.aragon.es/def/ei2a#isLegalPublicEntity -->

    <owl:DatatypeProperty rdf:about="http://opendata.aragon.es/def/ei2a#isLegalPublicEntity">
        <rdfs:domain rdf:resource="http://www.w3.org/ns/org#Organization"/>
        <rdfs:range rdf:resource="http://www.w3.org/2001/XMLSchema#boolean"/>
        <rdfs:comment xml:lang="es">Define si la unidad es o depende de una entidad de derecho público, según el artículo 2.2 de la Ley 30.92 (B_SW_DEP_EDP_PRINCIPAL)</rdfs:comment>
        <rdfs:comment xml:lang="en">It defines if the unit is a public entity, depending on article 2.2 from law 30.92.</rdfs:comment>
    </owl:DatatypeProperty>
    


    <!-- http://opendata.aragon.es/def/ei2a#isRegistrationOffice -->

    <owl:DatatypeProperty rdf:about="http://opendata.aragon.es/def/ei2a#isRegistrationOffice">
        <rdfs:domain rdf:resource="http://www.w3.org/ns/org#Organization"/>
        <rdfs:range rdf:resource="http://www.w3.org/2001/XMLSchema#boolean"/>
        <rdfs:comment xml:lang="es">Dentro de la administración pública, define si la oficina es una oficina de registro (B_OFICINA_REGISTRO)</rdfs:comment>
        <rdfs:comment xml:lang="en">It defines whether the office is a registration office in the public administration.</rdfs:comment>
    </owl:DatatypeProperty>
    


    <!-- http://opendata.aragon.es/def/ei2a#isSIRIntegration -->

    <owl:DatatypeProperty rdf:about="http://opendata.aragon.es/def/ei2a#isSIRIntegration">
        <rdfs:domain rdf:resource="http://www.w3.org/ns/org#Organization"/>
        <rdfs:range rdf:resource="http://www.w3.org/2001/XMLSchema#boolean"/>
        <rdfs:comment xml:lang="es">Dentro de la admininistración pública, indica si la oficina está integrada con el sistema de interconexión de registros (SIR) (B_SIR)</rdfs:comment>
        <rdfs:comment xml:lang="en">It indicate whether the office is integrated in a register interconnection system (SIR)</rdfs:comment>
    </owl:DatatypeProperty>
    


    <!-- http://opendata.aragon.es/def/ei2a#isTransactionOffice -->

    <owl:DatatypeProperty rdf:about="http://opendata.aragon.es/def/ei2a#isTransactionOffice">
        <rdfs:domain rdf:resource="http://www.w3.org/ns/org#Organization"/>
        <rdfs:range rdf:resource="http://www.w3.org/2001/XMLSchema#boolean"/>
        <rdfs:comment xml:lang="es">Dentro de la administración pública, indica si la oficina es una oficina de tramitación (B_OFICINA_TRAMITACION)</rdfs:comment>
        <rdfs:comment xml:lang="en">It indicates whether the office is an application office in the public administration.</rdfs:comment>
    </owl:DatatypeProperty>
    


    <!-- http://opendata.aragon.es/def/ei2a#kilometrePoint -->

    <owl:DatatypeProperty rdf:about="http://opendata.aragon.es/def/ei2a#kilometrePoint">
        <rdfs:domain rdf:resource="http://www.w3.org/ns/locn#Address"/>
        <rdfs:range rdf:resource="http://www.w3.org/2000/01/rdf-schema#Literal"/>
        <rdfs:comment xml:lang="es">Kilómetro vía</rdfs:comment>
        <rdfs:comment xml:lang="en">Km</rdfs:comment>
    </owl:DatatypeProperty>
    


    <!-- http://opendata.aragon.es/def/ei2a#language -->

    <owl:DatatypeProperty rdf:about="http://opendata.aragon.es/def/ei2a#language">
        <rdfs:domain rdf:resource="http://opendata.aragon.es/def/ei2a#Document"/>
        <rdfs:range rdf:resource="http://www.w3.org/2000/01/rdf-schema#Literal"/>
        <rdfs:comment xml:lang="en">Document language</rdfs:comment>
        <rdfs:comment xml:lang="es">Idioma del documento</rdfs:comment>
    </owl:DatatypeProperty>
    


    <!-- http://opendata.aragon.es/def/ei2a#mention -->

    <owl:DatatypeProperty rdf:about="http://opendata.aragon.es/def/ei2a#mention">
        <rdfs:domain rdf:resource="http://opendata.aragon.es/def/ei2a#SocialMediaMention"/>
        <rdfs:range rdf:resource="http://www.w3.org/2000/01/rdf-schema#Literal"/>
        <rdfs:comment xml:lang="es">Valor de la mención de la comunicación social</rdfs:comment>
        <rdfs:comment xml:lang="en">Value of the mention of social communication</rdfs:comment>
    </owl:DatatypeProperty>
    


    <!-- http://opendata.aragon.es/def/ei2a#mobile -->

    <owl:DatatypeProperty rdf:about="http://opendata.aragon.es/def/ei2a#mobile">
        <rdfs:domain>
            <owl:Class>
                <owl:unionOf rdf:parseType="Collection">
                    <rdf:Description rdf:about="http://www.w3.org/ns/org#Organization"/>
                    <rdf:Description rdf:about="http://www.w3.org/ns/org#Site"/>
                    <rdf:Description rdf:about="http://www.w3.org/ns/person#Person"/>
                </owl:unionOf>
            </owl:Class>
        </rdfs:domain>
        <rdfs:range rdf:resource="http://www.w3.org/2000/01/rdf-schema#Literal"/>
        <rdfs:comment xml:lang="en">Associated mobile phone number</rdfs:comment>
        <rdfs:comment xml:lang="es">Número de teléfono móvil asociado</rdfs:comment>
    </owl:DatatypeProperty>
    


    <!-- http://opendata.aragon.es/def/ei2a#nameDocument -->

    <owl:DatatypeProperty rdf:about="http://opendata.aragon.es/def/ei2a#nameDocument">
        <rdfs:domain rdf:resource="http://opendata.aragon.es/def/ei2a#Document"/>
        <rdfs:range rdf:resource="http://www.w3.org/2000/01/rdf-schema#Literal"/>
        <rdfs:comment xml:lang="en">Document name.</rdfs:comment>
        <rdfs:comment xml:lang="es">Nombre del documento</rdfs:comment>
    </owl:DatatypeProperty>
    


    <!-- http://opendata.aragon.es/def/ei2a#observations -->

    <owl:DatatypeProperty rdf:about="http://opendata.aragon.es/def/ei2a#observations">
        <rdfs:domain rdf:resource="http://opendata.aragon.es/def/ei2a#Document"/>
        <rdfs:range rdf:resource="http://www.w3.org/2000/01/rdf-schema#Literal"/>
        <rdfs:comment xml:lang="es">Observaciones</rdfs:comment>
        <rdfs:comment xml:lang="en">Observations</rdfs:comment>
    </owl:DatatypeProperty>
    


    <!-- http://opendata.aragon.es/def/ei2a#officialCreationDate -->

    <owl:DatatypeProperty rdf:about="http://opendata.aragon.es/def/ei2a#officialCreationDate">
        <rdfs:domain rdf:resource="http://www.w3.org/ns/org#Organization"/>
        <rdfs:range rdf:resource="http://www.w3.org/2001/XMLSchema#dateTime"/>
        <rdfs:comment xml:lang="en">Date of official creation in which a unit is created or established, according to its legal provision (D_VIG_ALTA_OFICIAL)</rdfs:comment>
        <rdfs:comment xml:lang="es">Fecha de creación oficial en la que se crea o establece una unidad, según su disposición legal (D_VIG_ALTA_OFICIAL)</rdfs:comment>
    </owl:DatatypeProperty>
    


    <!-- http://opendata.aragon.es/def/ei2a#officialLeavingDate -->

    <owl:DatatypeProperty rdf:about="http://opendata.aragon.es/def/ei2a#officialLeavingDate">
        <rdfs:domain rdf:resource="http://www.w3.org/ns/org#Organization"/>
        <rdfs:range rdf:resource="http://www.w3.org/2001/XMLSchema#dateTime"/>
        <rdfs:comment xml:lang="es">Fecha de Supresión oficial en la que se suprime la unidad (aunque no estén extinguidas todas las unidades dependientes de ella jerarquicamente), según una disposición legal</rdfs:comment>
        <rdfs:comment xml:lang="en">Official Suppression Date on which the unit is deleted (even if all units are not extinguished hierarchically), according to a legal provision</rdfs:comment>
    </owl:DatatypeProperty>
    


    <!-- http://opendata.aragon.es/def/ei2a#organizationName -->

    <owl:DatatypeProperty rdf:about="http://opendata.aragon.es/def/ei2a#organizationName">
        <rdfs:domain rdf:resource="http://www.w3.org/ns/org#Organization"/>
        <rdfs:range rdf:resource="http://www.w3.org/2000/01/rdf-schema#Literal"/>
        <rdfs:comment xml:lang="es">Nombre asociado a la organización. 
En el caso de entidades públicas corresponde con el nombre de la unidad (C_DNM_UNIDAD) (DIR3)</rdfs:comment>
        <rdfs:comment xml:lang="en">Organization´s name. 
Unity&apos;s name in public institution depending on DIR3.</rdfs:comment>
    </owl:DatatypeProperty>
    


    <!-- http://opendata.aragon.es/def/ei2a#originalFormat -->

    <owl:DatatypeProperty rdf:about="http://opendata.aragon.es/def/ei2a#originalFormat">
        <rdfs:domain rdf:resource="http://opendata.aragon.es/def/ei2a#Document"/>
        <rdfs:range rdf:resource="http://www.w3.org/2000/01/rdf-schema#Literal"/>
        <rdfs:comment xml:lang="es">Soporte o formato original del documento (digital,...)</rdfs:comment>
        <rdfs:comment xml:lang="en">Support or original document format (digital, ...)</rdfs:comment>
    </owl:DatatypeProperty>
    


    <!-- http://opendata.aragon.es/def/ei2a#parcel -->

    <owl:DatatypeProperty rdf:about="http://opendata.aragon.es/def/ei2a#parcel">
        <rdfs:domain rdf:resource="http://opendata.aragon.es/def/ei2a#RuralParcel"/>
        <rdfs:range rdf:resource="http://www.w3.org/2001/XMLSchema#nonNegativeInteger"/>
        <rdfs:comment xml:lang="es">Identificación de una parcela dentro del polígono correspondiente.</rdfs:comment>
        <rdfs:comment xml:lang="en">Identification of a parcel within the corresponding polygon.</rdfs:comment>
    </owl:DatatypeProperty>
    


    <!-- http://opendata.aragon.es/def/ei2a#passportID -->

    <owl:DatatypeProperty rdf:about="http://opendata.aragon.es/def/ei2a#passportID">
        <rdfs:domain rdf:resource="http://www.w3.org/ns/person#Person"/>
        <rdfs:range rdf:resource="http://www.w3.org/2000/01/rdf-schema#Literal"/>
        <rdfs:comment xml:lang="en">Identification number of the passport, that is to say, the document with international validity issued by the authorities of their respective country, which accredits a permit or legal authorization for a person to leave or enter it, through international ports or airports.</rdfs:comment>
        <rdfs:comment xml:lang="es">Número de identificación del pasaporte, es decir, del documento con validez internacional expedido por las autoridades de su respectivo país, que acredita un permiso o autorización legal para que una persona salga o ingrese del mismo, por los puertos o aeropuertos internacionales.</rdfs:comment>
    </owl:DatatypeProperty>
    


    <!-- http://opendata.aragon.es/def/ei2a#pasturePercentage -->

    <owl:DatatypeProperty rdf:about="http://opendata.aragon.es/def/ei2a#pasturePercentage">
        <rdfs:domain rdf:resource="http://opendata.aragon.es/def/ei2a#Compound"/>
        <rdfs:range rdf:resource="http://www.w3.org/2000/01/rdf-schema#Literal"/>
        <rdfs:comment xml:lang="en">Admissibility coefficient of pastures for aid</rdfs:comment>
        <rdfs:comment xml:lang="es">Coeficiente de admisibilidad de pastos para ayuda</rdfs:comment>
    </owl:DatatypeProperty>
    


    <!-- http://opendata.aragon.es/def/ei2a#pearsonCorrelation -->

    <owl:DatatypeProperty rdf:about="http://opendata.aragon.es/def/ei2a#pearsonCorrelation">
        <rdfs:domain rdf:resource="http://opendata.aragon.es/def/ei2a#Similarity"/>
        <rdfs:range rdf:resource="http://www.w3.org/2001/XMLSchema#float"/>
        <rdfs:comment xml:lang="en">Measurement of similarity between two documents based on the Pearson correlation</rdfs:comment>
        <rdfs:comment xml:lang="es">Medida de similitud entre dos documentos basada en la correlación de Pearson</rdfs:comment>
    </owl:DatatypeProperty>
    


    <!-- http://opendata.aragon.es/def/ei2a#pending -->

    <owl:DatatypeProperty rdf:about="http://opendata.aragon.es/def/ei2a#pending">
        <rdfs:domain rdf:resource="http://opendata.aragon.es/def/ei2a#Compound"/>
        <rdfs:range rdf:resource="http://www.w3.org/2000/01/rdf-schema#Literal"/>
        <rdfs:comment xml:lang="es">Pendiente media del recinto en porcentaje</rdfs:comment>
        <rdfs:comment xml:lang="en">verage slope of the compound or enclosure in percentage</rdfs:comment>
    </owl:DatatypeProperty>
    


    <!-- http://opendata.aragon.es/def/ei2a#personIdentifier -->

    <owl:DatatypeProperty rdf:about="http://opendata.aragon.es/def/ei2a#personIdentifier">
        <rdfs:subPropertyOf rdf:resource="http://www.w3.org/2004/02/skos/core#notation"/>
        <rdfs:domain rdf:resource="http://www.w3.org/ns/person#Person"/>
        <rdfs:range rdf:resource="http://www.w3.org/2000/01/rdf-schema#Literal"/>
    </owl:DatatypeProperty>
    


    <!-- http://opendata.aragon.es/def/ei2a#phone -->

    <owl:DatatypeProperty rdf:about="http://opendata.aragon.es/def/ei2a#phone">
        <rdfs:domain>
            <owl:Class>
                <owl:unionOf rdf:parseType="Collection">
                    <rdf:Description rdf:about="http://www.w3.org/ns/org#Organization"/>
                    <rdf:Description rdf:about="http://www.w3.org/ns/org#Site"/>
                    <rdf:Description rdf:about="http://www.w3.org/ns/person#Person"/>
                </owl:unionOf>
            </owl:Class>
        </rdfs:domain>
        <rdfs:range rdf:resource="http://www.w3.org/2000/01/rdf-schema#Literal"/>
        <rdfs:comment xml:lang="en">Associated non-mobile phone number</rdfs:comment>
        <rdfs:comment xml:lang="es">Número de teléfono no móvil asociado</rdfs:comment>
    </owl:DatatypeProperty>
    


    <!-- http://opendata.aragon.es/def/ei2a#polarity -->

    <owl:DatatypeProperty rdf:about="http://opendata.aragon.es/def/ei2a#polarity">
        <rdfs:domain rdf:resource="http://opendata.aragon.es/def/ei2a#SocialMedia"/>
        <rdfs:range rdf:resource="http://www.w3.org/2001/XMLSchema#float"/>
        <rdfs:comment xml:lang="es">Polaridad de una comunicación social</rdfs:comment>
        <rdfs:comment xml:lang="en">Polarity of a social communication</rdfs:comment>
    </owl:DatatypeProperty>
    


    <!-- http://opendata.aragon.es/def/ei2a#polygon -->

    <owl:DatatypeProperty rdf:about="http://opendata.aragon.es/def/ei2a#polygon">
        <rdfs:domain rdf:resource="http://opendata.aragon.es/def/ei2a#RuralParcel"/>
        <rdfs:range rdf:resource="http://www.w3.org/2001/XMLSchema#nonNegativeInteger"/>
        <rdfs:comment xml:lang="es">Identificador del número de polígono que forma parte de un determinado término municipal.</rdfs:comment>
        <rdfs:comment xml:lang="en">Identifier of the polygon number that is part of a certain municipality.</rdfs:comment>
    </owl:DatatypeProperty>
    


    <!-- http://opendata.aragon.es/def/ei2a#procedureIdentifier -->

    <owl:DatatypeProperty rdf:about="http://opendata.aragon.es/def/ei2a#procedureIdentifier">
        <rdfs:subPropertyOf rdf:resource="http://www.w3.org/2004/02/skos/core#notation"/>
        <rdfs:domain rdf:resource="http://opendata.aragon.es/def/ei2a#Procedure"/>
        <rdfs:range rdf:resource="http://www.w3.org/2000/01/rdf-schema#Literal"/>
    </owl:DatatypeProperty>
    


    <!-- http://opendata.aragon.es/def/ei2a#productiveIntensity -->

    <owl:DatatypeProperty rdf:about="http://opendata.aragon.es/def/ei2a#productiveIntensity">
        <rdfs:domain rdf:resource="http://opendata.aragon.es/def/ei2a#Compound"/>
        <rdfs:range rdf:resource="http://www.w3.org/2000/01/rdf-schema#Literal"/>
        <rdfs:comment xml:lang="es">Intensidad productiva</rdfs:comment>
        <rdfs:comment xml:lang="en">Productive intensity</rdfs:comment>
    </owl:DatatypeProperty>
    


    <!-- http://opendata.aragon.es/def/ei2a#propertyIdentifier -->

    <owl:DatatypeProperty rdf:about="http://opendata.aragon.es/def/ei2a#propertyIdentifier">
        <rdfs:domain>
            <owl:Class>
                <owl:unionOf rdf:parseType="Collection">
                    <rdf:Description rdf:about="http://opendata.aragon.es/def/ei2a#RuralParcel"/>
                    <rdf:Description rdf:about="http://opendata.aragon.es/def/ei2a#UrbanParcel"/>
                </owl:unionOf>
            </owl:Class>
        </rdfs:domain>
        <rdfs:range rdf:resource="http://www.w3.org/2001/XMLSchema#nonNegativeInteger"/>
        <rdfs:comment xml:lang="en">For rustic cadastral references corresponds to the identification of the property into the parcel.

For urban cadastral references corresponds to the identification of the property into the estate.</rdfs:comment>
        <rdfs:comment xml:lang="es">Para referencias catastrales rústicas corresponde con la identificación del inmueble dentro de una parcela.

Para referencias catastrales urbanas corresponde con la identificación del inmueble dentro de una finca.</rdfs:comment>
    </owl:DatatypeProperty>
    


    <!-- http://opendata.aragon.es/def/ei2a#reason -->

    <owl:DatatypeProperty rdf:about="http://opendata.aragon.es/def/ei2a#reason">
        <rdfs:domain rdf:resource="http://opendata.aragon.es/def/ei2a#SocialMedia"/>
        <rdfs:range rdf:resource="http://www.w3.org/2000/01/rdf-schema#Literal"/>
        <rdfs:comment xml:lang="es">Razón de la comunicación social</rdfs:comment>
        <rdfs:comment xml:lang="en">Reason for social communication</rdfs:comment>
    </owl:DatatypeProperty>
    


    <!-- http://opendata.aragon.es/def/ei2a#registrationDate -->

    <owl:DatatypeProperty rdf:about="http://opendata.aragon.es/def/ei2a#registrationDate">
        <rdfs:domain>
            <owl:Class>
                <owl:unionOf rdf:parseType="Collection">
                    <rdf:Description rdf:about="http://opendata.aragon.es/def/ei2a#Document"/>
                    <rdf:Description rdf:about="http://opendata.aragon.es/def/ei2a#PACAidsRequest"/>
                </owl:unionOf>
            </owl:Class>
        </rdfs:domain>
        <rdfs:range rdf:resource="http://www.w3.org/2001/XMLSchema#dateTime"/>
        <rdfs:comment xml:lang="es">Fecha de registro en el sistema informático (Fecha de captura)</rdfs:comment>
        <rdfs:comment xml:lang="en">Registration date in the computer system (Date of capture)</rdfs:comment>
    </owl:DatatypeProperty>
    


    <!-- http://opendata.aragon.es/def/ei2a#requestDate -->

    <owl:DatatypeProperty rdf:about="http://opendata.aragon.es/def/ei2a#requestDate">
        <rdfs:domain rdf:resource="http://opendata.aragon.es/def/ei2a#PACAidsRequest"/>
        <rdfs:range rdf:resource="http://www.w3.org/2001/XMLSchema#dateTimeStamp"/>
        <rdfs:comment xml:lang="en">Date of the request for PAC aids</rdfs:comment>
        <rdfs:comment xml:lang="es">Fecha de la solicitud de ayudas de la PAC</rdfs:comment>
    </owl:DatatypeProperty>
    


    <!-- http://opendata.aragon.es/def/ei2a#resolution -->

    <owl:DatatypeProperty rdf:about="http://opendata.aragon.es/def/ei2a#resolution">
        <rdfs:domain rdf:resource="http://www.w3.org/ns/locn#Geometry"/>
        <rdfs:range rdf:resource="http://www.w3.org/2000/01/rdf-schema#Literal"/>
        <rdfs:comment xml:lang="es">La resolución espacial de una imagen es una indicación del  tamaño del pixel expresada en términos de dimensiones sobre el terreno. Usualmente se  presenta por un valor único correspondiente a la longitud de un lado del cuadrado  correspondiente a dicho pixel. Así, una resolución espacial de 30 m significa que el pixel  representa un área de 30 m x 30 m sobre el terreno. Si el pixel fuera rectangular debería ser  representado por su largo y ancho, por ejemplo 56 m x 79 m. La resolución espacial es una  indicación del potencial de detalle que ofrece una imagen.

Si una imagen de satélite de 1 m  de resolución se imprime a una escala de 1/500000 se perdería el potencial de detalle que ofrece dicha imagen. La inversa también es cierta: si se imprime una imagen de baja resolución espacial, por ej. 500 m, a una escala muy fina sólo veríamos los pixeles individuales. Cuando efectuamos “zoom” repetido sobre una imagen digital (es decir,  cuando vamos “afinando” la escala) llega un momento en que comienzan a visualizarse los  pixeles, y a partir de ese punto aunque sigamos afinando la escala no se aumentará su nivel  de detalle llegando a dificultarse su interpretación.</rdfs:comment>
        <rdfs:comment xml:lang="en">The spatial resolution of an image is an indication of the size of the pixel expressed in terms of dimensions on the ground. Usually presented by a unique value corresponding to the length of one side of the square corresponding to said pixel. Thus, a spatial resolution of 30 m means that the pixel represents an area of ​​30 m x 30 m above the ground. If the pixel is rectangular it should be represented by its length and width, for example 56 m x 79 m. Spatial resolution is an indication of the detail potential offered by an image.

If a satellite image of 1 m resolution is printed on a scale of 1/500000 would lose the detail potential offered by that image. The reverse is also true: if an image with low spatial resolution is printed, eg. 500 m, on a very fine scale we would only see the individual pixels. When we zoom in on a digital image (that is, when we &quot;fine-tune&quot; the scale) there comes a moment when the pixels begin to be displayed, and from that point even if we continue to fine-tune the scale, it will not increase its level of detail Becoming difficult to interpret.</rdfs:comment>
    </owl:DatatypeProperty>
    


    <!-- http://opendata.aragon.es/def/ei2a#roleIdentifier -->

    <owl:DatatypeProperty rdf:about="http://opendata.aragon.es/def/ei2a#roleIdentifier">
        <rdfs:subPropertyOf rdf:resource="http://www.w3.org/2004/02/skos/core#notation"/>
        <rdfs:domain rdf:resource="http://www.w3.org/ns/org#Role"/>
        <rdfs:range rdf:resource="http://www.w3.org/2000/01/rdf-schema#Literal"/>
    </owl:DatatypeProperty>
    


    <!-- http://opendata.aragon.es/def/ei2a#roleName -->

    <owl:DatatypeProperty rdf:about="http://opendata.aragon.es/def/ei2a#roleName">
        <rdfs:domain rdf:resource="http://www.w3.org/ns/org#Role"/>
        <rdfs:range rdf:resource="http://www.w3.org/2000/01/rdf-schema#Literal"/>
        <rdfs:comment xml:lang="en">Name of role or role of a person in an organization</rdfs:comment>
        <rdfs:comment xml:lang="es">Nombre del cargo o rol de una persona en una organización</rdfs:comment>
    </owl:DatatypeProperty>
    


    <!-- http://opendata.aragon.es/def/ei2a#scale -->

    <owl:DatatypeProperty rdf:about="http://opendata.aragon.es/def/ei2a#scale">
        <rdfs:domain rdf:resource="http://www.w3.org/ns/locn#Geometry"/>
        <rdfs:range rdf:resource="http://www.w3.org/2000/01/rdf-schema#Literal"/>
        <rdfs:comment xml:lang="en">Concept closely related to the degree of detail with which we can visualize a given image.

The scale of an image or a map refers to the relative difference in size or distance between the objects in the image and the actual terrain. This difference is expressed as the relation between the distance on the image and the real earth. For example, a scale of 1: 100000 means that 1 cm on the map or image corresponds to 100000 cm (1 km) on the ground.</rdfs:comment>
        <rdfs:comment xml:lang="es">Concepto estrechamente relacionados con el grado de detalle con que podemos visualizar una dada imagen. 

La escala de una imagen o de un mapa hace referencia a la diferencia relativa de tamaño o distancia entre los objetos de la imagen y los reales terrenos. Esta diferencia se expresa como la relación entre la distancia sobre la imagen y la real terrena.. Así por ejemplo, una  escala de 1: 100000 significa que 1 cm en el mapa o imagen corresponde a 100000 cm (1  km) sobre el terreno.</rdfs:comment>
    </owl:DatatypeProperty>
    


    <!-- http://opendata.aragon.es/def/ei2a#sector -->

    <owl:DatatypeProperty rdf:about="http://opendata.aragon.es/def/ei2a#sector">
        <rdfs:domain rdf:resource="http://opendata.aragon.es/def/ei2a#CadastralRuralParcel"/>
        <rdfs:range rdf:resource="http://www.w3.org/2000/01/rdf-schema#Literal"/>
        <rdfs:comment xml:lang="en">Aggregate or land consolidation zone.</rdfs:comment>
        <rdfs:comment xml:lang="es">Agregado o zona de concentración parcelaria.</rdfs:comment>
    </owl:DatatypeProperty>
    


    <!-- http://opendata.aragon.es/def/ei2a#serieIdentifier -->

    <owl:DatatypeProperty rdf:about="http://opendata.aragon.es/def/ei2a#serieIdentifier">
        <rdfs:subPropertyOf rdf:resource="http://www.w3.org/2004/02/skos/core#notation"/>
        <rdfs:domain rdf:resource="http://opendata.aragon.es/def/ei2a#Series"/>
        <rdfs:range rdf:resource="http://www.w3.org/2000/01/rdf-schema#Literal"/>
    </owl:DatatypeProperty>
    


    <!-- http://opendata.aragon.es/def/ei2a#shareCoef -->

    <owl:DatatypeProperty rdf:about="http://opendata.aragon.es/def/ei2a#shareCoef">
        <rdfs:domain rdf:resource="http://opendata.aragon.es/def/ei2a#UrbanParcel"/>
        <rdfs:range rdf:resource="http://www.w3.org/2001/XMLSchema#float"/>
        <rdfs:comment xml:lang="en">Percentage ownership interest</rdfs:comment>
        <rdfs:comment xml:lang="es">Porcentaje de participación de una propiedad</rdfs:comment>
    </owl:DatatypeProperty>
    


    <!-- http://opendata.aragon.es/def/ei2a#siteIdentifier -->

    <owl:DatatypeProperty rdf:about="http://opendata.aragon.es/def/ei2a#siteIdentifier">
        <rdfs:subPropertyOf rdf:resource="http://www.w3.org/2004/02/skos/core#notation"/>
        <rdfs:domain rdf:resource="http://www.w3.org/ns/org#Site"/>
        <rdfs:range rdf:resource="http://www.w3.org/2000/01/rdf-schema#Literal"/>
    </owl:DatatypeProperty>
    


    <!-- http://opendata.aragon.es/def/ei2a#socialMediaSourceType -->

    <owl:DatatypeProperty rdf:about="http://opendata.aragon.es/def/ei2a#socialMediaSourceType">
        <rdfs:domain rdf:resource="http://opendata.aragon.es/def/ei2a#SocialMedia"/>
        <rdfs:range rdf:resource="http://www.w3.org/2000/01/rdf-schema#Literal"/>
        <rdfs:comment xml:lang="es">Tipo de la fuente de la comunicación social: texto, imagen, etc.</rdfs:comment>
        <rdfs:comment xml:lang="en">Type of the source of the social communication: text, image, etc.</rdfs:comment>
    </owl:DatatypeProperty>
    


    <!-- http://opendata.aragon.es/def/ei2a#staircaseIdentifier -->

    <owl:DatatypeProperty rdf:about="http://opendata.aragon.es/def/ei2a#staircaseIdentifier">
        <rdfs:domain rdf:resource="http://www.w3.org/ns/locn#Address"/>
        <rdfs:range rdf:resource="http://www.w3.org/2000/01/rdf-schema#Literal"/>
        <rdfs:comment xml:lang="es">Escalera de una dirección</rdfs:comment>
        <rdfs:comment xml:lang="en">Staricase of an address</rdfs:comment>
    </owl:DatatypeProperty>
    


    <!-- http://opendata.aragon.es/def/ei2a#startDate -->

    <owl:DatatypeProperty rdf:about="http://opendata.aragon.es/def/ei2a#startDate">
        <rdfs:domain rdf:resource="http://opendata.aragon.es/def/ei2a#Document"/>
        <rdfs:range rdf:resource="http://www.w3.org/2001/XMLSchema#dateTime"/>
        <rdfs:comment xml:lang="en">Document processing start date</rdfs:comment>
        <rdfs:comment xml:lang="es">Fecha de inicio de tramitación del documento</rdfs:comment>
    </owl:DatatypeProperty>
    


    <!-- http://opendata.aragon.es/def/ei2a#summary -->

    <owl:DatatypeProperty rdf:about="http://opendata.aragon.es/def/ei2a#summary">
        <rdfs:domain rdf:resource="http://opendata.aragon.es/def/ei2a#WebPage"/>
        <rdfs:range rdf:resource="http://www.w3.org/2000/01/rdf-schema#Literal"/>
        <rdfs:comment xml:lang="es">Resumen  de la web, subdominio o portal del Gobierno de Aragón analizada y procesada</rdfs:comment>
        <rdfs:comment xml:lang="en">Summary of the web, subdomain or portal of the Government of Aragon analyzed and processed</rdfs:comment>
    </owl:DatatypeProperty>
    


    <!-- http://opendata.aragon.es/def/ei2a#surface -->

    <owl:DatatypeProperty rdf:about="http://opendata.aragon.es/def/ei2a#surface">
        <rdfs:domain rdf:resource="http://opendata.aragon.es/def/ei2a#Compound"/>
        <rdfs:range rdf:resource="http://www.w3.org/2000/01/rdf-schema#Literal"/>
        <rdfs:comment xml:lang="en">Compound or enclosure surface</rdfs:comment>
        <rdfs:comment xml:lang="es">Superficie del recinto</rdfs:comment>
    </owl:DatatypeProperty>
    


    <!-- http://opendata.aragon.es/def/ei2a#surname1 -->

    <owl:DatatypeProperty rdf:about="http://opendata.aragon.es/def/ei2a#surname1">
        <rdfs:domain rdf:resource="http://www.w3.org/ns/person#Person"/>
        <rdfs:range rdf:resource="http://www.w3.org/2000/01/rdf-schema#Literal"/>
        <rdfs:comment xml:lang="en">First surname of a person</rdfs:comment>
        <rdfs:comment xml:lang="es">Primer apellido de una persona</rdfs:comment>
    </owl:DatatypeProperty>
    


    <!-- http://opendata.aragon.es/def/ei2a#surname2 -->

    <owl:DatatypeProperty rdf:about="http://opendata.aragon.es/def/ei2a#surname2">
        <rdfs:domain rdf:resource="http://www.w3.org/ns/person#Person"/>
        <rdfs:range rdf:resource="http://www.w3.org/2000/01/rdf-schema#Literal"/>
        <rdfs:comment xml:lang="en">Second last name of a person</rdfs:comment>
        <rdfs:comment xml:lang="es">Segundo apellido de una persona</rdfs:comment>
    </owl:DatatypeProperty>
    


    <!-- http://opendata.aragon.es/def/ei2a#typeAdministrativeRecord -->

    <owl:DatatypeProperty rdf:about="http://opendata.aragon.es/def/ei2a#typeAdministrativeRecord">
        <rdfs:domain rdf:resource="http://opendata.aragon.es/def/ei2a#AdministrativeRecord"/>
        <rdfs:range rdf:resource="http://www.w3.org/2000/01/rdf-schema#Literal"/>
        <rdfs:comment xml:lang="en">Administrative record type</rdfs:comment>
        <rdfs:comment xml:lang="en">Tipo de expediente</rdfs:comment>
    </owl:DatatypeProperty>
    


    <!-- http://opendata.aragon.es/def/ei2a#unitIdentifier -->

    <owl:DatatypeProperty rdf:about="http://opendata.aragon.es/def/ei2a#unitIdentifier">
        <rdfs:domain rdf:resource="http://www.w3.org/ns/locn#Address"/>
        <rdfs:range rdf:resource="http://www.w3.org/2000/01/rdf-schema#Literal"/>
        <rdfs:comment xml:lang="en">Address door</rdfs:comment>
        <rdfs:comment xml:lang="es">Puerta de una dirección</rdfs:comment>
    </owl:DatatypeProperty>
    


    <!-- http://opendata.aragon.es/def/ei2a#use -->

    <owl:DatatypeProperty rdf:about="http://opendata.aragon.es/def/ei2a#use">
        <rdfs:domain>
            <owl:Class>
                <owl:unionOf rdf:parseType="Collection">
                    <rdf:Description rdf:about="http://opendata.aragon.es/def/ei2a#Compound"/>
                    <rdf:Description rdf:about="http://opendata.aragon.es/def/ei2a#UrbanParcel"/>
                </owl:unionOf>
            </owl:Class>
        </rdfs:domain>
        <rdfs:range rdf:resource="http://www.w3.org/2000/01/rdf-schema#Literal"/>
        <rdfs:comment xml:lang="en">Main use to which an agricultural parcel is dedicated</rdfs:comment>
        <rdfs:comment xml:lang="es">Uso principal al que está dedicada una parcela agraria</rdfs:comment>
    </owl:DatatypeProperty>
    


    <!-- http://opendata.aragon.es/def/ei2a#zone -->

    <owl:DatatypeProperty rdf:about="http://opendata.aragon.es/def/ei2a#zone">
        <rdfs:domain rdf:resource="http://opendata.aragon.es/def/ei2a#Compound"/>
        <rdfs:range rdf:resource="http://www.w3.org/2000/01/rdf-schema#Literal"/>
        <rdfs:comment xml:lang="en">Area or zone of the compound</rdfs:comment>
        <rdfs:comment xml:lang="es">Zona o área del recinto</rdfs:comment>
    </owl:DatatypeProperty>
    


    <!-- http://purl.org/dc/elements/1.1/type -->

    <owl:DatatypeProperty rdf:about="http://purl.org/dc/elements/1.1/type"/>
    


    <!-- http://vocab.gtfs.org/terms#arrivalTime -->

    <owl:DatatypeProperty rdf:about="http://vocab.gtfs.org/terms#arrivalTime">
        <rdfs:domain rdf:resource="http://vocab.gtfs.org/terms#StopTime"/>
        <rdfs:range rdf:resource="http://www.w3.org/2001/XMLSchema#duration"/>
        <rdfs:comment xml:lang="en">Check the original specification for special cases</rdfs:comment>
        <rdfs:comment xml:lang="es">Compruebe la especificación original para casos especiales</rdfs:comment>
        <rdfs:label xml:lang="en">Arrival time</rdfs:label>
        <rdfs:label xml:lang="es">hora de llegada</rdfs:label>
        <rdfs:seeAlso rdf:resource="https://developers.google.com/transit/gtfs/reference#stop_times_fields"/>
        <status:term_status xml:lang="es">inestable</status:term_status>
        <status:term_status xml:lang="en">unstable</status:term_status>
    </owl:DatatypeProperty>
    


    <!-- http://vocab.gtfs.org/terms#dateAddition -->

    <owl:DatatypeProperty rdf:about="http://vocab.gtfs.org/terms#dateAddition">
        <rdfs:domain rdf:resource="http://vocab.gtfs.org/terms#CalendarDateRule"/>
        <rdfs:range rdf:resource="http://www.w3.org/2001/XMLSchema#boolean"/>
        <comment xml:lang="es">El campo exception_type en calendar_dates.txt - 1 es cierto, 2 es falso.</comment>
        <comment xml:lang="en">The exception_type field in calendar_dates.txt - 1 is true, 2 is false.</comment>
        <rdfs:comment xml:lang="en">A boolean whether to add (true) or remove (false) a date</rdfs:comment>
        <rdfs:comment xml:lang="es">Booleano que indica si el servicio se ha agregado (cierto) o suprimido (falso) en la fecha especificada</rdfs:comment>
        <rdfs:label xml:lang="en">Date Addition</rdfs:label>
        <rdfs:label xml:lang="es">incorporación de fecha</rdfs:label>
        <status:term_status xml:lang="es">inestable</status:term_status>
        <status:term_status xml:lang="en">unstable</status:term_status>
    </owl:DatatypeProperty>
    


    <!-- http://vocab.gtfs.org/terms#departureTime -->

    <owl:DatatypeProperty rdf:about="http://vocab.gtfs.org/terms#departureTime">
        <rdfs:domain rdf:resource="http://vocab.gtfs.org/terms#StopTime"/>
        <rdfs:range rdf:resource="http://www.w3.org/2001/XMLSchema#duration"/>
        <rdfs:comment xml:lang="en">Check the original specification for special cases</rdfs:comment>
        <rdfs:comment xml:lang="es">Compruebe la especificación original para casos especiales</rdfs:comment>
        <rdfs:label xml:lang="en">Departure time</rdfs:label>
        <rdfs:label xml:lang="es">hora de salida</rdfs:label>
        <rdfs:seeAlso rdf:resource="https://developers.google.com/transit/gtfs/reference#stop_times_fields"/>
        <status:term_status xml:lang="es">inestable</status:term_status>
        <status:term_status xml:lang="en">unstable</status:term_status>
    </owl:DatatypeProperty>
    


    <!-- http://vocab.gtfs.org/terms#friday -->

    <owl:DatatypeProperty rdf:about="http://vocab.gtfs.org/terms#friday">
        <rdfs:range rdf:resource="http://www.w3.org/2001/XMLSchema#boolean"/>
        <rdfs:comment xml:lang="en">Service is available on Friday</rdfs:comment>
        <rdfs:comment xml:lang="es">Servicio disponible los viernes</rdfs:comment>
        <rdfs:label xml:lang="en">Friday</rdfs:label>
        <rdfs:label xml:lang="es">viernes</rdfs:label>
        <status:term_status xml:lang="es">inestable</status:term_status>
        <status:term_status xml:lang="en">unstable</status:term_status>
    </owl:DatatypeProperty>
    


    <!-- http://vocab.gtfs.org/terms#monday -->

    <owl:DatatypeProperty rdf:about="http://vocab.gtfs.org/terms#monday">
        <rdfs:range rdf:resource="http://www.w3.org/2001/XMLSchema#boolean"/>
        <rdfs:comment xml:lang="en">Service is available on Monday</rdfs:comment>
        <rdfs:comment xml:lang="es">Servicio disponible los lunes</rdfs:comment>
        <rdfs:label xml:lang="en">Monday</rdfs:label>
        <rdfs:label xml:lang="es">lunes</rdfs:label>
        <status:term_status xml:lang="es">inestable</status:term_status>
        <status:term_status xml:lang="en">unstable</status:term_status>
    </owl:DatatypeProperty>
    


    <!-- http://vocab.gtfs.org/terms#saturday -->

    <owl:DatatypeProperty rdf:about="http://vocab.gtfs.org/terms#saturday">
        <rdfs:range rdf:resource="http://www.w3.org/2001/XMLSchema#boolean"/>
        <rdfs:comment xml:lang="en">Service is available on Saturday</rdfs:comment>
        <rdfs:comment xml:lang="es">Servicio disponible los sábados</rdfs:comment>
        <rdfs:label xml:lang="en">Saturday</rdfs:label>
        <rdfs:label xml:lang="es">sábado</rdfs:label>
        <status:term_status xml:lang="es">inestable</status:term_status>
        <status:term_status xml:lang="en">unstable</status:term_status>
    </owl:DatatypeProperty>
    


    <!-- http://vocab.gtfs.org/terms#stopSequence -->

    <owl:DatatypeProperty rdf:about="http://vocab.gtfs.org/terms#stopSequence">
        <rdfs:domain rdf:resource="http://vocab.gtfs.org/terms#StopTime"/>
        <rdfs:range rdf:resource="http://www.w3.org/2001/XMLSchema#nonNegativeInteger"/>
        <rdfs:comment xml:lang="es">Indica el orden de paradas para un viaje concreto. Los valores de gtfs:stopSequence deben ser enteros no negativos, deben aumentar durante el viaje referenciado por la propiedad gtfs:trip.</rdfs:comment>
        <rdfs:comment xml:lang="en">The stopSequence property identifies the order of the stops for a particular trip. The values must increase along the gtfs:Trip referenced in the gtfs:trip property.</rdfs:comment>
        <rdfs:label xml:lang="en">Stop sequence</rdfs:label>
        <rdfs:label xml:lang="es">secuencia de paradas</rdfs:label>
        <status:term_status xml:lang="es">inestable</status:term_status>
        <status:term_status xml:lang="en">unstable</status:term_status>
    </owl:DatatypeProperty>
    


    <!-- http://vocab.gtfs.org/terms#sunday -->

    <owl:DatatypeProperty rdf:about="http://vocab.gtfs.org/terms#sunday">
        <rdfs:range rdf:resource="http://www.w3.org/2001/XMLSchema#boolean"/>
        <rdfs:comment xml:lang="en">Service is available on Sunday</rdfs:comment>
        <rdfs:comment xml:lang="es">Servicio disponible los domingos</rdfs:comment>
        <rdfs:label xml:lang="en">Sunday</rdfs:label>
        <rdfs:label xml:lang="es">domingos</rdfs:label>
        <status:term_status xml:lang="es">inestable</status:term_status>
        <status:term_status xml:lang="en">unstable</status:term_status>
    </owl:DatatypeProperty>
    


    <!-- http://vocab.gtfs.org/terms#thursday -->

    <owl:DatatypeProperty rdf:about="http://vocab.gtfs.org/terms#thursday">
        <rdfs:range rdf:resource="http://www.w3.org/2001/XMLSchema#boolean"/>
        <rdfs:comment xml:lang="en">Service is available on Thursday</rdfs:comment>
        <rdfs:comment xml:lang="es">Servicio disponible los jueves</rdfs:comment>
        <rdfs:label xml:lang="en">Thursday</rdfs:label>
        <rdfs:label xml:lang="es">jueves</rdfs:label>
        <status:term_status xml:lang="es">inestable</status:term_status>
        <status:term_status xml:lang="en">unstable</status:term_status>
    </owl:DatatypeProperty>
    


    <!-- http://vocab.gtfs.org/terms#tuesday -->

    <owl:DatatypeProperty rdf:about="http://vocab.gtfs.org/terms#tuesday">
        <rdfs:range rdf:resource="http://www.w3.org/2001/XMLSchema#boolean"/>
        <rdfs:comment xml:lang="en">Service is available on Tuesday</rdfs:comment>
        <rdfs:comment xml:lang="es">Servicio disponible los martes</rdfs:comment>
        <rdfs:label xml:lang="en">Tuesday</rdfs:label>
        <rdfs:label xml:lang="es">martes</rdfs:label>
        <status:term_status xml:lang="es">inestable</status:term_status>
        <status:term_status xml:lang="en">unstable</status:term_status>
    </owl:DatatypeProperty>
    


    <!-- http://vocab.gtfs.org/terms#wednesday -->

    <owl:DatatypeProperty rdf:about="http://vocab.gtfs.org/terms#wednesday">
        <rdfs:range rdf:resource="http://www.w3.org/2001/XMLSchema#boolean"/>
        <rdfs:comment xml:lang="en">Service is available on Wednesday</rdfs:comment>
        <rdfs:comment xml:lang="es">Servicio disponible los miércoles</rdfs:comment>
        <rdfs:label xml:lang="en">Wednesday</rdfs:label>
        <rdfs:label xml:lang="es">miércoles</rdfs:label>
        <status:term_status xml:lang="es">inestable</status:term_status>
        <status:term_status xml:lang="en">unstable</status:term_status>
    </owl:DatatypeProperty>
    


    <!-- http://www.ontologydesignpatterns.org/ont/dul/DUL.owl#hasDataValue -->

    <owl:DatatypeProperty rdf:about="http://www.ontologydesignpatterns.org/ont/dul/DUL.owl#hasDataValue">
        <owl:equivalentProperty rdf:resource="http://www.semanticwater.com/WISDOM#hasValue"/>
        <rdfs:domain rdf:resource="http://www.ontologydesignpatterns.org/ont/dul/DUL.owl#Entity"/>
        <rdfs:comment>A datatype property that encodes values from a datatype for an Entity. 
There are several ways to encode values in DOLCE (Ultralite):

1) Directly assert an xsd:_ value to an Entity by using hasDataValue
2) Assert a Region for an Entity by using hasRegion, and then assert an xsd:_ value to that Region, by using hasRegionDataValue
3) Assert a Quality for an Entity by using hasQuality, then assert a Region for that Quality, and assert an xsd:_ value to that Region, by using hasRegionDataValue
4) When the value is required, but not directly observed, assert a Parameter for an xsd:_ value by using hasParameterDataValue, and then associate the Parameter to an Entity by using isConstraintFor
5) When the value is required, but not directly observed, you can also assert a Parameter for a Region by using parametrizes, and then assert an xsd:_ value to that Region, by using hasRegionDataValue

The five approaches obey different requirements. 
For example, a simple value can be easily asserted by using pattern (1), but if one needs to assert an interval between two values, a Region should be introduced to materialize that interval, as pattern (2) suggests. 
Furthermore, if one needs to distinguish the individual Quality of a value, e.g. the particular nature of the density of a substance, pattern (3) can be used. 
Patterns (4) and (5) should be used instead when a constraint or a selection is modeled, independently from the actual observation of values in the real world.</rdfs:comment>
        <rdfs:label xml:lang="it">ha valore</rdfs:label>
        <rdfs:label xml:lang="en">has data value</rdfs:label>
    </owl:DatatypeProperty>
    


    <!-- http://www.semanticwater.com/WISDOM#hasLength -->

    <owl:DatatypeProperty rdf:about="http://www.semanticwater.com/WISDOM#hasLength">
        <rdfs:subPropertyOf rdf:resource="http://www.semanticwater.com/WISDOM#hasPipeProperty"/>
        <rdf:type rdf:resource="http://www.w3.org/2002/07/owl#FunctionalProperty"/>
        <rdfs:range rdf:resource="http://www.w3.org/2001/XMLSchema#double"/>
        <rdfs:label xml:lang="en">hasLength</rdfs:label>
    </owl:DatatypeProperty>
    


    <!-- http://www.semanticwater.com/WISDOM#hasMeterProperty -->

    <owl:DatatypeProperty rdf:about="http://www.semanticwater.com/WISDOM#hasMeterProperty"/>
    


    <!-- http://www.semanticwater.com/WISDOM#hasNetworkPropertyValue -->

    <owl:DatatypeProperty rdf:about="http://www.semanticwater.com/WISDOM#hasNetworkPropertyValue">
        <rdfs:domain rdf:resource="http://www.semanticwater.com/WISDOM#PhysicalTopologicalEntity"/>
    </owl:DatatypeProperty>
    


    <!-- http://www.semanticwater.com/WISDOM#hasNominalDiameter -->

    <owl:DatatypeProperty rdf:about="http://www.semanticwater.com/WISDOM#hasNominalDiameter">
        <rdfs:subPropertyOf rdf:resource="http://www.semanticwater.com/WISDOM#hasNetworkPropertyValue"/>
        <rdf:type rdf:resource="http://www.w3.org/2002/07/owl#FunctionalProperty"/>
        <rdfs:range rdf:resource="http://www.w3.org/2001/XMLSchema#double"/>
        <rdfs:label xml:lang="en">hasNominalDiameter</rdfs:label>
    </owl:DatatypeProperty>
    


    <!-- http://www.semanticwater.com/WISDOM#hasPipeProperty -->

    <owl:DatatypeProperty rdf:about="http://www.semanticwater.com/WISDOM#hasPipeProperty">
        <rdfs:label xml:lang="en">hasPipeProperty</rdfs:label>
    </owl:DatatypeProperty>
    


    <!-- http://www.semanticwater.com/WISDOM#hasValue -->

    <owl:DatatypeProperty rdf:about="http://www.semanticwater.com/WISDOM#hasValue">
        <rdfs:subPropertyOf rdf:resource="http://www.w3.org/2002/07/owl#topDataProperty"/>
        <alignedWithWatERP>hasValue</alignedWithWatERP>
    </owl:DatatypeProperty>
    


    <!-- http://www.w3.org/ns/org#identifier -->

    <rdf:Description rdf:about="http://www.w3.org/ns/org#identifier">
        <rdfs:range rdf:resource="http://www.w3.org/2000/01/rdf-schema#Literal"/>
    </rdf:Description>
    


    <!-- 
    ///////////////////////////////////////////////////////////////////////////////////////
    //
    // Classes
    //
    ///////////////////////////////////////////////////////////////////////////////////////
     -->

    


    <!-- http://harmonet.org/harmonise.rdfs#Accommodation -->

    <owl:Class rdf:about="http://harmonet.org/harmonise.rdfs#Accommodation">
        <rdfs:subClassOf rdf:resource="http://www.w3.org/ns/org#Organization"/>
        <rdfs:comment>The Accommodation aggregated concept is the primary accommodation entity. An accommodation is in one location and is managed by an organiser. It may physically consist of a number of buildings in proximity to one another. However, if an accommodation is spread across a number of locations then these are treated as multiple accommodations.
An accommodation may consist of a hotel, or a bed and breakfast, or a pension, or any other form of accommodation which provides private-room, catered services to guests. The self-catering and camping sectors are excluded from the scope of the accommodation concept. However, the accommodation ontology is structured in such a way as to facilitate the broadening of the sub domain in the future. 

An accommodation is made up of a number of units (often bedrooms). The accommodation has facilities which are available on a per-accommodation basis (accommodation-level facilities), such as a swimming pool or car park. The units also have facilities, which are available on a per-unit basis (unit-level facilities), such as hair-dryers.</rdfs:comment>
        <rdfs:label>Accommodation</rdfs:label>
    </owl:Class>
    


    <!-- http://harmonet.org/harmonise.rdfs#Attraction -->

    <owl:Class rdf:about="http://harmonet.org/harmonise.rdfs#Attraction">
        <rdfs:subClassOf rdf:resource="http://www.w3.org/ns/org#Organization"/>
        <rdfs:comment>An attraction has much in common with an accommodation and has many similar properties. This reflects the fact that both are tourism offerings, both are static (i.e. do not move from place to place), both are available most or all of the time, and both have associated costs.</rdfs:comment>
        <rdfs:label>Attraction</rdfs:label>
    </owl:Class>
    


    <!-- http://harmonet.org/harmonise.rdfs#Award -->

    <owl:Class rdf:about="http://harmonet.org/harmonise.rdfs#Award">
        <rdfs:comment>This aggregated concept provides information about the award or standard allocated to a tourism offering such as an accommodation or a restaurant. The aggregated concept reflects the reality that there are many awarding bodies, including the AA, the ADAC, the national tourism organisations, etc. The awardRange specifies the maximal value an offering can achieve. Usual gradings like ‘+’ and ‘-‘ are represented by the values ‘.3’ and ‘.7’.</rdfs:comment>
        <rdfs:label>Award</rdfs:label>
    </owl:Class>
    


    <!-- http://harmonet.org/harmonise.rdfs#Date -->

    <owl:Class rdf:about="http://harmonet.org/harmonise.rdfs#Date">
        <rdfs:comment>The Date aggregated concept contains year, month and day-of-month values. Each date aggregated concept represents one calendar day. The dateText property allows the name of a particular day (e.g. Christmas) to be included.</rdfs:comment>
        <rdfs:label>Date</rdfs:label>
    </owl:Class>
    


    <!-- http://harmonet.org/harmonise.rdfs#DateRange -->

    <owl:Class rdf:about="http://harmonet.org/harmonise.rdfs#DateRange">
        <rdfs:comment>The DateRange aggregated concept represents a number of consecutive days. It includes a start date and an end date, both of which are included in the DateRange. Thus, for example, the DateRange.startDate might be 01 March 2003, the DateRange.endDate might be 5 March 2003, and the DateRange would include the days 01,02,03,04 and 05 March 2003.</rdfs:comment>
        <rdfs:label>DateRange</rdfs:label>
    </owl:Class>
    


    <!-- http://harmonet.org/harmonise.rdfs#Facility -->

    <owl:Class rdf:about="http://harmonet.org/harmonise.rdfs#Facility">
        <rdfs:comment>This aggregated concept aggregates information about a facility. Such a construct is useful in different tourism domains, e.g. accommodation or gastronomy. Facilities may be associated with an accommodation, or with a single unit within an accommodation, or have some other, non-accommodation scope. This is reflected in the Extent property. Facilities may be available to all, or may be restricted to certain categories of user (e.g. golf course available only to penthouse guests). Lists of unit and accommodation facilities are provided in Appendix A.</rdfs:comment>
        <rdfs:label>Facility</rdfs:label>
    </owl:Class>
    


    <!-- http://harmonet.org/harmonise.rdfs#Gastro -->

    <owl:Class rdf:about="http://harmonet.org/harmonise.rdfs#Gastro">
        <rdfs:subClassOf rdf:resource="http://www.w3.org/ns/org#Organization"/>
        <rdfs:comment>The Gastro aggregated concept is the primary food and drink entity. A gastro is in one location and is managed by one organisation. It may physically consist of a number of buildings in proximity to one another. However, if a gastro is spread across a number of locations then these are treated as multiple gastros. Also, if a single establishment includes two different offerings (e.g. a bar, with basic bar food, and a restaurant with a la carte gourmet offerings), this is treated as two gastros, which are related to one another.
A gastro may consist of a restaurant, a pub, a mountain hut, a sandwich shop, or any other form of location which provides prepared food or drink for consumption on or off the premises. 

A gastro has much in common with an accommodation, such as a location, an organiser, etc. However, it also has many attributes of its own, particularly those which focus on the food and drink available in the gastro. 

The key attributes of a gastro, which differ from those of an accommodation are 
-	The gastroType of the gastro 
-	The cuisine served (which may be primarily drink, in some cases)
-	The profile values (e.g. whether or not outside catering is provided, whether picnics are allowed, etc.)
-	The facility values (e.g. whether there are separate children’s dining areas, whether there is a smoking room, etc.)
The profile and facility values are considered as extensions to the existing (accommodation) profile and facility values.</rdfs:comment>
        <rdfs:label>Gastro</rdfs:label>
    </owl:Class>
    


    <!-- http://harmonet.org/harmonise.rdfs#ListValue -->

    <owl:Class rdf:about="http://harmonet.org/harmonise.rdfs#ListValue">
        <rdfs:comment>The ListValue aggregated concept contains a value of a value list defined globally within the complete HarmoNET network as well as a value of a domain specific value list together with the name of the domain. The HarmoNET-wide unique value enables a mapping between domain specific value lists while the domain specific value avoids a loss of information in case a precise mapping is not possible.</rdfs:comment>
        <rdfs:label>ListValue</rdfs:label>
    </owl:Class>
    


    <!-- http://harmonet.org/harmonise.rdfs#PointOfTime -->

    <owl:Class rdf:about="http://harmonet.org/harmonise.rdfs#PointOfTime">
        <rdfs:comment>The aggregated concept PointOfTime specifies a point of time consisting of a date and a daytime.</rdfs:comment>
        <rdfs:label>PointOfTime</rdfs:label>
    </owl:Class>
    


    <!-- http://harmonet.org/harmonise.rdfs#Profile -->

    <owl:Class rdf:about="http://harmonet.org/harmonise.rdfs#Profile">
        <rdfs:comment>The Profile aggregated concept is used to hold multiple attribute-value pairs which characterise a tourism resource or offering. These may be at accommodation, room or other level, depending on the parent concept. The profile consists of multiple profileField concepts.</rdfs:comment>
        <rdfs:label>Profile</rdfs:label>
    </owl:Class>
    


    <!-- http://harmonet.org/harmonise.rdfs#ProfileField -->

    <owl:Class rdf:about="http://harmonet.org/harmonise.rdfs#ProfileField">
        <rdfs:comment>The ProfileField Aggregated Concept is a simple attribute-value pair construct. It links a profile field to a value. Thus, on an accommodation level, it might link the number of rooms with a shower, to an integer value, to indicated that an accommodation has (say) 39 rooms with a shower. On a unit level, it might indicate that a room is wheelchair-accessible. Lists of profile values are available, at the accommodation and unit level, in Appendix A.</rdfs:comment>
        <rdfs:label>ProfileField</rdfs:label>
    </owl:Class>
    


    <!-- http://harmonet.org/harmonise.rdfs#ReferencedValue -->

    <owl:Class rdf:about="http://harmonet.org/harmonise.rdfs#ReferencedValue">
        <rdfs:comment>The ReferencedValue aggregated concept contains a value and the name of the domain the value is defined in.</rdfs:comment>
        <rdfs:label>ReferencedValue</rdfs:label>
    </owl:Class>
    


    <!-- http://harmonet.org/harmonise.rdfs#Service -->

    <owl:Class rdf:about="http://harmonet.org/harmonise.rdfs#Service"/>
    


    <!-- http://harmonet.org/harmonise.rdfs#Timeline -->

    <owl:Class rdf:about="http://harmonet.org/harmonise.rdfs#Timeline">
        <rdfs:comment>The Timeline aggregated concept represents a complex timeline, e.g. the opening times of an accommodation, an event, a restaurant, etc. By using the various aggregated concepts outlined above, it specifies the dates and days when the resource is open, and the times of day when access to the resource can be gained (e.g. Reception opening hours). It reflects the complexity of time models by also including a free-text Exceptions element, which can be used to explain any unusual deviations from the Timeline.</rdfs:comment>
        <rdfs:label>Timeline</rdfs:label>
    </owl:Class>
    


    <!-- http://opendata.aragon.es/def/ei2a#DatatypeProperty -->

    <owl:Class rdf:about="http://opendata.aragon.es/def/ei2a#DatatypeProperty"/>
    


    <!-- http://opendata.aragon.es/def/ei2a#AdministrativeLevel -->

    <owl:Class rdf:about="http://opendata.aragon.es/def/ei2a#AdministrativeLevel">
        <owl:equivalentClass>
            <owl:Class>
                <owl:oneOf rdf:parseType="Collection">
                    <rdf:Description rdf:about="http://opendata.aragon.es/def/ei2a#AdministraciónAutonómica"/>
                    <rdf:Description rdf:about="http://opendata.aragon.es/def/ei2a#AdministraciónDeJusticia"/>
                    <rdf:Description rdf:about="http://opendata.aragon.es/def/ei2a#AdministraciónDelEstado"/>
                    <rdf:Description rdf:about="http://opendata.aragon.es/def/ei2a#AdministraciónLocal"/>
                    <rdf:Description rdf:about="http://opendata.aragon.es/def/ei2a#OtrasInstituciones"/>
                    <rdf:Description rdf:about="http://opendata.aragon.es/def/ei2a#Universidades"/>
                </owl:oneOf>
            </owl:Class>
        </owl:equivalentClass>
        <rdfs:comment xml:lang="en">Administration level that represents the territorial level of administration to which a unit or office belongs and in which they exercise their powers, according to article 2.1 of Law 39/2015.

For those organizations within the ontology whose type isórganoAdministrativo, the level of administration is considered mandatory.

The domain of values that presents this class are: AdministraciónDelEstado, 
AdministraciónAutonómica, AdministraciónLocal, Universidades, OtrasInstituciones, AdministraciónDeJusticia.

For more information regarding these values, consult the Electronic Administration Portal (PAE, https://administracionelectronica.gob.es) and the Attributes Manual (https://administracionelectronica.gob.es/ctt/resources/Soluciones/238/Area%20descargas/Manual%20de%20Atributos.pdf?idIniciativa=238&amp;idElemento=420)</rdfs:comment>
        <rdfs:comment xml:lang="es">Nivel de administración que representa el nivel territorial de administración al que pertenece una unidad u oficina y en el cual ejercen sus competencias, según el artículo 2.1 de la Ley 39/2015. 

Para aquellas organizaciones dentro de la ontología cuyo tipo sea órganoAdministrativo, el nivel de administración se considera obligatorio.

El dominio de valores que presenta esta clase son: AdministraciónDelEstado, 
AdministraciónAutonómica, AdministraciónLocal, Universidades, OtrasInstituciones, AdministraciónDeJusticia.

Para más información relativa a estos valores consultar sobre el  Portal de Administración electrónica (PAE, https://administracionelectronica.gob.es) y el manual de atributos (https://administracionelectronica.gob.es/ctt/resources/Soluciones/238/Area%20descargas/Manual%20de%20Atributos.pdf?idIniciativa=238&amp;idElemento=420)</rdfs:comment>
    </owl:Class>
    


    <!-- http://opendata.aragon.es/def/ei2a#AdministrativeRecord -->

    <owl:Class rdf:about="http://opendata.aragon.es/def/ei2a#AdministrativeRecord">
        <rdfs:subClassOf rdf:resource="http://opendata.aragon.es/def/ei2a#Document"/>
        <rdfs:comment xml:lang="es">Conjunto de documentos que corresponden a una determinada cuestión y que conforman el expediente administrativo.</rdfs:comment>
        <rdfs:comment xml:lang="en">Set of documents that correspond to a certain question and that form the administrative record.</rdfs:comment>
    </owl:Class>
    


    <!-- http://opendata.aragon.es/def/ei2a#AdministrativeRecordStatus -->

    <owl:Class rdf:about="http://opendata.aragon.es/def/ei2a#AdministrativeRecordStatus">
        <owl:equivalentClass>
            <owl:Class>
                <owl:oneOf rdf:parseType="Collection">
                    <rdf:Description rdf:about="http://opendata.aragon.es/def/ei2a#close"/>
                    <rdf:Description rdf:about="http://opendata.aragon.es/def/ei2a#indexForClosedRemission"/>
                    <rdf:Description rdf:about="http://opendata.aragon.es/def/ei2a#open"/>
                </owl:oneOf>
            </owl:Class>
        </owl:equivalentClass>
        <rdfs:comment xml:lang="es">Estado del expediente en el momento de intercambio.  Esta clase es una clase enumerada que tiene los siguientes valores: close, indexForCloseRemission, open.

De acuerdo a la Guía de aplicación de la Norma Técnica de Interoperabilidad de Expediente Electrónico (edición 2016), el expediente puede estar cerrado, abierto o índice para remisión cerrado.</rdfs:comment>
        <rdfs:comment xml:lang="en">Status of the administrative record at the time of exchange. This class is an enumerated class that has the following values: close, indexForCloseRemission, open.

According to the Application Guide of the Technical Standard for Electronic File Interoperability (2016 edition), the administrative record may be closed, open or closed reference index.</rdfs:comment>
    </owl:Class>
    


    <!-- http://opendata.aragon.es/def/ei2a#ArableSubparcel -->

    <owl:Class rdf:about="http://opendata.aragon.es/def/ei2a#ArableSubparcel">
        <rdfs:subClassOf rdf:resource="http://opendata.aragon.es/def/ei2a#Compound"/>
    </owl:Class>
    


    <!-- http://opendata.aragon.es/def/ei2a#BankAccount -->

    <owl:Class rdf:about="http://opendata.aragon.es/def/ei2a#BankAccount">
        <rdfs:subClassOf>
            <owl:Restriction>
                <owl:onProperty rdf:resource="http://opendata.aragon.es/def/ei2a#bankAccountIdentifier"/>
                <owl:cardinality rdf:datatype="http://www.w3.org/2001/XMLSchema#nonNegativeInteger">1</owl:cardinality>
            </owl:Restriction>
        </rdfs:subClassOf>
        <owl:hasKey rdf:parseType="Collection">
            <rdf:Description rdf:about="http://opendata.aragon.es/def/ei2a#bankAccountIdentifier"/>
        </owl:hasKey>
        <rdfs:comment xml:lang="es">Contrato financiero con una entidad bancaria en virtud del cual se registran el balance y los subsiguientes movimientos de dinero del cliente. 	

Con el objetivo de facilitar el tratamiento automático de pagos y cobros transfronterizos, se utiliza el código International Bank Account Number (IBAN). Este código es un código alfanumérico que identifica una cuenta bancaria determinada en una entidad financiera en cualquier lugar del mundo (si el país está adherido al sistema IBAN). Es decir, a cada cuenta le corresponde un único IBAN mediante el cual se identifica el país, la entidad, la oficina y la cuenta.</rdfs:comment>
        <rdfs:comment xml:lang="en">Financial contract with a banking entity under which the balance and the subsequent money movements of the customer are recorded.

The International Bank Account Number (IBAN) is used to facilitate the automatic processing of cross-border payments and charges. This code is an alphanumeric code that identifies a particular bank account in a financial institution anywhere in the world (if the country is an IBAN member). That is, each account corresponds to a single IBAN that identifies the country, entity, office and account.</rdfs:comment>
    </owl:Class>
    


    <!-- http://opendata.aragon.es/def/ei2a#CadastralParcel -->

    <owl:Class rdf:about="http://opendata.aragon.es/def/ei2a#CadastralParcel">
        <rdfs:subClassOf>
            <owl:Restriction>
                <owl:onProperty rdf:resource="http://opendata.aragon.es/def/ei2a#cadastralParcelIdentifier"/>
                <owl:cardinality rdf:datatype="http://www.w3.org/2001/XMLSchema#nonNegativeInteger">1</owl:cardinality>
            </owl:Restriction>
        </rdfs:subClassOf>
        <owl:hasKey rdf:parseType="Collection">
            <rdf:Description rdf:about="http://opendata.aragon.es/def/ei2a#cadastralParcelIdentifier"/>
        </owl:hasKey>
        <rdfs:comment xml:lang="es">Porción de terreno o superficie terrestre, que puede ser descrito por algunos elementos tales como geometría, identificador único y referencia catastral.</rdfs:comment>
        <rdfs:comment xml:lang="en">Portion of land or land surface, which can be described by some elements such as geometry, unique identifier and cadastral reference.</rdfs:comment>
    </owl:Class>
    


    <!-- http://opendata.aragon.es/def/ei2a#CadastralRuralParcel -->

    <owl:Class rdf:about="http://opendata.aragon.es/def/ei2a#CadastralRuralParcel">
        <rdfs:subClassOf rdf:resource="http://opendata.aragon.es/def/ei2a#RuralParcel"/>
        <rdfs:comment xml:lang="es">Porción de terreno o superficie terrestre rural, que puede ser descrito por algunos elementos tales como geometría, identificador único y referencia catastral.</rdfs:comment>
        <rdfs:comment xml:lang="en">Portion of  rural land or land surface, which can be described by some elements such as geometry, unique identifier and cadastral reference.</rdfs:comment>
    </owl:Class>
    


    <!-- http://opendata.aragon.es/def/ei2a#Citation -->

    <owl:Class rdf:about="http://opendata.aragon.es/def/ei2a#Citation">
        <rdfs:comment xml:lang="es">Citación de una entidad (pesona, organización o localización) en una web, subdominios y/o portal del Gobierno de Aragón. Es una relación n-aria</rdfs:comment>
        <rdfs:comment xml:lang="en">Citation of an entity (person, organization or location) in a web, subdomains and / or portal of the Government of Aragon. Represents an n-ary relation</rdfs:comment>
    </owl:Class>
    


    <!-- http://opendata.aragon.es/def/ei2a#Compound -->

    <owl:Class rdf:about="http://opendata.aragon.es/def/ei2a#Compound">
        <owl:equivalentClass rdf:resource="http://opendata.aragon.es/def/ei2a#Subparcel"/>
        <rdfs:subClassOf rdf:resource="http://opendata.aragon.es/def/ei2a#RuralParcel"/>
        <rdfs:comment xml:lang="en">Compound, fundamental unit of SIGPAC. Continuous surface of land, within a parcel, with the same stable agricultural use. In each rural plot there may be one or several enclosures depending on the crop or group of crops that is carried out in it.</rdfs:comment>
        <rdfs:comment xml:lang="es">Recinto, unidad fundamental del SIGPAC.  Superficie continúa de terreno, dentro deuna parcela, con un mismo uso agrícola estable. En cada parcela rural puede haber uno o varios recintos en función del cultivo o grupo de cultivos que se realice en ella.</rdfs:comment>
    </owl:Class>
    


    <!-- http://opendata.aragon.es/def/ei2a#CreditCard -->

    <owl:Class rdf:about="http://opendata.aragon.es/def/ei2a#CreditCard">
        <rdfs:subClassOf>
            <owl:Restriction>
                <owl:onProperty rdf:resource="http://opendata.aragon.es/def/ei2a#creditCardIdentifier"/>
                <owl:cardinality rdf:datatype="http://www.w3.org/2001/XMLSchema#nonNegativeInteger">1</owl:cardinality>
            </owl:Restriction>
        </rdfs:subClassOf>
        <owl:hasKey rdf:parseType="Collection">
            <rdf:Description rdf:about="http://opendata.aragon.es/def/ei2a#creditCardIdentifier"/>
        </owl:hasKey>
        <rdfs:comment xml:lang="en">Card issued by a banking entity that allows certain transactions to be performed from an ATM and the purchase of goods and services on credit; It is usually plastic and has a magnetic stripe on one of its faces.</rdfs:comment>
        <rdfs:comment xml:lang="es">Tarjeta emitida por una entidad bancaria que permite realizar ciertas operaciones desde un cajero automático y la compra de bienes y servicios a crédito; generalmente es de plástico y tiene una banda magnética en una de sus caras.</rdfs:comment>
    </owl:Class>
    


    <!-- http://opendata.aragon.es/def/ei2a#Crop -->

    <owl:Class rdf:about="http://opendata.aragon.es/def/ei2a#Crop">
        <rdfs:comment xml:lang="en">Crop</rdfs:comment>
        <rdfs:comment xml:lang="es">Cultivo</rdfs:comment>
    </owl:Class>
    


    <!-- http://opendata.aragon.es/def/ei2a#CropVariety -->

    <owl:Class rdf:about="http://opendata.aragon.es/def/ei2a#CropVariety">
        <rdfs:comment xml:lang="en">Crop variety</rdfs:comment>
        <rdfs:comment xml:lang="es">Variedad de cultivo</rdfs:comment>
    </owl:Class>
    


    <!-- http://opendata.aragon.es/def/ei2a#Document -->

    <owl:Class rdf:about="http://opendata.aragon.es/def/ei2a#Document">
        <rdfs:subClassOf>
            <owl:Restriction>
                <owl:onProperty rdf:resource="http://opendata.aragon.es/def/ei2a#documentIdentifier"/>
                <owl:cardinality rdf:datatype="http://www.w3.org/2001/XMLSchema#nonNegativeInteger">1</owl:cardinality>
            </owl:Restriction>
        </rdfs:subClassOf>
        <owl:hasKey rdf:parseType="Collection">
            <rdf:Description rdf:about="http://opendata.aragon.es/def/ei2a#documentIdentifier"/>
        </owl:hasKey>
        <rdfs:comment xml:lang="es">Entidad que representa un documento genérico y que contiene información común a todos los tipos de documentos. Cuando se requiera se podrá generar una especialización (subclase) por tipo de documento similar al de expediente.</rdfs:comment>
        <rdfs:comment xml:lang="en">Entity that represents a generic document that contains information common to all types of documents. When required, a specialization (subclass) can be generated by type of document similar to the administrative record.</rdfs:comment>
    </owl:Class>
    


    <!-- http://opendata.aragon.es/def/ei2a#DocumentCategory -->

    <owl:Class rdf:about="http://opendata.aragon.es/def/ei2a#DocumentCategory">
        <owl:equivalentClass>
            <owl:Class>
                <owl:oneOf rdf:parseType="Collection">
                    <rdf:Description rdf:about="http://opendata.aragon.es/def/ei2a#Agregación"/>
                    <rdf:Description rdf:about="http://opendata.aragon.es/def/ei2a#DocumentoSimple"/>
                    <rdf:Description rdf:about="http://opendata.aragon.es/def/ei2a#Expediente"/>
                    <rdf:Description rdf:about="http://opendata.aragon.es/def/ei2a#Fondo"/>
                    <rdf:Description rdf:about="http://opendata.aragon.es/def/ei2a#GrupoDeFondos"/>
                    <rdf:Description rdf:about="http://opendata.aragon.es/def/ei2a#Serie"/>
                </owl:oneOf>
            </owl:Class>
        </owl:equivalentClass>
        <rdfs:comment xml:lang="en">Category of the document that is being processed.

The domain of values that presents this class are: Agregación, DocumentoSimple, 
Expediente, Fondo, GrupoDeFondos, Serie.</rdfs:comment>
        <rdfs:comment xml:lang="es">Categoría del documento que se está tratando.

El dominio de valores que presenta esta clase son: Agregación, DocumentoSimple, 
Expediente, Fondo, GrupoDeFondos, Serie.</rdfs:comment>
    </owl:Class>
    


    <!-- http://opendata.aragon.es/def/ei2a#DocumentOrigin -->

    <owl:Class rdf:about="http://opendata.aragon.es/def/ei2a#DocumentOrigin">
        <owl:equivalentClass>
            <owl:Class>
                <owl:oneOf rdf:parseType="Collection">
                    <rdf:Description rdf:about="http://opendata.aragon.es/def/ei2a#Administración"/>
                    <rdf:Description rdf:about="http://opendata.aragon.es/def/ei2a#Ciudadano"/>
                </owl:oneOf>
            </owl:Class>
        </owl:equivalentClass>
        <rdfs:comment xml:lang="en">Origin of a particular document.

The domain of values that presents this class are:	Administración, Ciudadano.</rdfs:comment>
        <rdfs:comment xml:lang="es">Procedencia de un determinado documento.

El dominio de valores que presenta esta clase son:	Administración, Ciudadano.</rdfs:comment>
    </owl:Class>
    


    <!-- http://opendata.aragon.es/def/ei2a#DocumentStatus -->

    <owl:Class rdf:about="http://opendata.aragon.es/def/ei2a#DocumentStatus">
        <owl:equivalentClass>
            <owl:Class>
                <owl:oneOf rdf:parseType="Collection">
                    <rdf:Description rdf:about="http://opendata.aragon.es/def/ei2a#Anulado"/>
                    <rdf:Description rdf:about="http://opendata.aragon.es/def/ei2a#Borrador"/>
                    <rdf:Description rdf:about="http://opendata.aragon.es/def/ei2a#Copia"/>
                    <rdf:Description rdf:about="http://opendata.aragon.es/def/ei2a#Original"/>
                    <rdf:Description rdf:about="http://opendata.aragon.es/def/ei2a#PendienteDeFirma"/>
                </owl:oneOf>
            </owl:Class>
        </owl:equivalentClass>
        <rdfs:comment xml:lang="es">Estado del documento.

El dominio de valores que presenta esta clase son: Original, Borrador, Copia, PendienteDeFirma, Anulado.</rdfs:comment>
        <rdfs:comment xml:lang="en">Status of the document.

The domain of values that presents this class are: Original, Borrador, Copia, PendienteDeFirma, Anulado.</rdfs:comment>
    </owl:Class>
    


    <!-- http://opendata.aragon.es/def/ei2a#EventAgenda -->

    <owl:Class rdf:about="http://opendata.aragon.es/def/ei2a#EventAgenda">
        <rdfs:subClassOf rdf:resource="http://purl.org/NET/c4dm/event.owl#Event"/>
        <rdfs:comment xml:lang="en">Event as an agenda that has its description, start date, end date, start time, end time, duration, place, etc.</rdfs:comment>
        <rdfs:comment xml:lang="es">Evento a modo de agenda que tiene su descripción, fecha de inicio, fecha de fin, hora de inicio, hora de fin, duración, lugar, etc.</rdfs:comment>
    </owl:Class>
    


    <!-- http://opendata.aragon.es/def/ei2a#EventHistory -->

    <owl:Class rdf:about="http://opendata.aragon.es/def/ei2a#EventHistory">
        <rdfs:subClassOf rdf:resource="http://purl.org/NET/c4dm/event.owl#Event"/>
        <rdfs:comment xml:lang="en">Event as a record of changes (for example, grant subsidy).</rdfs:comment>
        <rdfs:comment xml:lang="es">Evento a modo de registro de cambios (por ejemplo, la concesión de una subvención).</rdfs:comment>
    </owl:Class>
    


    <!-- http://opendata.aragon.es/def/ei2a#FunctionalOrganizationStatus -->

    <owl:Class rdf:about="http://opendata.aragon.es/def/ei2a#FunctionalOrganizationStatus">
        <owl:equivalentClass>
            <owl:Class>
                <owl:oneOf rdf:parseType="Collection">
                    <rdf:Description rdf:about="http://opendata.aragon.es/def/ei2a#Anulado"/>
                    <rdf:Description rdf:about="http://opendata.aragon.es/def/ei2a#Extinguido"/>
                    <rdf:Description rdf:about="http://opendata.aragon.es/def/ei2a#Transitorio"/>
                    <rdf:Description rdf:about="http://opendata.aragon.es/def/ei2a#Vigente"/>
                </owl:oneOf>
            </owl:Class>
        </owl:equivalentClass>
        <rdfs:comment xml:lang="en">Catalog of states or situations of an organic unit or office.

The domain of the values that presents this class are: Anulado, Extinguido, Transitorio, Vigente.

For more information regarding these values, consult the Electronic Administration Portal (PAE, https://administracionelectronica.gob.es) and the Attributes Manual (https://administracionelectronica.gob.es/ctt/resources/Soluciones/238/Area%20descargas/Manual%20de%20Atributos.pdf?idIniciativa=238&amp;idElemento=420).</rdfs:comment>
        <rdfs:comment xml:lang="es">Catálogo de estados o situaciones de una unidad orgánica u oficina.

El dominio de los valores que presenta esta clase son: Anulado, Extinguido, Transitorio, Vigente.

Para más información relativa a estos valores consultar sobre el  Portal de Administración electrónica (PAE, https://administracionelectronica.gob.es) y el manual de atributos (https://administracionelectronica.gob.es/ctt/resources/Soluciones/238/Area%20descargas/Manual%20de%20Atributos.pdf?idIniciativa=238&amp;idElemento=420).</rdfs:comment>
    </owl:Class>
    


    <!-- http://opendata.aragon.es/def/ei2a#GeometryCollection -->

    <owl:Class rdf:about="http://opendata.aragon.es/def/ei2a#GeometryCollection">
        <rdfs:subClassOf rdf:resource="http://www.w3.org/ns/locn#Geometry"/>
        <rdfs:comment xml:lang="es">Super-clase que agrupa todas las representaciones geométricas compuestas.</rdfs:comment>
        <rdfs:comment xml:lang="en">Super-class grouping all composite geometrical representations.</rdfs:comment>
    </owl:Class>
    


    <!-- http://opendata.aragon.es/def/ei2a#LOPDLevel -->

    <owl:Class rdf:about="http://opendata.aragon.es/def/ei2a#LOPDLevel">
        <owl:equivalentClass>
            <owl:Class>
                <owl:oneOf rdf:parseType="Collection">
                    <rdf:Description rdf:about="http://opendata.aragon.es/def/ei2a#Alto"/>
                    <rdf:Description rdf:about="http://opendata.aragon.es/def/ei2a#Básico"/>
                    <rdf:Description rdf:about="http://opendata.aragon.es/def/ei2a#Medio"/>
                </owl:oneOf>
            </owl:Class>
        </owl:equivalentClass>
        <rdfs:comment xml:lang="en">Level of protection of the data of a document.

The values domain that presents this class are: Básico, Medio, Alto.

Default Basic.</rdfs:comment>
        <rdfs:comment xml:lang="es">Nivel de protección de los datos de un documento.

El dominio de valores que presenta esta clase son: Básico, Medio, Alto.

Por defecto Básico.</rdfs:comment>
    </owl:Class>
    


    <!-- http://opendata.aragon.es/def/ei2a#Line -->

    <owl:Class rdf:about="http://opendata.aragon.es/def/ei2a#Line">
        <rdfs:subClassOf rdf:resource="http://www.w3.org/ns/locn#Geometry"/>
        <rdfs:comment xml:lang="es">Representa una serie de puntos conectados por líneas.</rdfs:comment>
        <rdfs:comment xml:lang="en">Represents a series of points connected by lines.</rdfs:comment>
    </owl:Class>
    


    <!-- http://opendata.aragon.es/def/ei2a#MultiLine -->

    <owl:Class rdf:about="http://opendata.aragon.es/def/ei2a#MultiLine">
        <rdfs:subClassOf rdf:resource="http://opendata.aragon.es/def/ei2a#GeometryCollection"/>
        <rdfs:comment xml:lang="es">Describe una forma geométrica compuesta de varios recursos línea (Line).</rdfs:comment>
        <rdfs:comment xml:lang="en">Describes a geometric shape composed of several Line resources.</rdfs:comment>
    </owl:Class>
    


    <!-- http://opendata.aragon.es/def/ei2a#MultiPoint -->

    <owl:Class rdf:about="http://opendata.aragon.es/def/ei2a#MultiPoint">
        <rdfs:subClassOf rdf:resource="http://opendata.aragon.es/def/ei2a#GeometryCollection"/>
        <rdfs:comment xml:lang="es">Describe una colección de recursos de puntos (Point) que definen la representación geométrica de un recurso.</rdfs:comment>
        <rdfs:comment xml:lang="en">Describes a collection of Point resources, which define a resource&apos;s geometric representation.</rdfs:comment>
    </owl:Class>
    


    <!-- http://opendata.aragon.es/def/ei2a#MultiPolygon -->

    <owl:Class rdf:about="http://opendata.aragon.es/def/ei2a#MultiPolygon">
        <rdfs:subClassOf rdf:resource="http://opendata.aragon.es/def/ei2a#GeometryCollection"/>
        <rdfs:comment xml:lang="es">Describe una forma geométrica compuesta por varios recursos de polígono (Polygon)</rdfs:comment>
        <rdfs:comment xml:lang="en">Describes a geometric shape composed of several Polygon resources.</rdfs:comment>
    </owl:Class>
    


    <!-- http://opendata.aragon.es/def/ei2a#OliveGroveSubparcel -->

    <owl:Class rdf:about="http://opendata.aragon.es/def/ei2a#OliveGroveSubparcel">
        <rdfs:subClassOf rdf:resource="http://opendata.aragon.es/def/ei2a#Compound"/>
    </owl:Class>
    


    <!-- http://opendata.aragon.es/def/ei2a#OrganizationType -->

    <owl:Class rdf:about="http://opendata.aragon.es/def/ei2a#OrganizationType">
        <owl:equivalentClass>
            <owl:Class>
                <owl:oneOf rdf:parseType="Collection">
                    <rdf:Description rdf:about="http://opendata.aragon.es/def/ei2a#empresa"/>
                    <rdf:Description rdf:about="http://opendata.aragon.es/def/ei2a#escuela"/>
                    <rdf:Description rdf:about="http://opendata.aragon.es/def/ei2a#fundación"/>
                    <rdf:Description rdf:about="http://opendata.aragon.es/def/ei2a#oficinaDeTurismo"/>
                    <rdf:Description rdf:about="http://opendata.aragon.es/def/ei2a#puntoDeInformación"/>
                    <rdf:Description rdf:about="http://opendata.aragon.es/def/ei2a#órganoAdministrativo"/>
                </owl:oneOf>
            </owl:Class>
        </owl:equivalentClass>
        <rdfs:comment xml:lang="es">Tipo de organización que se está representando, indicando si es de carácter público o privado.

El dominio de los valores que presenta esta clase son: empresa, 	órganoAdministrativo</rdfs:comment>
        <rdfs:comment xml:lang="en">Type of organization being represented, indicating whether it is public or private.

The domain of the values that presents this class are: empresa, 	órganoAdministrativo.</rdfs:comment>
    </owl:Class>
    


    <!-- http://opendata.aragon.es/def/ei2a#PACAidsRequest -->

    <owl:Class rdf:about="http://opendata.aragon.es/def/ei2a#PACAidsRequest">
        <rdfs:comment xml:lang="en">Application for PAC aids (Common Agricultural Policy)</rdfs:comment>
        <rdfs:comment xml:lang="es">Solicitud de ayudas PAC (Política Agrícola Común)</rdfs:comment>
    </owl:Class>
    


    <!-- http://opendata.aragon.es/def/ei2a#PersonGender -->

    <owl:Class rdf:about="http://opendata.aragon.es/def/ei2a#PersonGender">
        <owl:equivalentClass>
            <owl:Class>
                <owl:oneOf rdf:parseType="Collection">
                    <rdf:Description rdf:about="http://opendata.aragon.es/def/ei2a#Femenino"/>
                    <rdf:Description rdf:about="http://opendata.aragon.es/def/ei2a#Masculino"/>
                </owl:oneOf>
            </owl:Class>
        </owl:equivalentClass>
        <rdfs:comment xml:lang="en">Gender or sex of the person.

It is always registered the sex that appears in the document proving the identity of the person (male or female)</rdfs:comment>
        <rdfs:comment xml:lang="es">Género o sexo de la persona.

Se registrará siempre el sexo que conste en el documento acreditativo de la identidad de la persona (Masculino o Femenino)</rdfs:comment>
    </owl:Class>
    


    <!-- http://opendata.aragon.es/def/ei2a#PersonalIdentifierSystem -->

    <owl:Class rdf:about="http://opendata.aragon.es/def/ei2a#PersonalIdentifierSystem">
        <owl:hasKey rdf:parseType="Collection">
            <rdf:Description rdf:about="http://www.w3.org/ns/org#identifier"/>
        </owl:hasKey>
        <rdfs:comment xml:lang="es">Sistema en el que se hace una identificación de persona.  El objetivo es poder tener vinculado el identificador unívoco de una Persona con todos los posibles identificadores de personas que se tenga en otros sistemas.</rdfs:comment>
        <rdfs:comment xml:lang="en">System in which a person identification is made. The objective is to be able to have linked the unique identifier of a Person with all the possible identifiers of people that you have in other systems.</rdfs:comment>
    </owl:Class>
    


    <!-- http://opendata.aragon.es/def/ei2a#Point -->

    <owl:Class rdf:about="http://opendata.aragon.es/def/ei2a#Point">
        <owl:equivalentClass rdf:resource="http://www.w3.org/2003/01/geo/wgs84_pos#Point"/>
        <rdfs:subClassOf rdf:resource="http://www.w3.org/ns/locn#Geometry"/>
        <rdfs:comment xml:lang="es">Punto identificado unívocamente que puede ser descrito usando un sistema de coordenadas.</rdfs:comment>
        <rdfs:comment xml:lang="en">Uniquely identified point that can be described using a coordinate system.</rdfs:comment>
    </owl:Class>
    


    <!-- http://opendata.aragon.es/def/ei2a#Polygon -->

    <owl:Class rdf:about="http://opendata.aragon.es/def/ei2a#Polygon">
        <rdfs:subClassOf rdf:resource="http://www.w3.org/ns/locn#Geometry"/>
        <rdfs:comment xml:lang="en">A closed area defined by an exterior boundary, and optionally one or more interior boundaries.</rdfs:comment>
        <rdfs:comment xml:lang="es">Área cerrada definida por un límite exterior, y opcionalmente uno o más límites interiores.</rdfs:comment>
    </owl:Class>
    


    <!-- http://opendata.aragon.es/def/ei2a#Procedure -->

    <owl:Class rdf:about="http://opendata.aragon.es/def/ei2a#Procedure">
        <rdfs:subClassOf>
            <owl:Restriction>
                <owl:onProperty rdf:resource="http://opendata.aragon.es/def/ei2a#procedureIdentifier"/>
                <owl:cardinality rdf:datatype="http://www.w3.org/2001/XMLSchema#nonNegativeInteger">1</owl:cardinality>
            </owl:Restriction>
        </rdfs:subClassOf>
        <owl:hasKey rdf:parseType="Collection">
            <rdf:Description rdf:about="http://opendata.aragon.es/def/ei2a#procedureIdentifier"/>
        </owl:hasKey>
        <rdfs:comment xml:lang="es">Clasificación otorgada en relación con las posibilidades de trámites electrónicos y desarrollo de la e-admin en Aragón.</rdfs:comment>
        <rdfs:comment xml:lang="en">Classification granted in relation to the possibilities of electronic procedures and development of e-admin in Aragon.</rdfs:comment>
    </owl:Class>
    


    <!-- http://opendata.aragon.es/def/ei2a#PropertyType -->

    <owl:Class rdf:about="http://opendata.aragon.es/def/ei2a#PropertyType">
        <owl:equivalentClass>
            <owl:Class>
                <owl:oneOf rdf:parseType="Collection">
                    <rdf:Description rdf:about="http://opendata.aragon.es/def/ei2a#Rural"/>
                    <rdf:Description rdf:about="http://opendata.aragon.es/def/ei2a#Urbana"/>
                </owl:oneOf>
            </owl:Class>
        </owl:equivalentClass>
        <rdfs:comment xml:lang="es">Tipo de la referencia catastral. 

Esta clase es una clase enumerada que tiene los siguientes valores: 	Urbana, 	Rural.</rdfs:comment>
        <rdfs:comment xml:lang="en">Type of cadastral reference.

This class is an enumerated class that has the following values: Urban, Rural.</rdfs:comment>
    </owl:Class>
    


    <!-- http://opendata.aragon.es/def/ei2a#PublicEntityType -->

    <owl:Class rdf:about="http://opendata.aragon.es/def/ei2a#PublicEntityType">
        <owl:equivalentClass>
            <owl:Class>
                <owl:oneOf rdf:parseType="Collection">
                    <rdf:Description rdf:about="http://opendata.aragon.es/def/ei2a#AgenciaEstatal"/>
                    <rdf:Description rdf:about="http://opendata.aragon.es/def/ei2a#AgrupaciónSecretarial"/>
                    <rdf:Description rdf:about="http://opendata.aragon.es/def/ei2a#Auxiliar"/>
                    <rdf:Description rdf:about="http://opendata.aragon.es/def/ei2a#Ayuntamiento"/>
                    <rdf:Description rdf:about="http://opendata.aragon.es/def/ei2a#Cabildo"/>
                    <rdf:Description rdf:about="http://opendata.aragon.es/def/ei2a#CentroEducativo"/>
                    <rdf:Description rdf:about="http://opendata.aragon.es/def/ei2a#ColegioProfesional"/>
                    <rdf:Description rdf:about="http://opendata.aragon.es/def/ei2a#Comarca"/>
                    <rdf:Description rdf:about="http://opendata.aragon.es/def/ei2a#ComunidadAutónoma"/>
                    <rdf:Description rdf:about="http://opendata.aragon.es/def/ei2a#Cámara"/>
                    <rdf:Description rdf:about="http://opendata.aragon.es/def/ei2a#DiputaciónProvincialForal"/>
                    <rdf:Description rdf:about="http://opendata.aragon.es/def/ei2a#EntidadDerechoPúblico"/>
                    <rdf:Description rdf:about="http://opendata.aragon.es/def/ei2a#EntidadLocalMenor"/>
                    <rdf:Description rdf:about="http://opendata.aragon.es/def/ei2a#EntidadPúblicaEmpresarial"/>
                    <rdf:Description rdf:about="http://opendata.aragon.es/def/ei2a#FundaciónEstatal"/>
                    <rdf:Description rdf:about="http://opendata.aragon.es/def/ei2a#General"/>
                    <rdf:Description rdf:about="http://opendata.aragon.es/def/ei2a#Mancomunidad"/>
                    <rdf:Description rdf:about="http://opendata.aragon.es/def/ei2a#Ministerio"/>
                    <rdf:Description rdf:about="http://opendata.aragon.es/def/ei2a#OficinaDeTurismoYPuntoDeInformación"/>
                    <rdf:Description rdf:about="http://opendata.aragon.es/def/ei2a#OrganismoAutónomo"/>
                    <rdf:Description rdf:about="http://opendata.aragon.es/def/ei2a#SinClasificar"/>
                    <rdf:Description rdf:about="http://opendata.aragon.es/def/ei2a#Universidad"/>
                </owl:oneOf>
            </owl:Class>
        </owl:equivalentClass>
        <rdfs:comment xml:lang="es">Tipo de entidad pública clasificando distintos tipos de entidades que constituyen la administración pública. Por lo general, representa una estructura de unidades orgánicas que constituye una entidad (órgano/organismos) de la administración pública.

El dominio de valores que presenta esta clase son: AgenciaEstatal, Auxiliar (Para Oficinas), Ayuntamiento, Cabildo, ColegioProfesional, Comarca,  ComunidadAutónoma, Cámara, DiputaciónProvincialForal, 	EntidadDerechoPúblico, EntidadLocalMenor, EntidadPúblicaEmpresarial, 	FundaciónEstatal, General (Para Oficinas), Mancomunidad, Ministerio, OrganismoAutónomo, SinClasificar, Universidad.

Para más información relativa a estos valores consultar sobre el  Portal de Administración electrónica (PAE, https://administracionelectronica.gob.es) y el manual de atributos (https://administracionelectronica.gob.es/ctt/resources/Soluciones/238/Area%20descargas/Manual%20de%20Atributos.pdf?idIniciativa=238&amp;idElemento=420).</rdfs:comment>
        <rdfs:comment xml:lang="en">Type of public entity classifying different types of entities that constitute the public administration. In general, it represents a structure of organic units that constitutes an entity (organ / agencies) of the public administration.

The domain of values that presents this class are: AgenciaEstatal, Auxiliar (Para Oficinas), Ayuntamiento, Cabildo, ColegioProfesional, Comarca,  ComunidadAutónoma, Cámara, DiputaciónProvincialForal, 	EntidadDerechoPúblico, EntidadLocalMenor, EntidadPúblicaEmpresarial, 	FundaciónEstatal, General (Para Oficinas), Mancomunidad, Ministerio, OrganismoAutónomo, SinClasificar, Universidad.

For more information regarding these values, consult the Electronic Administration Portal (PAE, https://administracionelectronica.gob.es) and the Attributes Manual (https://administracionelectronica.gob.es/ctt/resources/Soluciones/238/Area%20descargas/Manual%20de%20Atributos.pdf?idIniciativa=238&amp;idElemento=420).</rdfs:comment>
    </owl:Class>
    


    <!-- http://opendata.aragon.es/def/ei2a#ReferenceSystem -->

    <owl:Class rdf:about="http://opendata.aragon.es/def/ei2a#ReferenceSystem">
        <owl:equivalentClass>
            <owl:Class>
                <owl:oneOf rdf:parseType="Collection">
                    <rdf:Description rdf:about="http://opendata.aragon.es/def/ei2a#ETRS89"/>
                    <rdf:Description rdf:about="http://opendata.aragon.es/def/ei2a#WGS84"/>
                </owl:oneOf>
            </owl:Class>
        </owl:equivalentClass>
        <rdfs:comment xml:lang="es">La clase ReferenceSystem (ei2a: ReferenceSystem) representa un sistema de referencia que permite expresar la posición de determinados elementos utilizando sus coordenadas.  Esta clase es una clase enumerada que tiene los siguientes valores:

 - ETRS89
 - WGS84

ETRS89 (European Terrestrial Reference System) es un sistema de referencia europeo gestionado por organismos públicos, basado en sistemas internacionales, y diseñado acorde a los requisitos de precisión actuales.

WGS84 (World Geodetic System) es un sistema de referencia internacional gestionado por el DoD de los EEUU y utilizado, inicialmente, para expresar las posiciones de los satélites GPS. 

En el caso español, según el Real Decreto 1071/2007 del 27 de Julio por el que se regula el sistema geodésico de referencia oficial en España, debe ser ETRS89.</rdfs:comment>
        <rdfs:comment xml:lang="en">The ReferenceSystem class (ei2a: ReferenceSystem) represents a reference system that allows you to express the position of certain elements using their coordinates. This class is an enumerated class that has the following values:

  - ETRS89
  - WGS84

ETRS89 (European Terrestrial Reference System) is a European reference system managed by public bodies, based on international systems, and designed according to current precision requirements.

WGS84 (World Geodetic System) is an international reference system managed by the US DoD and used, initially, to express the positions of the GPS satellites.

In the Spanish case, according to Royal Decree 1071/2007 of July 27, which regulates the geodesic reference system in Spain, it must be ETRS89.</rdfs:comment>
    </owl:Class>
    


    <!-- http://opendata.aragon.es/def/ei2a#RuralParcel -->

    <owl:Class rdf:about="http://opendata.aragon.es/def/ei2a#RuralParcel">
        <rdfs:comment xml:lang="es">Porción de terreno o superficie terrestre de tipo rústico.</rdfs:comment>
        <rdfs:comment xml:lang="en">Portion of land or land surface of rustic type.</rdfs:comment>
    </owl:Class>
    


    <!-- http://opendata.aragon.es/def/ei2a#RuralParcelOrigin -->

    <owl:Class rdf:about="http://opendata.aragon.es/def/ei2a#RuralParcelOrigin">
        <owl:equivalentClass>
            <owl:Class>
                <owl:oneOf rdf:parseType="Collection">
                    <rdf:Description rdf:about="http://opendata.aragon.es/def/ei2a#SIGPAC"/>
                    <rdf:Description rdf:about="http://opendata.aragon.es/def/ei2a#cadastral"/>
                </owl:oneOf>
            </owl:Class>
        </owl:equivalentClass>
        <rdfs:comment xml:lang="en">Origin of a rural plot (cadastral, SIGPAC)</rdfs:comment>
        <rdfs:comment xml:lang="es">Procedencia de una parcela rural (catastral, SIGPAC)</rdfs:comment>
    </owl:Class>
    


    <!-- http://opendata.aragon.es/def/ei2a#Series -->

    <owl:Class rdf:about="http://opendata.aragon.es/def/ei2a#Series">
        <rdfs:subClassOf>
            <owl:Restriction>
                <owl:onProperty rdf:resource="http://opendata.aragon.es/def/ei2a#serieIdentifier"/>
                <owl:cardinality rdf:datatype="http://www.w3.org/2001/XMLSchema#nonNegativeInteger">1</owl:cardinality>
            </owl:Restriction>
        </rdfs:subClassOf>
        <owl:hasKey rdf:parseType="Collection">
            <rdf:Description rdf:about="http://opendata.aragon.es/def/ei2a#serieIdentifier"/>
        </owl:hasKey>
        <rdfs:comment xml:lang="es">Documentación producida por un organismo en el desarrollo de una actividad concreta y regulada por una norma de procedimiento.

Indica la categoría del documento que se está tratando  (Cuadro de clasificación funcional, http://www.aragon.es/archivo/AreasTematicas/02_recursos_archivo/ci.01_Cuadro_fondos.detalleDepartamento)</rdfs:comment>
        <rdfs:comment xml:lang="en">Documentation produced by an agency in the development of a specific activity and regulated by a procedural rule.

Indicates the category of the document being treated (Functional classification table, http://www.aragon.es/archivo/AreasTematicas/02_recursos_archivo/ci.01_Directory_fondos.detalleDepartment)</rdfs:comment>
    </owl:Class>
    


    <!-- http://opendata.aragon.es/def/ei2a#Similarity -->

    <owl:Class rdf:about="http://opendata.aragon.es/def/ei2a#Similarity">
        <rdfs:comment xml:lang="es">Entidad que recoge información sobre medidas de similitud entre dos páginas web pertenecientes a la misma categoría</rdfs:comment>
        <rdfs:comment xml:lang="en">Entity that collects information on measures of similarity between two web pages belonging to the same category</rdfs:comment>
    </owl:Class>
    


    <!-- http://opendata.aragon.es/def/ei2a#SocialMedia -->

    <owl:Class rdf:about="http://opendata.aragon.es/def/ei2a#SocialMedia">
        <rdfs:comment xml:lang="en">Concept for collecting information from social media</rdfs:comment>
        <rdfs:comment xml:lang="es">Concepto para recoger información de medios de comunicación social</rdfs:comment>
    </owl:Class>
    


    <!-- http://opendata.aragon.es/def/ei2a#SocialMediaHashtag -->

    <owl:Class rdf:about="http://opendata.aragon.es/def/ei2a#SocialMediaHashtag">
        <rdfs:comment xml:lang="es">Palabras o frases (sin espacios) precedidas de un signo almohadilla #. Permite que los usuarios puedan participar en conversaciones sobre un tema particular, y de esta manera quedar agrupadas bajo una misma etiqueta</rdfs:comment>
        <rdfs:comment xml:lang="en">Words or phrases (without spaces) preceded by a pound sign #. It allows users to participate in conversations on a particular topic, and thus be grouped under the same label</rdfs:comment>
    </owl:Class>
    


    <!-- http://opendata.aragon.es/def/ei2a#SocialMediaMention -->

    <owl:Class rdf:about="http://opendata.aragon.es/def/ei2a#SocialMediaMention">
        <rdfs:comment xml:lang="es">Mención en una comunicación social</rdfs:comment>
        <rdfs:comment xml:lang="en">Mention in a social communication</rdfs:comment>
    </owl:Class>
    


    <!-- http://opendata.aragon.es/def/ei2a#SocialMediaSources -->

    <owl:Class rdf:about="http://opendata.aragon.es/def/ei2a#SocialMediaSources">
        <owl:equivalentClass>
            <owl:Class>
                <owl:oneOf rdf:parseType="Collection">
                    <rdf:Description rdf:about="http://opendata.aragon.es/def/ei2a#diariodelaltoaragon"/>
                    <rdf:Description rdf:about="http://opendata.aragon.es/def/ei2a#diariodeteruel"/>
                    <rdf:Description rdf:about="http://opendata.aragon.es/def/ei2a#facebook"/>
                    <rdf:Description rdf:about="http://opendata.aragon.es/def/ei2a#facebook_geoposts"/>
                    <rdf:Description rdf:about="http://opendata.aragon.es/def/ei2a#flickr"/>
                    <rdf:Description rdf:about="http://opendata.aragon.es/def/ei2a#heraldodearagon"/>
                    <rdf:Description rdf:about="http://opendata.aragon.es/def/ei2a#instagram"/>
                    <rdf:Description rdf:about="http://opendata.aragon.es/def/ei2a#periodicodearagon"/>
                    <rdf:Description rdf:about="http://opendata.aragon.es/def/ei2a#twitter"/>
                    <rdf:Description rdf:about="http://opendata.aragon.es/def/ei2a#wikipedia"/>
                    <rdf:Description rdf:about="http://opendata.aragon.es/def/ei2a#youtube"/>
                </owl:oneOf>
            </owl:Class>
        </owl:equivalentClass>
    </owl:Class>
    


    <!-- http://opendata.aragon.es/def/ei2a#Subparcel -->

    <owl:Class rdf:about="http://opendata.aragon.es/def/ei2a#Subparcel">
        <rdfs:comment xml:lang="es">La subpacerla propia del catastro en el nuevo sistema se denomina recinto. Se establece como equivalente del concepto Recinto para  poder reflejar información histórica en la que se denominaba subparcela y la información actual denominada como recinto.</rdfs:comment>
        <rdfs:comment xml:lang="en">The subparcel proper of the cadastre in the new system is called Compond. It is established as an equivalent of the concept of a Compound in order to reflect historical information in what was called a Subparcel and the current information known as the Compound.</rdfs:comment>
    </owl:Class>
    


    <!-- http://opendata.aragon.es/def/ei2a#TypeGeometryModel -->

    <owl:Class rdf:about="http://opendata.aragon.es/def/ei2a#TypeGeometryModel">
        <owl:equivalentClass>
            <owl:Class>
                <owl:oneOf rdf:parseType="Collection">
                    <rdf:Description rdf:about="http://opendata.aragon.es/def/ei2a#Raster"/>
                    <rdf:Description rdf:about="http://opendata.aragon.es/def/ei2a#Vectorial"/>
                </owl:oneOf>
            </owl:Class>
        </owl:equivalentClass>
        <rdfs:comment xml:lang="es">La clase TypeGeometryModel (ei2a: TypeGeometryModel) representa un tipo de modelo lógico que hacen referencia a cómo se muestran y organizan las variables y objetos para lograr una representación lo más adecuada posible y que da lugar a un tipo de capa de información espacial.  Esta clase es una clase enumerada que tiene los siguientes valores:

 - Raster
 - Vectorial

En el formato de tipo raster se divide el espacio en un conjunto regular de celdillas, cada una de estas celdillas contiene un número que puede ser el identificador de un objeto (si se trata de una capa que contiene objetos) o del valor de una variable (si la capa contiene esta variable).

En el formato de tipo vectorial los diferentes objetos se representan mediante formas geométricas (puntos, líneas o polígonos, esto es, vectores).</rdfs:comment>
        <rdfs:comment xml:lang="en">The TypeGeometryModel class (ei2a: TypeGeometryModel) represents a type of logical model that refers to how variables and objects are displayed and organized to achieve the most appropriate representation possible and which results in a spatial information layer type. This class is an enumerated class that has the following values:

  - Raster
  - Vectorial

In the raster format the space is divided into a regular set of cells, each of these cells contains a number that can be the identifier of an object (if it is a layer containing objects) or the value of a variable (If the layer contains this variable).

In the format of vectorial type the different objects are represented by geometric forms (points, lines or polygons, that is, vectors).</rdfs:comment>
    </owl:Class>
    


    <!-- http://opendata.aragon.es/def/ei2a#UrbanParcel -->

    <owl:Class rdf:about="http://opendata.aragon.es/def/ei2a#UrbanParcel">
        <rdfs:comment xml:lang="es">Bien inmueble urbano. Se entiende como un suelo de naturaleza urbana :

 - El clasificado como urbano, urbanizado o equivalente por el planeamiento urbanístico correspondiente.

 - El que tenga la consideración de urbanizable o aquel para el que los instrumentos de ordenación territorial y urbanística prevea o permita su paso a la situación de suelo urbanizado, y esté incluido en sectores o ámbitos espaciales delimitados, así como el suelo de este tipo una vez aprobado el instrumento urbanístico que establezca las determinaciones para su desarrollo.

 - El integrado de forma efectiva en la trama de dotaciones y servicios propios de los núcleos de población.

 - El ocupado por los núcleos o asentamientos de población aislados, en su caso, del núcleo principal, cualquiera que sea el hábitat en que se localicen y con independencia del grado de concentración de las edificaciones.

 - El suelo ya transformado por contar con los servicios urbanos establecidos por la legislación urbanística o, en su defecto, por disponer de acceso rodado, abastecimiento de agua, evacuación de aguas y suministro de energía eléctrica.

 -El consolidado por la edificación, en la forma y con las características que establezca la legislación urbanística correspondiente.</rdfs:comment>
        <rdfs:comment xml:lang="en">Urban parcel. It is understood as a soil of urban nature:

 - The classified as urban, urbanized or equivalent by the corresponding urban planning.

 - The one that has the status of urban development or one for which the instruments of territorial and urban planning foresee or allow their passage to the situation of urbanized land, and is included in sectors or defined space areas, as well as the soil of this type Once approved the urban planning instrument that establishes the determinations for its development.

 - The integrated of effective form in the network of endowments and services typical of the population centers.

 - Occupied by nuclei or population settlements isolated, if any, from the main nucleus, regardless of the habitat in which they are located and regardless of the degree of concentration of the buildings.

 - The land already transformed by having urban services established by urban planning legislation or, failing that, by having access to roads, water supply, water drainage and electricity supply.

 - Consolidated by the building, in the form and with the characteristics established by the corresponding urban legislation.</rdfs:comment>
    </owl:Class>
    


    <!-- http://opendata.aragon.es/def/ei2a#VineyardSubparcel -->

    <owl:Class rdf:about="http://opendata.aragon.es/def/ei2a#VineyardSubparcel">
        <rdfs:subClassOf rdf:resource="http://opendata.aragon.es/def/ei2a#Compound"/>
    </owl:Class>
    


    <!-- http://opendata.aragon.es/def/ei2a#WebPage -->

    <owl:Class rdf:about="http://opendata.aragon.es/def/ei2a#WebPage">
        <rdfs:comment xml:lang="es">Entidad que recoge información sobre webs, subdominios y portales del Gobierno de Aragón</rdfs:comment>
        <rdfs:comment xml:lang="en">Entity that collects information on webs, subdomains and portals of the Government of Aragon</rdfs:comment>
    </owl:Class>
    


    <!-- http://opendata.aragon.es/def/ei2a#WoodenSubparcel -->

    <owl:Class rdf:about="http://opendata.aragon.es/def/ei2a#WoodenSubparcel">
        <rdfs:subClassOf rdf:resource="http://opendata.aragon.es/def/ei2a#Compound"/>
    </owl:Class>
    


    <!-- http://opendata.aragon.es/def/ei2a/categorization#GeneralCategorization -->

    <owl:Class rdf:about="http://opendata.aragon.es/def/ei2a/categorization#GeneralCategorization"/>
    


    <!-- http://purl.oclc.org/NET/ssnx/ssn#Accuracy -->

    <owl:Class rdf:about="http://purl.oclc.org/NET/ssnx/ssn#Accuracy">
        <rdfs:subClassOf rdf:resource="http://purl.oclc.org/NET/ssnx/ssn#MeasurementProperty"/>
        <dc:source>skos:exactMatch &apos;measurement accuracy/accuracy&apos; [VIM 2.13] 
		                    http://www.bipm.org/utils/common/documents/jcgm/JCGM_200_2008.pdf</dc:source>
        <rdfs:comment>The closeness of agreement between the value of an observation and the true value of the observed quality.</rdfs:comment>
        <rdfs:isDefinedBy>http://purl.oclc.org/NET/ssnx/ssn</rdfs:isDefinedBy>
        <rdfs:label>Accuracy</rdfs:label>
        <rdfs:seeAlso>http://www.w3.org/2005/Incubator/ssn/wiki/SSN_Sensor#MeasuringCapability</rdfs:seeAlso>
    </owl:Class>
    


    <!-- http://purl.oclc.org/NET/ssnx/ssn#DetectionLimit -->

    <owl:Class rdf:about="http://purl.oclc.org/NET/ssnx/ssn#DetectionLimit">
        <rdfs:subClassOf rdf:resource="http://purl.oclc.org/NET/ssnx/ssn#MeasurementProperty"/>
        <dc:source>skos:exactMatch &apos;detection limit&apos; [VIM 4.18] 
                                 http://www.bipm.org/utils/common/documents/jcgm/JCGM_200_2008.pdf</dc:source>
        <rdfs:comment>An observed value for which the probability of falsely claiming the absence of a component in a material is Î², given a probability Î± of falsely claiming its presence.</rdfs:comment>
        <rdfs:isDefinedBy>http://purl.oclc.org/NET/ssnx/ssn</rdfs:isDefinedBy>
        <rdfs:label>detection limit</rdfs:label>
        <rdfs:seeAlso>http://www.w3.org/2005/Incubator/ssn/wiki/SSN_Sensor#MeasuringCapability</rdfs:seeAlso>
    </owl:Class>
    


    <!-- http://purl.oclc.org/NET/ssnx/ssn#Device -->

    <owl:Class rdf:about="http://purl.oclc.org/NET/ssnx/ssn#Device">
        <rdfs:subClassOf rdf:resource="http://www.ontologydesignpatterns.org/ont/dul/DUL.owl#DesignedArtifact"/>
        <alignedWithSaref>saref:Device</alignedWithSaref>
        <dc:source>http://www.w3.org/2005/Incubator/ssn/</dc:source>
        <rdfs:comment>A device is a physical piece of technology - a system in a box. Devices may of course be built of smaller devices and software components (i.e. systems have components).</rdfs:comment>
        <rdfs:isDefinedBy>http://purl.oclc.org/NET/ssnx/ssn</rdfs:isDefinedBy>
        <rdfs:label>Device</rdfs:label>
        <rdfs:seeAlso>http://www.w3.org/2005/Incubator/ssn/wiki/SSN_Device#Device</rdfs:seeAlso>
    </owl:Class>
    


    <!-- http://purl.oclc.org/NET/ssnx/ssn#Drift -->

    <owl:Class rdf:about="http://purl.oclc.org/NET/ssnx/ssn#Drift">
        <rdfs:subClassOf rdf:resource="http://purl.oclc.org/NET/ssnx/ssn#MeasurementProperty"/>
        <dc:source>skos:exactMatch &apos;instrumental drift&apos; [VIM 4.21]
                                  http://www.bipm.org/utils/common/documents/jcgm/JCGM_200_2008.pdf</dc:source>
        <rdfs:comment>A, continuous or incremental, change in the reported values of observations over time for an unchanging quality.</rdfs:comment>
        <rdfs:isDefinedBy>http://purl.oclc.org/NET/ssnx/ssn</rdfs:isDefinedBy>
        <rdfs:label>Drift</rdfs:label>
        <rdfs:seeAlso>http://www.w3.org/2005/Incubator/ssn/wiki/SSN_Sensor#MeasuringCapability</rdfs:seeAlso>
    </owl:Class>
    


    <!-- http://purl.oclc.org/NET/ssnx/ssn#FeatureOfInterest -->

    <owl:Class rdf:about="http://purl.oclc.org/NET/ssnx/ssn#FeatureOfInterest">
        <rdfs:subClassOf>
            <owl:Restriction>
                <owl:onProperty rdf:resource="http://purl.oclc.org/NET/ssnx/ssn#hasProperty"/>
                <owl:someValuesFrom rdf:resource="http://purl.oclc.org/NET/ssnx/ssn#Property"/>
            </owl:Restriction>
        </rdfs:subClassOf>
        <rdfs:subClassOf>
            <owl:Restriction>
                <owl:onProperty rdf:resource="http://purl.oclc.org/NET/ssnx/ssn#hasProperty"/>
                <owl:allValuesFrom rdf:resource="http://purl.oclc.org/NET/ssnx/ssn#Property"/>
            </owl:Restriction>
        </rdfs:subClassOf>
        <alignedWithWatERP>FeatureOfInterest</alignedWithWatERP>
        <dc:source>skos:exactMatch &apos;feature&apos; [O&amp;M] 
		                    http://www.opengeospatial.org/standards/om</dc:source>
        <rdfs:comment>A feature is an abstraction of real world phenomena (thing, person, event, etc).</rdfs:comment>
        <rdfs:isDefinedBy>http://purl.oclc.org/NET/ssnx/ssn</rdfs:isDefinedBy>
        <rdfs:label>FeatureOfInterest</rdfs:label>
        <rdfs:seeAlso>http://www.w3.org/2005/Incubator/ssn/wiki/SSN_Skeleton#Skeleton</rdfs:seeAlso>
    </owl:Class>
    


    <!-- http://purl.oclc.org/NET/ssnx/ssn#Frequency -->

    <owl:Class rdf:about="http://purl.oclc.org/NET/ssnx/ssn#Frequency">
        <rdfs:subClassOf rdf:resource="http://purl.oclc.org/NET/ssnx/ssn#MeasurementProperty"/>
        <rdfs:comment>The smallest possible time between one observation and the next.</rdfs:comment>
        <rdfs:isDefinedBy>http://purl.oclc.org/NET/ssnx/ssn</rdfs:isDefinedBy>
        <rdfs:label>Frequency</rdfs:label>
        <rdfs:seeAlso>http://www.w3.org/2005/Incubator/ssn/wiki/SSN_Sensor#MeasuringCapability</rdfs:seeAlso>
    </owl:Class>
    


    <!-- http://purl.oclc.org/NET/ssnx/ssn#Latency -->

    <owl:Class rdf:about="http://purl.oclc.org/NET/ssnx/ssn#Latency">
        <rdfs:subClassOf rdf:resource="http://purl.oclc.org/NET/ssnx/ssn#MeasurementProperty"/>
        <rdfs:comment>The time between a request for an observation and the sensor providing a result.</rdfs:comment>
        <rdfs:isDefinedBy>http://purl.oclc.org/NET/ssnx/ssn</rdfs:isDefinedBy>
        <rdfs:label>Latency</rdfs:label>
        <rdfs:seeAlso>http://www.w3.org/2005/Incubator/ssn/wiki/SSN_Sensor#MeasuringCapability</rdfs:seeAlso>
    </owl:Class>
    


    <!-- http://purl.oclc.org/NET/ssnx/ssn#MeasurementCapability -->

    <owl:Class rdf:about="http://purl.oclc.org/NET/ssnx/ssn#MeasurementCapability">
        <rdfs:subClassOf rdf:resource="http://purl.oclc.org/NET/ssnx/ssn#Property"/>
        <rdfs:subClassOf>
            <owl:Restriction>
                <owl:onProperty rdf:resource="http://purl.oclc.org/NET/ssnx/ssn#forProperty"/>
                <owl:allValuesFrom rdf:resource="http://purl.oclc.org/NET/ssnx/ssn#Property"/>
            </owl:Restriction>
        </rdfs:subClassOf>
        <rdfs:subClassOf>
            <owl:Restriction>
                <owl:onProperty rdf:resource="http://purl.oclc.org/NET/ssnx/ssn#hasMeasurementProperty"/>
                <owl:allValuesFrom rdf:resource="http://purl.oclc.org/NET/ssnx/ssn#MeasurementProperty"/>
            </owl:Restriction>
        </rdfs:subClassOf>
        <dc:source>Similar idea to MeasurementCapability in MMI Device Ontology
                                  http://marinemetadata.org/community/teams/ontdevices

But the the two express the relationship between constraints and multiple measurement properties differently.

The conditions linked to a MeasurementCapability are skos:exactMatch to &apos;influence quantity&apos; [VIM 2.52]
http://www.bipm.org/utils/common/documents/jcgm/JCGM_200_2008.pdf</dc:source>
        <rdfs:comment>Collects together measurement properties (accuracy, range, precision, etc) and the environmental conditions in which those properties hold, representing a specification of a sensor&apos;s capability in those conditions.

The conditions specified here are those that affect the measurement properties, while those in OperatingRange represent the sensor&apos;s standard operating conditions, including conditions that don&apos;t affect the observations.</rdfs:comment>
        <rdfs:isDefinedBy>http://purl.oclc.org/NET/ssnx/ssn</rdfs:isDefinedBy>
        <rdfs:label>Measurement Capability</rdfs:label>
        <rdfs:seeAlso>http://www.w3.org/2005/Incubator/ssn/wiki/SSN_Sensor#MeasuringCapability</rdfs:seeAlso>
    </owl:Class>
    


    <!-- http://purl.oclc.org/NET/ssnx/ssn#MeasurementProperty -->

    <owl:Class rdf:about="http://purl.oclc.org/NET/ssnx/ssn#MeasurementProperty">
        <rdfs:subClassOf rdf:resource="http://purl.oclc.org/NET/ssnx/ssn#Property"/>
        <rdfs:comment>An identifiable and observable characteristic of a sensor&apos;s observations or ability to make observations.</rdfs:comment>
        <rdfs:isDefinedBy>http://purl.oclc.org/NET/ssnx/ssn</rdfs:isDefinedBy>
        <rdfs:label>Measurement  Property</rdfs:label>
        <rdfs:seeAlso>http://www.w3.org/2005/Incubator/ssn/wiki/SSN_Sensor#MeasuringCapability</rdfs:seeAlso>
    </owl:Class>
    


    <!-- http://purl.oclc.org/NET/ssnx/ssn#MeasurementRange -->

    <owl:Class rdf:about="http://purl.oclc.org/NET/ssnx/ssn#MeasurementRange">
        <rdfs:subClassOf rdf:resource="http://purl.oclc.org/NET/ssnx/ssn#MeasurementProperty"/>
        <dc:source>skos:exactMatch &apos;measuring interval/measurement range&apos; [VIM 4.7]
                                  http://www.bipm.org/utils/common/documents/jcgm/JCGM_200_2008.pdf</dc:source>
        <rdfs:comment>The set of values that the sensor can return as the result of an observation under the defined conditions with the defined measurement properties.  (If no conditions are specified or the conditions do not specify a range for the observed qualities, the measurement range is to be taken as the condition for the observed qualities.)</rdfs:comment>
        <rdfs:isDefinedBy>http://purl.oclc.org/NET/ssnx/ssn</rdfs:isDefinedBy>
        <rdfs:label>Measurement  Range</rdfs:label>
        <rdfs:seeAlso>http://www.w3.org/2005/Incubator/ssn/wiki/SSN_Sensor#MeasuringCapability</rdfs:seeAlso>
    </owl:Class>
    


    <!-- http://purl.oclc.org/NET/ssnx/ssn#Precision -->

    <owl:Class rdf:about="http://purl.oclc.org/NET/ssnx/ssn#Precision">
        <rdfs:subClassOf rdf:resource="http://purl.oclc.org/NET/ssnx/ssn#MeasurementProperty"/>
        <dc:source>skos:exactMatch &apos;measurement precision/precision&apos; [VIM 2.15]
                                   http://www.bipm.org/utils/common/documents/jcgm/JCGM_200_2008.pdf</dc:source>
        <rdfs:comment>The closeness of agreement between replicate observations on an unchanged or similar quality value: i.e., a measure of a sensor&apos;s ability to consitently reproduce an observation.</rdfs:comment>
        <rdfs:isDefinedBy>http://purl.oclc.org/NET/ssnx/ssn</rdfs:isDefinedBy>
        <rdfs:label>Precision</rdfs:label>
        <rdfs:seeAlso>http://www.w3.org/2005/Incubator/ssn/wiki/SSN_Sensor#MeasuringCapability</rdfs:seeAlso>
    </owl:Class>
    


    <!-- http://purl.oclc.org/NET/ssnx/ssn#Property -->

    <owl:Class rdf:about="http://purl.oclc.org/NET/ssnx/ssn#Property">
        <rdfs:subClassOf rdf:resource="http://www.ontologydesignpatterns.org/ont/dul/DUL.owl#Quality"/>
        <rdfs:subClassOf>
            <owl:Restriction>
                <owl:onProperty rdf:resource="http://purl.oclc.org/NET/ssnx/ssn#isPropertyOf"/>
                <owl:someValuesFrom rdf:resource="http://purl.oclc.org/NET/ssnx/ssn#FeatureOfInterest"/>
            </owl:Restriction>
        </rdfs:subClassOf>
        <alignedWithIFC>IfcProperty</alignedWithIFC>
        <alignedWithSaref>saref:Property</alignedWithSaref>
        <alignedWithWatERP>Phenomenon</alignedWithWatERP>
        <dc:source>skos:exactMatch &apos;property&apos; [O&amp;M] 
		                    http://www.opengeospatial.org/standards/om</dc:source>
        <rdfs:comment>An observable Quality of an Event or Object.  That is, not a quality of an abstract entity as is also allowed by DUL&apos;s Quality, but rather an aspect of an entity that is intrinsic to and cannot exist without the entity and is observable by a sensor.</rdfs:comment>
        <rdfs:isDefinedBy>http://purl.oclc.org/NET/ssnx/ssn</rdfs:isDefinedBy>
        <rdfs:label>Property</rdfs:label>
        <rdfs:seeAlso>http://www.w3.org/2005/Incubator/ssn/wiki/SSN_Skeleton#Skeleton</rdfs:seeAlso>
    </owl:Class>
    


    <!-- http://purl.oclc.org/NET/ssnx/ssn#Resolution -->

    <owl:Class rdf:about="http://purl.oclc.org/NET/ssnx/ssn#Resolution">
        <rdfs:subClassOf rdf:resource="http://purl.oclc.org/NET/ssnx/ssn#MeasurementProperty"/>
        <dc:source>skos:exactMatch &apos;resolution&apos; [VIM 4.14]
                                  http://www.bipm.org/utils/common/documents/jcgm/JCGM_200_2008.pdf</dc:source>
        <rdfs:comment>The smallest difference in the value of a quality being observed that would result in perceptably different values of observation results.</rdfs:comment>
        <rdfs:isDefinedBy>http://purl.oclc.org/NET/ssnx/ssn</rdfs:isDefinedBy>
        <rdfs:label>Resolution</rdfs:label>
        <rdfs:seeAlso>http://www.w3.org/2005/Incubator/ssn/wiki/SSN_Sensor#MeasuringCapability</rdfs:seeAlso>
    </owl:Class>
    


    <!-- http://purl.oclc.org/NET/ssnx/ssn#ResponseTime -->

    <owl:Class rdf:about="http://purl.oclc.org/NET/ssnx/ssn#ResponseTime">
        <rdfs:subClassOf rdf:resource="http://purl.oclc.org/NET/ssnx/ssn#MeasurementProperty"/>
        <dc:source>skos:exactMatch &apos;step response time&apos; [VIM 4.23]
                                  http://www.bipm.org/utils/common/documents/jcgm/JCGM_200_2008.pdf</dc:source>
        <rdfs:comment>The time between a (step) change inthe value of an observed quality and a sensor (possibly with specified error) &apos;settling&apos; on an observed value.</rdfs:comment>
        <rdfs:isDefinedBy>http://purl.oclc.org/NET/ssnx/ssn</rdfs:isDefinedBy>
        <rdfs:label>Response time</rdfs:label>
        <rdfs:seeAlso>http://www.w3.org/2005/Incubator/ssn/wiki/SSN_Sensor#MeasuringCapability</rdfs:seeAlso>
    </owl:Class>
    


    <!-- http://purl.oclc.org/NET/ssnx/ssn#Selectivity -->

    <owl:Class rdf:about="http://purl.oclc.org/NET/ssnx/ssn#Selectivity">
        <rdfs:subClassOf rdf:resource="http://purl.oclc.org/NET/ssnx/ssn#MeasurementProperty"/>
        <dc:source>skos:exactMatch &apos;selectivity&apos; [VIM 4.13]
                                 http://www.bipm.org/utils/common/documents/jcgm/JCGM_200_2008.pdf</dc:source>
        <rdfs:comment>Selectivity is a property of a sensor whereby it provides observed values for one or more qualities such that the values of each quality are independent of other qualities in the phenomenon, body, or substance being investigated.</rdfs:comment>
        <rdfs:isDefinedBy>http://purl.oclc.org/NET/ssnx/ssn</rdfs:isDefinedBy>
        <rdfs:label>Selectivity</rdfs:label>
        <rdfs:seeAlso>http://www.w3.org/2005/Incubator/ssn/wiki/SSN_Sensor#MeasuringCapability</rdfs:seeAlso>
    </owl:Class>
    


    <!-- http://purl.oclc.org/NET/ssnx/ssn#Sensitivity -->

    <owl:Class rdf:about="http://purl.oclc.org/NET/ssnx/ssn#Sensitivity">
        <rdfs:subClassOf rdf:resource="http://purl.oclc.org/NET/ssnx/ssn#MeasurementProperty"/>
        <dc:source>skos:exactMatch &apos;sensitivity&apos; [VIM 4.12]
                                  http://www.bipm.org/utils/common/documents/jcgm/JCGM_200_2008.pdf</dc:source>
        <rdfs:comment>Sensitivity is the quotient of the change in a result of sensor and the corresponding change in a value of a quality being observed.</rdfs:comment>
        <rdfs:isDefinedBy>http://purl.oclc.org/NET/ssnx/ssn</rdfs:isDefinedBy>
        <rdfs:label>Sensitivity</rdfs:label>
        <rdfs:seeAlso>http://www.w3.org/2005/Incubator/ssn/wiki/SSN_Sensor#MeasuringCapability</rdfs:seeAlso>
    </owl:Class>
    


    <!-- http://purl.oclc.org/NET/ssnx/ssn#Sensor -->

    <owl:Class rdf:about="http://purl.oclc.org/NET/ssnx/ssn#Sensor">
        <rdfs:subClassOf rdf:resource="http://purl.oclc.org/NET/ssnx/ssn#Device"/>
        <rdfs:subClassOf>
            <owl:Restriction>
                <owl:onProperty rdf:resource="http://purl.oclc.org/NET/ssnx/ssn#hasMeasurementCapability"/>
                <owl:allValuesFrom rdf:resource="http://purl.oclc.org/NET/ssnx/ssn#MeasurementCapability"/>
            </owl:Restriction>
        </rdfs:subClassOf>
        <rdfs:subClassOf>
            <owl:Restriction>
                <owl:onProperty rdf:resource="http://purl.oclc.org/NET/ssnx/ssn#observes"/>
                <owl:allValuesFrom rdf:resource="http://purl.oclc.org/NET/ssnx/ssn#Property"/>
            </owl:Restriction>
        </rdfs:subClassOf>
        <rdfs:subClassOf>
            <owl:Restriction>
                <owl:onProperty rdf:resource="http://www.semanticwater.com/WISDOM#atAsset"/>
                <owl:maxQualifiedCardinality rdf:datatype="http://www.w3.org/2001/XMLSchema#nonNegativeInteger">1</owl:maxQualifiedCardinality>
                <owl:onClass rdf:resource="http://www.semanticwater.com/WISDOM#DesignedAsset"/>
            </owl:Restriction>
        </rdfs:subClassOf>
        <rdfs:subClassOf>
            <owl:Restriction>
                <owl:onProperty rdf:resource="http://www.semanticwater.com/WISDOM#deployedAtEntity"/>
                <owl:maxQualifiedCardinality rdf:datatype="http://www.w3.org/2001/XMLSchema#nonNegativeInteger">1</owl:maxQualifiedCardinality>
                <owl:onClass rdf:resource="http://purl.oclc.org/NET/ssnx/ssn#FeatureOfInterest"/>
            </owl:Restriction>
        </rdfs:subClassOf>
        <alignedWithIFC>IfcSensor</alignedWithIFC>
        <alignedWithSaref>saref:Sensor</alignedWithSaref>
        <dc:source>skos:exactMatch &apos;sensor&apos; [SensorML OGC-0700]
		                    http://www.opengeospatial.org/standards/sensorml 

                                skos:closeMatch &apos;observation procedure&apos; [O&amp;M] 
                                http://www.opengeospatial.org/standards/om 

O&amp;M allows sensors, methods, instruments, systems, algorithms and process chains as the processUsed of an observation; this ontology allows a similar range of things (any thing that can do sensing), just they are all grouped under the term sensor (which is thus wider than the O&amp;M concept).</dc:source>
        <rdfs:comment>A sensor can do (implements) sensing: that is, a sensor is any entity that can follow a sensing method and thus observe some Property of a FeatureOfInterest.  Sensors may be physical devices, computational methods, a laboratory setup with a person following a method, or any other thing that can follow a Sensing Method to observe a Property.</rdfs:comment>
        <rdfs:isDefinedBy>http://purl.oclc.org/NET/ssnx/ssn</rdfs:isDefinedBy>
        <rdfs:label>Sensor</rdfs:label>
        <rdfs:seeAlso>http://www.w3.org/2005/Incubator/ssn/wiki/SSN_Skeleton#Skeleton</rdfs:seeAlso>
    </owl:Class>
    


    <!-- http://schema.org/Person -->

    <rdf:Description rdf:about="http://schema.org/Person">
        <owl:equivalentClass rdf:resource="http://xmlns.com/foaf/0.1/Person"/>
    </rdf:Description>
    


    <!-- http://vocab.gtfs.org/terms#CalendarDateRule -->

    <owl:Class rdf:about="http://vocab.gtfs.org/terms#CalendarDateRule">
        <rdfs:subClassOf rdf:resource="http://vocab.gtfs.org/terms#ServiceRule"/>
        <comment xml:lang="en">a row from calendar_dates.txt</comment>
        <comment xml:lang="es">una línea en calendar_dates.txt</comment>
        <rdfs:comment xml:lang="en">Defines service availability for a specific date</rdfs:comment>
        <rdfs:comment xml:lang="es">Indica la disponibilidad de servicio para una fecha concreta</rdfs:comment>
        <rdfs:label xml:lang="en">Calendar date rule</rdfs:label>
        <rdfs:label xml:lang="es">Regla de fecha de calendario</rdfs:label>
        <rdfs:seeAlso rdf:resource="https://developers.google.com/transit/gtfs/reference#calendar_dates_fields"/>
        <status:term_status xml:lang="es">inestable</status:term_status>
        <status:term_status xml:lang="en">unstable</status:term_status>
    </owl:Class>
    


    <!-- http://vocab.gtfs.org/terms#CalendarRule -->

    <owl:Class rdf:about="http://vocab.gtfs.org/terms#CalendarRule">
        <rdfs:subClassOf rdf:resource="http://vocab.gtfs.org/terms#ServiceRule"/>
        <comment xml:lang="en">a row from calendar.txt</comment>
        <comment xml:lang="es">una línea de calendar.txt</comment>
        <rdfs:comment xml:lang="es">Define en qué días de la semana el servicio está disponible para un periodo concreto.</rdfs:comment>
        <rdfs:comment xml:lang="en">Defines on which days of the week for a certain period the service is available.</rdfs:comment>
        <rdfs:label xml:lang="en">Calendar rule</rdfs:label>
        <rdfs:label xml:lang="es">Regla de calendario</rdfs:label>
        <status:term_status xml:lang="es">inestable</status:term_status>
        <status:term_status xml:lang="en">unstable</status:term_status>
    </owl:Class>
    


    <!-- http://vocab.gtfs.org/terms#Route -->

    <owl:Class rdf:about="http://vocab.gtfs.org/terms#Route">
        <rdfs:comment xml:lang="en">A gtfs:Route is a commercial route followed entirely or partly by gtfs:Trips</rdfs:comment>
        <rdfs:comment xml:lang="es">Una gtfs:Route es un grupo de viajes (gtfs:Trips) que se muestran a los usuarios como servicio independiente</rdfs:comment>
        <rdfs:label xml:lang="en">Route</rdfs:label>
        <rdfs:label xml:lang="es">Ruta</rdfs:label>
        <rdfs:seeAlso rdf:resource="https://developers.google.com/transit/gtfs/reference#routes_fields"/>
        <status:term_status xml:lang="es">inestable</status:term_status>
        <status:term_status xml:lang="en">unstable</status:term_status>
    </owl:Class>
    


    <!-- http://vocab.gtfs.org/terms#RouteType -->

    <owl:Class rdf:about="http://vocab.gtfs.org/terms#RouteType">
        <rdfs:comment xml:lang="es">Describe el tipo de transporte usado en una ruta</rdfs:comment>
        <rdfs:comment xml:lang="en">Describes the type of transportation used on a route</rdfs:comment>
        <rdfs:label xml:lang="en">Route type</rdfs:label>
        <rdfs:label xml:lang="es">Tipo de ruta</rdfs:label>
        <status:term_status xml:lang="es">inestable</status:term_status>
        <status:term_status xml:lang="en">unstable</status:term_status>
    </owl:Class>
    


    <!-- http://vocab.gtfs.org/terms#Service -->

    <owl:Class rdf:about="http://vocab.gtfs.org/terms#Service">
        <comment xml:lang="en">A gtfs:Service is a set of gtfs:ServiceRules which can be found in both calendar.txt as calendar_dates.txt</comment>
        <comment xml:lang="es">Un gtfs:Service es un conjunto de gtfs:ServiceRules que pueden ser encontradas en calendar.txt y calendar_dates.txt</comment>
        <rdfs:comment xml:lang="en">A gtfs:Service identifies a set of dates when a service is available for one or more routes</rdfs:comment>
        <rdfs:comment xml:lang="es">Un gtfs:Service indica el conjunto de fechas en el que el servicio está disponible para una o más rutas</rdfs:comment>
        <rdfs:label xml:lang="en">Service</rdfs:label>
        <rdfs:label xml:lang="es">Servicio</rdfs:label>
        <rdfs:seeAlso rdf:resource="https://developers.google.com/transit/gtfs/reference#calendar_dates_fields"/>
        <rdfs:seeAlso rdf:resource="https://developers.google.com/transit/gtfs/reference#calendar_fields"/>
        <status:term_status xml:lang="es">inestable</status:term_status>
        <status:term_status xml:lang="en">unstable</status:term_status>
    </owl:Class>
    


    <!-- http://vocab.gtfs.org/terms#ServiceRule -->

    <owl:Class rdf:about="http://vocab.gtfs.org/terms#ServiceRule">
        <rdfs:comment xml:lang="en">One or more service rules define a set of dates</rdfs:comment>
        <rdfs:comment xml:lang="es">Una o más reglas de servicio definen un conjunto de fechas</rdfs:comment>
        <rdfs:label xml:lang="es">Regla de servicio</rdfs:label>
        <rdfs:label xml:lang="en">Service rule</rdfs:label>
        <status:term_status xml:lang="es">inestable</status:term_status>
        <status:term_status xml:lang="en">unstable</status:term_status>
    </owl:Class>
    


    <!-- http://vocab.gtfs.org/terms#Stop -->

    <owl:Class rdf:about="http://vocab.gtfs.org/terms#Stop">
        <rdfs:comment xml:lang="en">A location where passengers board or disembark from a transit vehicle.</rdfs:comment>
        <rdfs:comment xml:lang="es">Un lugar donde los pasajeros suben o bajan de un vehículo de transporte público.</rdfs:comment>
        <rdfs:label xml:lang="es">Parada</rdfs:label>
        <rdfs:label xml:lang="en">Stop</rdfs:label>
        <rdfs:seeAlso rdf:resource="https://developers.google.com/transit/gtfs/reference#stops_fields"/>
        <status:term_status xml:lang="es">estable</status:term_status>
        <status:term_status xml:lang="en">stable</status:term_status>
    </owl:Class>
    


    <!-- http://vocab.gtfs.org/terms#StopTime -->

    <owl:Class rdf:about="http://vocab.gtfs.org/terms#StopTime">
        <rdfs:comment xml:lang="es">Describe una hora de parada como parte de un viaje</rdfs:comment>
        <rdfs:comment xml:lang="en">Describes a stop time as part of a trip</rdfs:comment>
        <rdfs:label xml:lang="es">Hora de parada</rdfs:label>
        <rdfs:label xml:lang="en">Stop time</rdfs:label>
        <rdfs:seeAlso rdf:resource="https://developers.google.com/transit/gtfs/reference#stop_times_fields"/>
        <status:term_status xml:lang="es">inestable</status:term_status>
        <status:term_status xml:lang="en">unstable</status:term_status>
    </owl:Class>
    


    <!-- http://vocab.gtfs.org/terms#Trip -->

    <owl:Class rdf:about="http://vocab.gtfs.org/terms#Trip">
        <rdfs:comment xml:lang="en">A collection of gtfs:StopTimes followed by a transit vehicle</rdfs:comment>
        <rdfs:comment xml:lang="es">Trayecto de dos o más paradas realizadas por un vehículo que se produce a una gtfs:StopTime</rdfs:comment>
        <rdfs:label xml:lang="en">Trip</rdfs:label>
        <rdfs:label xml:lang="es">Viaje</rdfs:label>
        <rdfs:seeAlso rdf:resource="https://developers.google.com/transit/gtfs/reference#trips_fields"/>
        <status:term_status xml:lang="es">inestable</status:term_status>
        <status:term_status xml:lang="en">unstable</status:term_status>
    </owl:Class>
    


    <!-- http://www.ontologydesignpatterns.org/ont/dul/DUL.owl#DesignedArtifact -->

    <owl:Class rdf:about="http://www.ontologydesignpatterns.org/ont/dul/DUL.owl#DesignedArtifact">
        <rdfs:subClassOf rdf:resource="http://www.ontologydesignpatterns.org/ont/dul/DUL.owl#PhysicalArtifact"/>
        <rdfs:subClassOf rdf:resource="http://www.semanticwater.com/WISDOM#SampledFeature"/>
        <alignedWithIFC>IfcAsset</alignedWithIFC>
        <alignedWithWatERP>Infrastructure</alignedWithWatERP>
        <rdfs:comment>A PhysicalArtifact that is also described by a Design. This excludes simple recycling or refunctionalization of natural objects. Most common sense &apos;artifacts&apos; can be included in this class: cars, lamps, houses, chips, etc.</rdfs:comment>
        <rdfs:label xml:lang="it">Artefatto progettato</rdfs:label>
        <rdfs:label xml:lang="en">Designed artifact</rdfs:label>
    </owl:Class>
    


    <!-- http://www.ontologydesignpatterns.org/ont/dul/DUL.owl#Entity -->

    <owl:Class rdf:about="http://www.ontologydesignpatterns.org/ont/dul/DUL.owl#Entity">
        <alignedWithIFC>IfcObject</alignedWithIFC>
        <rdfs:comment rdf:datatype="http://www.w3.org/2001/XMLSchema#string">Anything: real, possible, or imaginary, which some modeller wants to talk about for some purpose.</rdfs:comment>
        <rdfs:label xml:lang="en">Entity</rdfs:label>
        <rdfs:label xml:lang="it">Entità</rdfs:label>
    </owl:Class>
    


    <!-- http://www.ontologydesignpatterns.org/ont/dul/DUL.owl#Object -->

    <owl:Class rdf:about="http://www.ontologydesignpatterns.org/ont/dul/DUL.owl#Object">
        <rdfs:subClassOf rdf:resource="http://www.ontologydesignpatterns.org/ont/dul/DUL.owl#Entity"/>
        <rdfs:subClassOf>
            <owl:Restriction>
                <owl:onProperty rdf:resource="http://www.ontologydesignpatterns.org/ont/dul/DUL.owl#hasConstituent"/>
                <owl:allValuesFrom rdf:resource="http://www.ontologydesignpatterns.org/ont/dul/DUL.owl#Object"/>
            </owl:Restriction>
        </rdfs:subClassOf>
        <owl:disjointWith rdf:resource="http://www.ontologydesignpatterns.org/ont/dul/DUL.owl#Quality"/>
        <rdfs:comment rdf:datatype="http://www.w3.org/2001/XMLSchema#string">Any physical, social, or mental object, or a substance</rdfs:comment>
        <rdfs:label xml:lang="en">Object</rdfs:label>
        <rdfs:label xml:lang="it">Oggetto</rdfs:label>
    </owl:Class>
    


    <!-- http://www.ontologydesignpatterns.org/ont/dul/DUL.owl#PhysicalArtifact -->

    <owl:Class rdf:about="http://www.ontologydesignpatterns.org/ont/dul/DUL.owl#PhysicalArtifact">
        <rdfs:subClassOf rdf:resource="http://www.ontologydesignpatterns.org/ont/dul/DUL.owl#PhysicalObject"/>
        <alignedWithIFC>IfcProduct</alignedWithIFC>
        <rdfs:comment rdf:datatype="http://www.w3.org/2001/XMLSchema#string">Any PhysicalObject that isDescribedBy a Plan .
This axiomatization is weak, but allows to talk of artifacts in a very general sense, i.e. including recycled objects, objects with an intentional functional change, natural objects that are given a certain function, even though they are not modified or structurally designed, etc. PhysicalArtifact(s) are not considered disjoint from PhysicalBody(s), in order to allow a dual classification when needed. E.g.,
FunctionalSubstance(s) are included here as well.
Immaterial (non-physical) artifacts (e.g. texts, ideas, cultural movements, corporations, communities, etc. can be modelled as social objects (see SocialObject), which are all &apos;artifactual&apos; in the weak sense assumed here.</rdfs:comment>
        <rdfs:label xml:lang="it">Artefatto fisico</rdfs:label>
        <rdfs:label xml:lang="en">Physical artifact</rdfs:label>
    </owl:Class>
    


    <!-- http://www.ontologydesignpatterns.org/ont/dul/DUL.owl#PhysicalObject -->

    <owl:Class rdf:about="http://www.ontologydesignpatterns.org/ont/dul/DUL.owl#PhysicalObject">
        <rdfs:subClassOf rdf:resource="http://www.ontologydesignpatterns.org/ont/dul/DUL.owl#Object"/>
        <rdfs:comment rdf:datatype="http://www.w3.org/2001/XMLSchema#string">Any Object that has a proper space region. The prototypical physical object has also an associated mass, but the nature of its mass can greatly vary based on the epistemological status of the object (scientifically measured, subjectively possible, imaginary).</rdfs:comment>
        <rdfs:label xml:lang="it">Oggetto fisico</rdfs:label>
        <rdfs:label xml:lang="en">Physical object</rdfs:label>
    </owl:Class>
    


    <!-- http://www.ontologydesignpatterns.org/ont/dul/DUL.owl#Quality -->

    <owl:Class rdf:about="http://www.ontologydesignpatterns.org/ont/dul/DUL.owl#Quality">
        <rdfs:subClassOf rdf:resource="http://www.ontologydesignpatterns.org/ont/dul/DUL.owl#Entity"/>
        <rdfs:subClassOf>
            <owl:Restriction>
                <owl:onProperty rdf:resource="http://www.ontologydesignpatterns.org/ont/dul/DUL.owl#isQualityOf"/>
                <owl:someValuesFrom rdf:resource="http://www.ontologydesignpatterns.org/ont/dul/DUL.owl#Entity"/>
            </owl:Restriction>
        </rdfs:subClassOf>
        <rdfs:subClassOf>
            <owl:Restriction>
                <owl:onProperty rdf:resource="http://www.ontologydesignpatterns.org/ont/dul/DUL.owl#hasConstituent"/>
                <owl:allValuesFrom rdf:resource="http://www.ontologydesignpatterns.org/ont/dul/DUL.owl#Quality"/>
            </owl:Restriction>
        </rdfs:subClassOf>
        <rdfs:comment>Any aspect of an Entity (but not a part of it), which cannot exist without that Entity. For example, the way the surface of a specific PhysicalObject looks like is a Quality, while the encoding of that Quality into e.g. a PhysicalAttribute should be modeled as a Region. 
From the design viewpoint, the Quality-Region distinction is useful only when individual aspects of an Entity are considered in a domain of discourse. 
For example, in an automotive context, it would be irrelevant to consider the aspects of car windows for a specific car, unless the factory wants to check a specific window against design parameters (anomaly detection). 
On the other hand, in an antiques context, the individual aspects for a specific piece of furniture are a major focus of attention, and may constitute the actual added value, because the design parameters for old furniture are often not fixed, and may not be viewed as &apos;anomalies&apos;.</rdfs:comment>
        <rdfs:label xml:lang="en">Quality</rdfs:label>
        <rdfs:label xml:lang="it">Qualità</rdfs:label>
    </owl:Class>
    


    <!-- http://www.ontologydesignpatterns.org/ont/dul/DUL.owl#Region -->

    <owl:Class rdf:about="http://www.ontologydesignpatterns.org/ont/dul/DUL.owl#Region">
        <rdfs:subClassOf rdf:resource="http://www.ontologydesignpatterns.org/ont/dul/DUL.owl#Quality"/>
        <rdfs:subClassOf>
            <owl:Restriction>
                <owl:onProperty rdf:resource="http://www.ontologydesignpatterns.org/ont/dul/DUL.owl#hasConstituent"/>
                <owl:allValuesFrom rdf:resource="http://www.ontologydesignpatterns.org/ont/dul/DUL.owl#Region"/>
            </owl:Restriction>
        </rdfs:subClassOf>
        <rdfs:comment rdf:datatype="http://www.w3.org/2001/XMLSchema#string">Any region in a dimensional space (a dimensional space is a maximal Region), which can be used as a value for a quality of an Entity . For example, TimeInterval, SpaceRegion, PhysicalAttribute, Amount, SocialAttribute are all subclasses of Region. 
Regions are not data values in the ordinary knowledge representation sense; in order to get patterns for modelling data, see the properties: representsDataValue and hasDataValue</rdfs:comment>
        <rdfs:label xml:lang="en">Region</rdfs:label>
        <rdfs:label xml:lang="it">Regione</rdfs:label>
    </owl:Class>
    


    <!-- http://www.semanticwater.com/WISDOM#AbstractionNode -->

    <owl:Class rdf:about="http://www.semanticwater.com/WISDOM#AbstractionNode">
        <rdfs:subClassOf rdf:resource="http://www.semanticwater.com/WISDOM#TerminalNode"/>
        <alignedWithWatERP>Source</alignedWithWatERP>
    </owl:Class>
    


    <!-- http://www.semanticwater.com/WISDOM#Arc -->

    <owl:Class rdf:about="http://www.semanticwater.com/WISDOM#Arc">
        <rdfs:subClassOf rdf:resource="http://www.semanticwater.com/WISDOM#PhysicalTopologicalEntity"/>
        <alignedWithIFC>IfcEdge</alignedWithIFC>
        <alignedWithInspire>Link</alignedWithInspire>
    </owl:Class>
    


    <!-- http://www.semanticwater.com/WISDOM#Chamber -->

    <owl:Class rdf:about="http://www.semanticwater.com/WISDOM#Chamber">
        <rdfs:subClassOf rdf:resource="http://www.semanticwater.com/WISDOM#StorageAsset"/>
        <alignedWithIFC>IfcDistributionChamberElement</alignedWithIFC>
    </owl:Class>
    


    <!-- http://www.semanticwater.com/WISDOM#ChlorineSensor -->

    <owl:Class rdf:about="http://www.semanticwater.com/WISDOM#ChlorineSensor">
        <rdfs:subClassOf rdf:resource="http://www.semanticwater.com/WISDOM#WaterSensor"/>
    </owl:Class>
    


    <!-- http://www.semanticwater.com/WISDOM#CleanMain -->

    <owl:Class rdf:about="http://www.semanticwater.com/WISDOM#CleanMain">
        <rdfs:subClassOf rdf:resource="http://www.semanticwater.com/WISDOM#WaterPipe"/>
        <owl:disjointWith rdf:resource="http://www.semanticwater.com/WISDOM#WastePipe"/>
    </owl:Class>
    


    <!-- http://www.semanticwater.com/WISDOM#CleanPumpingStation -->

    <owl:Class rdf:about="http://www.semanticwater.com/WISDOM#CleanPumpingStation">
        <rdfs:subClassOf rdf:resource="http://www.semanticwater.com/WISDOM#PumpingStation"/>
    </owl:Class>
    


    <!-- http://www.semanticwater.com/WISDOM#CleanTreatmentWorks -->

    <owl:Class rdf:about="http://www.semanticwater.com/WISDOM#CleanTreatmentWorks">
        <rdfs:subClassOf rdf:resource="http://www.semanticwater.com/WISDOM#TreatmentWorks"/>
    </owl:Class>
    


    <!-- http://www.semanticwater.com/WISDOM#CombinedChamber -->

    <owl:Class rdf:about="http://www.semanticwater.com/WISDOM#CombinedChamber">
        <rdfs:subClassOf rdf:resource="http://www.semanticwater.com/WISDOM#WasteChamber"/>
    </owl:Class>
    


    <!-- http://www.semanticwater.com/WISDOM#CombinedPumpingStation -->

    <owl:Class rdf:about="http://www.semanticwater.com/WISDOM#CombinedPumpingStation">
        <rdfs:subClassOf rdf:resource="http://www.semanticwater.com/WISDOM#WastePumpingStation"/>
    </owl:Class>
    


    <!-- http://www.semanticwater.com/WISDOM#CombinedTreatmentWorks -->

    <owl:Class rdf:about="http://www.semanticwater.com/WISDOM#CombinedTreatmentWorks">
        <rdfs:subClassOf rdf:resource="http://www.semanticwater.com/WISDOM#TreatmentWorks"/>
    </owl:Class>
    


    <!-- http://www.semanticwater.com/WISDOM#ConnectingSewer -->

    <owl:Class rdf:about="http://www.semanticwater.com/WISDOM#ConnectingSewer">
        <rdfs:subClassOf rdf:resource="http://www.semanticwater.com/WISDOM#WasteDistributionMain"/>
    </owl:Class>
    


    <!-- http://www.semanticwater.com/WISDOM#ConsumptionAppliance -->

    <owl:Class rdf:about="http://www.semanticwater.com/WISDOM#ConsumptionAppliance">
        <rdfs:subClassOf rdf:resource="http://www.semanticwater.com/WISDOM#DomesticDevice"/>
        <alignedWithSaref>saref:Appliance</alignedWithSaref>
        <alignedWithWatERP>Appliance</alignedWithWatERP>
    </owl:Class>
    


    <!-- http://www.semanticwater.com/WISDOM#ConsumptionNode -->

    <owl:Class rdf:about="http://www.semanticwater.com/WISDOM#ConsumptionNode">
        <rdfs:subClassOf rdf:resource="http://www.semanticwater.com/WISDOM#PhysicalNode"/>
        <alignedWithWatERP>Sink</alignedWithWatERP>
    </owl:Class>
    


    <!-- http://www.semanticwater.com/WISDOM#DesignedAsset -->

    <owl:Class rdf:about="http://www.semanticwater.com/WISDOM#DesignedAsset">
        <rdfs:subClassOf rdf:resource="http://www.ontologydesignpatterns.org/ont/dul/DUL.owl#DesignedArtifact"/>
    </owl:Class>
    


    <!-- http://www.semanticwater.com/WISDOM#DischargeNode -->

    <owl:Class rdf:about="http://www.semanticwater.com/WISDOM#DischargeNode">
        <rdfs:subClassOf rdf:resource="http://www.semanticwater.com/WISDOM#TerminalNode"/>
    </owl:Class>
    


    <!-- http://www.semanticwater.com/WISDOM#DistributionMain -->

    <owl:Class rdf:about="http://www.semanticwater.com/WISDOM#DistributionMain">
        <rdfs:subClassOf rdf:resource="http://www.semanticwater.com/WISDOM#CleanMain"/>
        <rdfs:label xml:lang="en">DistributionMain</rdfs:label>
    </owl:Class>
    


    <!-- http://www.semanticwater.com/WISDOM#DomesticDevice -->

    <owl:Class rdf:about="http://www.semanticwater.com/WISDOM#DomesticDevice">
        <rdfs:subClassOf rdf:resource="http://purl.oclc.org/NET/ssnx/ssn#Device"/>
    </owl:Class>
    


    <!-- http://www.semanticwater.com/WISDOM#ElecProperty -->

    <owl:Class rdf:about="http://www.semanticwater.com/WISDOM#ElecProperty">
        <rdfs:subClassOf rdf:resource="http://www.semanticwater.com/WISDOM#WaterNetworkProperty"/>
    </owl:Class>
    


    <!-- http://www.semanticwater.com/WISDOM#Fitting -->

    <owl:Class rdf:about="http://www.semanticwater.com/WISDOM#Fitting">
        <owl:equivalentClass rdf:resource="http://www.semanticwater.com/WISDOM#FittingNode"/>
        <rdfs:subClassOf rdf:resource="http://www.ontologydesignpatterns.org/ont/dul/DUL.owl#DesignedArtifact"/>
        <alignedWithIFC>IfcPipeFitting</alignedWithIFC>
        <rdfs:label xml:lang="en">Fitting</rdfs:label>
    </owl:Class>
    


    <!-- http://www.semanticwater.com/WISDOM#FittingNode -->

    <owl:Class rdf:about="http://www.semanticwater.com/WISDOM#FittingNode">
        <rdfs:subClassOf rdf:resource="http://www.semanticwater.com/WISDOM#PhysicalNode"/>
    </owl:Class>
    


    <!-- http://www.semanticwater.com/WISDOM#FlowSensor -->

    <owl:Class rdf:about="http://www.semanticwater.com/WISDOM#FlowSensor">
        <rdfs:subClassOf rdf:resource="http://www.semanticwater.com/WISDOM#WaterSensor"/>
    </owl:Class>
    


    <!-- http://www.semanticwater.com/WISDOM#FlowType -->

    <owl:Class rdf:about="http://www.semanticwater.com/WISDOM#FlowType">
        <rdfs:subClassOf rdf:resource="http://www.semanticwater.com/WISDOM#WaterNetworkProperty"/>
    </owl:Class>
    


    <!-- http://www.semanticwater.com/WISDOM#FluidDynamicsProperty -->

    <owl:Class rdf:about="http://www.semanticwater.com/WISDOM#FluidDynamicsProperty">
        <rdfs:subClassOf rdf:resource="http://www.semanticwater.com/WISDOM#WaterNetworkProperty"/>
    </owl:Class>
    


    <!-- http://www.semanticwater.com/WISDOM#FoulChamber -->

    <owl:Class rdf:about="http://www.semanticwater.com/WISDOM#FoulChamber">
        <rdfs:subClassOf rdf:resource="http://www.semanticwater.com/WISDOM#WasteChamber"/>
    </owl:Class>
    


    <!-- http://www.semanticwater.com/WISDOM#FoulPipe -->

    <owl:Class rdf:about="http://www.semanticwater.com/WISDOM#FoulPipe">
        <rdfs:subClassOf rdf:resource="http://www.semanticwater.com/WISDOM#WasteDistributionMain"/>
    </owl:Class>
    


    <!-- http://www.semanticwater.com/WISDOM#FoulPumpingStation -->

    <owl:Class rdf:about="http://www.semanticwater.com/WISDOM#FoulPumpingStation">
        <rdfs:subClassOf rdf:resource="http://www.semanticwater.com/WISDOM#WastePumpingStation"/>
    </owl:Class>
    


    <!-- http://www.semanticwater.com/WISDOM#FoulTreatmentWorks -->

    <owl:Class rdf:about="http://www.semanticwater.com/WISDOM#FoulTreatmentWorks">
        <rdfs:subClassOf rdf:resource="http://www.semanticwater.com/WISDOM#TreatmentWorks"/>
    </owl:Class>
    


    <!-- http://www.semanticwater.com/WISDOM#FullPipeFlow -->

    <owl:Class rdf:about="http://www.semanticwater.com/WISDOM#FullPipeFlow">
        <rdfs:subClassOf rdf:resource="http://www.semanticwater.com/WISDOM#FlowType"/>
    </owl:Class>
    


    <!-- http://www.semanticwater.com/WISDOM#Hydrant -->

    <owl:Class rdf:about="http://www.semanticwater.com/WISDOM#Hydrant">
        <rdfs:subClassOf rdf:resource="http://www.ontologydesignpatterns.org/ont/dul/DUL.owl#DesignedArtifact"/>
        <rdfs:subClassOf rdf:resource="http://www.semanticwater.com/WISDOM#ConsumptionNode"/>
        <rdfs:label xml:lang="en">Hydrant</rdfs:label>
    </owl:Class>
    


    <!-- http://www.semanticwater.com/WISDOM#LevelSensor -->

    <owl:Class rdf:about="http://www.semanticwater.com/WISDOM#LevelSensor">
        <rdfs:subClassOf rdf:resource="http://www.semanticwater.com/WISDOM#WaterSensor"/>
    </owl:Class>
    


    <!-- http://www.semanticwater.com/WISDOM#Main -->

    <owl:Class rdf:about="http://www.semanticwater.com/WISDOM#Main">
        <owl:equivalentClass rdf:resource="http://www.semanticwater.com/WISDOM#Pipe"/>
        <rdfs:subClassOf rdf:resource="http://www.ontologydesignpatterns.org/ont/dul/DUL.owl#DesignedArtifact"/>
        <alignedWithIFC>IfcPipeSegment</alignedWithIFC>
        <alignedWithInspire>Pipe</alignedWithInspire>
        <rdfs:label xml:lang="en">Main</rdfs:label>
    </owl:Class>
    


    <!-- http://www.semanticwater.com/WISDOM#Material -->

    <owl:Class rdf:about="http://www.semanticwater.com/WISDOM#Material">
        <rdfs:subClassOf rdf:resource="http://www.semanticwater.com/WISDOM#WaterNetworkStaticProperty"/>
        <alignedWithIFC>IfcMaterial</alignedWithIFC>
    </owl:Class>
    


    <!-- http://www.semanticwater.com/WISDOM#NaturalArtifact -->

    <owl:Class rdf:about="http://www.semanticwater.com/WISDOM#NaturalArtifact">
        <rdfs:subClassOf rdf:resource="http://www.ontologydesignpatterns.org/ont/dul/DUL.owl#PhysicalArtifact"/>
    </owl:Class>
    


    <!-- http://www.semanticwater.com/WISDOM#Node -->

    <owl:Class rdf:about="http://www.semanticwater.com/WISDOM#Node">
        <rdfs:subClassOf rdf:resource="http://www.semanticwater.com/WISDOM#PhysicalTopologicalEntity"/>
        <rdfs:subClassOf>
            <owl:Restriction>
                <owl:onProperty rdf:resource="http://www.semanticwater.com/WISDOM#atAsset"/>
                <owl:maxQualifiedCardinality rdf:datatype="http://www.w3.org/2001/XMLSchema#nonNegativeInteger">1</owl:maxQualifiedCardinality>
                <owl:onClass rdf:resource="http://www.semanticwater.com/WISDOM#DesignedAsset"/>
            </owl:Restriction>
        </rdfs:subClassOf>
        <alignedWithIFC>IfcVertex</alignedWithIFC>
        <alignedWithInspire>Node</alignedWithInspire>
    </owl:Class>
    


    <!-- http://www.semanticwater.com/WISDOM#OpenChannelFlow -->

    <owl:Class rdf:about="http://www.semanticwater.com/WISDOM#OpenChannelFlow">
        <rdfs:subClassOf rdf:resource="http://www.semanticwater.com/WISDOM#FlowType"/>
    </owl:Class>
    


    <!-- http://www.semanticwater.com/WISDOM#Percentage_LevelSensor -->

    <owl:Class rdf:about="http://www.semanticwater.com/WISDOM#Percentage_LevelSensor">
        <rdfs:subClassOf rdf:resource="http://www.semanticwater.com/WISDOM#WaterSensor"/>
    </owl:Class>
    


    <!-- http://www.semanticwater.com/WISDOM#PhysicalArc -->

    <owl:Class rdf:about="http://www.semanticwater.com/WISDOM#PhysicalArc">
        <rdfs:subClassOf rdf:resource="http://www.semanticwater.com/WISDOM#Arc"/>
        <alignedWithInspire>UtilityLink</alignedWithInspire>
        <alignedWithWatERP>Transport</alignedWithWatERP>
    </owl:Class>
    


    <!-- http://www.semanticwater.com/WISDOM#PhysicalNode -->

    <owl:Class rdf:about="http://www.semanticwater.com/WISDOM#PhysicalNode">
        <rdfs:subClassOf rdf:resource="http://www.semanticwater.com/WISDOM#Node"/>
        <alignedWithInspire>Appurtenance</alignedWithInspire>
    </owl:Class>
    


    <!-- http://www.semanticwater.com/WISDOM#PhysicalQuantity -->

    <owl:Class rdf:about="http://www.semanticwater.com/WISDOM#PhysicalQuantity">
        <rdfs:subClassOf rdf:resource="http://www.ontologydesignpatterns.org/ont/dul/DUL.owl#Region"/>
        <alignedWithIFC>IfcPhysicalSimpleQuantity</alignedWithIFC>
    </owl:Class>
    


    <!-- http://www.semanticwater.com/WISDOM#PhysicalTopologicalEntity -->

    <owl:Class rdf:about="http://www.semanticwater.com/WISDOM#PhysicalTopologicalEntity">
        <rdfs:subClassOf rdf:resource="http://www.ontologydesignpatterns.org/ont/dul/DUL.owl#Entity"/>
        <rdfs:subClassOf>
            <owl:Restriction>
                <owl:onProperty rdf:resource="http://www.semanticwater.com/WISDOM#hasFeatureOfInterest"/>
                <owl:allValuesFrom rdf:resource="http://purl.oclc.org/NET/ssnx/ssn#FeatureOfInterest"/>
            </owl:Restriction>
        </rdfs:subClassOf>
        <alignedWithIFC>IfcTopologicalRepresentationItem</alignedWithIFC>
        <alignedWithInspire>Network::NetworkElement</alignedWithInspire>
        <alignedWithWatERP>WaterResource</alignedWithWatERP>
    </owl:Class>
    


    <!-- http://www.semanticwater.com/WISDOM#Pipe -->

    <owl:Class rdf:about="http://www.semanticwater.com/WISDOM#Pipe">
        <rdfs:subClassOf rdf:resource="http://www.semanticwater.com/WISDOM#PhysicalArc"/>
    </owl:Class>
    


    <!-- http://www.semanticwater.com/WISDOM#PipeShape -->

    <owl:Class rdf:about="http://www.semanticwater.com/WISDOM#PipeShape">
        <rdfs:subClassOf rdf:resource="http://www.semanticwater.com/WISDOM#WaterNetworkStaticProperty"/>
    </owl:Class>
    


    <!-- http://www.semanticwater.com/WISDOM#PotablePumpingStation -->

    <owl:Class rdf:about="http://www.semanticwater.com/WISDOM#PotablePumpingStation">
        <rdfs:subClassOf rdf:resource="http://www.semanticwater.com/WISDOM#CleanPumpingStation"/>
    </owl:Class>
    


    <!-- http://www.semanticwater.com/WISDOM#PressureSensor -->

    <owl:Class rdf:about="http://www.semanticwater.com/WISDOM#PressureSensor">
        <rdfs:subClassOf rdf:resource="http://www.semanticwater.com/WISDOM#WaterSensor"/>
    </owl:Class>
    


    <!-- http://www.semanticwater.com/WISDOM#PumpNode -->

    <owl:Class rdf:about="http://www.semanticwater.com/WISDOM#PumpNode">
        <owl:equivalentClass rdf:resource="http://www.semanticwater.com/WISDOM#PumpingStation"/>
        <rdfs:subClassOf rdf:resource="http://www.semanticwater.com/WISDOM#TransformationNode"/>
    </owl:Class>
    


    <!-- http://www.semanticwater.com/WISDOM#PumpSpinRate -->

    <owl:Class rdf:about="http://www.semanticwater.com/WISDOM#PumpSpinRate">
        <rdfs:subClassOf rdf:resource="http://www.semanticwater.com/WISDOM#WaterNetworkProperty"/>
    </owl:Class>
    


    <!-- http://www.semanticwater.com/WISDOM#PumpSpinRateSensor -->

    <owl:Class rdf:about="http://www.semanticwater.com/WISDOM#PumpSpinRateSensor">
        <rdfs:subClassOf rdf:resource="http://www.semanticwater.com/WISDOM#WaterSensor"/>
    </owl:Class>
    


    <!-- http://www.semanticwater.com/WISDOM#PumpingStation -->

    <owl:Class rdf:about="http://www.semanticwater.com/WISDOM#PumpingStation">
        <rdfs:subClassOf rdf:resource="http://www.semanticwater.com/WISDOM#DesignedAsset"/>
    </owl:Class>
    


    <!-- http://www.semanticwater.com/WISDOM#RainfallSensor -->

    <owl:Class rdf:about="http://www.semanticwater.com/WISDOM#RainfallSensor">
        <rdfs:subClassOf rdf:resource="http://www.semanticwater.com/WISDOM#WaterSensor"/>
    </owl:Class>
    


    <!-- http://www.semanticwater.com/WISDOM#RawPumpingStation -->

    <owl:Class rdf:about="http://www.semanticwater.com/WISDOM#RawPumpingStation">
        <rdfs:subClassOf rdf:resource="http://www.semanticwater.com/WISDOM#CleanPumpingStation"/>
    </owl:Class>
    


    <!-- http://www.semanticwater.com/WISDOM#SampledFeature -->

    <owl:Class rdf:about="http://www.semanticwater.com/WISDOM#SampledFeature">
        <rdfs:subClassOf rdf:resource="http://purl.oclc.org/NET/ssnx/ssn#FeatureOfInterest"/>
        <alignedWithWatERP>SampledFeature</alignedWithWatERP>
        <rdfs:comment>FeatureOfInerest which can have sensors deployed to make observations regarding its properties</rdfs:comment>
    </owl:Class>
    


    <!-- http://www.semanticwater.com/WISDOM#Screen_LevelSensor -->

    <owl:Class rdf:about="http://www.semanticwater.com/WISDOM#Screen_LevelSensor">
        <rdfs:subClassOf rdf:resource="http://www.semanticwater.com/WISDOM#WaterSensor"/>
    </owl:Class>
    


    <!-- http://www.semanticwater.com/WISDOM#ServiceReservoir -->

    <owl:Class rdf:about="http://www.semanticwater.com/WISDOM#ServiceReservoir">
        <rdfs:subClassOf rdf:resource="http://www.semanticwater.com/WISDOM#StorageAsset"/>
    </owl:Class>
    


    <!-- http://www.semanticwater.com/WISDOM#SewageFitting -->

    <owl:Class rdf:about="http://www.semanticwater.com/WISDOM#SewageFitting">
        <rdfs:subClassOf rdf:resource="http://www.semanticwater.com/WISDOM#Fitting"/>
    </owl:Class>
    


    <!-- http://www.semanticwater.com/WISDOM#SpillSensor -->

    <owl:Class rdf:about="http://www.semanticwater.com/WISDOM#SpillSensor">
        <rdfs:subClassOf rdf:resource="http://www.semanticwater.com/WISDOM#WaterSensor"/>
    </owl:Class>
    


    <!-- http://www.semanticwater.com/WISDOM#StationaryWater -->

    <owl:Class rdf:about="http://www.semanticwater.com/WISDOM#StationaryWater">
        <rdfs:subClassOf rdf:resource="http://www.semanticwater.com/WISDOM#FlowType"/>
    </owl:Class>
    


    <!-- http://www.semanticwater.com/WISDOM#StorageAsset -->

    <owl:Class rdf:about="http://www.semanticwater.com/WISDOM#StorageAsset">
        <owl:equivalentClass rdf:resource="http://www.semanticwater.com/WISDOM#StorageNode"/>
        <rdfs:subClassOf rdf:resource="http://www.semanticwater.com/WISDOM#DesignedAsset"/>
        <alignedWithIFC>IfcFlowStorageDevice</alignedWithIFC>
    </owl:Class>
    


    <!-- http://www.semanticwater.com/WISDOM#StorageNode -->

    <owl:Class rdf:about="http://www.semanticwater.com/WISDOM#StorageNode">
        <rdfs:subClassOf rdf:resource="http://www.semanticwater.com/WISDOM#PhysicalNode"/>
        <alignedWithWatERP>Storage</alignedWithWatERP>
    </owl:Class>
    


    <!-- http://www.semanticwater.com/WISDOM#StormOverflowChamber -->

    <owl:Class rdf:about="http://www.semanticwater.com/WISDOM#StormOverflowChamber">
        <rdfs:subClassOf rdf:resource="http://www.semanticwater.com/WISDOM#WasteChamber"/>
    </owl:Class>
    


    <!-- http://www.semanticwater.com/WISDOM#SurfacePumpingStation -->

    <owl:Class rdf:about="http://www.semanticwater.com/WISDOM#SurfacePumpingStation">
        <rdfs:subClassOf rdf:resource="http://www.semanticwater.com/WISDOM#WastePumpingStation"/>
    </owl:Class>
    


    <!-- http://www.semanticwater.com/WISDOM#SurfaceTreatmentWorks -->

    <owl:Class rdf:about="http://www.semanticwater.com/WISDOM#SurfaceTreatmentWorks">
        <rdfs:subClassOf rdf:resource="http://www.semanticwater.com/WISDOM#TreatmentWorks"/>
    </owl:Class>
    


    <!-- http://www.semanticwater.com/WISDOM#SurfaceWaterChamber -->

    <owl:Class rdf:about="http://www.semanticwater.com/WISDOM#SurfaceWaterChamber">
        <rdfs:subClassOf rdf:resource="http://www.semanticwater.com/WISDOM#WasteChamber"/>
    </owl:Class>
    


    <!-- http://www.semanticwater.com/WISDOM#Tap -->

    <owl:Class rdf:about="http://www.semanticwater.com/WISDOM#Tap">
        <rdfs:subClassOf rdf:resource="http://www.semanticwater.com/WISDOM#ConsumptionAppliance"/>
    </owl:Class>
    


    <!-- http://www.semanticwater.com/WISDOM#TemperatureSensor -->

    <owl:Class rdf:about="http://www.semanticwater.com/WISDOM#TemperatureSensor">
        <rdfs:subClassOf rdf:resource="http://www.semanticwater.com/WISDOM#WaterSensor"/>
    </owl:Class>
    


    <!-- http://www.semanticwater.com/WISDOM#TerminalNode -->

    <owl:Class rdf:about="http://www.semanticwater.com/WISDOM#TerminalNode">
        <rdfs:subClassOf rdf:resource="http://www.semanticwater.com/WISDOM#PhysicalNode"/>
        <alignedWithIFC>IfcFlowTerminal</alignedWithIFC>
    </owl:Class>
    


    <!-- http://www.semanticwater.com/WISDOM#Tidal_guageSensor -->

    <owl:Class rdf:about="http://www.semanticwater.com/WISDOM#Tidal_guageSensor">
        <rdfs:subClassOf rdf:resource="http://www.semanticwater.com/WISDOM#WaterSensor"/>
    </owl:Class>
    


    <!-- http://www.semanticwater.com/WISDOM#TransformationNode -->

    <owl:Class rdf:about="http://www.semanticwater.com/WISDOM#TransformationNode">
        <rdfs:subClassOf rdf:resource="http://www.semanticwater.com/WISDOM#PhysicalNode"/>
        <alignedWithWatERP>Transformation</alignedWithWatERP>
    </owl:Class>
    


    <!-- http://www.semanticwater.com/WISDOM#TreatedEffluentChamber -->

    <owl:Class rdf:about="http://www.semanticwater.com/WISDOM#TreatedEffluentChamber">
        <rdfs:subClassOf rdf:resource="http://www.semanticwater.com/WISDOM#WasteChamber"/>
    </owl:Class>
    


    <!-- http://www.semanticwater.com/WISDOM#TreatmentNode -->

    <owl:Class rdf:about="http://www.semanticwater.com/WISDOM#TreatmentNode">
        <owl:equivalentClass rdf:resource="http://www.semanticwater.com/WISDOM#TreatmentWorks"/>
        <rdfs:subClassOf rdf:resource="http://www.semanticwater.com/WISDOM#TransformationNode"/>
    </owl:Class>
    


    <!-- http://www.semanticwater.com/WISDOM#TreatmentWorks -->

    <owl:Class rdf:about="http://www.semanticwater.com/WISDOM#TreatmentWorks">
        <rdfs:subClassOf rdf:resource="http://www.semanticwater.com/WISDOM#DesignedAsset"/>
        <alignedWithIFC>IfcFlowTreatmentDevice</alignedWithIFC>
    </owl:Class>
    


    <!-- http://www.semanticwater.com/WISDOM#ValveNode -->

    <owl:Class rdf:about="http://www.semanticwater.com/WISDOM#ValveNode">
        <rdfs:subClassOf rdf:resource="http://www.semanticwater.com/WISDOM#PhysicalNode"/>
    </owl:Class>
    


    <!-- http://www.semanticwater.com/WISDOM#ValveOpenness -->

    <owl:Class rdf:about="http://www.semanticwater.com/WISDOM#ValveOpenness">
        <rdfs:subClassOf rdf:resource="http://www.semanticwater.com/WISDOM#WaterNetworkSetpoint"/>
    </owl:Class>
    


    <!-- http://www.semanticwater.com/WISDOM#VelocitySensor -->

    <owl:Class rdf:about="http://www.semanticwater.com/WISDOM#VelocitySensor">
        <rdfs:subClassOf rdf:resource="http://www.semanticwater.com/WISDOM#WaterSensor"/>
    </owl:Class>
    


    <!-- http://www.semanticwater.com/WISDOM#Volume -->

    <owl:Class rdf:about="http://www.semanticwater.com/WISDOM#Volume">
        <rdfs:subClassOf rdf:resource="http://www.semanticwater.com/WISDOM#PhysicalQuantity"/>
        <alignedWithIFC>IfcQuantityVolume</alignedWithIFC>
    </owl:Class>
    


    <!-- http://www.semanticwater.com/WISDOM#WasteChamber -->

    <owl:Class rdf:about="http://www.semanticwater.com/WISDOM#WasteChamber">
        <rdfs:subClassOf rdf:resource="http://www.semanticwater.com/WISDOM#Chamber"/>
    </owl:Class>
    


    <!-- http://www.semanticwater.com/WISDOM#WasteDistributionMain -->

    <owl:Class rdf:about="http://www.semanticwater.com/WISDOM#WasteDistributionMain">
        <rdfs:subClassOf rdf:resource="http://www.semanticwater.com/WISDOM#WastePipe"/>
    </owl:Class>
    


    <!-- http://www.semanticwater.com/WISDOM#WastePipe -->

    <owl:Class rdf:about="http://www.semanticwater.com/WISDOM#WastePipe">
        <rdfs:subClassOf rdf:resource="http://www.semanticwater.com/WISDOM#Main"/>
        <rdfs:subClassOf>
            <owl:Restriction>
                <owl:onProperty rdf:resource="http://www.semanticwater.com/WISDOM#hasMaterial"/>
                <owl:allValuesFrom rdf:resource="http://www.semanticwater.com/WISDOM#Material"/>
            </owl:Restriction>
        </rdfs:subClassOf>
        <rdfs:subClassOf>
            <owl:Restriction>
                <owl:onProperty rdf:resource="http://www.semanticwater.com/WISDOM#hasLength"/>
                <owl:maxQualifiedCardinality rdf:datatype="http://www.w3.org/2001/XMLSchema#nonNegativeInteger">1</owl:maxQualifiedCardinality>
                <owl:onDataRange rdf:resource="http://www.w3.org/2001/XMLSchema#double"/>
            </owl:Restriction>
        </rdfs:subClassOf>
        <alignedWithInspire>SewerPipe</alignedWithInspire>
    </owl:Class>
    


    <!-- http://www.semanticwater.com/WISDOM#WastePumpingStation -->

    <owl:Class rdf:about="http://www.semanticwater.com/WISDOM#WastePumpingStation">
        <rdfs:subClassOf rdf:resource="http://www.semanticwater.com/WISDOM#PumpingStation"/>
    </owl:Class>
    


    <!-- http://www.semanticwater.com/WISDOM#WaterBody -->

    <owl:Class rdf:about="http://www.semanticwater.com/WISDOM#WaterBody">
        <rdfs:subClassOf rdf:resource="http://www.semanticwater.com/WISDOM#NaturalArtifact"/>
        <rdfs:subClassOf rdf:resource="http://www.semanticwater.com/WISDOM#SampledFeature"/>
        <alignedWithWatERP>BodyOfWater</alignedWithWatERP>
    </owl:Class>
    


    <!-- http://www.semanticwater.com/WISDOM#WaterNetworkProperty -->

    <owl:Class rdf:about="http://www.semanticwater.com/WISDOM#WaterNetworkProperty">
        <rdfs:subClassOf rdf:resource="http://purl.oclc.org/NET/ssnx/ssn#Property"/>
    </owl:Class>
    


    <!-- http://www.semanticwater.com/WISDOM#WaterNetworkSetpoint -->

    <owl:Class rdf:about="http://www.semanticwater.com/WISDOM#WaterNetworkSetpoint">
        <rdfs:subClassOf rdf:resource="http://www.semanticwater.com/WISDOM#WaterNetworkProperty"/>
    </owl:Class>
    


    <!-- http://www.semanticwater.com/WISDOM#WaterNetworkStaticProperty -->

    <owl:Class rdf:about="http://www.semanticwater.com/WISDOM#WaterNetworkStaticProperty">
        <rdfs:subClassOf rdf:resource="http://www.semanticwater.com/WISDOM#WaterNetworkProperty"/>
    </owl:Class>
    


    <!-- http://www.semanticwater.com/WISDOM#WaterPipe -->

    <owl:Class rdf:about="http://www.semanticwater.com/WISDOM#WaterPipe">
        <rdfs:subClassOf rdf:resource="http://www.semanticwater.com/WISDOM#Main"/>
        <alignedWithInspire>WaterPipe</alignedWithInspire>
    </owl:Class>
    


    <!-- http://www.semanticwater.com/WISDOM#WaterQualityProperty -->

    <owl:Class rdf:about="http://www.semanticwater.com/WISDOM#WaterQualityProperty">
        <rdfs:subClassOf rdf:resource="http://www.semanticwater.com/WISDOM#WaterNetworkProperty"/>
    </owl:Class>
    


    <!-- http://www.semanticwater.com/WISDOM#WaterSensor -->

    <owl:Class rdf:about="http://www.semanticwater.com/WISDOM#WaterSensor">
        <rdfs:subClassOf rdf:resource="http://purl.oclc.org/NET/ssnx/ssn#Sensor"/>
        <alignedWithIFC>IfcFlowInstrument</alignedWithIFC>
    </owl:Class>
    


    <!-- http://www.semanticwater.com/WISDOM#WaterTower -->

    <owl:Class rdf:about="http://www.semanticwater.com/WISDOM#WaterTower">
        <rdfs:subClassOf rdf:resource="http://www.semanticwater.com/WISDOM#StorageAsset"/>
    </owl:Class>
    


    <!-- http://www.semanticwater.com/WISDOM#WaterType -->

    <owl:Class rdf:about="http://www.semanticwater.com/WISDOM#WaterType">
        <rdfs:subClassOf rdf:resource="http://www.semanticwater.com/WISDOM#WaterNetworkProperty"/>
    </owl:Class>
    


    <!-- http://www.semanticwater.com/WISDOM#WaterVehicle -->

    <owl:Class rdf:about="http://www.semanticwater.com/WISDOM#WaterVehicle">
        <rdfs:subClassOf rdf:resource="http://www.semanticwater.com/WISDOM#PhysicalArc"/>
    </owl:Class>
    


    <!-- http://www.semanticwater.com/WISDOM#Well -->

    <owl:Class rdf:about="http://www.semanticwater.com/WISDOM#Well">
        <rdfs:subClassOf rdf:resource="http://www.semanticwater.com/WISDOM#WaterBody"/>
    </owl:Class>
    


    <!-- http://www.w3.org/2003/01/geo/wgs84_pos#Point -->

    <owl:Class rdf:about="http://www.w3.org/2003/01/geo/wgs84_pos#Point">
        <rdfs:subClassOf rdf:resource="http://www.w3.org/2003/01/geo/wgs84_pos#SpatialThing"/>
        <rdfs:comment>A point, typically described using a coordinate system relative to Earth, such as WGS84.</rdfs:comment>
        <rdfs:comment>Uniquely identified by lat/long/alt. i.e.

spaciallyIntersects(P1, P2) :- lat(P1, LAT), long(P1, LONG), alt(P1, ALT),
  lat(P2, LAT), long(P2, LONG), alt(P2, ALT).

sameThing(P1, P2) :- type(P1, Point), type(P2, Point), spaciallyIntersects(P1, P2).</rdfs:comment>
        <rdfs:label>point</rdfs:label>
    </owl:Class>
    


    <!-- http://www.w3.org/2003/01/geo/wgs84_pos#SpatialThing -->

    <owl:Class rdf:about="http://www.w3.org/2003/01/geo/wgs84_pos#SpatialThing">
        <rdfs:comment xml:lang="en">Anything with spatial extent, i.e. size, shape, or position.
 e.g. people, places, bowling balls, as well as abstract areas like cubes.</rdfs:comment>
        <rdfs:comment xml:lang="es">Cualquier cosa con extensión espacial: tamaño, forma o posición. Por ejemplo: Personas, lugares, bolas de bolos, así como áreas abstractas como cubos.</rdfs:comment>
        <rdfs:label>SpatialThing</rdfs:label>
    </owl:Class>
    


    <!-- http://www.w3.org/ns/locn#Geometry -->

    <rdf:Description rdf:about="http://www.w3.org/ns/locn#Geometry">
        <rdfs:comment xml:lang="es">Pproporciona los medios para identificar una ubicación expresada como un punto, línea, polígono, etc. utilizando coordenadas en algún sistema de referencia de coordenadas.</rdfs:comment>
    </rdf:Description>
    


    <!-- http://www.w3.org/ns/org#FormalOrganization -->

    <rdf:Description rdf:about="http://www.w3.org/ns/org#FormalOrganization">
        <rdfs:subClassOf rdf:resource="http://www.w3.org/ns/org#Organization"/>
    </rdf:Description>
    


    <!-- http://www.w3.org/ns/org#Organization -->

    <rdf:Description rdf:about="http://www.w3.org/ns/org#Organization">
        <rdfs:subClassOf>
            <owl:Restriction>
                <owl:onProperty rdf:resource="http://www.w3.org/ns/org#identifier"/>
                <owl:cardinality rdf:datatype="http://www.w3.org/2001/XMLSchema#nonNegativeInteger">1</owl:cardinality>
            </owl:Restriction>
        </rdfs:subClassOf>
    </rdf:Description>
    


    <!-- http://www.w3.org/ns/org#Role -->

    <rdf:Description rdf:about="http://www.w3.org/ns/org#Role">
        <rdfs:subClassOf>
            <owl:Restriction>
                <owl:onProperty rdf:resource="http://opendata.aragon.es/def/ei2a#roleIdentifier"/>
                <owl:cardinality rdf:datatype="http://www.w3.org/2001/XMLSchema#nonNegativeInteger">1</owl:cardinality>
            </owl:Restriction>
        </rdfs:subClassOf>
        <owl:hasKey rdf:parseType="Collection">
            <rdf:Description rdf:about="http://opendata.aragon.es/def/ei2a#roleIdentifier"/>
        </owl:hasKey>
    </rdf:Description>
    


    <!-- http://www.w3.org/ns/org#Site -->

    <rdf:Description rdf:about="http://www.w3.org/ns/org#Site">
        <owl:hasKey rdf:parseType="Collection">
            <rdf:Description rdf:about="http://opendata.aragon.es/def/ei2a#siteIdentifier"/>
        </owl:hasKey>
    </rdf:Description>
    


    <!-- http://www.w3.org/ns/person#Person -->

    <rdf:Description rdf:about="http://www.w3.org/ns/person#Person">
        <rdfs:subClassOf>
            <owl:Restriction>
                <owl:onProperty rdf:resource="http://opendata.aragon.es/def/ei2a#personIdentifier"/>
                <owl:cardinality rdf:datatype="http://www.w3.org/2001/XMLSchema#nonNegativeInteger">1</owl:cardinality>
            </owl:Restriction>
        </rdfs:subClassOf>
        <owl:hasKey rdf:parseType="Collection">
            <rdf:Description rdf:about="http://opendata.aragon.es/def/ei2a#personIdentifier"/>
        </owl:hasKey>
    </rdf:Description>
    


    <!-- http://xmlns.com/foaf/0.1/Organization -->

    <rdf:Description rdf:about="http://xmlns.com/foaf/0.1/Organization">
        <owl:disjointWith rdf:resource="http://xmlns.com/foaf/0.1/Person"/>
    </rdf:Description>
    


    <!-- http://xmlns.com/foaf/0.1/Person -->

    <rdf:Description rdf:about="http://xmlns.com/foaf/0.1/Person">
        <rdfs:subClassOf rdf:resource="http://xmlns.com/foaf/0.1/Agent"/>
        <owl:hasKey rdf:parseType="Collection">
            <rdf:Description rdf:about="http://www.w3.org/ns/org#identifier"/>
        </owl:hasKey>
    </rdf:Description>
    


    <!-- 
    ///////////////////////////////////////////////////////////////////////////////////////
    //
    // Individuals
    //
    ///////////////////////////////////////////////////////////////////////////////////////
     -->

    


    <!-- http://harmonet.org/harmonise.rdfs#accommodationType -->

    <owl:NamedIndividual rdf:about="http://harmonet.org/harmonise.rdfs#accommodationType"/>
    


    <!-- http://harmonet.org/harmonise.rdfs#award -->

    <owl:NamedIndividual rdf:about="http://harmonet.org/harmonise.rdfs#award"/>
    


    <!-- http://harmonet.org/harmonise.rdfs#awardAchieved -->

    <owl:NamedIndividual rdf:about="http://harmonet.org/harmonise.rdfs#awardAchieved">
        <rdf:type rdf:resource="http://opendata.aragon.es/def/ei2a#DatatypeProperty"/>
    </owl:NamedIndividual>
    


    <!-- http://harmonet.org/harmonise.rdfs#awardingBody -->

    <owl:NamedIndividual rdf:about="http://harmonet.org/harmonise.rdfs#awardingBody">
        <rdf:type rdf:resource="http://opendata.aragon.es/def/ei2a#DatatypeProperty"/>
    </owl:NamedIndividual>
    


    <!-- http://harmonet.org/harmonise.rdfs#facility -->

    <owl:NamedIndividual rdf:about="http://harmonet.org/harmonise.rdfs#facility"/>
    


    <!-- http://harmonet.org/harmonise.rdfs#fieldName -->

    <owl:NamedIndividual rdf:about="http://harmonet.org/harmonise.rdfs#fieldName">
        <rdf:type rdf:resource="http://opendata.aragon.es/def/ei2a#DatatypeProperty"/>
    </owl:NamedIndividual>
    


    <!-- http://harmonet.org/harmonise.rdfs#fieldValue -->

    <owl:NamedIndividual rdf:about="http://harmonet.org/harmonise.rdfs#fieldValue">
        <rdf:type rdf:resource="http://opendata.aragon.es/def/ei2a#DatatypeProperty"/>
    </owl:NamedIndividual>
    


    <!-- http://harmonet.org/harmonise.rdfs#gastroType -->

    <owl:NamedIndividual rdf:about="http://harmonet.org/harmonise.rdfs#gastroType"/>
    


    <!-- http://harmonet.org/harmonise.rdfs#organiser -->

    <owl:NamedIndividual rdf:about="http://harmonet.org/harmonise.rdfs#organiser"/>
    


    <!-- http://harmonet.org/harmonise.rdfs#profile -->

    <owl:NamedIndividual rdf:about="http://harmonet.org/harmonise.rdfs#profile"/>
    


    <!-- http://harmonet.org/harmonise.rdfs#profileField -->

    <owl:NamedIndividual rdf:about="http://harmonet.org/harmonise.rdfs#profileField"/>
    


    <!-- http://harmonet.org/harmonise.rdfs#type -->

    <owl:NamedIndividual rdf:about="http://harmonet.org/harmonise.rdfs#type"/>
    


    <!-- http://opendata.aragon.es/def/ei2a#Administración -->

    <owl:NamedIndividual rdf:about="http://opendata.aragon.es/def/ei2a#Administración">
        <rdf:type rdf:resource="http://opendata.aragon.es/def/ei2a#DocumentOrigin"/>
    </owl:NamedIndividual>
    


    <!-- http://opendata.aragon.es/def/ei2a#AdministraciónAutonómica -->

    <owl:NamedIndividual rdf:about="http://opendata.aragon.es/def/ei2a#AdministraciónAutonómica">
        <rdf:type rdf:resource="http://opendata.aragon.es/def/ei2a#AdministrativeLevel"/>
    </owl:NamedIndividual>
    


    <!-- http://opendata.aragon.es/def/ei2a#AdministraciónDeJusticia -->

    <owl:NamedIndividual rdf:about="http://opendata.aragon.es/def/ei2a#AdministraciónDeJusticia">
        <rdf:type rdf:resource="http://opendata.aragon.es/def/ei2a#AdministrativeLevel"/>
    </owl:NamedIndividual>
    


    <!-- http://opendata.aragon.es/def/ei2a#AdministraciónDelEstado -->

    <owl:NamedIndividual rdf:about="http://opendata.aragon.es/def/ei2a#AdministraciónDelEstado">
        <rdf:type rdf:resource="http://opendata.aragon.es/def/ei2a#AdministrativeLevel"/>
    </owl:NamedIndividual>
    


    <!-- http://opendata.aragon.es/def/ei2a#AdministraciónLocal -->

    <owl:NamedIndividual rdf:about="http://opendata.aragon.es/def/ei2a#AdministraciónLocal">
        <rdf:type rdf:resource="http://opendata.aragon.es/def/ei2a#AdministrativeLevel"/>
    </owl:NamedIndividual>
    


    <!-- http://opendata.aragon.es/def/ei2a#AgenciaEstatal -->

    <owl:NamedIndividual rdf:about="http://opendata.aragon.es/def/ei2a#AgenciaEstatal">
        <rdf:type rdf:resource="http://opendata.aragon.es/def/ei2a#PublicEntityType"/>
    </owl:NamedIndividual>
    


    <!-- http://opendata.aragon.es/def/ei2a#Agregación -->

    <owl:NamedIndividual rdf:about="http://opendata.aragon.es/def/ei2a#Agregación">
        <rdf:type rdf:resource="http://opendata.aragon.es/def/ei2a#DocumentCategory"/>
    </owl:NamedIndividual>
    


    <!-- http://opendata.aragon.es/def/ei2a#AgrupaciónSecretarial -->

    <owl:NamedIndividual rdf:about="http://opendata.aragon.es/def/ei2a#AgrupaciónSecretarial">
        <rdf:type rdf:resource="http://opendata.aragon.es/def/ei2a#PublicEntityType"/>
    </owl:NamedIndividual>
    


    <!-- http://opendata.aragon.es/def/ei2a#Alto -->

    <owl:NamedIndividual rdf:about="http://opendata.aragon.es/def/ei2a#Alto">
        <rdf:type rdf:resource="http://opendata.aragon.es/def/ei2a#LOPDLevel"/>
    </owl:NamedIndividual>
    


    <!-- http://opendata.aragon.es/def/ei2a#Anulado -->

    <owl:NamedIndividual rdf:about="http://opendata.aragon.es/def/ei2a#Anulado">
        <rdf:type rdf:resource="http://opendata.aragon.es/def/ei2a#DocumentStatus"/>
        <rdf:type rdf:resource="http://opendata.aragon.es/def/ei2a#FunctionalOrganizationStatus"/>
    </owl:NamedIndividual>
    


    <!-- http://opendata.aragon.es/def/ei2a#Auxiliar -->

    <owl:NamedIndividual rdf:about="http://opendata.aragon.es/def/ei2a#Auxiliar">
        <rdf:type rdf:resource="http://opendata.aragon.es/def/ei2a#PublicEntityType"/>
    </owl:NamedIndividual>
    


    <!-- http://opendata.aragon.es/def/ei2a#Ayuntamiento -->

    <owl:NamedIndividual rdf:about="http://opendata.aragon.es/def/ei2a#Ayuntamiento">
        <rdf:type rdf:resource="http://opendata.aragon.es/def/ei2a#PublicEntityType"/>
    </owl:NamedIndividual>
    


    <!-- http://opendata.aragon.es/def/ei2a#Borrador -->

    <owl:NamedIndividual rdf:about="http://opendata.aragon.es/def/ei2a#Borrador">
        <rdf:type rdf:resource="http://opendata.aragon.es/def/ei2a#DocumentStatus"/>
    </owl:NamedIndividual>
    


    <!-- http://opendata.aragon.es/def/ei2a#Básico -->

    <owl:NamedIndividual rdf:about="http://opendata.aragon.es/def/ei2a#Básico">
        <rdf:type rdf:resource="http://opendata.aragon.es/def/ei2a#LOPDLevel"/>
    </owl:NamedIndividual>
    


    <!-- http://opendata.aragon.es/def/ei2a#Cabildo -->

    <owl:NamedIndividual rdf:about="http://opendata.aragon.es/def/ei2a#Cabildo">
        <rdf:type rdf:resource="http://opendata.aragon.es/def/ei2a#PublicEntityType"/>
    </owl:NamedIndividual>
    


    <!-- http://opendata.aragon.es/def/ei2a#CentroEducativo -->

    <owl:NamedIndividual rdf:about="http://opendata.aragon.es/def/ei2a#CentroEducativo">
        <rdf:type rdf:resource="http://opendata.aragon.es/def/ei2a#PublicEntityType"/>
    </owl:NamedIndividual>
    


    <!-- http://opendata.aragon.es/def/ei2a#Ciudadano -->

    <owl:NamedIndividual rdf:about="http://opendata.aragon.es/def/ei2a#Ciudadano">
        <rdf:type rdf:resource="http://opendata.aragon.es/def/ei2a#DocumentOrigin"/>
    </owl:NamedIndividual>
    


    <!-- http://opendata.aragon.es/def/ei2a#ColegioProfesional -->

    <owl:NamedIndividual rdf:about="http://opendata.aragon.es/def/ei2a#ColegioProfesional">
        <rdf:type rdf:resource="http://opendata.aragon.es/def/ei2a#PublicEntityType"/>
    </owl:NamedIndividual>
    


    <!-- http://opendata.aragon.es/def/ei2a#Comarca -->

    <owl:NamedIndividual rdf:about="http://opendata.aragon.es/def/ei2a#Comarca">
        <rdf:type rdf:resource="http://opendata.aragon.es/def/ei2a#PublicEntityType"/>
    </owl:NamedIndividual>
    


    <!-- http://opendata.aragon.es/def/ei2a#ComunidadAutónoma -->

    <owl:NamedIndividual rdf:about="http://opendata.aragon.es/def/ei2a#ComunidadAutónoma">
        <rdf:type rdf:resource="http://opendata.aragon.es/def/ei2a#PublicEntityType"/>
    </owl:NamedIndividual>
    


    <!-- http://opendata.aragon.es/def/ei2a#Copia -->

    <owl:NamedIndividual rdf:about="http://opendata.aragon.es/def/ei2a#Copia">
        <rdf:type rdf:resource="http://opendata.aragon.es/def/ei2a#DocumentStatus"/>
    </owl:NamedIndividual>
    


    <!-- http://opendata.aragon.es/def/ei2a#Cámara -->

    <owl:NamedIndividual rdf:about="http://opendata.aragon.es/def/ei2a#Cámara">
        <rdf:type rdf:resource="http://opendata.aragon.es/def/ei2a#PublicEntityType"/>
    </owl:NamedIndividual>
    


    <!-- http://opendata.aragon.es/def/ei2a#DiputaciónProvincialForal -->

    <owl:NamedIndividual rdf:about="http://opendata.aragon.es/def/ei2a#DiputaciónProvincialForal">
        <rdf:type rdf:resource="http://opendata.aragon.es/def/ei2a#PublicEntityType"/>
    </owl:NamedIndividual>
    


    <!-- http://opendata.aragon.es/def/ei2a#DocumentoSimple -->

    <owl:NamedIndividual rdf:about="http://opendata.aragon.es/def/ei2a#DocumentoSimple">
        <rdf:type rdf:resource="http://opendata.aragon.es/def/ei2a#DocumentCategory"/>
    </owl:NamedIndividual>
    


    <!-- http://opendata.aragon.es/def/ei2a#ETRS89 -->

    <owl:NamedIndividual rdf:about="http://opendata.aragon.es/def/ei2a#ETRS89">
        <rdf:type rdf:resource="http://opendata.aragon.es/def/ei2a#ReferenceSystem"/>
    </owl:NamedIndividual>
    


    <!-- http://opendata.aragon.es/def/ei2a#EntidadDerechoPúblico -->

    <owl:NamedIndividual rdf:about="http://opendata.aragon.es/def/ei2a#EntidadDerechoPúblico">
        <rdf:type rdf:resource="http://opendata.aragon.es/def/ei2a#PublicEntityType"/>
    </owl:NamedIndividual>
    


    <!-- http://opendata.aragon.es/def/ei2a#EntidadLocalMenor -->

    <owl:NamedIndividual rdf:about="http://opendata.aragon.es/def/ei2a#EntidadLocalMenor">
        <rdf:type rdf:resource="http://opendata.aragon.es/def/ei2a#PublicEntityType"/>
    </owl:NamedIndividual>
    


    <!-- http://opendata.aragon.es/def/ei2a#EntidadPúblicaEmpresarial -->

    <owl:NamedIndividual rdf:about="http://opendata.aragon.es/def/ei2a#EntidadPúblicaEmpresarial">
        <rdf:type rdf:resource="http://opendata.aragon.es/def/ei2a#PublicEntityType"/>
    </owl:NamedIndividual>
    


    <!-- http://opendata.aragon.es/def/ei2a#Expediente -->

    <owl:NamedIndividual rdf:about="http://opendata.aragon.es/def/ei2a#Expediente">
        <rdf:type rdf:resource="http://opendata.aragon.es/def/ei2a#DocumentCategory"/>
    </owl:NamedIndividual>
    


    <!-- http://opendata.aragon.es/def/ei2a#Extinguido -->

    <owl:NamedIndividual rdf:about="http://opendata.aragon.es/def/ei2a#Extinguido">
        <rdf:type rdf:resource="http://opendata.aragon.es/def/ei2a#FunctionalOrganizationStatus"/>
    </owl:NamedIndividual>
    


    <!-- http://opendata.aragon.es/def/ei2a#Femenino -->

    <owl:NamedIndividual rdf:about="http://opendata.aragon.es/def/ei2a#Femenino">
        <rdf:type rdf:resource="http://opendata.aragon.es/def/ei2a#PersonGender"/>
    </owl:NamedIndividual>
    


    <!-- http://opendata.aragon.es/def/ei2a#Fondo -->

    <owl:NamedIndividual rdf:about="http://opendata.aragon.es/def/ei2a#Fondo">
        <rdf:type rdf:resource="http://opendata.aragon.es/def/ei2a#DocumentCategory"/>
    </owl:NamedIndividual>
    


    <!-- http://opendata.aragon.es/def/ei2a#FundaciónEstatal -->

    <owl:NamedIndividual rdf:about="http://opendata.aragon.es/def/ei2a#FundaciónEstatal">
        <rdf:type rdf:resource="http://opendata.aragon.es/def/ei2a#PublicEntityType"/>
    </owl:NamedIndividual>
    


    <!-- http://opendata.aragon.es/def/ei2a#General -->

    <owl:NamedIndividual rdf:about="http://opendata.aragon.es/def/ei2a#General">
        <rdf:type rdf:resource="http://opendata.aragon.es/def/ei2a#PublicEntityType"/>
    </owl:NamedIndividual>
    


    <!-- http://opendata.aragon.es/def/ei2a#GrupoDeFondos -->

    <owl:NamedIndividual rdf:about="http://opendata.aragon.es/def/ei2a#GrupoDeFondos">
        <rdf:type rdf:resource="http://opendata.aragon.es/def/ei2a#DocumentCategory"/>
    </owl:NamedIndividual>
    


    <!-- http://opendata.aragon.es/def/ei2a#Mancomunidad -->

    <owl:NamedIndividual rdf:about="http://opendata.aragon.es/def/ei2a#Mancomunidad">
        <rdf:type rdf:resource="http://opendata.aragon.es/def/ei2a#PublicEntityType"/>
    </owl:NamedIndividual>
    


    <!-- http://opendata.aragon.es/def/ei2a#Masculino -->

    <owl:NamedIndividual rdf:about="http://opendata.aragon.es/def/ei2a#Masculino">
        <rdf:type rdf:resource="http://opendata.aragon.es/def/ei2a#PersonGender"/>
    </owl:NamedIndividual>
    


    <!-- http://opendata.aragon.es/def/ei2a#Medio -->

    <owl:NamedIndividual rdf:about="http://opendata.aragon.es/def/ei2a#Medio">
        <rdf:type rdf:resource="http://opendata.aragon.es/def/ei2a#LOPDLevel"/>
    </owl:NamedIndividual>
    


    <!-- http://opendata.aragon.es/def/ei2a#Ministerio -->

    <owl:NamedIndividual rdf:about="http://opendata.aragon.es/def/ei2a#Ministerio">
        <rdf:type rdf:resource="http://opendata.aragon.es/def/ei2a#PublicEntityType"/>
    </owl:NamedIndividual>
    


    <!-- http://opendata.aragon.es/def/ei2a#OficinaDeTurismoYPuntoDeInformación -->

    <owl:NamedIndividual rdf:about="http://opendata.aragon.es/def/ei2a#OficinaDeTurismoYPuntoDeInformación">
        <rdf:type rdf:resource="http://opendata.aragon.es/def/ei2a#PublicEntityType"/>
    </owl:NamedIndividual>
    


    <!-- http://opendata.aragon.es/def/ei2a#OrganismoAutónomo -->

    <owl:NamedIndividual rdf:about="http://opendata.aragon.es/def/ei2a#OrganismoAutónomo">
        <rdf:type rdf:resource="http://opendata.aragon.es/def/ei2a#PublicEntityType"/>
    </owl:NamedIndividual>
    


    <!-- http://opendata.aragon.es/def/ei2a#Original -->

    <owl:NamedIndividual rdf:about="http://opendata.aragon.es/def/ei2a#Original">
        <rdf:type rdf:resource="http://opendata.aragon.es/def/ei2a#DocumentStatus"/>
    </owl:NamedIndividual>
    


    <!-- http://opendata.aragon.es/def/ei2a#OtrasInstituciones -->

    <owl:NamedIndividual rdf:about="http://opendata.aragon.es/def/ei2a#OtrasInstituciones">
        <rdf:type rdf:resource="http://opendata.aragon.es/def/ei2a#AdministrativeLevel"/>
    </owl:NamedIndividual>
    


    <!-- http://opendata.aragon.es/def/ei2a#PendienteDeFirma -->

    <owl:NamedIndividual rdf:about="http://opendata.aragon.es/def/ei2a#PendienteDeFirma">
        <rdf:type rdf:resource="http://opendata.aragon.es/def/ei2a#DocumentStatus"/>
    </owl:NamedIndividual>
    


    <!-- http://opendata.aragon.es/def/ei2a#Raster -->

    <owl:NamedIndividual rdf:about="http://opendata.aragon.es/def/ei2a#Raster">
        <rdf:type rdf:resource="http://opendata.aragon.es/def/ei2a#TypeGeometryModel"/>
    </owl:NamedIndividual>
    


    <!-- http://opendata.aragon.es/def/ei2a#Rural -->

    <owl:NamedIndividual rdf:about="http://opendata.aragon.es/def/ei2a#Rural">
        <rdf:type rdf:resource="http://opendata.aragon.es/def/ei2a#PropertyType"/>
    </owl:NamedIndividual>
    


    <!-- http://opendata.aragon.es/def/ei2a#SIGPAC -->

    <owl:NamedIndividual rdf:about="http://opendata.aragon.es/def/ei2a#SIGPAC">
        <rdf:type rdf:resource="http://opendata.aragon.es/def/ei2a#RuralParcelOrigin"/>
    </owl:NamedIndividual>
    


    <!-- http://opendata.aragon.es/def/ei2a#Serie -->

    <owl:NamedIndividual rdf:about="http://opendata.aragon.es/def/ei2a#Serie">
        <rdf:type rdf:resource="http://opendata.aragon.es/def/ei2a#DocumentCategory"/>
    </owl:NamedIndividual>
    


    <!-- http://opendata.aragon.es/def/ei2a#SinClasificar -->

    <owl:NamedIndividual rdf:about="http://opendata.aragon.es/def/ei2a#SinClasificar">
        <rdf:type rdf:resource="http://opendata.aragon.es/def/ei2a#PublicEntityType"/>
    </owl:NamedIndividual>
    


    <!-- http://opendata.aragon.es/def/ei2a#Transitorio -->

    <owl:NamedIndividual rdf:about="http://opendata.aragon.es/def/ei2a#Transitorio">
        <rdf:type rdf:resource="http://opendata.aragon.es/def/ei2a#FunctionalOrganizationStatus"/>
    </owl:NamedIndividual>
    


    <!-- http://opendata.aragon.es/def/ei2a#Universidad -->

    <owl:NamedIndividual rdf:about="http://opendata.aragon.es/def/ei2a#Universidad">
        <rdf:type rdf:resource="http://opendata.aragon.es/def/ei2a#PublicEntityType"/>
    </owl:NamedIndividual>
    


    <!-- http://opendata.aragon.es/def/ei2a#Universidades -->

    <owl:NamedIndividual rdf:about="http://opendata.aragon.es/def/ei2a#Universidades">
        <rdf:type rdf:resource="http://opendata.aragon.es/def/ei2a#AdministrativeLevel"/>
    </owl:NamedIndividual>
    


    <!-- http://opendata.aragon.es/def/ei2a#Urbana -->

    <owl:NamedIndividual rdf:about="http://opendata.aragon.es/def/ei2a#Urbana">
        <rdf:type rdf:resource="http://opendata.aragon.es/def/ei2a#PropertyType"/>
    </owl:NamedIndividual>
    


    <!-- http://opendata.aragon.es/def/ei2a#Vectorial -->

    <owl:NamedIndividual rdf:about="http://opendata.aragon.es/def/ei2a#Vectorial">
        <rdf:type rdf:resource="http://opendata.aragon.es/def/ei2a#TypeGeometryModel"/>
    </owl:NamedIndividual>
    


    <!-- http://opendata.aragon.es/def/ei2a#Vigente -->

    <owl:NamedIndividual rdf:about="http://opendata.aragon.es/def/ei2a#Vigente">
        <rdf:type rdf:resource="http://opendata.aragon.es/def/ei2a#FunctionalOrganizationStatus"/>
    </owl:NamedIndividual>
    


    <!-- http://opendata.aragon.es/def/ei2a#WGS84 -->

    <owl:NamedIndividual rdf:about="http://opendata.aragon.es/def/ei2a#WGS84">
        <rdf:type rdf:resource="http://opendata.aragon.es/def/ei2a#ReferenceSystem"/>
    </owl:NamedIndividual>
    


    <!-- http://opendata.aragon.es/def/ei2a#cadastral -->

    <owl:NamedIndividual rdf:about="http://opendata.aragon.es/def/ei2a#cadastral">
        <rdf:type rdf:resource="http://opendata.aragon.es/def/ei2a#RuralParcelOrigin"/>
    </owl:NamedIndividual>
    


    <!-- http://opendata.aragon.es/def/ei2a#close -->

    <owl:NamedIndividual rdf:about="http://opendata.aragon.es/def/ei2a#close">
        <rdf:type rdf:resource="http://opendata.aragon.es/def/ei2a#AdministrativeRecordStatus"/>
    </owl:NamedIndividual>
    


    <!-- http://opendata.aragon.es/def/ei2a#diariodelaltoaragon -->

    <owl:NamedIndividual rdf:about="http://opendata.aragon.es/def/ei2a#diariodelaltoaragon">
        <rdf:type rdf:resource="http://opendata.aragon.es/def/ei2a#SocialMediaSources"/>
    </owl:NamedIndividual>
    


    <!-- http://opendata.aragon.es/def/ei2a#diariodeteruel -->

    <owl:NamedIndividual rdf:about="http://opendata.aragon.es/def/ei2a#diariodeteruel">
        <rdf:type rdf:resource="http://opendata.aragon.es/def/ei2a#SocialMediaSources"/>
    </owl:NamedIndividual>
    


    <!-- http://opendata.aragon.es/def/ei2a#empresa -->

    <owl:NamedIndividual rdf:about="http://opendata.aragon.es/def/ei2a#empresa">
        <rdf:type rdf:resource="http://opendata.aragon.es/def/ei2a#OrganizationType"/>
    </owl:NamedIndividual>
    


    <!-- http://opendata.aragon.es/def/ei2a#escuela -->

    <owl:NamedIndividual rdf:about="http://opendata.aragon.es/def/ei2a#escuela">
        <rdf:type rdf:resource="http://opendata.aragon.es/def/ei2a#OrganizationType"/>
    </owl:NamedIndividual>
    


    <!-- http://opendata.aragon.es/def/ei2a#facebook -->

    <owl:NamedIndividual rdf:about="http://opendata.aragon.es/def/ei2a#facebook">
        <rdf:type rdf:resource="http://opendata.aragon.es/def/ei2a#SocialMediaSources"/>
    </owl:NamedIndividual>
    


    <!-- http://opendata.aragon.es/def/ei2a#facebook_geoposts -->

    <owl:NamedIndividual rdf:about="http://opendata.aragon.es/def/ei2a#facebook_geoposts">
        <rdf:type rdf:resource="http://opendata.aragon.es/def/ei2a#SocialMediaSources"/>
    </owl:NamedIndividual>
    


    <!-- http://opendata.aragon.es/def/ei2a#flickr -->

    <owl:NamedIndividual rdf:about="http://opendata.aragon.es/def/ei2a#flickr">
        <rdf:type rdf:resource="http://opendata.aragon.es/def/ei2a#SocialMediaSources"/>
    </owl:NamedIndividual>
    


    <!-- http://opendata.aragon.es/def/ei2a#fundación -->

    <owl:NamedIndividual rdf:about="http://opendata.aragon.es/def/ei2a#fundación">
        <rdf:type rdf:resource="http://opendata.aragon.es/def/ei2a#OrganizationType"/>
    </owl:NamedIndividual>
    


    <!-- http://opendata.aragon.es/def/ei2a#heraldodearagon -->

    <owl:NamedIndividual rdf:about="http://opendata.aragon.es/def/ei2a#heraldodearagon">
        <rdf:type rdf:resource="http://opendata.aragon.es/def/ei2a#SocialMediaSources"/>
    </owl:NamedIndividual>
    


    <!-- http://opendata.aragon.es/def/ei2a#indexForClosedRemission -->

    <owl:NamedIndividual rdf:about="http://opendata.aragon.es/def/ei2a#indexForClosedRemission">
        <rdf:type rdf:resource="http://opendata.aragon.es/def/ei2a#AdministrativeRecordStatus"/>
    </owl:NamedIndividual>
    


    <!-- http://opendata.aragon.es/def/ei2a#instagram -->

    <owl:NamedIndividual rdf:about="http://opendata.aragon.es/def/ei2a#instagram">
        <rdf:type rdf:resource="http://opendata.aragon.es/def/ei2a#SocialMediaSources"/>
    </owl:NamedIndividual>
    


    <!-- http://opendata.aragon.es/def/ei2a#oficinaDeTurismo -->

    <owl:NamedIndividual rdf:about="http://opendata.aragon.es/def/ei2a#oficinaDeTurismo">
        <rdf:type rdf:resource="http://opendata.aragon.es/def/ei2a#OrganizationType"/>
    </owl:NamedIndividual>
    


    <!-- http://opendata.aragon.es/def/ei2a#open -->

    <owl:NamedIndividual rdf:about="http://opendata.aragon.es/def/ei2a#open">
        <rdf:type rdf:resource="http://opendata.aragon.es/def/ei2a#AdministrativeRecordStatus"/>
    </owl:NamedIndividual>
    


    <!-- http://opendata.aragon.es/def/ei2a#periodicodearagon -->

    <owl:NamedIndividual rdf:about="http://opendata.aragon.es/def/ei2a#periodicodearagon">
        <rdf:type rdf:resource="http://opendata.aragon.es/def/ei2a#SocialMediaSources"/>
    </owl:NamedIndividual>
    


    <!-- http://opendata.aragon.es/def/ei2a#puntoDeInformación -->

    <owl:NamedIndividual rdf:about="http://opendata.aragon.es/def/ei2a#puntoDeInformación">
        <rdf:type rdf:resource="http://opendata.aragon.es/def/ei2a#OrganizationType"/>
    </owl:NamedIndividual>
    


    <!-- http://opendata.aragon.es/def/ei2a#twitter -->

    <owl:NamedIndividual rdf:about="http://opendata.aragon.es/def/ei2a#twitter">
        <rdf:type rdf:resource="http://opendata.aragon.es/def/ei2a#SocialMediaSources"/>
    </owl:NamedIndividual>
    


    <!-- http://opendata.aragon.es/def/ei2a#wikipedia -->

    <owl:NamedIndividual rdf:about="http://opendata.aragon.es/def/ei2a#wikipedia">
        <rdf:type rdf:resource="http://opendata.aragon.es/def/ei2a#SocialMediaSources"/>
    </owl:NamedIndividual>
    


    <!-- http://opendata.aragon.es/def/ei2a#youtube -->

    <owl:NamedIndividual rdf:about="http://opendata.aragon.es/def/ei2a#youtube">
        <rdf:type rdf:resource="http://opendata.aragon.es/def/ei2a#SocialMediaSources"/>
    </owl:NamedIndividual>
    


    <!-- http://opendata.aragon.es/def/ei2a#órganoAdministrativo -->

    <owl:NamedIndividual rdf:about="http://opendata.aragon.es/def/ei2a#órganoAdministrativo">
        <rdf:type rdf:resource="http://opendata.aragon.es/def/ei2a#OrganizationType"/>
    </owl:NamedIndividual>
    


    <!-- http://vocab.gtfs.org/terms#Bus -->

    <owl:NamedIndividual rdf:about="http://vocab.gtfs.org/terms#Bus">
        <rdf:type rdf:resource="http://vocab.gtfs.org/terms#RouteType"/>
        <rdfs:comment xml:lang="en">Used for short- and long-distance bus routes.</rdfs:comment>
        <rdfs:comment xml:lang="es">Utilizado para rutas en autobús de corta y larga distancia.</rdfs:comment>
        <rdfs:label xml:lang="es">Autobús</rdfs:label>
        <rdfs:label xml:lang="en">Bus</rdfs:label>
        <status:term_status xml:lang="es">inestable</status:term_status>
        <status:term_status xml:lang="en">unstable</status:term_status>
    </owl:NamedIndividual>
    


    <!-- http://vocab.gtfs.org/terms#CableCar -->

    <owl:NamedIndividual rdf:about="http://vocab.gtfs.org/terms#CableCar">
        <rdf:type rdf:resource="http://vocab.gtfs.org/terms#RouteType"/>
        <rdfs:comment xml:lang="en">Used for street-level cable cars where the cable runs beneath the car.</rdfs:comment>
        <rdfs:comment xml:lang="es">Utilizado para funiculares en superficie en donde el cable pasa por debajo del vehículo.</rdfs:comment>
        <rdfs:label xml:lang="en">Cable car</rdfs:label>
        <rdfs:label xml:lang="es">Funicular</rdfs:label>
        <status:term_status xml:lang="es">inestable</status:term_status>
        <status:term_status xml:lang="en">unstable</status:term_status>
    </owl:NamedIndividual>
    


    <!-- http://vocab.gtfs.org/terms#Ferry -->

    <owl:NamedIndividual rdf:about="http://vocab.gtfs.org/terms#Ferry">
        <rdf:type rdf:resource="http://vocab.gtfs.org/terms#RouteType"/>
        <rdfs:comment xml:lang="en">Used for short- and long-distance boat service.</rdfs:comment>
        <rdfs:comment xml:lang="es">Utilizado para servicio de transporte público fluvial o marítimo de corta y larga distancia.</rdfs:comment>
        <rdfs:label xml:lang="en">Ferry</rdfs:label>
        <rdfs:label xml:lang="es">Ferry, transbordador</rdfs:label>
        <status:term_status xml:lang="es">inestable</status:term_status>
        <status:term_status xml:lang="en">unstable</status:term_status>
    </owl:NamedIndividual>
    


    <!-- http://vocab.gtfs.org/terms#Funicular -->

    <owl:NamedIndividual rdf:about="http://vocab.gtfs.org/terms#Funicular">
        <rdf:type rdf:resource="http://vocab.gtfs.org/terms#RouteType"/>
        <rdfs:comment xml:lang="en">Any rail system designed for steep inclines.</rdfs:comment>
        <rdfs:comment xml:lang="es">Cualquier sistema por raíl diseñado para recorridos con una gran inclinación.</rdfs:comment>
        <rdfs:label xml:lang="en">Funicular</rdfs:label>
        <rdfs:label xml:lang="es">Funicular</rdfs:label>
        <status:term_status xml:lang="es">inestable</status:term_status>
        <status:term_status xml:lang="en">unstable</status:term_status>
    </owl:NamedIndividual>
    


    <!-- http://vocab.gtfs.org/terms#Gondola -->

    <owl:NamedIndividual rdf:about="http://vocab.gtfs.org/terms#Gondola">
        <rdf:type rdf:resource="http://vocab.gtfs.org/terms#RouteType"/>
        <rdfs:comment xml:lang="en">Gondola, Suspended cable car. Typically used for aerial cable cars where the car is suspended from the cable.</rdfs:comment>
        <rdfs:comment xml:lang="es">Normalmente se utiliza para medios de transporte público por cable en donde el vehículo queda suspendido de un cable.</rdfs:comment>
        <rdfs:label xml:lang="en">Gondola, Suspended cable car</rdfs:label>
        <rdfs:label xml:lang="es">Teleférico, telecabina</rdfs:label>
        <status:term_status xml:lang="es">inestable</status:term_status>
        <status:term_status xml:lang="en">unstable</status:term_status>
    </owl:NamedIndividual>
    


    <!-- http://vocab.gtfs.org/terms#LightRail -->

    <owl:NamedIndividual rdf:about="http://vocab.gtfs.org/terms#LightRail">
        <rdf:type rdf:resource="http://vocab.gtfs.org/terms#RouteType"/>
        <rdfs:comment xml:lang="en">Any light rail or street level system within a metropolitan area.</rdfs:comment>
        <rdfs:comment xml:lang="es">Cualquier metro ligero o sistema ferroviario en superficie dentro de un área metropolitana.</rdfs:comment>
        <rdfs:label xml:lang="en">Tram, Streetcar, Light rail</rdfs:label>
        <rdfs:label xml:lang="es">Tranvía, metro ligero</rdfs:label>
        <status:term_status xml:lang="es">inestable</status:term_status>
        <status:term_status xml:lang="en">unstable</status:term_status>
    </owl:NamedIndividual>
    


    <!-- http://vocab.gtfs.org/terms#Rail -->

    <owl:NamedIndividual rdf:about="http://vocab.gtfs.org/terms#Rail">
        <rdf:type rdf:resource="http://vocab.gtfs.org/terms#RouteType"/>
        <rdfs:comment xml:lang="en">Used for intercity or long-distance travel.</rdfs:comment>
        <rdfs:comment xml:lang="es">Utilizado para viajes de cercanías, interurbanos o de larga distancia.</rdfs:comment>
        <rdfs:label xml:lang="en">Rail</rdfs:label>
        <rdfs:label xml:lang="es">Tren</rdfs:label>
        <status:term_status xml:lang="es">inestable</status:term_status>
        <status:term_status xml:lang="en">unstable</status:term_status>
    </owl:NamedIndividual>
    


    <!-- http://vocab.gtfs.org/terms#Subway -->

    <owl:NamedIndividual rdf:about="http://vocab.gtfs.org/terms#Subway">
        <rdf:type rdf:resource="http://vocab.gtfs.org/terms#RouteType"/>
        <rdfs:comment xml:lang="en">Any underground rail system within a metropolitan area.</rdfs:comment>
        <rdfs:comment xml:lang="es">Cualquier sistema ferroviario subterráneo dentro de un área metropolitana.</rdfs:comment>
        <rdfs:label xml:lang="es">Subterráneo, metro</rdfs:label>
        <rdfs:label xml:lang="en">Subway, Metro</rdfs:label>
        <status:term_status xml:lang="es">inestable</status:term_status>
        <status:term_status xml:lang="en">unstable</status:term_status>
    </owl:NamedIndividual>
    


    <!-- http://www.semanticwater.com/WISDOM#CombinedWasteWater -->

    <owl:NamedIndividual rdf:about="http://www.semanticwater.com/WISDOM#CombinedWasteWater">
        <rdf:type rdf:resource="http://www.semanticwater.com/WISDOM#WaterType"/>
    </owl:NamedIndividual>
    


    <!-- http://www.semanticwater.com/WISDOM#FlowRateProperty -->

    <owl:NamedIndividual rdf:about="http://www.semanticwater.com/WISDOM#FlowRateProperty">
        <rdf:type rdf:resource="http://www.semanticwater.com/WISDOM#FluidDynamicsProperty"/>
    </owl:NamedIndividual>
    


    <!-- http://www.semanticwater.com/WISDOM#FoulWasteWater -->

    <owl:NamedIndividual rdf:about="http://www.semanticwater.com/WISDOM#FoulWasteWater">
        <rdf:type rdf:resource="http://www.semanticwater.com/WISDOM#WaterType"/>
    </owl:NamedIndividual>
    


    <!-- http://www.semanticwater.com/WISDOM#LevelProperty -->

    <owl:NamedIndividual rdf:about="http://www.semanticwater.com/WISDOM#LevelProperty">
        <rdf:type rdf:resource="http://www.semanticwater.com/WISDOM#FluidDynamicsProperty"/>
    </owl:NamedIndividual>
    


    <!-- http://www.semanticwater.com/WISDOM#LevelProperty_Percentage -->

    <owl:NamedIndividual rdf:about="http://www.semanticwater.com/WISDOM#LevelProperty_Percentage">
        <rdf:type rdf:resource="http://www.semanticwater.com/WISDOM#FluidDynamicsProperty"/>
    </owl:NamedIndividual>
    


    <!-- http://www.semanticwater.com/WISDOM#LevelProperty_Screen -->

    <owl:NamedIndividual rdf:about="http://www.semanticwater.com/WISDOM#LevelProperty_Screen">
        <rdf:type rdf:resource="http://www.semanticwater.com/WISDOM#FluidDynamicsProperty"/>
    </owl:NamedIndividual>
    


    <!-- http://www.semanticwater.com/WISDOM#LevelProperty_Tidal -->

    <owl:NamedIndividual rdf:about="http://www.semanticwater.com/WISDOM#LevelProperty_Tidal">
        <rdf:type rdf:resource="http://www.semanticwater.com/WISDOM#FluidDynamicsProperty"/>
    </owl:NamedIndividual>
    


    <!-- http://www.semanticwater.com/WISDOM#MDPE -->

    <owl:NamedIndividual rdf:about="http://www.semanticwater.com/WISDOM#MDPE">
        <rdf:type rdf:resource="http://www.semanticwater.com/WISDOM#Material"/>
    </owl:NamedIndividual>
    


    <!-- http://www.semanticwater.com/WISDOM#PotableWater -->

    <owl:NamedIndividual rdf:about="http://www.semanticwater.com/WISDOM#PotableWater">
        <rdf:type rdf:resource="http://www.semanticwater.com/WISDOM#WaterType"/>
    </owl:NamedIndividual>
    


    <!-- http://www.semanticwater.com/WISDOM#PressureProperty -->

    <owl:NamedIndividual rdf:about="http://www.semanticwater.com/WISDOM#PressureProperty">
        <rdf:type rdf:resource="http://www.semanticwater.com/WISDOM#FluidDynamicsProperty"/>
    </owl:NamedIndividual>
    


    <!-- http://www.semanticwater.com/WISDOM#PureWater -->

    <owl:NamedIndividual rdf:about="http://www.semanticwater.com/WISDOM#PureWater">
        <rdf:type rdf:resource="http://www.semanticwater.com/WISDOM#WaterType"/>
    </owl:NamedIndividual>
    


    <!-- http://www.semanticwater.com/WISDOM#RainfallProperty -->

    <owl:NamedIndividual rdf:about="http://www.semanticwater.com/WISDOM#RainfallProperty">
        <rdf:type rdf:resource="http://www.semanticwater.com/WISDOM#FluidDynamicsProperty"/>
    </owl:NamedIndividual>
    


    <!-- http://www.semanticwater.com/WISDOM#RawWater -->

    <owl:NamedIndividual rdf:about="http://www.semanticwater.com/WISDOM#RawWater">
        <rdf:type rdf:resource="http://www.semanticwater.com/WISDOM#WaterType"/>
    </owl:NamedIndividual>
    


    <!-- http://www.semanticwater.com/WISDOM#SpillProperty -->

    <owl:NamedIndividual rdf:about="http://www.semanticwater.com/WISDOM#SpillProperty">
        <rdf:type rdf:resource="http://www.semanticwater.com/WISDOM#FluidDynamicsProperty"/>
    </owl:NamedIndividual>
    


    <!-- http://www.semanticwater.com/WISDOM#SurfaceRunoff -->

    <owl:NamedIndividual rdf:about="http://www.semanticwater.com/WISDOM#SurfaceRunoff">
        <rdf:type rdf:resource="http://www.semanticwater.com/WISDOM#WaterType"/>
    </owl:NamedIndividual>
    


    <!-- http://www.semanticwater.com/WISDOM#TemperatureProperty -->

    <owl:NamedIndividual rdf:about="http://www.semanticwater.com/WISDOM#TemperatureProperty">
        <rdf:type rdf:resource="http://www.semanticwater.com/WISDOM#FluidDynamicsProperty"/>
    </owl:NamedIndividual>
    


    <!-- http://www.semanticwater.com/WISDOM#TotalVolumeProperty -->

    <owl:NamedIndividual rdf:about="http://www.semanticwater.com/WISDOM#TotalVolumeProperty">
        <rdf:type rdf:resource="http://www.semanticwater.com/WISDOM#FluidDynamicsProperty"/>
    </owl:NamedIndividual>
    


    <!-- http://www.semanticwater.com/WISDOM#TreatedEffluent -->

    <owl:NamedIndividual rdf:about="http://www.semanticwater.com/WISDOM#TreatedEffluent">
        <rdf:type rdf:resource="http://www.semanticwater.com/WISDOM#WaterType"/>
    </owl:NamedIndividual>
    


    <!-- http://www.semanticwater.com/WISDOM#TurbidityProperty -->

    <owl:NamedIndividual rdf:about="http://www.semanticwater.com/WISDOM#TurbidityProperty">
        <rdf:type rdf:resource="http://www.semanticwater.com/WISDOM#FluidDynamicsProperty"/>
    </owl:NamedIndividual>
    


    <!-- http://www.semanticwater.com/WISDOM#VoltageProperty -->

    <owl:NamedIndividual rdf:about="http://www.semanticwater.com/WISDOM#VoltageProperty">
        <rdf:type rdf:resource="http://www.semanticwater.com/WISDOM#ElecProperty"/>
    </owl:NamedIndividual>
    


    <!-- http://www.semanticwater.com/WISDOM#WaterVelocityProperty -->

    <owl:NamedIndividual rdf:about="http://www.semanticwater.com/WISDOM#WaterVelocityProperty">
        <rdf:type rdf:resource="http://www.semanticwater.com/WISDOM#FluidDynamicsProperty"/>
    </owl:NamedIndividual>
    


    <!-- http://www.semanticwater.com/WISDOM#box -->

    <owl:NamedIndividual rdf:about="http://www.semanticwater.com/WISDOM#box">
        <rdf:type rdf:resource="http://www.semanticwater.com/WISDOM#PipeShape"/>
    </owl:NamedIndividual>
    


    <!-- http://www.semanticwater.com/WISDOM#circular -->

    <owl:NamedIndividual rdf:about="http://www.semanticwater.com/WISDOM#circular">
        <rdf:type rdf:resource="http://www.semanticwater.com/WISDOM#PipeShape"/>
    </owl:NamedIndividual>
    


    <!-- http://www.semanticwater.com/WISDOM#eggShaped -->

    <owl:NamedIndividual rdf:about="http://www.semanticwater.com/WISDOM#eggShaped">
        <rdf:type rdf:resource="http://www.semanticwater.com/WISDOM#PipeShape"/>
    </owl:NamedIndividual>
    <rdf:Description>
        <foaf:mbox>Pieter.Colpaert@UGent.be</foaf:mbox>
        <foaf:name>Pieter Colpaert</foaf:name>
    </rdf:Description>
    <rdf:Description>
        <foaf:mbox>abyrd@conveyal.com</foaf:mbox>
        <foaf:name>Andrew Byrd</foaf:name>
    </rdf:Description>
    


    <!-- 
    ///////////////////////////////////////////////////////////////////////////////////////
    //
    // Annotations
    //
    ///////////////////////////////////////////////////////////////////////////////////////
     -->

    <rdf:Description rdf:about="http://harmonet.org/harmonise.rdfs#accommodationType">
        <rdfs:comment>one of a defined value domain</rdfs:comment>
        <rdfs:label>accommodationType</rdfs:label>
    </rdf:Description>
    <rdf:Description rdf:about="http://harmonet.org/harmonise.rdfs#award">
        <rdfs:comment>f</rdfs:comment>
        <rdfs:label>award</rdfs:label>
    </rdf:Description>
    <rdf:Description rdf:about="http://harmonet.org/harmonise.rdfs#awardAchieved">
        <rdfs:label>awardAchieved</rdfs:label>
    </rdf:Description>
    <rdf:Description rdf:about="http://harmonet.org/harmonise.rdfs#awardingBody">
        <rdfs:label>awardingBody</rdfs:label>
    </rdf:Description>
    <rdf:Description rdf:about="http://harmonet.org/harmonise.rdfs#facility">
        <rdfs:label>facility</rdfs:label>
    </rdf:Description>
    <rdf:Description rdf:about="http://harmonet.org/harmonise.rdfs#fieldName">
        <rdfs:label>fieldName</rdfs:label>
    </rdf:Description>
    <rdf:Description rdf:about="http://harmonet.org/harmonise.rdfs#fieldValue">
        <rdfs:label>fieldValue</rdfs:label>
    </rdf:Description>
    <rdf:Description rdf:about="http://harmonet.org/harmonise.rdfs#gastroType">
        <rdfs:comment>The type of  gastro : a pub, a restaurant, a cafe, etc.</rdfs:comment>
        <rdfs:label>gastroType</rdfs:label>
    </rdf:Description>
    <rdf:Description rdf:about="http://harmonet.org/harmonise.rdfs#organiser">
        <rdfs:label>organiser</rdfs:label>
    </rdf:Description>
    <rdf:Description rdf:about="http://harmonet.org/harmonise.rdfs#profile">
        <rdfs:label>profile</rdfs:label>
    </rdf:Description>
    <rdf:Description rdf:about="http://harmonet.org/harmonise.rdfs#profileField">
        <rdfs:label>profileField</rdfs:label>
        <rdfs:comment>A field in the profile. This could be, for an accommodation site, the number of rooms with a shower. For a room, it could be whether smoking is permitted, etc.</rdfs:comment>
    </rdf:Description>
    <rdf:Description rdf:about="http://harmonet.org/harmonise.rdfs#type">
        <rdfs:label>type</rdfs:label>
    </rdf:Description>
    <rdf:Description rdf:about="http://purl.org/NET/c4dm/event.owl#literal_factor">
        <rdfs:comment xml:lang="es">Habla de un evento el cual puede ser descrito como un literal.
Esta propiedad no debería ser usada, pero debería ser incluida por otra más específica. Por ejemplo el tiempo en grados celsius debería ser incluida dentro del evento de temperatura.</rdfs:comment>
    </rdf:Description>
    <rdf:Description rdf:about="http://www.w3.org/2001/XMLSchema#unsignedLong">
        <rdfs:comment xml:lang="es">Bloque</rdfs:comment>
    </rdf:Description>
    <rdf:Description rdf:about="http://www.w3.org/2003/01/geo/wgs84_pos#">
        <rdfs:label>geo</rdfs:label>
        <rdfs:comment>Recent changes to this namespace:
$Log: wgs84_pos.rdf,v $
Revision 1.22  2009/04/20 15:00:30  timbl
Remove the time bits which have been deal with elsewhere eg in iCal.

Revision 1.21  2009/04/20 12:52:47  timbl
try again

Revision 1.20  2009/04/20 12:42:11  timbl
Add Event (edited ages ago and never checked in), and location (following discussion http://chatlogs.planetrdf.com/swig/2009-04-20#T12-36-09)

Revision 1.19  2009/04/20 12:36:31  timbl
Add Event (edited ages ago and never checked in), and location (following discussion http://chatlogs.planetrdf.com/swig/2009-04-20#T12-36-09)

Revision 1.18  2006/02/01 22:01:04  danbri
Clarified that lat and long are decimal degrees, and that alt is decimal metres about local reference ellipsoid

Revision 1.17  2004/02/06 17:38:12  danbri
Fixed a bad commit screwup

Revision 1.15  2003/04/19 11:24:08  danbri
Fixed the typo even more.

Revision 1.14  2003/04/19 11:16:56  danbri
fixed a typo

Revision 1.13  2003/02/19 22:27:27  connolly
relaxed domain constraints on lat/long/alt from Point to SpatialThing

Revision 1.12  2003/01/12 01:41:41  danbri
Trying local copy of XSLT doc.

Revision 1.11  2003/01/12 01:20:18  danbri
added a link to morten&apos;s xslt rdfs viewer.

Revision 1.10  2003/01/11 18:56:49  danbri
Removed datatype range from lat and long properties, since they would
have required each occurance of the property to mention the datatype.

Revision 1.9  2003/01/11 11:41:31  danbri
Another typo; repaired rdfs:Property to rdf:Property x4

Revision 1.8  2003/01/11 11:05:02  danbri
Added an rdfs:range for each lat/long/alt property,
http://www.w3.org/2001/XMLSchema#float

Revision 1.7  2003/01/10 20:25:16  danbri
Longer rdfs:comment for Point, trying to be Earth-centric and neutral about
coordinate system(s) at the same time. Feedback welcomed.

Revision 1.6  2003/01/10 20:18:30  danbri
Added CVS log comments into the RDF/XML as an rdfs:comment property of the
vocabulary. Note that this is not common practice (but seems both harmless
and potentially useful).


revision 1.5
date: 2003/01/10 20:14:31;  author: danbri;  state: Exp;  lines: +16 -5
Updated schema:
Added a dc:date, added url for more info. Changed the rdfs:label of the
namespace from gp to geo. Added a class Point, set as the rdfs:domain of
each property. Added XML comment on the lat_long property suggesting that
we might not need it (based on #rdfig commentary from implementors).

revision 1.4
date: 2003/01/10 20:01:07;  author: danbri;  state: Exp;  lines: +6 -5
Fixed typo; several rdfs:about attributes are now rdf:about. Thanks to MortenF in
#rdfig for catching this error.

revision 1.3
date: 2003/01/10 11:59:03;  author: danbri;  state: Exp;  lines: +4 -3
fixed buglet in vocab, added more wgs links

revision 1.2
date: 2003/01/10 11:01:11;  author: danbri;  state: Exp;  lines: +4 -4
Removed alt from the as-a-flat-string property, and switched from
space separated to comma separated.

revision 1.1
date: 2003/01/10 10:53:23;  author: danbri;  state: Exp;
basic geo vocab</rdfs:comment>
    </rdf:Description>
    <rdf:Description rdf:about="http://www.w3.org/2003/01/geo/wgs84_pos#lat_long">
        <rdfs:comment>A comma-separated representation of a latitude, longitude coordinate.</rdfs:comment>
        <rdfs:label>lat/long</rdfs:label>
    </rdf:Description>
    <rdf:Description rdf:about="http://www.w3.org/ns/locn#address">
        <rdfs:comment xml:lang="es">La relación de propiedad locn:address asocia cualquier recurso con la clase locn: Address</rdfs:comment>
    </rdf:Description>
    <rdf:Description rdf:about="http://www.w3.org/ns/locn#addressArea">
        <rdfs:comment xml:lang="es">El nombre de una zona geográfica o localidad que agrupa un gupo de objetos con dirección sin ser una unidad administrativa. 
Debería ser una parte de una ciudad, vecindario o pueblo. El dominio de locn:addressArea es locn:Address.</rdfs:comment>
    </rdf:Description>
    <rdf:Description rdf:about="http://www.w3.org/ns/locn#addressId">
        <rdfs:comment xml:lang="es">El concepto de añadir un identificador único global para cada instancia de una dirección es una parte crucial de las especificaciones de INSPIRE.
El dominio de locn:addressId es locn:Address.</rdfs:comment>
    </rdf:Description>
    <rdf:Description rdf:about="http://www.w3.org/ns/locn#fullAddress">
        <rdfs:comment xml:lang="es">Dirección completa de una propiedad escrita como una cades, con o sin formato. El dominio de locn:fullAddres es locn:Address.</rdfs:comment>
    </rdf:Description>
    <rdf:Description rdf:about="http://www.w3.org/ns/person#birthName">
        <rdfs:comment xml:lang="es">Todos los datos asociados con un individuo están sujetos a cambios. Los nombres pueden cambiar para una variedad de razones, ya sean formales o informales, y la nueva información puede poner de manifiesto que una corrección o aclaración se puede hacer sobre un registro existente. Los nombres de nacimiento tienden a ser persistentes, sin embargo y por esta razón, pueden estar registrados por algunos sistemas de información del sector público. No hay granularidad de nombres de nacimiento - el nombre completo debe ser registrado en un único campo</rdfs:comment>
    </rdf:Description>
    <rdf:Description rdf:about="http://www.w3.org/ns/person#citizenship">
        <rdfs:comment xml:lang="es">La relación de ciudadanía vincula a una Persona con una Jurisdicción que ha conferido derechos de ciudadanía a la persona tal como el derecho a votar, a recibir cierta protección de la comunidad oa la emisión de un pasaporte. Las múltiples ciudadanías se registran como múltiples instancias de la relación de ciudadanía.</rdfs:comment>
    </rdf:Description>
    <rdf:Description rdf:about="http://www.w3.org/ns/person#countryOfBirth">
        <rdfs:comment xml:lang="es">País de nacimiento de una persona</rdfs:comment>
    </rdf:Description>
    <rdf:Description rdf:about="http://www.w3.org/ns/person#countryOfDeath">
        <rdfs:comment xml:lang="es">País de fallecimiento de una persona</rdfs:comment>
    </rdf:Description>
    <rdf:Description rdf:about="http://www.w3.org/ns/person#patronymicName">
        <rdfs:comment xml:lang="es">Los nombres patronímicos son importantes en algunos países. Islandia no tiene un concepto de apellido como muchos otros países europeos, por ejemplo. En Bulgaria y Rusia, los nombres patronímicos están en uso diario, por ejemplo, el &quot;Sergeyevich&quot; (Сергеевич) en &quot;Mikhail Sergeyevich Gorbachev&quot; (Михаил Сергеевич Горбачёв).</rdfs:comment>
    </rdf:Description>
    <rdf:Description rdf:about="http://www.w3.org/ns/person#placeOfBirth">
        <rdfs:comment xml:lang="es">Lugar de nacimiento de una persona.</rdfs:comment>
    </rdf:Description>
    <rdf:Description rdf:about="http://www.w3.org/ns/person#placeOfDeath">
        <rdfs:comment xml:lang="es">Lugar de fallecimiento de una persona.</rdfs:comment>
    </rdf:Description>
    <rdf:Description rdf:about="http://www.w3.org/ns/person#residency">
        <rdfs:comment xml:lang="es">Residencia que típicamente asocia a un individuo con un subconjunto de los derechos de un ciudadano.</rdfs:comment>
    </rdf:Description>
    


    <!-- 
    ///////////////////////////////////////////////////////////////////////////////////////
    //
    // General axioms
    //
    ///////////////////////////////////////////////////////////////////////////////////////
     -->

    <rdf:Description>
        <rdf:type rdf:resource="http://www.w3.org/2002/07/owl#AllDisjointClasses"/>
        <owl:members rdf:parseType="Collection">
            <rdf:Description rdf:about="http://opendata.aragon.es/def/ei2a#ArableSubparcel"/>
            <rdf:Description rdf:about="http://opendata.aragon.es/def/ei2a#OliveGroveSubparcel"/>
            <rdf:Description rdf:about="http://opendata.aragon.es/def/ei2a#VineyardSubparcel"/>
            <rdf:Description rdf:about="http://opendata.aragon.es/def/ei2a#WoodenSubparcel"/>
        </owl:members>
    </rdf:Description>
</rdf:RDF>



<!-- Generated by the OWL API (version 4.2.6.20160910-2108) https://github.com/owlcs/owlapi -->

