<?xml version="1.0"?>
<rdf:RDF xmlns="http://data.europa.eu/esco/model#"
     xml:base="http://data.europa.eu/esco/model"
     xmlns:itm="http://data.europa.eu/esco/flow#"
     xmlns:owl="http://www.w3.org/2002/07/owl#"
     xmlns:dsv="http://purl.org/iso25964/DataSet/Versioning#"
     xmlns:owl2xml="http://www.w3.org/2006/12/owl2-xml#"
     xmlns:iso-thes="http://purl.org/iso25964/skos-thes#"
     xmlns:xsd="http://www.w3.org/2001/XMLSchema#"
     xmlns:voaf="http://purl.org/vocommons/voaf#"
     xmlns:skos="http://www.w3.org/2004/02/skos/core#"
     xmlns:rdfs="http://www.w3.org/2000/01/rdf-schema#"
     xmlns:skos2="http://data.europa.eu/esco/skos2#"
     xmlns:skos-xl="http://www.w3.org/2008/05/skos-xl#"
     xmlns:ConceptScheme="http://data.europa.eu/esco/ConceptScheme/"
     xmlns:rdf="http://www.w3.org/1999/02/22-rdf-syntax-ns#"
     xmlns:terms="http://purl.org/dc/terms/"
     xmlns:escowf="http://data.europa.eu/esco/model/workflow#"
     xmlns:esco="http://data.europa.eu/esco/model#"
     xmlns:xml="http://www.w3.org/XML/1998/namespace"
     xmlns:vs="http://www.w3.org/2003/06/sw-vocab-status/ns#"
     xmlns:prov="http://www.w3.org/ns/prov#"
     xmlns:foaf="http://xmlns.com/foaf/0.1/"
     xmlns:dc="http://purl.org/dc/elements/1.1/">
    <owl:Ontology rdf:about="http://data.europa.eu/esco/model">
        <owl:versionIRI rdf:resource="http://data.europa.eu/esco/model/1.2"/>
        <owl:imports rdf:resource="http://www.w3.org/1999/02/22-rdf-syntax-ns#"/>
        <owl:imports rdf:resource="http://data.europa.eu/esco/flow"/>
        <owl:imports rdf:resource="http://www.w3.org/2008/05/skos-xl"/>
        <owl:imports rdf:resource="http://data.europa.eu/esco/skos2"/>
        <owl:imports rdf:resource="http://purl.org/iso25964/skos-thes"/>
        <owl:imports rdf:resource="http://www.w3.org/2004/02/skos/core"/>
        <terms:modified rdf:datatype="http://www.w3.org/2001/XMLSchema#date">2016-06-03</terms:modified>				
        <terms:contributor>Agis Papantoniou (Everis, CogniZone)</terms:contributor>
        <terms:creator>Johan De Smedt (TenForce)</terms:creator>
        <terms:contributor>Karel Kremer (TenForce)</terms:contributor>
        <terms:contributor>Massimiliano Molinari (DG-EMPL, Reviewer)</terms:contributor>
        <terms:contributor>Pieter Fannes (Everis, CogniZone)</terms:contributor>
        <terms:contributor>Martin Le Vrang (DG-EMPL, Approver)</terms:contributor>
        <terms:contributor>Laurent BÃ©gin (Mondeca)</terms:contributor>
        <terms:contributor>Niels Vandekeybus (TenForce)</terms:contributor>
        <terms:title xml:lang="en">The ESCO ontology</terms:title>
        <owl:versionInfo rdf:datatype="http://www.w3.org/2001/XMLSchema#string">1.2</owl:versionInfo>
        <owl:incompatibleWith rdf:resource="http://data.europa.eu/esco/model/1.0"/>
        <terms:contributor>Bernard Vatan (Mondeca)</terms:contributor>
        <rdfs:comment xml:lang="en">The ontology of the taxonomy &quot;European Skills, Competences, qualifications and Occupations&quot;.

The ontology considers three ESCO pillars (or taxonomy) and 2 registers.
The three pillars are:
- Occupation
- Skill (and competences)
- Qualification

For the construction and use of the ESCO pillars, the following modelling artefacts are used:
- SKOS mapping properties to relate ESCO pillar concepts to concepts in other (external) taxonomies (e.g. ISCED-FoET and ISCO08.  More mappings can be added in the future.)
- Tagging ESCO pillar concepts by other (external) taxonomies (NUTS, EQF, NACE, ...), these taggings are defined using ESCO structures
- Capture gender specifics on the labels of the ESCO pillar concepts
- Rich ESCO concept relationships holding a description and other specific characteristics of the relation between two ESCO pillar concepts.

ESCO maintains two additional registers:
- Awarding Body
- Work Context
Awarding Bodies typically are referenced by ESCO qualifications.
Occupations can have one or more work context.
</rdfs:comment>
    </owl:Ontology>



    <!--
    ///////////////////////////////////////////////////////////////////////////////////////
    //
    // Annotation properties
    //
    ///////////////////////////////////////////////////////////////////////////////////////
     -->




    <!-- http://data.europa.eu/esco/model#expirationNote -->

    <owl:AnnotationProperty rdf:about="http://data.europa.eu/esco/model#expirationNote">
        <terms:modified rdf:datatype="http://www.w3.org/2001/XMLSchema#date">2013-12-03</terms:modified>
        <rdfs:isDefinedBy rdf:resource="http://data.europa.eu/esco/model"/>
        <rdfs:label xml:lang="en">ESCO expiration note</rdfs:label>
        <rdfs:seeAlso rdf:resource="http://data.europa.eu/esco/model#expirationPeriod"/>
        <owl:deprecated rdf:datatype="http://www.w3.org/2001/XMLSchema#boolean">true</owl:deprecated>
        <vs:term_status>rejected</vs:term_status>
        <skos:changeNote xml:lang="en">ESCO v0 -&gt; ESCO v1.
Should be part of http://www.w3.org/2004/02/skos/core#definition.
An expiration period typically should be given formaly by the &quot;xsd:duration&quot; typed property http://data.europa.eu/esco/model#expirationPeriod

ESCO v0 has expiration notes on 3 qualifications (also having a definition).  These expiration notes need to be appended to the respective definition note.by:
- add two line breaks
- add the expiration note.
The formal property esco:expirationPeriod needs to be set manually to express a duration.</skos:changeNote>
        <skos:definition xml:lang="en">A note documenting an expiry period or date</skos:definition>
        <skos:historyNote xml:lang="en">Deprecated with Model version 1.</skos:historyNote>
        <rdfs:subPropertyOf rdf:resource="http://www.w3.org/2004/02/skos/core#note"/>
    </owl:AnnotationProperty>



    <!-- http://data.europa.eu/esco/model#iscoLabel -->

    <owl:AnnotationProperty rdf:about="http://data.europa.eu/esco/model#iscoLabel">
        <rule rdf:datatype="http://www.w3.org/2001/XMLSchema#string">There may be at most 1 iscoLabel per language for any OcupationGroup.</rule>
        <terms:modified rdf:datatype="http://www.w3.org/2001/XMLSchema#date">2013-12-03</terms:modified>
        <rdfs:comment xml:lang="en">The ISCO label of an occupation group.
Provided in case the preferred label has been replaced by an esco specific one.

Typically this can happen in order not to have duplicate preferred labels in the ESCO thesaurus.</rdfs:comment>
        <rdfs:isDefinedBy rdf:resource="http://data.europa.eu/esco/model"/>
        <rdfs:label xml:lang="en">isco label</rdfs:label>
        <rdfs:seeAlso rdf:resource="http://data.europa.eu/esco/ConceptScheme/ISCO2008"/>
        <rdfs:seeAlso rdf:resource="http://data.europa.eu/esco/model#originalLabel"/>
        <owl:deprecated rdf:datatype="http://www.w3.org/2001/XMLSchema#boolean">true</owl:deprecated>
        <vs:term_status>released</vs:term_status>
        <skos:changeNote xml:lang="en">Generalized and replaced by: http://data.europa.eu/esco/model#originalLabel

ESCO v0 -&gt; ESCO v1 (read also change note on: http://data.europa.eu/esco/ConceptScheme/ISCO2008)
The ESCOv1 (= v0.0) concepts (that are a copy of ISCO2008 concepts) should keep existing label in ESCOv0 and iscoLabel is removed.
The ISCO2008 concepts should keep the preferred label (per language) the property esco:iscoLabel is replaced by the property esco:originalLabel (http://data.europa.eu/esco/model#originalLabel)

Conversion needs to convert the existing ISCO labels in two ways:
- as esco:iscoLabel which MAY NOT be modified (READ-ONLY)
- as xl:label where ESCO can overrule the terminology from ISCO to conform to SKOS label requirements.</skos:changeNote>
        <skos:historyNote xml:lang="en">Deprecated with Model version 1.</skos:historyNote>
        <rdfs:subPropertyOf rdf:resource="http://www.w3.org/2000/01/rdf-schema#label"/>
    </owl:AnnotationProperty>



    <!-- http://data.europa.eu/esco/model#learningOutcomeNote -->

    <owl:AnnotationProperty rdf:about="http://data.europa.eu/esco/model#learningOutcomeNote">
        <terms:issued rdf:datatype="http://www.w3.org/2001/XMLSchema#date">2013-06-27</terms:issued>
        <terms:modified rdf:datatype="http://www.w3.org/2001/XMLSchema#date">2013-12-03</terms:modified>
        <rdfs:comment xml:lang="en">a note documenting the learning outcomes.</rdfs:comment>
        <rdfs:isDefinedBy rdf:resource="http://data.europa.eu/esco/model"/>
        <rdfs:label xml:lang="en">editorial note</rdfs:label>
        <owl:deprecated rdf:datatype="http://www.w3.org/2001/XMLSchema#boolean">true</owl:deprecated>
        <vs:term_status>rejected</vs:term_status>
        <skos:changeNote xml:lang="en">The deprecated note must be transferred.
- either be part of the definition (http://www.w3.org/2004/02/skos/core#definition) of the subject
- or be part of the ESCO relationship (see http://data.europa.eu/esco/model#Relationship) providing the description of the subject.

ESCOv0 -&gt; ESCOv
ESCO v0 has two (subject) Qualification concepts with a learningOutcome Note (and no definition note).
On conversion to ESCOv1 model, these should be replaced by a http://www.w3.org/2004/02/skos/core#definition</skos:changeNote>
        <skos:historyNote xml:lang="en">Deprecated with Model version 1.</skos:historyNote>
        <rdfs:subPropertyOf rdf:resource="http://www.w3.org/2004/02/skos/core#note"/>
    </owl:AnnotationProperty>



    <!-- http://data.europa.eu/esco/model#originalLabel -->

    <owl:AnnotationProperty rdf:about="http://data.europa.eu/esco/model#originalLabel">
        <rule rdf:datatype="http://www.w3.org/2001/XMLSchema#string">There may be at most 1 originalLabel per language for any Concept.</rule>
        <terms:issued rdf:datatype="http://www.w3.org/2001/XMLSchema#date">2013-12-03</terms:issued>
        <terms:modified rdf:datatype="http://www.w3.org/2001/XMLSchema#date">2013-12-03</terms:modified>
        <rdfs:comment xml:lang="en">The original label of a concept of a support taxonomy.
Provided in case the preferred label has been replaced by an ESCO specific one.

Typically used on arguable names for exceptional concepts like &apos;Country&apos;</rdfs:comment>
        <rdfs:isDefinedBy rdf:resource="http://data.europa.eu/esco/model"/>
        <rdfs:label xml:lang="en">original label</rdfs:label>
        <vs:term_status>proposed</vs:term_status>
        <rdfs:subPropertyOf rdf:resource="http://www.w3.org/2000/01/rdf-schema#label"/>
        <rdfs:range rdf:resource="http://www.w3.org/1999/02/22-rdf-syntax-ns#PlainLiteral"/>
    </owl:AnnotationProperty>



    <!-- http://data.europa.eu/esco/model#regulatedProfessionNote -->

    <owl:AnnotationProperty rdf:about="http://data.europa.eu/esco/model#regulatedProfessionNote">
        <terms:modified rdf:datatype="http://www.w3.org/2001/XMLSchema#date">2014-08-26</terms:modified>
        <rdfs:comment xml:lang="en">The subject occupation is regulated according the description in the note.  The note typically contains a hyperlink.</rdfs:comment>
        <rdfs:isDefinedBy rdf:resource="http://data.europa.eu/esco/model"/>
        <rdfs:label xml:lang="en">regultated profession note</rdfs:label>
        <vs:term_status>proposed</vs:term_status>
        <rdfs:subPropertyOf rdf:resource="http://www.w3.org/2004/02/skos/core#note"/>
        <rdfs:domain rdf:resource="http://data.europa.eu/esco/model#Occupation"/>
    </owl:AnnotationProperty>



    <!-- http://data.europa.eu/esco/model#rule -->

    <owl:AnnotationProperty rdf:about="http://data.europa.eu/esco/model#rule">
        <owl:deprecated rdf:datatype="http://www.w3.org/2001/XMLSchema#boolean">true</owl:deprecated>
    </owl:AnnotationProperty>



    <!-- http://data.europa.eu/esco/model#sortString -->

    <owl:AnnotationProperty rdf:about="http://data.europa.eu/esco/model#sortString">
        <terms:issued rdf:datatype="http://www.w3.org/2001/XMLSchema#date">2014-04-08</terms:issued>
        <terms:modified rdf:datatype="http://www.w3.org/2001/XMLSchema#date">2014-04-08</terms:modified>
        <rdfs:comment xml:lang="en">The formatted string used to establish sorting among concepts.
Deprecated by use of skos:OrderedCollection and iso-thes:subordinateArray</rdfs:comment>
        <rdfs:isDefinedBy rdf:resource="http://data.europa.eu/esco/model"/>
        <rdfs:label xml:lang="en">sorting string</rdfs:label>
        <rdfs:seeAlso rdf:resource="http://purl.org/iso25964/skos-thes#subordinateArray"/>
        <rdfs:seeAlso rdf:resource="http://www.w3.org/2004/02/skos/core#OrderedCollection"/>
        <owl:deprecated rdf:datatype="http://www.w3.org/2001/XMLSchema#boolean">true</owl:deprecated>
        <vs:term_status>rejected</vs:term_status>
        <vs:term_status rdf:datatype="http://www.w3.org/2001/XMLSchema#string">rejected</vs:term_status>
        <rdfs:range rdf:resource="http://www.w3.org/2000/01/rdf-schema#Literal"/>
    </owl:AnnotationProperty>



    <!-- http://www.w3.org/2003/06/sw-vocab-status/ns#term_status -->

    <owl:AnnotationProperty rdf:about="http://www.w3.org/2003/06/sw-vocab-status/ns#term_status">
        <terms:issued rdf:datatype="http://www.w3.org/2001/XMLSchema#date">2013-12-05</terms:issued>
        <terms:modified rdf:datatype="http://www.w3.org/2001/XMLSchema#date">2013-12-05</terms:modified>
        <rdfs:isDefinedBy rdf:resource="http://www.w3.org/2003/06/sw-vocab-status/ns"/>
        <rdfs:label xml:lang="en">model axiom or term status</rdfs:label>
        <vs:term_status rdf:datatype="http://www.w3.org/2001/XMLSchema#string">proposed</vs:term_status>
        <rdfs:range rdf:resource="http://data.europa.eu/esco/model#termStatusDataType"/>
    </owl:AnnotationProperty>



    <!--
    ///////////////////////////////////////////////////////////////////////////////////////
    //
    // Datatypes
    //
    ///////////////////////////////////////////////////////////////////////////////////////
     -->




    <!-- http://data.europa.eu/esco/Notation/EQF2012 -->

    <rdfs:Datatype rdf:about="http://data.europa.eu/esco/Notation/EQF2012">
        <rdfs:isDefinedBy rdf:resource="http://data.europa.eu/esco/model"/>
        <vs:term_status>released</vs:term_status>
    </rdfs:Datatype>



    <!-- http://data.europa.eu/esco/Notation/FoET2013 -->

    <rdfs:Datatype rdf:about="http://data.europa.eu/esco/Notation/FoET2013">
        <rdfs:isDefinedBy rdf:resource="http://data.europa.eu/esco/model"/>
        <vs:term_status>released</vs:term_status>
    </rdfs:Datatype>



    <!-- http://data.europa.eu/esco/Notation/ISCO08 -->

    <rdfs:Datatype rdf:about="http://data.europa.eu/esco/Notation/ISCO08">
        <rdfs:isDefinedBy rdf:resource="http://data.europa.eu/esco/model"/>
        <vs:term_status>released</vs:term_status>
    </rdfs:Datatype>



    <!-- http://data.europa.eu/esco/Notation/ISCO88 -->

    <rdfs:Datatype rdf:about="http://data.europa.eu/esco/Notation/ISCO88">
        <rdfs:isDefinedBy rdf:resource="http://data.europa.eu/esco/model"/>
        <owl:deprecated rdf:datatype="http://www.w3.org/2001/XMLSchema#boolean">true</owl:deprecated>
        <vs:term_status>deprecated</vs:term_status>
    </rdfs:Datatype>



    <!-- http://data.europa.eu/esco/Notation/NACEr2.code -->

    <rdfs:Datatype rdf:about="http://data.europa.eu/esco/Notation/NACEr2.code">
        <rdfs:isDefinedBy rdf:resource="http://data.europa.eu/esco/model"/>
        <vs:term_status>released</vs:term_status>
    </rdfs:Datatype>



    <!-- http://data.europa.eu/esco/Notation/NACEr2.section -->

    <rdfs:Datatype rdf:about="http://data.europa.eu/esco/Notation/NACEr2.section">
        <rdfs:isDefinedBy rdf:resource="http://data.europa.eu/esco/model"/>
        <vs:term_status>released</vs:term_status>
    </rdfs:Datatype>



    <!-- http://data.europa.eu/esco/Notation/NUTS.regionCode -->

    <rdfs:Datatype rdf:about="http://data.europa.eu/esco/Notation/NUTS.regionCode">
        <rdfs:isDefinedBy rdf:resource="http://data.europa.eu/esco/model"/>
        <vs:term_status>released</vs:term_status>
    </rdfs:Datatype>



    <!-- http://data.europa.eu/esco/Notation/eCF30 -->

    <rdfs:Datatype rdf:about="http://data.europa.eu/esco/Notation/eCF30">
        <rdfs:isDefinedBy rdf:resource="http://data.europa.eu/esco/model"/>
        <vs:term_status>released</vs:term_status>
    </rdfs:Datatype>



    <!-- http://data.europa.eu/esco/model#editorialStatusDataType -->

    <rdfs:Datatype rdf:about="http://data.europa.eu/esco/model#editorialStatusDataType">
        <terms:modified rdf:datatype="http://www.w3.org/2001/XMLSchema#string">2013-12-05</terms:modified>
        <rdfs:comment xml:lang="en">list of status values used for managing ESCO vocabulary changes.
The editorial status is only managed by a human with the role of taxonomy editor.

On creation, the default status is &quot;prepared&quot;.  The label or concept is considered not final.
When finalizing the business releaavance and the related editorial review process, the status can be set to &quot;proposed&quot;.
After a formal validation process by the business, the status can be set to approved.
When a review considers the label or concept not relevant any more, the publication status is (automatically) set to &quot;obsolete&quot; by the relevant deprecation action.
</rdfs:comment>
        <rdfs:isDefinedBy rdf:resource="http://data.europa.eu/esco/model"/>
        <rdfs:label rdf:datatype="http://www.w3.org/2001/XMLSchema#string">thesaurus concept and label editorial status type</rdfs:label>
        <vs:term_status>proposed</vs:term_status>
        <owl:equivalentClass>
            <rdfs:Datatype>
                <owl:unionOf rdf:parseType="Collection">
                    <rdfs:Datatype>
                        <owl:onDatatype rdf:resource="http://www.w3.org/2001/XMLSchema#string"/>
                        <owl:withRestrictions rdf:parseType="Collection">
                            <rdf:Description>
                                <xsd:pattern rdf:datatype="http://www.w3.org/2001/XMLSchema#string">approved</xsd:pattern>
                            </rdf:Description>
                        </owl:withRestrictions>
                    </rdfs:Datatype>
                    <rdfs:Datatype>
                        <owl:onDatatype rdf:resource="http://www.w3.org/2001/XMLSchema#string"/>
                        <owl:withRestrictions rdf:parseType="Collection">
                            <rdf:Description>
                                <xsd:pattern rdf:datatype="http://www.w3.org/2001/XMLSchema#string">prepared</xsd:pattern>
                            </rdf:Description>
                        </owl:withRestrictions>
                    </rdfs:Datatype>
                    <rdfs:Datatype>
                        <owl:onDatatype rdf:resource="http://www.w3.org/2001/XMLSchema#string"/>
                        <owl:withRestrictions rdf:parseType="Collection">
                            <rdf:Description>
                                <xsd:pattern rdf:datatype="http://www.w3.org/2001/XMLSchema#string">proposed</xsd:pattern>
                            </rdf:Description>
                        </owl:withRestrictions>
                    </rdfs:Datatype>
                </owl:unionOf>
            </rdfs:Datatype>
        </owl:equivalentClass>
    </rdfs:Datatype>



    <!-- http://data.europa.eu/esco/model#statusDataType -->

    <rdfs:Datatype rdf:about="http://data.europa.eu/esco/model#statusDataType">
        <terms:modified rdf:datatype="http://www.w3.org/2001/XMLSchema#string">2013-12-05</terms:modified>
        <rdfs:comment xml:lang="en">list of status values used for managing ESCO release status.
On creation of a concept or label, the default state is &quot;to be reviewed&quot;
On deprecation of a concept the concept state becomed &quot;obsolete&quot;
When a wrongly deprecated concept is revived, the state becomes &quot;to be reviewed&quot;
When the thesaurus is published, the statuss becomes &quot;released&quot;

All state changes are system managed.</rdfs:comment>
        <rdfs:isDefinedBy rdf:resource="http://data.europa.eu/esco/model"/>
        <rdfs:label rdf:datatype="http://www.w3.org/2001/XMLSchema#string">thesaurus concept and label publaction status type</rdfs:label>
        <vs:term_status>proposed</vs:term_status>
        <owl:equivalentClass>
            <rdfs:Datatype>
                <owl:unionOf rdf:parseType="Collection">
                    <rdfs:Datatype>
                        <owl:onDatatype rdf:resource="http://www.w3.org/2001/XMLSchema#string"/>
                        <owl:withRestrictions rdf:parseType="Collection">
                            <rdf:Description>
                                <xsd:pattern rdf:datatype="http://www.w3.org/2001/XMLSchema#string">obsolete</xsd:pattern>
                            </rdf:Description>
                        </owl:withRestrictions>
                    </rdfs:Datatype>
                    <rdfs:Datatype>
                        <owl:onDatatype rdf:resource="http://www.w3.org/2001/XMLSchema#string"/>
                        <owl:withRestrictions rdf:parseType="Collection">
                            <rdf:Description>
                                <xsd:pattern rdf:datatype="http://www.w3.org/2001/XMLSchema#string">released</xsd:pattern>
                            </rdf:Description>
                        </owl:withRestrictions>
                    </rdfs:Datatype>
                    <rdfs:Datatype>
                        <owl:onDatatype rdf:resource="http://www.w3.org/2001/XMLSchema#string"/>
                        <owl:withRestrictions rdf:parseType="Collection">
                            <rdf:Description>
                                <xsd:pattern rdf:datatype="http://www.w3.org/2001/XMLSchema#string">to be reviewed</xsd:pattern>
                            </rdf:Description>
                        </owl:withRestrictions>
                    </rdfs:Datatype>
                </owl:unionOf>
            </rdfs:Datatype>
        </owl:equivalentClass>
    </rdfs:Datatype>



    <!-- http://data.europa.eu/esco/model#termStatusDataType -->

    <rdfs:Datatype rdf:about="http://data.europa.eu/esco/model#termStatusDataType">
        <terms:modified rdf:datatype="http://www.w3.org/2001/XMLSchema#string">2013-12-05</terms:modified>
        <rdfs:comment xml:lang="en">list of status values used for managing ESCO ontology changes.</rdfs:comment>
        <rdfs:isDefinedBy rdf:resource="http://data.europa.eu/esco/model"/>
        <rdfs:label rdf:datatype="http://www.w3.org/2001/XMLSchema#string">term status type</rdfs:label>
        <vs:term_status>proposed</vs:term_status>
        <owl:equivalentClass>
            <rdfs:Datatype>
                <owl:unionOf rdf:parseType="Collection">
                    <rdfs:Datatype>
                        <owl:onDatatype rdf:resource="http://www.w3.org/2001/XMLSchema#string"/>
                        <owl:withRestrictions rdf:parseType="Collection">
                            <rdf:Description>
                                <xsd:pattern rdf:datatype="http://www.w3.org/2001/XMLSchema#string">approved</xsd:pattern>
                            </rdf:Description>
                        </owl:withRestrictions>
                    </rdfs:Datatype>
                    <rdfs:Datatype>
                        <owl:onDatatype rdf:resource="http://www.w3.org/2001/XMLSchema#string"/>
                        <owl:withRestrictions rdf:parseType="Collection">
                            <rdf:Description>
                                <xsd:pattern rdf:datatype="http://www.w3.org/2001/XMLSchema#string">prepared</xsd:pattern>
                            </rdf:Description>
                        </owl:withRestrictions>
                    </rdfs:Datatype>
                    <rdfs:Datatype>
                        <owl:onDatatype rdf:resource="http://www.w3.org/2001/XMLSchema#string"/>
                        <owl:withRestrictions rdf:parseType="Collection">
                            <rdf:Description>
                                <xsd:pattern rdf:datatype="http://www.w3.org/2001/XMLSchema#string">proposed</xsd:pattern>
                            </rdf:Description>
                        </owl:withRestrictions>
                    </rdfs:Datatype>
                    <rdfs:Datatype>
                        <owl:onDatatype rdf:resource="http://www.w3.org/2001/XMLSchema#string"/>
                        <owl:withRestrictions rdf:parseType="Collection">
                            <rdf:Description>
                                <xsd:pattern rdf:datatype="http://www.w3.org/2001/XMLSchema#string">rejected</xsd:pattern>
                            </rdf:Description>
                        </owl:withRestrictions>
                    </rdfs:Datatype>
                    <rdfs:Datatype>
                        <owl:onDatatype rdf:resource="http://www.w3.org/2001/XMLSchema#string"/>
                        <owl:withRestrictions rdf:parseType="Collection">
                            <rdf:Description>
                                <xsd:pattern rdf:datatype="http://www.w3.org/2001/XMLSchema#string">released</xsd:pattern>
                            </rdf:Description>
                        </owl:withRestrictions>
                    </rdfs:Datatype>
                    <rdfs:Datatype>
                        <owl:onDatatype rdf:resource="http://www.w3.org/2001/XMLSchema#string"/>
                        <owl:withRestrictions rdf:parseType="Collection">
                            <rdf:Description>
                                <xsd:pattern rdf:datatype="http://www.w3.org/2001/XMLSchema#string">to be reviewed</xsd:pattern>
                            </rdf:Description>
                        </owl:withRestrictions>
                    </rdfs:Datatype>
                </owl:unionOf>
            </rdfs:Datatype>
        </owl:equivalentClass>
    </rdfs:Datatype>



    <!-- http://www.w3.org/2001/XMLSchema#duration -->

    <rdfs:Datatype rdf:about="http://www.w3.org/2001/XMLSchema#duration"/>



    <!--
    ///////////////////////////////////////////////////////////////////////////////////////
    //
    // Object Properties
    //
    ///////////////////////////////////////////////////////////////////////////////////////
     -->




    <!-- http://data.europa.eu/esco/model#ISCO88Code -->

    <owl:ObjectProperty rdf:about="http://data.europa.eu/esco/model#ISCO88Code">
        <rdfs:subPropertyOf rdf:resource="http://purl.org/dc/terms/subject"/>
        <terms:issued rdf:datatype="http://www.w3.org/2001/XMLSchema#date">2013-06-27</terms:issued>
        <terms:modified rdf:datatype="http://www.w3.org/2001/XMLSchema#date">2013-12-03</terms:modified>
        <rdfs:comment xml:lang="en">The parent ISCO 88 codes of a specific occupation.
The format is &apos;&apos;&lt;code&gt;[,&lt;code&gt;]*&apos;&apos;^^xsd:string

e.g &apos;&apos;3139,3131&apos;&apos;^^xsd:string  means the occupation has 2 parent occupation groups in isco88. One with iscocode 3139 and one with iscocode 3131</rdfs:comment>
        <rdfs:isDefinedBy rdf:resource="http://data.europa.eu/esco/model"/>
        <rdfs:label xml:lang="en">ISCO88 Code</rdfs:label>
        <rdfs:seeAlso rdf:resource="http://data.europa.eu/esco/ConceptScheme/ISCO2008"/>
        <rdfs:seeAlso rdf:resource="http://data.europa.eu/esco/model#memberOfISCOGroup"/>
        <owl:deprecated rdf:datatype="http://www.w3.org/2001/XMLSchema#boolean">true</owl:deprecated>
        <vs:term_status>rejected</vs:term_status>
        <skos:changeNote xml:lang="en">ESCO v0 -&gt; ESCO v1 must create http://data.europa.eu/esco/model#memberOfISCOGroup (esco:memberOfISCOGroup a sub-property of skos:broadMatch) based on the detailed list of ISCO codes.
Read also change note on: http://data.europa.eu/esco/ConceptScheme/ISCO2008

Esco v0 has 4761 statements.</skos:changeNote>
        <skos:historyNote xml:lang="en">Deprecated with Model version 1.</skos:historyNote>
    </owl:ObjectProperty>



    <!-- http://data.europa.eu/esco/model#additionalNote -->

    <owl:ObjectProperty rdf:about="http://data.europa.eu/esco/model#additionalNote">
        <rdfs:range rdf:resource="http://data.europa.eu/esco/model#NodeLiteral"/>
        <rdfs:comment xml:lang="en"></rdfs:comment>
        <rdfs:isDefinedBy rdf:resource="http://data.europa.eu/esco/model"/>
        <rdfs:label xml:lang="en">Additional note</rdfs:label>
        <rdfs:seeAlso rdf:resource="http://data.europa.eu/esco/model#NodeLiteral"/>
    </owl:ObjectProperty>



    <!-- http://data.europa.eu/esco/model#awardingBodyDescription -->

    <owl:ObjectProperty rdf:about="http://data.europa.eu/esco/model#awardingBodyDescription">
        <rdfs:domain rdf:resource="http://data.europa.eu/esco/model#Qualification"/>
        <rdfs:range rdf:resource="http://www.w3.org/1999/02/22-rdf-syntax-ns#XMLLiteral"/>
    </owl:ObjectProperty>



    <!-- http://data.europa.eu/esco/model#broaderInstance -->

    <owl:ObjectProperty rdf:about="http://data.europa.eu/esco/model#broaderInstance">
        <rdfs:subPropertyOf rdf:resource="http://data.europa.eu/esco/model#memberOfGroup"/>
        <rdfs:subPropertyOf rdf:resource="http://purl.org/iso25964/skos-thes#broaderInstantial"/>
        <owl:inverseOf rdf:resource="http://data.europa.eu/esco/model#narrowerInstance"/>
        <rdfs:domain rdf:resource="http://data.europa.eu/esco/model#MemberConcept"/>
        <rdfs:domain rdf:resource="http://data.europa.eu/esco/model#SimpleConcept"/>
        <rdfs:range rdf:resource="http://data.europa.eu/esco/model#LeafGroupConcept"/>
        <terms:issued rdf:datatype="http://www.w3.org/2001/XMLSchema#date">2013-06-27</terms:issued>
        <terms:modified rdf:datatype="http://www.w3.org/2001/XMLSchema#date">2016-06-08</terms:modified>
        <rdfs:comment xml:lang="en">The Leaf Group the (subject) ESCO member concept (Skill or Occupation or Qualification) belongs to.
Only member properties having a Leaf Group type as broader concept must have this property,  Specializations of member concepts (like Faceted Concepts) do not have this property.</rdfs:comment>
        <rdfs:isDefinedBy rdf:resource="http://data.europa.eu/esco/model"/>
        <rdfs:label xml:lang="en">broader instance</rdfs:label>
        <owl:deprecated rdf:datatype="http://www.w3.org/2001/XMLSchema#boolean">true</owl:deprecated>
        <vs:term_status rdf:datatype="http://www.w3.org/2001/XMLSchema#string">deprecated</vs:term_status>
    </owl:ObjectProperty>



    <!-- http://data.europa.eu/esco/model#codeList -->

    <owl:ObjectProperty rdf:about="http://data.europa.eu/esco/model#codeList">
        <rdfs:range rdf:resource="http://www.w3.org/2004/02/skos/core#ConceptScheme"/>
        <terms:created rdf:datatype="http://www.w3.org/2001/XMLSchema#date">2016-06-21</terms:created>
        <terms:modified rdf:datatype="http://www.w3.org/2001/XMLSchema#date">2016-06-21</terms:modified>
        <rdfs:isDefinedBy rdf:resource="http://data.europa.eu/esco/model"/>
        <rdfs:label>has code list</rdfs:label>
        <rdfs:seeAlso rdf:resource="http://data.europa.eu/esco/model#Structure"/>
        <rdfs:seeAlso rdf:resource="http://data.europa.eu/esco/model#codedProperty"/>
        <vs:term_status>proposed</vs:term_status>
    </owl:ObjectProperty>



    <!-- http://data.europa.eu/esco/model#codedProperty -->

    <owl:ObjectProperty rdf:about="http://data.europa.eu/esco/model#codedProperty">
        <rdfs:range rdf:resource="http://www.w3.org/1999/02/22-rdf-syntax-ns#Property"/>
        <terms:created rdf:datatype="http://www.w3.org/2001/XMLSchema#date">2016-06-21</terms:created>
        <terms:modified rdf:datatype="http://www.w3.org/2001/XMLSchema#date">2016-06-21</terms:modified>
        <rdfs:isDefinedBy rdf:resource="http://data.europa.eu/esco/model"/>
        <rdfs:label>has coded property</rdfs:label>
        <rdfs:seeAlso rdf:resource="http://data.europa.eu/esco/model#Structure"/>
        <rdfs:seeAlso rdf:resource="http://data.europa.eu/esco/model#codeList"/>
        <vs:term_status>proposed</vs:term_status>
    </owl:ObjectProperty>



    <!-- http://data.europa.eu/esco/model#constructedFrom -->

    <owl:ObjectProperty rdf:about="http://data.europa.eu/esco/model#constructedFrom">
        <rdfs:subPropertyOf rdf:resource="http://www.w3.org/2004/02/skos/core#broaderTransitive"/>
        <rdfs:domain rdf:resource="http://data.europa.eu/esco/model#FacetedConcept"/>
        <rdfs:range rdf:resource="http://data.europa.eu/esco/model#MemberConcept"/>
        <rdfs:range rdf:resource="http://data.europa.eu/esco/model#SimpleConcept"/>
        <rule rdf:datatype="http://www.w3.org/2001/XMLSchema#string">If:
- FC esco:constructedFrom SC
- FC esco:plusUF UF
- lang(UF/xl:literalForm) = L
- SC xl:prefLabel PLsc
- lang(PLsc/xl:literalForm) = L
Then
- PLsc iso-thes:plusUFTerm UF
- UF iso-thes:plusUseTerm PLsc</rule>
        <terms:issued rdf:datatype="http://www.w3.org/2001/XMLSchema#date">2014-02-03</terms:issued>
        <terms:modified rdf:datatype="http://www.w3.org/2001/XMLSchema#date">2016-06-08</terms:modified>
        <rdfs:comment xml:lang="en">The unique (simple) ESCO concept used to construct the (subject) faceted ESCO concept.

Example (started): Simple concept Teacher is specialized to identify teacher at different education levels.
- The simple (member) occupation is: &quot;Teacher&quot;
- Assume we have a classification of the levels of education (e.g. &quot;primary school&quot;, &quot;high school&quot;, &quot;university&quot;)
- The constructed faceted (member) concepts that will be:
  &quot;primary school teacher&quot;, &quot;high school teacher&quot; and &quot;university teacher&quot; (this last one occasionally re-labeled as &quot;university professor&quot;)
- Each of the constructed faceted (member) concepts will indicate the &quot;teacher&quot; also as a skos:broader concept.
- Each of the constructed faceted (member) concepts will indicate the &quot;teacher&quot; as the esco:constructedFrom concept.

Example (completed): Nesting facets - Teacher of a subject at a school level
- Assume we have a classification of subjects of education (e.g. &quot;mother tongue&quot;, &quot;mathematics&quot;, &quot;theorethical quantum mechanics&quot;).
  Two facet groups are created for this facet (education subject):
  1) Facet Group: Basic Education Subjects (with &quot;mother tongue&quot;, &quot;mathematics&quot;)
  2) Facet Group: Advanced Education Subjects (with &quot;mother tongue&quot;, &quot;mathematics&quot;, &quot;theorethical quantum mechanics&quot;)
- The faceted concepts of the &apos;started&apos; part of the example (&quot;primary school teacher&quot;, &quot;high school teacher&quot;, &quot;university teacher&quot;)
   can be further specialized with the &apos;Basic Education Subjects&apos; or &apos;Advanced Education Subjects&apos;.
- The resulting constructed facets can be &quot;high school teacher mathematics&quot;, &quot;university teacher mathematics&quot;, &quot;university teacher theorethical quantum mechanics&quot;, ...
- The skos:broader for the new faceted concepts are:
  1) for &quot;university teacher mathematics&quot; and for &quot;university teacher theorethical quantum mechanics&quot; : &quot;university teacher&quot;
  2) for &quot;high school teacher mathematics&quot; : &quot;high school teacher&quot;
  3) ...
- Each of these (more) specialized faceted concepts all have the (simple) ESCO occupation &quot;Teacher&quot; as value for esco:constructedFrom</rdfs:comment>
        <rdfs:isDefinedBy rdf:resource="http://data.europa.eu/esco/model"/>
        <rdfs:label xml:lang="en">constructed from ESCO concept</rdfs:label>
        <owl:deprecated rdf:datatype="http://www.w3.org/2001/XMLSchema#boolean">true</owl:deprecated>
        <vs:term_status rdf:datatype="http://www.w3.org/2001/XMLSchema#string">rejected</vs:term_status>
    </owl:ObjectProperty>



    <!-- http://data.europa.eu/esco/model#facet -->

    <owl:ObjectProperty rdf:about="http://data.europa.eu/esco/model#facet">
        <rdfs:domain>
            <owl:Class>
                <owl:unionOf rdf:parseType="Collection">
                    <rdf:Description rdf:about="http://www.w3.org/2004/02/skos/core#Collection"/>
                    <rdf:Description rdf:about="http://www.w3.org/2004/02/skos/core#Concept"/>
                </owl:unionOf>
            </owl:Class>
        </rdfs:domain>
        <rdfs:range rdf:resource="http://data.europa.eu/esco/model#FacetConceptGroup"/>
        <terms:issued rdf:datatype="http://www.w3.org/2001/XMLSchema#date">2013-12-03</terms:issued>
        <terms:modified rdf:datatype="http://www.w3.org/2001/XMLSchema#date">2016-06-08</terms:modified>
        <rdfs:comment xml:lang="en">The facet concept group, a group of concepts used to expand:
- the subject (ESCO) concept
  or
- all the members concepts of the subject Collection
to build ESCO (compound) faceted concepts.

An ESCO concept may have different aspects or facets that can specialize the ESCO concept.
A well known example is the (foreign) language skills.
- the main aspect of the (foreign) language skill is the identification of the foreign language
  The specialized concepts thus constructed are:
   - (foreign) language skill Albanian,
   - (foreign) labguage skill Bulgarian,
   - ...
- the (main) facet (e.g. a set of languages) occasional is extended by (sub-) facets that can be added. E.g. a (sub-) facet of language (skill) are the specialized levels defined by CEFR writing, understanding interactively, ...)

The relationship between facet groups (in the example above &quot;language&quot; and &quot;CEFR language skill level&quot; can be made 2-way (from &quot;language&quot; to &quot;language skill level&quot; and the inverse). In addition, the &quot;(foreign) language skill&quot; can have as facet (i.e. be specialized) by as well &quot;language&quot; as by &quot;CEFR language skill level&quot;.  As a result, the ESCO concept &quot;(foreign) language skill&quot; can be specialized in two different ways:
- first by language then by language skill level
  or
- first by language skill level then by language
Both navigation hierarchies ultimatly hold the same set of (compound) faceted concepts (e.g. &quot;(foreign) language skill&quot; &quot;writing&quot; &quot;Bulgarian&quot;.
In general:
- concept
- - &amp;lt;concept by facet group 1&amp;gt;
- - - [concept + facet group 1 member]
- - - - &amp;lt;[concept + facet group 1 member] by facet group 2&amp;gt;
- - - - - [concept + facet group 1 member + facet group 2 member]
- - - - - ... (other facet group 2 members)
- - - ... (other facet group 1 members)
- - &amp;lt;concept by facet group 2&amp;gt;
- - - [concept + facet group 2 member]
- - - - &amp;lt;[concept + facet group 2 member] by facet group 1&amp;gt;
- - - - - [concept + facet group 2 member + facet group 1 member]
- - - - - ... (other facet group 1 members)
- - - ... (other facet group 2 members)</rdfs:comment>
        <rdfs:isDefinedBy rdf:resource="http://data.europa.eu/esco/model"/>
        <rdfs:label xml:lang="en">specializing facet</rdfs:label>
        <owl:deprecated rdf:datatype="http://www.w3.org/2001/XMLSchema#boolean">true</owl:deprecated>
        <vs:term_status rdf:datatype="http://www.w3.org/2001/XMLSchema#string">rejected</vs:term_status>
    </owl:ObjectProperty>



    <!-- http://data.europa.eu/esco/model#hasAccreditation -->

    <owl:ObjectProperty rdf:about="http://data.europa.eu/esco/model#hasAccreditation">
        <rdfs:domain rdf:resource="http://data.europa.eu/esco/model#Qualification"/>
        <rdfs:range rdf:resource="http://data.europa.eu/esco/model#Accreditation"/>
        <rdfs:comment xml:lang="en"></rdfs:comment>
        <rdfs:isDefinedBy rdf:resource="http://data.europa.eu/esco/model"/>
        <rdfs:label xml:lang="en">has accreditation</rdfs:label>
        <rdfs:seeAlso rdf:resource="http://data.europa.eu/esco/model#Accreditation"/>
    </owl:ObjectProperty>



    <!-- http://data.europa.eu/esco/model#hasAssociation -->

    <owl:ObjectProperty rdf:about="http://data.europa.eu/esco/model#hasAssociation">
        <rdf:type rdf:resource="http://www.w3.org/2002/07/owl#InverseFunctionalProperty"/>
        <rdfs:range rdf:resource="http://data.europa.eu/esco/model#AssociationObject"/>
        <rdfs:comment xml:lang="en">The detailed (typed, annotated and documented) association (see http://data.europa.eu/esco/model#AssociationObject) from a resource (e.g. a qualification) to a node in an other established framework.
			The association identifies a related semantic asset from another established framework. The inverse relation of esco:isAssociationFor entails the property esco:hasAssociation.</rdfs:comment>
        <rdfs:comment xml:lang="en">Used to express a learning outcome of a qualification as a relation from a qualification to an ESCO skill, competence or knowdledge.</rdfs:comment>
        <rdfs:comment xml:lang="en">Used to link a qualification to a qualification framework level.</rdfs:comment>
        <rdfs:comment xml:lang="en">Used to related a qualification to an occupation from a national, regional or international occupation classification system.</rdfs:comment>
        <rdfs:isDefinedBy rdf:resource="http://data.europa.eu/esco/model"/>
        <rdfs:label xml:lang="en">has association</rdfs:label>
        <rdfs:seeAlso rdf:resource="http://data.europa.eu/esco/model#AssociationObject"/>
        <rdfs:seeAlso rdf:resource="http://data.europa.eu/esco/model#isAssociationFor"/>
    </owl:ObjectProperty>



    <!-- http://data.europa.eu/esco/model#hasAwardingActivity -->

    <owl:ObjectProperty rdf:about="http://data.europa.eu/esco/model#hasAwardingActivity">
        <rdfs:domain rdf:resource="http://data.europa.eu/esco/model#Qualification"/>
        <rdfs:range rdf:resource="http://data.europa.eu/esco/model#AwardingActivity"/>
        <rdfs:comment xml:lang="en">an awarding activity of a qualification</rdfs:comment>
        <rdfs:isDefinedBy rdf:resource="http://data.europa.eu/esco/model"/>
        <rdfs:label xml:lang="en">has awarding activity</rdfs:label>
        <rdfs:seeAlso rdf:resource="http://data.europa.eu/esco/model#AwardingActivity"/>
    </owl:ObjectProperty>



    <!-- http://data.europa.eu/esco/model#hasAwardingBody -->

    <owl:ObjectProperty rdf:about="http://data.europa.eu/esco/model#hasAwardingBody">
        <rdfs:subPropertyOf rdf:resource="http://purl.org/dc/terms/subject"/>
        <rdfs:range rdf:resource="http://data.europa.eu/esco/model#AwardingBody"/>
        <terms:issued rdf:datatype="http://www.w3.org/2001/XMLSchema#date">2013-06-27</terms:issued>
        <terms:modified rdf:datatype="http://www.w3.org/2001/XMLSchema#date">2013-06-27</terms:modified>
        <rdfs:comment xml:lang="en">The institutiution, organisation or company that issues the (subject) qualification (certification).</rdfs:comment>
        <rdfs:isDefinedBy rdf:resource="http://data.europa.eu/esco/model"/>
        <rdfs:label xml:lang="en">has awarding body</rdfs:label>
        <vs:term_status>released</vs:term_status>
    </owl:ObjectProperty>



    <!-- http://data.europa.eu/esco/model#hasDivisionCharacteristic -->

    <owl:ObjectProperty rdf:about="http://data.europa.eu/esco/model#hasDivisionCharacteristic">
        <rdfs:domain rdf:resource="http://purl.org/iso25964/skos-thes#ThesaurusArray"/>
        <rdfs:range rdf:resource="http://data.europa.eu/esco/model#FacetConceptGroup"/>
        <terms:issued rdf:datatype="http://www.w3.org/2001/XMLSchema#date">2014-03-07</terms:issued>
        <terms:modified rdf:datatype="http://www.w3.org/2001/XMLSchema#date">2016-06-08</terms:modified>
        <rdfs:comment xml:lang="en">The ESCO facet group the thesaurus array is being built from.

When an ESCO concept is specialized by a facet group, the ESCO thesaurus introduces that set (or branch) of specializations with a Thesaurus.Array.

Example: The occupation &quot;Teacher&quot; can be specialized by &apos;education level&apos; or by &apos;education subject&apos;.
At concept development time this is typically specified with respective esco:facet properties, one identifying the facet-group for education level, anoher identifying the facet-group holding the instructed subject areas.
At concept publication time, each specializing facet will be represented as an iso-thes:ThesaurusArray having as members the (compound) faceted concepts.
For each ESCO thesaurus array this property (esco:hasDivisionCharacteristic) recalls the FacetGroup it was created for.

Note: Complementary to esco:hasDivisionCharacteristic the iso-thes:superOrdinate identifies the ESCO member concept used to create the faceted concepts that are members of the thesaurus array.</rdfs:comment>
        <rdfs:isDefinedBy rdf:resource="http://data.europa.eu/esco/model"/>
        <rdfs:label xml:lang="en">division characteristic</rdfs:label>
        <rdfs:seeAlso rdf:resource="http://data.europa.eu/esco/model#facet"/>
        <rdfs:seeAlso rdf:resource="http://purl.org/iso25964/skos-thes#superOrdinate"/>
        <owl:deprecated rdf:datatype="http://www.w3.org/2001/XMLSchema#boolean">true</owl:deprecated>
        <vs:term_status rdf:datatype="http://www.w3.org/2001/XMLSchema#string">rejected</vs:term_status>
    </owl:ObjectProperty>



    <!-- http://data.europa.eu/esco/model#hasEQFLevel -->

    <owl:ObjectProperty rdf:about="http://data.europa.eu/esco/model#hasEQFLevel">
        <rdfs:subPropertyOf rdf:resource="http://purl.org/dc/terms/subject"/>
        <rdfs:range rdf:resource="http://data.europa.eu/esco/model#EQFLevel"/>
        <terms:issued rdf:datatype="http://www.w3.org/2001/XMLSchema#date">2013-06-27</terms:issued>
        <terms:modified rdf:datatype="http://www.w3.org/2001/XMLSchema#date">2013-06-27</terms:modified>
        <rdfs:comment xml:lang="en">The level (as specified by the European Qualification Framework) applicable to the subject qualification.</rdfs:comment>
        <rdfs:isDefinedBy rdf:resource="http://data.europa.eu/esco/model"/>
        <rdfs:label xml:lang="en">has EQF Level</rdfs:label>
        <owl:deprecated rdf:datatype="http://www.w3.org/2001/XMLSchema#boolean">true</owl:deprecated>
        <vs:term_status rdf:datatype="http://www.w3.org/2001/XMLSchema#string">deprecated</vs:term_status>
    </owl:ObjectProperty>



    <!-- http://data.europa.eu/esco/model#hasEntryRequirement -->

    <owl:ObjectProperty rdf:about="http://data.europa.eu/esco/model#hasEntryRequirement">
        <rdfs:domain rdf:resource="http://data.europa.eu/esco/model#Qualification"/>
        <rdfs:range rdf:resource="http://data.europa.eu/esco/model#EntryRequirement"/>
        <rdfs:comment xml:lang="en">an entry requirement of a qualification</rdfs:comment>
        <rdfs:isDefinedBy rdf:resource="http://data.europa.eu/esco/model"/>
        <rdfs:label xml:lang="en">has entry requirement</rdfs:label>
        <rdfs:seeAlso rdf:resource="http://data.europa.eu/esco/model#EntryRequirement"/>
    </owl:ObjectProperty>



    <!-- http://data.europa.eu/esco/model#hasFacet -->

    <owl:ObjectProperty rdf:about="http://data.europa.eu/esco/model#hasFacet">
        <rdfs:domain rdf:resource="http://data.europa.eu/esco/model#FacetedConcept"/>
        <rdfs:range rdf:resource="http://www.w3.org/2004/02/skos/core#Concept"/>
        <terms:issued rdf:datatype="http://www.w3.org/2001/XMLSchema#date">2013-12-03</terms:issued>
        <terms:modified rdf:datatype="http://www.w3.org/2001/XMLSchema#date">2016-06-08</terms:modified>
        <rdfs:comment xml:lang="en">A faceted ESCO concept (e.g.) is a compound concept constructed from an ESCO pillar concept and one or more facets.
The typical example is the (foreign) language skills.
- The ESCO concept is the skill: foreign language expertise.
The facets are:
  - the specific language of the expertise (en, fr, el, bg, nl ... )
  - the skill levels defined by CEFR (writing, understanding interactively, ...).</rdfs:comment>
        <rdfs:isDefinedBy rdf:resource="http://data.europa.eu/esco/model"/>
        <rdfs:label xml:lang="en">has facet</rdfs:label>
        <owl:deprecated rdf:datatype="http://www.w3.org/2001/XMLSchema#boolean">true</owl:deprecated>
        <vs:term_status rdf:datatype="http://www.w3.org/2001/XMLSchema#string">rejected</vs:term_status>
    </owl:ObjectProperty>



    <!-- http://data.europa.eu/esco/model#hasFoETCode -->

    <owl:ObjectProperty rdf:about="http://data.europa.eu/esco/model#hasFoETCode">
        <rdfs:subPropertyOf rdf:resource="http://purl.org/dc/terms/subject"/>
        <rdfs:range rdf:resource="http://data.europa.eu/esco/model#FoETCode"/>
        <terms:issued rdf:datatype="http://www.w3.org/2001/XMLSchema#date">2013-12-03</terms:issued>
        <terms:modified rdf:datatype="http://www.w3.org/2001/XMLSchema#date">2013-12-03</terms:modified>
        <rdfs:comment xml:lang="en">A tagging concept identifying the Field of Education Code as specified by the UNESCO Institute for Statistics (UIS).</rdfs:comment>
        <rdfs:isDefinedBy rdf:resource="http://data.europa.eu/esco/model"/>
        <rdfs:label xml:lang="en">has FoET Code</rdfs:label>
        <owl:deprecated rdf:datatype="http://www.w3.org/2001/XMLSchema#boolean">true</owl:deprecated>
        <vs:term_status>deprecated</vs:term_status>
    </owl:ObjectProperty>



    <!-- http://data.europa.eu/esco/model#hasGroupMember -->

    <owl:ObjectProperty rdf:about="http://data.europa.eu/esco/model#hasGroupMember">
        <rdfs:subPropertyOf rdf:resource="http://www.w3.org/2004/02/skos/core#narrowerTransitive"/>
        <owl:inverseOf rdf:resource="http://data.europa.eu/esco/model#memberOfGroup"/>
        <rdfs:domain rdf:resource="http://data.europa.eu/esco/model#GroupConcept"/>
        <rdfs:range rdf:resource="http://data.europa.eu/esco/model#MemberConcept"/>
        <terms:issued rdf:datatype="http://www.w3.org/2001/XMLSchema#date">2013-12-03</terms:issued>
        <terms:modified rdf:datatype="http://www.w3.org/2001/XMLSchema#date">2016-06-10</terms:modified>
        <rdfs:comment xml:lang="en">Identifies the member Concept of the (subject) Group concept.</rdfs:comment>
        <rdfs:isDefinedBy rdf:resource="http://data.europa.eu/esco/model"/>
        <rdfs:label xml:lang="en">has group member</rdfs:label>
        <owl:deprecated rdf:datatype="http://www.w3.org/2001/XMLSchema#boolean">true</owl:deprecated>
        <vs:term_status rdf:datatype="http://www.w3.org/2001/XMLSchema#string">deprecated</vs:term_status>
    </owl:ObjectProperty>



    <!-- http://data.europa.eu/esco/model#hasISCED-FCode -->

    <owl:ObjectProperty rdf:about="http://data.europa.eu/esco/model#hasISCED-FCode">
        <rdfs:subPropertyOf rdf:resource="http://purl.org/dc/terms/subject"/>
        <rdfs:range rdf:resource="http://www.w3.org/2004/02/skos/core#Concept"/>
        <terms:created rdf:datatype="http://www.w3.org/2001/XMLSchema#date">2016-06-10</terms:created>
        <terms:modified rdf:datatype="http://www.w3.org/2001/XMLSchema#date">2016-06-10</terms:modified>
        <rdfs:comment xml:lang="en">A tagging concept identifying the ISCED 2013 FoET classification code (Field of Education Code). It is used to indicate the thematic area of a qualification.</rdfs:comment>
        <rdfs:isDefinedBy rdf:resource="http://data.europe.eu/esco/model"/>
        <rdfs:label xml:lang="en">ISCED FoET Code</rdfs:label>
        <vs:term_status rdf:datatype="http://www.w3.org/2001/XMLSchema#string">proposed</vs:term_status>
    </owl:ObjectProperty>



    <!-- http://data.europa.eu/esco/model#hasLabelRole -->

    <owl:ObjectProperty rdf:about="http://data.europa.eu/esco/model#hasLabelRole">
        <rdfs:subPropertyOf rdf:resource="http://purl.org/dc/terms/subject"/>
        <rdfs:domain rdf:resource="http://data.europa.eu/esco/model#Label"/>
        <rdfs:range rdf:resource="http://data.europa.eu/esco/model#LabelRole"/>
        <terms:issued rdf:datatype="http://www.w3.org/2001/XMLSchema#date">2013-12-03</terms:issued>
        <terms:modified rdf:datatype="http://www.w3.org/2001/XMLSchema#date">2013-12-03</terms:modified>
        <rdfs:comment xml:lang="en">A tagging concept providing the gender specific typing of an ESCO label.
Each ESCO label can have
- at most 1 label that is standard male and zero or more labels that are male
- at most 1 label that is standard female and zero or more labels that are female
- any label that is not male or female is considered neutral
- a male respectively female preferred label is the standard male respectively standard female label
</rdfs:comment>
        <rdfs:isDefinedBy rdf:resource="http://data.europa.eu/esco/model"/>
        <rdfs:label xml:lang="en">has label role</rdfs:label>
        <vs:term_status>released</vs:term_status>
    </owl:ObjectProperty>



    <!-- http://data.europa.eu/esco/model#hasNACECode -->

    <owl:ObjectProperty rdf:about="http://data.europa.eu/esco/model#hasNACECode">
        <rdfs:subPropertyOf rdf:resource="http://purl.org/dc/terms/subject"/>
        <rdfs:range rdf:resource="http://data.europa.eu/esco/model#NACECode"/>
        <terms:issued rdf:datatype="http://www.w3.org/2001/XMLSchema#date">2013-12-03</terms:issued>
        <terms:modified rdf:datatype="http://www.w3.org/2001/XMLSchema#date">2013-12-03</terms:modified>
        <rdfs:comment xml:lang="en">A tagging concept using the NACE codes to specify the industry sector of the tagged subject.</rdfs:comment>
        <rdfs:isDefinedBy rdf:resource="http://data.europa.eu/esco/model"/>
        <rdfs:label xml:lang="en">has NACE code</rdfs:label>
        <vs:term_status>released</vs:term_status>
    </owl:ObjectProperty>



    <!-- http://data.europa.eu/esco/model#hasPolyHierarchy -->

    <owl:ObjectProperty rdf:about="http://data.europa.eu/esco/model#hasPolyHierarchy">
        <rdfs:domain rdf:resource="http://data.europa.eu/esco/model#ConceptScheme"/>
    </owl:ObjectProperty>



    <!-- http://data.europa.eu/esco/model#hasRecognition -->

    <owl:ObjectProperty rdf:about="http://data.europa.eu/esco/model#hasRecognition">
        <rdfs:domain rdf:resource="http://data.europa.eu/esco/model#Qualification"/>
        <rdfs:range rdf:resource="http://data.europa.eu/esco/model#Recognition"/>
        <rdfs:comment xml:lang="en"></rdfs:comment>
        <rdfs:isDefinedBy rdf:resource="http://data.europa.eu/esco/model"/>
        <rdfs:label xml:lang="en">has recogition</rdfs:label>
        <rdfs:seeAlso rdf:resource="http://data.europa.eu/esco/model#Recognition"/>
    </owl:ObjectProperty>



    <!-- http://data.europa.eu/esco/model#hasRelationship -->

    <owl:ObjectProperty rdf:about="http://data.europa.eu/esco/model#hasRelationship">
        <rdf:type rdf:resource="http://www.w3.org/2002/07/owl#InverseFunctionalProperty"/>
        <rdfs:domain rdf:resource="http://data.europa.eu/esco/model#Concept"/>
        <rdfs:range rdf:resource="http://data.europa.eu/esco/model#Relationship"/>
        <terms:issued rdf:datatype="http://www.w3.org/2001/XMLSchema#date">2013-12-03</terms:issued>
        <terms:modified rdf:datatype="http://www.w3.org/2001/XMLSchema#date">2014-11-14</terms:modified>
        <rdfs:comment xml:lang="en">The detailed (typed, annotated and documented) ESCO relationship (see http://data.europa.eu/esco/model#Relationship) for the subject ESCO concept.

The relationship identifies a related ESCO concept.
The inverse relations of esco:refersConcept and of esco:isRelationshipFor entail the property esco:hasRelationship.
The relationship properties provide formal semantics to the ESCO concept relationship.</rdfs:comment>
        <rdfs:isDefinedBy rdf:resource="http://data.europa.eu/esco/model"/>
        <rdfs:label xml:lang="en">has ESCO relationship</rdfs:label>
        <rdfs:seeAlso rdf:resource="http://data.europa.eu/esco/model#Relationship"/>
        <rdfs:seeAlso rdf:resource="http://data.europa.eu/esco/model#isRelationshipFor"/>
        <rdfs:seeAlso rdf:resource="http://data.europa.eu/esco/model#refersConcept"/>
        <owl:deprecated rdf:datatype="http://www.w3.org/2001/XMLSchema#boolean">true</owl:deprecated>
        <vs:term_status rdf:datatype="http://www.w3.org/2001/XMLSchema#string">deprecated</vs:term_status>
    </owl:ObjectProperty>



    <!-- http://data.europa.eu/esco/model#hasRelationshipList -->

    <owl:ObjectProperty rdf:about="http://data.europa.eu/esco/model#hasRelationshipList">
        <rdfs:domain rdf:resource="http://data.europa.eu/esco/model#Concept"/>
        <rdfs:range rdf:resource="http://www.w3.org/1999/02/22-rdf-syntax-ns#List"/>
        <terms:issued rdf:datatype="http://www.w3.org/2001/XMLSchema#date">2014-10-23</terms:issued>
        <terms:modified rdf:datatype="http://www.w3.org/2001/XMLSchema#date">2016-06-08</terms:modified>
        <rdfs:comment xml:lang="en">The ordered set of relationships starting at the subject ESCO pillar concept.

For any resource, every item in the list given as the value of the
      esco:hasRelationshipList property is also a value of the esco:hasRelationship property.</rdfs:comment>
        <rdfs:isDefinedBy rdf:resource="http://data.europa.eu/esco/model"/>
        <rdfs:label xml:lang="en">has ESCO relationship list</rdfs:label>
        <rdfs:seeAlso rdf:resource="http://data.europa.eu/esco/model#Relationship"/>
        <rdfs:seeAlso rdf:resource="http://data.europa.eu/esco/model#hasRelationship"/>
        <owl:deprecated rdf:datatype="http://www.w3.org/2001/XMLSchema#boolean">true</owl:deprecated>
        <vs:term_status rdf:datatype="http://www.w3.org/2001/XMLSchema#string">rejected</vs:term_status>
    </owl:ObjectProperty>



    <!-- http://data.europa.eu/esco/model#hasRelationshipType -->

    <owl:ObjectProperty rdf:about="http://data.europa.eu/esco/model#hasRelationshipType">
        <rdfs:subPropertyOf rdf:resource="http://purl.org/dc/terms/subject"/>
        <rdfs:domain rdf:resource="http://data.europa.eu/esco/model#Relationship"/>
        <rdfs:range rdf:resource="http://data.europa.eu/esco/model#RelationshipType"/>
        <terms:issued rdf:datatype="http://www.w3.org/2001/XMLSchema#date">2014-04-16</terms:issued>
        <terms:modified rdf:datatype="http://www.w3.org/2001/XMLSchema#date">2014-04-16</terms:modified>
        <rdfs:comment xml:lang="en">A tagging concept detailing the type of the (subject) ESCO relationship</rdfs:comment>
        <rdfs:isDefinedBy rdf:resource="http://data.europa.eu/esco/model"/>
        <rdfs:label xml:lang="en">has ESCO relationship type</rdfs:label>
        <owl:deprecated rdf:datatype="http://www.w3.org/2001/XMLSchema#boolean">true</owl:deprecated>
        <vs:term_status>rejected</vs:term_status>
    </owl:ObjectProperty>



    <!-- http://data.europa.eu/esco/model#hasTopConceptList -->

    <owl:ObjectProperty rdf:about="http://data.europa.eu/esco/model#hasTopConceptList">
        <rdfs:domain rdf:resource="http://www.w3.org/2004/02/skos/core#ConceptScheme"/>
        <rdfs:range rdf:resource="http://www.w3.org/1999/02/22-rdf-syntax-ns#List"/>
        <terms:issued rdf:datatype="http://www.w3.org/2001/XMLSchema#date">2014-11-14</terms:issued>
        <terms:modified rdf:datatype="http://www.w3.org/2001/XMLSchema#date">2016-06-08</terms:modified>
        <rdfs:comment xml:lang="en">The ordered set of top concepts of the subject conceptscheme.

For any resource, every item in the list given as the value of the
      esco:hasTopConceptList property is also a value of the skos:hasTopConcept property.</rdfs:comment>
        <rdfs:isDefinedBy rdf:resource="http://data.europa.eu/esco/model"/>
        <rdfs:label xml:lang="en">has top concept list</rdfs:label>
        <rdfs:seeAlso rdf:resource="http://www.w3.org/2004/02/skos/core#hasTopConcept"/>
        <owl:deprecated rdf:datatype="http://www.w3.org/2001/XMLSchema#boolean">true</owl:deprecated>
        <vs:term_status rdf:datatype="http://www.w3.org/2001/XMLSchema#string">rejected</vs:term_status>
    </owl:ObjectProperty>



    <!-- http://data.europa.eu/esco/model#hasWorkContext -->

    <owl:ObjectProperty rdf:about="http://data.europa.eu/esco/model#hasWorkContext">
        <rdfs:subPropertyOf rdf:resource="http://purl.org/dc/terms/subject"/>
        <rdfs:range rdf:resource="http://data.europa.eu/esco/model#WorkContext"/>
        <terms:issued rdf:datatype="http://www.w3.org/2001/XMLSchema#date">2014-08-10</terms:issued>
        <terms:modified rdf:datatype="http://www.w3.org/2001/XMLSchema#date">2014-08-10</terms:modified>
        <rdfs:comment xml:lang="en">The possible working context of the (subject) occupation.</rdfs:comment>
        <rdfs:isDefinedBy rdf:resource="http://data.europa.eu/esco/model"/>
        <rdfs:label xml:lang="en">can have work context</rdfs:label>
        <vs:term_status>proposed</vs:term_status>
    </owl:ObjectProperty>



    <!-- http://data.europa.eu/esco/model#isAssociationFor -->

    <owl:ObjectProperty rdf:about="http://data.europa.eu/esco/model#isAssociationFor">
        <rdf:type rdf:resource="http://www.w3.org/2002/07/owl#FunctionalProperty"/>
        <rdfs:domain rdf:resource="http://data.europa.eu/esco/model#AssociationObject"/>
        <rdfs:comment xml:lang="en">The resource being described (the resource the association starts from e.g. a qualification). This property entails the inverse property http://data.europa.eu/esco/model#hasAssociation.</rdfs:comment>
        <rdfs:isDefinedBy rdf:resource="http://data.europa.eu/esco/model"/>
        <rdfs:label xml:lang="en">association from</rdfs:label>
        <rdfs:seeAlso rdf:resource="http://data.europa.eu/esco/model#AssociationObject"/>
        <rdfs:seeAlso rdf:resource="http://data.europa.eu/esco/model#hasAssociation"/>
    </owl:ObjectProperty>



    <!-- http://data.europa.eu/esco/model#isCompetenceFor -->

    <owl:ObjectProperty rdf:about="http://data.europa.eu/esco/model#isCompetenceFor">
        <rdfs:subPropertyOf rdf:resource="http://www.w3.org/2004/02/skos/core#related"/>
        <owl:inverseOf rdf:resource="http://data.europa.eu/esco/model#relatedCompetence"/>
        <rdfs:domain rdf:resource="http://data.europa.eu/esco/model#Skill"/>
        <rdfs:range rdf:resource="http://data.europa.eu/esco/model#Qualification"/>
        <terms:issued rdf:datatype="http://www.w3.org/2001/XMLSchema#date">2014-11-14</terms:issued>
        <terms:modified rdf:datatype="http://www.w3.org/2001/XMLSchema#date">2014-11-14</terms:modified>
        <rdfs:comment xml:lang="en">The inverse of esco:relatedCompetence.</rdfs:comment>
        <rdfs:isDefinedBy rdf:resource="http://data.europa.eu/esco/model"/>
        <rdfs:label xml:lang="en">is a learning outcome of</rdfs:label>
        <owl:deprecated rdf:datatype="http://www.w3.org/2001/XMLSchema#boolean">true</owl:deprecated>
        <vs:term_status rdf:datatype="http://www.w3.org/2001/XMLSchema#string">deprecated</vs:term_status>
    </owl:ObjectProperty>



    <!-- http://data.europa.eu/esco/model#isEssentialSkillFor -->

    <owl:ObjectProperty rdf:about="http://data.europa.eu/esco/model#isEssentialSkillFor">
        <rdfs:subPropertyOf rdf:resource="http://www.w3.org/2004/02/skos/core#related"/>
        <owl:inverseOf rdf:resource="http://data.europa.eu/esco/model#relatedEssentialSkill"/>
        <rdfs:domain rdf:resource="http://data.europa.eu/esco/model#Skill"/>
        <rdfs:range>
            <owl:Class>
                <owl:unionOf rdf:parseType="Collection">
                    <rdf:Description rdf:about="http://data.europa.eu/esco/model#Occupation"/>
                    <rdf:Description rdf:about="http://data.europa.eu/esco/model#Skill"/>
                </owl:unionOf>
            </owl:Class>
        </rdfs:range>
        <terms:issued rdf:datatype="http://www.w3.org/2001/XMLSchema#date">2014-08-10</terms:issued>
        <terms:modified rdf:datatype="http://www.w3.org/2001/XMLSchema#date">2014-08-10</terms:modified>
        <rdfs:comment xml:lang="en">The inverse of esco:relatedEssentialSkill.</rdfs:comment>
        <rdfs:isDefinedBy rdf:resource="http://data.europa.eu/esco/model"/>
        <rdfs:label xml:lang="en">is essential skill for</rdfs:label>
        <vs:term_status rdf:datatype="http://www.w3.org/2001/XMLSchema#string">proposed</vs:term_status>
    </owl:ObjectProperty>



    <!-- http://data.europa.eu/esco/model#isIndirect -->

    <owl:ObjectProperty rdf:about="http://data.europa.eu/esco/model#isIndirect">
        <rdfs:domain rdf:resource="http://data.europa.eu/esco/model#Concept"/>
    </owl:ObjectProperty>



    <!-- http://data.europa.eu/esco/model#isLegallyRequiredQualificationFor -->

    <owl:ObjectProperty rdf:about="http://data.europa.eu/esco/model#isLegallyRequiredQualificationFor">
        <rdfs:subPropertyOf rdf:resource="http://www.w3.org/2004/02/skos/core#related"/>
        <owl:inverseOf rdf:resource="http://data.europa.eu/esco/model#relatedLegallyRequiredQualification"/>
        <rdfs:domain rdf:resource="http://data.europa.eu/esco/model#Qualification"/>
        <rdfs:range>
            <owl:Class>
                <owl:unionOf rdf:parseType="Collection">
                    <rdf:Description rdf:about="http://data.europa.eu/esco/model#Occupation"/>
                    <rdf:Description rdf:about="http://data.europa.eu/esco/model#Skill"/>
                </owl:unionOf>
            </owl:Class>
        </rdfs:range>
        <terms:issued rdf:datatype="http://www.w3.org/2001/XMLSchema#date">2014-11-14</terms:issued>
        <terms:modified rdf:datatype="http://www.w3.org/2001/XMLSchema#date">2014-11-14</terms:modified>
        <rdfs:comment xml:lang="en">The inverse of esco:relatedLegallyRequiredQualification</rdfs:comment>
        <rdfs:isDefinedBy rdf:resource="http://data.europa.eu/esco/model"/>
        <rdfs:label xml:lang="en">is legally required qualification for</rdfs:label>
        <vs:term_status rdf:datatype="http://www.w3.org/2001/XMLSchema#string">rejected</vs:term_status>
				<owl:deprecated rdf:datatype="http://www.w3.org/2001/XMLSchema#boolean">true</owl:deprecated>
    </owl:ObjectProperty>



    <!-- http://data.europa.eu/esco/model#isOptionalSkillFor -->

    <owl:ObjectProperty rdf:about="http://data.europa.eu/esco/model#isOptionalSkillFor">
        <rdfs:subPropertyOf rdf:resource="http://www.w3.org/2004/02/skos/core#related"/>
        <owl:inverseOf rdf:resource="http://data.europa.eu/esco/model#relatedOptionalSkill"/>
        <rdfs:domain rdf:resource="http://data.europa.eu/esco/model#Skill"/>
        <rdfs:range>
            <owl:Class>
                <owl:unionOf rdf:parseType="Collection">
                    <rdf:Description rdf:about="http://data.europa.eu/esco/model#Occupation"/>
                    <rdf:Description rdf:about="http://data.europa.eu/esco/model#Skill"/>
                </owl:unionOf>
            </owl:Class>
        </rdfs:range>
        <terms:issued rdf:datatype="http://www.w3.org/2001/XMLSchema#date">2014-08-10</terms:issued>
        <terms:modified rdf:datatype="http://www.w3.org/2001/XMLSchema#date">2014-08-10</terms:modified>
        <rdfs:comment xml:lang="en">The inverse of esco:relatedOptionalSkill.</rdfs:comment>
        <rdfs:isDefinedBy rdf:resource="http://data.europa.eu/esco/model"/>
        <rdfs:label xml:lang="en">is optional skill for</rdfs:label>
        <vs:term_status rdf:datatype="http://www.w3.org/2001/XMLSchema#string">proposed</vs:term_status>
    </owl:ObjectProperty>



    <!-- http://data.europa.eu/esco/model#isQualificationFor -->

    <owl:ObjectProperty rdf:about="http://data.europa.eu/esco/model#isQualificationFor">
        <rdfs:subPropertyOf rdf:resource="http://www.w3.org/2004/02/skos/core#related"/>
        <owl:inverseOf rdf:resource="http://data.europa.eu/esco/model#relatedQualification"/>
        <rdfs:domain rdf:resource="http://data.europa.eu/esco/model#Qualification"/>
        <rdfs:range>
            <owl:Class>
                <owl:unionOf rdf:parseType="Collection">
                    <rdf:Description rdf:about="http://data.europa.eu/esco/model#Occupation"/>
                    <rdf:Description rdf:about="http://data.europa.eu/esco/model#Skill"/>
                </owl:unionOf>
            </owl:Class>
        </rdfs:range>
        <terms:issued rdf:datatype="http://www.w3.org/2001/XMLSchema#date">2014-11-14</terms:issued>
        <terms:modified rdf:datatype="http://www.w3.org/2001/XMLSchema#date">2014-11-14</terms:modified>
        <rdfs:comment xml:lang="en">The inverse of esco:relatedQualification.</rdfs:comment>
        <rdfs:isDefinedBy rdf:resource="http://data.europa.eu/esco/model"/>
        <rdfs:label xml:lang="en">is qualification for</rdfs:label>
        <owl:deprecated rdf:datatype="http://www.w3.org/2001/XMLSchema#boolean">true</owl:deprecated>				   <vs:term_status rdf:datatype="http://www.w3.org/2001/XMLSchema#string">reject</vs:term_status>
    </owl:ObjectProperty>



    <!-- http://data.europa.eu/esco/model#isRelationshipFor -->

    <owl:ObjectProperty rdf:about="http://data.europa.eu/esco/model#isRelationshipFor">
        <rdf:type rdf:resource="http://www.w3.org/2002/07/owl#FunctionalProperty"/>
        <rdfs:domain rdf:resource="http://data.europa.eu/esco/model#Relationship"/>
        <rdfs:range rdf:resource="http://data.europa.eu/esco/model#Concept"/>
        <terms:issued rdf:datatype="http://www.w3.org/2001/XMLSchema#date">2013-12-03</terms:issued>
        <terms:modified rdf:datatype="http://www.w3.org/2001/XMLSchema#date">2017-02-10</terms:modified>
        <rdfs:comment xml:lang="en">The ESCO concept the (subject) relationship starts from (see http://data.europa.eu/esco/model#Relationship).</rdfs:comment>
        <rdfs:isDefinedBy rdf:resource="http://data.europa.eu/esco/model"/>
        <rdfs:label xml:lang="en">from ESCO concept</rdfs:label>
        <owl:deprecated rdf:datatype="http://www.w3.org/2001/XMLSchema#boolean">true</owl:deprecated>
        <vs:term_status rdf:datatype="http://www.w3.org/2001/XMLSchema#string">rejected</vs:term_status>
    </owl:ObjectProperty>



    <!-- http://data.europa.eu/esco/model#language -->

    <owl:ObjectProperty rdf:about="http://data.europa.eu/esco/model#language"/>



    <!-- http://data.europa.eu/esco/model#location -->

    <owl:ObjectProperty rdf:about="http://data.europa.eu/esco/model#location">
        <rdfs:subPropertyOf rdf:resource="http://purl.org/dc/terms/subject"/>
        <rdfs:range rdf:resource="http://data.europa.eu/esco/model#Location"/>
        <terms:issued rdf:datatype="http://www.w3.org/2001/XMLSchema#date">2013-06-27</terms:issued>
        <terms:modified rdf:datatype="http://www.w3.org/2001/XMLSchema#date">2013-06-27</terms:modified>
        <rdfs:comment xml:lang="en">The Country or region the subject is associated with.
Typically a tagging concept.</rdfs:comment>
        <rdfs:isDefinedBy rdf:resource="http://data.europa.eu/esco/model"/>
        <rdfs:label xml:lang="en">location</rdfs:label>
        <vs:term_status>proposed</vs:term_status>
        <vs:term_status>released</vs:term_status>
    </owl:ObjectProperty>



    <!-- http://data.europa.eu/esco/model#memberOfGroup -->

    <owl:ObjectProperty rdf:about="http://data.europa.eu/esco/model#memberOfGroup">
        <rdfs:subPropertyOf rdf:resource="http://www.w3.org/2004/02/skos/core#broaderTransitive"/>
        <rdfs:domain rdf:resource="http://data.europa.eu/esco/model#MemberConcept"/>
        <rdfs:range rdf:resource="http://data.europa.eu/esco/model#GroupConcept"/>
        <owl:propertyChainAxiom rdf:parseType="Collection">
            <rdf:Description rdf:about="http://data.europa.eu/esco/model#broaderInstance"/>
            <rdf:Description rdf:about="http://www.w3.org/2004/02/skos/core#broaderTransitive"/>
        </owl:propertyChainAxiom>
        <owl:propertyChainAxiom rdf:parseType="Collection">
            <rdf:Description rdf:about="http://data.europa.eu/esco/model#constructedFrom"/>
            <rdf:Description rdf:about="http://data.europa.eu/esco/model#broaderInstance"/>
            <rdf:Description rdf:about="http://www.w3.org/2004/02/skos/core#broaderTransitive"/>
        </owl:propertyChainAxiom>
        <terms:issued rdf:datatype="http://www.w3.org/2001/XMLSchema#date">2013-06-27</terms:issued>
        <terms:modified rdf:datatype="http://www.w3.org/2001/XMLSchema#date">2016-06-08</terms:modified>
        <rdfs:comment xml:lang="en">The ESCO Group (pillar) concept containing the subject ESCO concept as a member.</rdfs:comment>
        <rdfs:isDefinedBy rdf:resource="http://data.europa.eu/esco/model"/>
        <rdfs:label xml:lang="en">containing group</rdfs:label>
        <owl:deprecated rdf:datatype="http://www.w3.org/2001/XMLSchema#boolean">true</owl:deprecated>
        <vs:term_status rdf:datatype="http://www.w3.org/2001/XMLSchema#string">deprecated</vs:term_status>
    </owl:ObjectProperty>



    <!-- http://data.europa.eu/esco/model#memberOfISCOGroup -->

    <owl:ObjectProperty rdf:about="http://data.europa.eu/esco/model#memberOfISCOGroup">
        <terms:issued rdf:datatype="http://www.w3.org/2001/XMLSchema#date">2013-12-03</terms:issued>
        <terms:modified rdf:datatype="http://www.w3.org/2001/XMLSchema#date">2013-12-03</terms:modified>
        <rdfs:comment xml:lang="en">The direct hierarchical broader ISCO concept of the (subject) ESCO occupation.
The &apos;direct&apos; (or one step) relationship is to be understood in terms of extending the ISCO taxonomy the (object) concept belongs to.

The ISCO concept may be of any ISCO version.  The ISCO version can be determined by the inScheme property on the ISCO concept and the version information on the ISCO concept scheme (referenced by the object - i.e. by the ISCO concept).</rdfs:comment>
        <rdfs:isDefinedBy rdf:resource="http://data.europa.eu/esco/model"/>
        <rdfs:label xml:lang="en">belongs to ISCO Group with code</rdfs:label>
        <vs:term_status rdf:datatype="http://www.w3.org/2001/XMLSchema#string">proposed</vs:term_status>
    </owl:ObjectProperty>



    <!-- http://data.europa.eu/esco/model#narrowerInstance -->

    <owl:ObjectProperty rdf:about="http://data.europa.eu/esco/model#narrowerInstance">
        <rdfs:subPropertyOf rdf:resource="http://data.europa.eu/esco/model#hasGroupMember"/>
        <rdfs:subPropertyOf rdf:resource="http://purl.org/iso25964/skos-thes#narrowerInstantial"/>
        <rdfs:domain rdf:resource="http://data.europa.eu/esco/model#LeafGroupConcept"/>
        <rdfs:range rdf:resource="http://data.europa.eu/esco/model#MemberConcept"/>
        <rdfs:range rdf:resource="http://data.europa.eu/esco/model#SimpleConcept"/>
        <terms:issued rdf:datatype="http://www.w3.org/2001/XMLSchema#date">2013-06-27</terms:issued>
        <terms:modified rdf:datatype="http://www.w3.org/2001/XMLSchema#date">2016-06-10</terms:modified>
        <rdfs:comment xml:lang="en">The ESCO concepts (occupation, skill or qualification) that are immediate (one step) narrower concepts of the (subject) leaf group.  These narrower concepts are top level (member) concepts of the subject leaf concept group.

The (subject) leaf group may have more members, not provided by its esco:narrowerInstance properties.  Typically, these other members are specializations (e.g. faceted concepts) of the top level members of the (subject) leaf concept group.</rdfs:comment>
        <rdfs:isDefinedBy rdf:resource="http://data.europa.eu/esco/model"/>
        <rdfs:label xml:lang="en">narrower instance</rdfs:label>
        <owl:deprecated rdf:datatype="http://www.w3.org/2001/XMLSchema#boolean">true</owl:deprecated>
        <vs:term_status rdf:datatype="http://www.w3.org/2001/XMLSchema#string">deprecated</vs:term_status>
    </owl:ObjectProperty>



    <!-- http://data.europa.eu/esco/model#noteLiteral -->

    <owl:ObjectProperty rdf:about="http://data.europa.eu/esco/model#noteLiteral">
        <rdfs:range rdf:resource="http://www.w3.org/1999/02/22-rdf-syntax-ns#XMLLiteral"/>
    </owl:ObjectProperty>



    <!-- http://data.europa.eu/esco/model#plusUF -->

    <owl:ObjectProperty rdf:about="http://data.europa.eu/esco/model#plusUF">
        <rdfs:domain rdf:resource="http://data.europa.eu/esco/model#SimpleConcept"/>
        <rdfs:range rdf:resource="http://purl.org/iso25964/skos-thes#SplitNonPreferredTerm"/>
        <owl:propertyChainAxiom rdf:parseType="Collection">
            <rdf:Description rdf:about="http://www.w3.org/2008/05/skos-xl#prefLabel"/>
            <rdf:Description rdf:about="http://purl.org/iso25964/skos-thes#plusUFTerm"/>
        </owl:propertyChainAxiom>
        <terms:issued rdf:datatype="http://www.w3.org/2001/XMLSchema#date">2014-02-18</terms:issued>
        <terms:modified rdf:datatype="http://www.w3.org/2001/XMLSchema#date">2016-06-08</terms:modified>
        <rdfs:comment xml:lang="en">A compound equivalence label for the subject concept.
The subject concept is a Simple ESCO concept used as a component of a Faceted ESCO concept (i.e. a compound concept).
The label of this faceted concept is a compound term (i.e. a split non preferred term) and the value of esco:plusUF (i.e. a UF++).
There can be any number of compound terms per language and per faceted concept.</rdfs:comment>
        <rdfs:isDefinedBy rdf:resource="http://data.europa.eu/esco/model"/>
        <rdfs:label xml:lang="en">compound term</rdfs:label>
        <owl:deprecated rdf:datatype="http://www.w3.org/2001/XMLSchema#boolean">true</owl:deprecated>
        <vs:term_status>rejected</vs:term_status>
    </owl:ObjectProperty>



    <!-- http://data.europa.eu/esco/model#refersConcept -->

    <owl:ObjectProperty rdf:about="http://data.europa.eu/esco/model#refersConcept">
        <rdf:type rdf:resource="http://www.w3.org/2002/07/owl#FunctionalProperty"/>
        <rdfs:domain rdf:resource="http://data.europa.eu/esco/model#Relationship"/>
        <rdfs:range rdf:resource="http://data.europa.eu/esco/model#Concept"/>
        <terms:issued rdf:datatype="http://www.w3.org/2001/XMLSchema#date">2013-12-03</terms:issued>
        <terms:modified rdf:datatype="http://www.w3.org/2001/XMLSchema#date">2014-02-03</terms:modified>
        <rdfs:comment xml:lang="en">The ESCO concept referred by the (subject) ESCO relationship.
The esco:Relationship gives a more elaborate semantic description of related ESCO concepts.  These related concepts are identied by the esco:Relationship propertief
- esco:isRelationshipFor
- esco:refersConcept
Further semantics are provided by
- a relationshipt type
- a description
- .. (other possible extensions)</rdfs:comment>
        <rdfs:isDefinedBy rdf:resource="http://data.europa.eu/esco/model"/>
        <rdfs:label xml:lang="en">to ESCO concept</rdfs:label>
        <vs:term_status rdf:datatype="http://www.w3.org/2001/XMLSchema#string">proposed</vs:term_status>
    </owl:ObjectProperty>



    <!-- http://data.europa.eu/esco/model#relatedCompetence -->

    <owl:ObjectProperty rdf:about="http://data.europa.eu/esco/model#relatedCompetence">
        <rdfs:subPropertyOf rdf:resource="http://www.w3.org/2004/02/skos/core#related"/>
        <rdfs:domain rdf:resource="http://data.europa.eu/esco/model#Qualification"/>
        <rdfs:range rdf:resource="http://data.europa.eu/esco/model#Skill"/>
        <terms:issued rdf:datatype="http://www.w3.org/2001/XMLSchema#date">2013-12-03</terms:issued>
        <terms:modified rdf:datatype="http://www.w3.org/2001/XMLSchema#date">2014-11-09</terms:modified>
        <rdfs:comment xml:lang="en">The ESCO skill/competence related to (or asserted by) the subject ESCO qualification.
I.e. when asserted on a subject qualification, the related competence is a learning outcome of that qualification.</rdfs:comment>
        <rdfs:isDefinedBy rdf:resource="http://data.europa.eu/esco/model"/>
        <rdfs:label xml:lang="en">has learning outcome</rdfs:label>
        <owl:deprecated rdf:datatype="http://www.w3.org/2001/XMLSchema#boolean">true</owl:deprecated>
        <vs:term_status>rejected</vs:term_status>
    </owl:ObjectProperty>



    <!-- http://data.europa.eu/esco/model#relatedEssentialSkill -->

    <owl:ObjectProperty rdf:about="http://data.europa.eu/esco/model#relatedEssentialSkill">
        <rdfs:subPropertyOf rdf:resource="http://www.w3.org/2004/02/skos/core#related"/>
        <rdfs:domain>
            <owl:Class>
                <owl:unionOf rdf:parseType="Collection">
                    <rdf:Description rdf:about="http://data.europa.eu/esco/model#Occupation"/>
                    <rdf:Description rdf:about="http://data.europa.eu/esco/model#Skill"/>
                </owl:unionOf>
            </owl:Class>
        </rdfs:domain>
        <rdfs:range rdf:resource="http://data.europa.eu/esco/model#Skill"/>
        <terms:issued rdf:datatype="http://www.w3.org/2001/XMLSchema#date">2013-12-03</terms:issued>
        <terms:modified rdf:datatype="http://www.w3.org/2001/XMLSchema#date">2013-12-03</terms:modified>
        <rdfs:comment xml:lang="en">The ESCO skill or competence that is essential for the subject occupation or skill.</rdfs:comment>
        <rdfs:isDefinedBy rdf:resource="http://data.europa.eu/esco/model"/>
        <rdfs:label xml:lang="en">has essential skill</rdfs:label>
        <vs:term_status rdf:datatype="http://www.w3.org/2001/XMLSchema#string">proposed</vs:term_status>
    </owl:ObjectProperty>



    <!-- http://data.europa.eu/esco/model#relatedLegallyRequiredQualification -->

    <owl:ObjectProperty rdf:about="http://data.europa.eu/esco/model#relatedLegallyRequiredQualification">
        <rdfs:subPropertyOf rdf:resource="http://www.w3.org/2004/02/skos/core#related"/>
        <rdfs:domain>
            <owl:Class>
                <owl:unionOf rdf:parseType="Collection">
                    <rdf:Description rdf:about="http://data.europa.eu/esco/model#Occupation"/>
                    <rdf:Description rdf:about="http://data.europa.eu/esco/model#Skill"/>
                </owl:unionOf>
            </owl:Class>
        </rdfs:domain>
        <rdfs:range rdf:resource="http://data.europa.eu/esco/model#Qualification"/>
        <terms:issued rdf:datatype="http://www.w3.org/2001/XMLSchema#date">2013-12-03</terms:issued>
        <terms:modified rdf:datatype="http://www.w3.org/2001/XMLSchema#date">2013-12-03</terms:modified>
        <rdfs:comment xml:lang="en">The ESCO qualification (certification) that is legally required for the subject occupation or skill.
Details for the requirements must be given in the relationship description.

Occasionally, such a description must hold a hyperlink to the relevant professions database (e.g. http://ec.europa.eu/internal_market/qualifications/regprof/index.cfm?action=profession&amp;id_profession=12142).
In case the legal requirement is region specific, the relationship:
- should detail the restriction in the relation description
- could be tagged with a location or NUTS code (see http://data.europa.eu/esco/model#location)</rdfs:comment>
        <rdfs:isDefinedBy rdf:resource="http://data.europa.eu/esco/model"/>
        <rdfs:label xml:lang="en">legally required qualification</rdfs:label>
        <rdfs:seeAlso rdf:resource="http://data.europa.eu/esco/model#Relationship"/>
        <rdfs:seeAlso rdf:resource="http://data.europa.eu/esco/model#location"/>
        <owl:deprecated rdf:datatype="http://www.w3.org/2001/XMLSchema#boolean">true</owl:deprecated>
        <vs:term_status rdf:datatype="http://www.w3.org/2001/XMLSchema#string">deprecated</vs:term_status>
    </owl:ObjectProperty>



    <!-- http://data.europa.eu/esco/model#relatedOptionalSkill -->

    <owl:ObjectProperty rdf:about="http://data.europa.eu/esco/model#relatedOptionalSkill">
        <rdfs:subPropertyOf rdf:resource="http://www.w3.org/2004/02/skos/core#related"/>
        <rdfs:domain>
            <owl:Class>
                <owl:unionOf rdf:parseType="Collection">
                    <rdf:Description rdf:about="http://data.europa.eu/esco/model#Occupation"/>
                    <rdf:Description rdf:about="http://data.europa.eu/esco/model#Skill"/>
                </owl:unionOf>
            </owl:Class>
        </rdfs:domain>
        <rdfs:range rdf:resource="http://data.europa.eu/esco/model#Skill"/>
        <terms:issued rdf:datatype="http://www.w3.org/2001/XMLSchema#date">2013-12-03</terms:issued>
        <terms:modified rdf:datatype="http://www.w3.org/2001/XMLSchema#date">2013-12-03</terms:modified>
        <rdfs:comment xml:lang="en">The ESCO skill or competence that is relevant (but optional) for the subject occuption.</rdfs:comment>
        <rdfs:isDefinedBy rdf:resource="http://data.europa.eu/esco/model"/>
        <rdfs:label xml:lang="en">has optional skill</rdfs:label>
        <vs:term_status rdf:datatype="http://www.w3.org/2001/XMLSchema#string">proposed</vs:term_status>
    </owl:ObjectProperty>



    <!-- http://data.europa.eu/esco/model#relatedQualification -->

    <owl:ObjectProperty rdf:about="http://data.europa.eu/esco/model#relatedQualification">
        <rdfs:subPropertyOf rdf:resource="http://www.w3.org/2004/02/skos/core#related"/>
        <rdfs:domain>
            <owl:Class>
                <owl:unionOf rdf:parseType="Collection">
                    <rdf:Description rdf:about="http://data.europa.eu/esco/model#Occupation"/>
                    <rdf:Description rdf:about="http://data.europa.eu/esco/model#Skill"/>
                </owl:unionOf>
            </owl:Class>
        </rdfs:domain>
        <rdfs:range rdf:resource="http://data.europa.eu/esco/model#Qualification"/>
        <terms:issued rdf:datatype="http://www.w3.org/2001/XMLSchema#date">2013-12-03</terms:issued>
        <terms:modified rdf:datatype="http://www.w3.org/2001/XMLSchema#date">2017-02-10</terms:modified>
        <rdfs:comment xml:lang="en">The ESCO qualification (certification) that is required for the subject occupation or skill.</rdfs:comment>
        <rdfs:isDefinedBy rdf:resource="http://data.europa.eu/esco/model"/>
        <rdfs:label xml:lang="en">qualification</rdfs:label>
        <owl:deprecated rdf:datatype="http://www.w3.org/2001/XMLSchema#boolean">true</owl:deprecated>
        <vs:term_status rdf:datatype="http://www.w3.org/2001/XMLSchema#string">deprecated</vs:term_status>
    </owl:ObjectProperty>



    <!-- http://data.europa.eu/esco/model#relevantURL -->

    <owl:ObjectProperty rdf:about="http://data.europa.eu/esco/model#relevantURL">
        <rdfs:domain>
            <owl:Class>
                <owl:unionOf rdf:parseType="Collection">
                    <rdf:Description rdf:about="http://data.europa.eu/esco/model#Label"/>
                    <rdf:Description rdf:about="http://www.w3.org/2004/02/skos/core#Concept"/>
                </owl:unionOf>
            </owl:Class>
        </rdfs:domain>
        <rdfs:range rdf:resource="http://www.w3.org/2000/01/rdf-schema#Literal"/>
        <owl:deprecated rdf:datatype="http://www.w3.org/2001/XMLSchema#boolean">true</owl:deprecated>
        <vs:term_status rdf:datatype="http://www.w3.org/2001/XMLSchema#string">deprecated</vs:term_status>				
    </owl:ObjectProperty>



    <!-- http://data.europa.eu/esco/model#replacedBy -->

    <owl:ObjectProperty rdf:about="http://data.europa.eu/esco/model#replacedBy">
        <owl:inverseOf rdf:resource="http://data.europa.eu/esco/model#replaces"/>
        <rdf:type rdf:resource="http://www.w3.org/2002/07/owl#TransitiveProperty"/>
        <rdfs:domain rdf:resource="http://www.w3.org/2004/02/skos/core#Concept"/>
        <rdfs:range rdf:resource="http://www.w3.org/2004/02/skos/core#Concept"/>
        <rule>PREFIX esco: &lt;http://data.europa.eu/esco/model#&gt;
			PREFIX terms &lt;http://purl.org/dc/terms/&gt;
			PREFIX rdf &lt;http://www.w3.org/1999/02/22-rdf-syntax-ns#&gt;

			CONSTRUCT
				{  ?A  esco:replacedBy ?B . }
			WHERE
				{
				   ?A  terms:isReplacedBy ?B ;  rdf:type  esco:Concept .
				   ?B  rdf:type  esco:Concept .
				}
		</rule>
        <terms:issued rdf:datatype="http://www.w3.org/2001/XMLSchema#date">2013-12-03</terms:issued>
        <terms:modified rdf:datatype="http://www.w3.org/2001/XMLSchema#date">2015-04-21</terms:modified>
        <rdfs:comment xml:lang="en">Typical for a deprecated concept that has been replaced by one or more other concepts.</rdfs:comment>
        <rdfs:isDefinedBy rdf:resource="http://data.europa.eu/esco/model"/>
        <rdfs:label xml:lang="en">replaced by</rdfs:label>
        <vs:term_status rdf:datatype="http://www.w3.org/2001/XMLSchema#string">proposed</vs:term_status>
    </owl:ObjectProperty>



    <!-- http://data.europa.eu/esco/model#replacedByTransitive -->

    <owl:ObjectProperty rdf:about="http://data.europa.eu/esco/model#replacedByTransitive">
        <owl:inverseOf rdf:resource="http://data.europa.eu/esco/model#replacesTransitive"/>
        <rdfs:domain rdf:resource="http://www.w3.org/2004/02/skos/core#Concept"/>
        <rdfs:range rdf:resource="http://www.w3.org/2004/02/skos/core#Concept"/>
        <terms:issued rdf:datatype="http://www.w3.org/2001/XMLSchema#date">2014-05-30</terms:issued>
        <terms:modified rdf:datatype="http://www.w3.org/2001/XMLSchema#date">2015-04-10</terms:modified>
        <rdfs:comment xml:lang="en">Typical for a chain of changes and deprecations of a concept over different versions.</rdfs:comment>
        <rdfs:isDefinedBy rdf:resource="http://data.europa.eu/esco/model"/>
        <rdfs:label xml:lang="en">transitive replaced by</rdfs:label>
        <owl:deprecated rdf:datatype="http://www.w3.org/2001/XMLSchema#boolean">true</owl:deprecated>
        <vs:term_status rdf:datatype="http://www.w3.org/2001/XMLSchema#string">rejected</vs:term_status>
    </owl:ObjectProperty>



    <!-- http://data.europa.eu/esco/model#replaces -->

    <owl:ObjectProperty rdf:about="http://data.europa.eu/esco/model#replaces">
        <rdf:type rdf:resource="http://www.w3.org/2002/07/owl#TransitiveProperty"/>
        <rdfs:domain rdf:resource="http://www.w3.org/2004/02/skos/core#Concept"/>
        <rdfs:range rdf:resource="http://www.w3.org/2004/02/skos/core#Concept"/>
        <rule>PREFIX esco: &lt;http://data.europa.eu/esco/model#&gt;
			PREFIX terms &lt;http://purl.org/dc/terms/&gt;
			PREFIX rdf &lt;http://www.w3.org/1999/02/22-rdf-syntax-ns#&gt;

			CONSTRUCT
				{  ?A  esco:replaces ?B . }
			WHERE
				{
				   ?A  terms:replaces ?B ;  rdf:type  esco:Concept .
				   ?B  rdf:type  esco:Concept .
				}
		</rule>
        <terms:issued rdf:datatype="http://www.w3.org/2001/XMLSchema#date">2013-12-17</terms:issued>
        <terms:modified rdf:datatype="http://www.w3.org/2001/XMLSchema#date">2015-04-21</terms:modified>
        <rdfs:comment xml:lang="en">Typical for a deprecated concept that replaces one or more other concepts.</rdfs:comment>
        <rdfs:isDefinedBy rdf:resource="http://data.europa.eu/esco/model"/>
        <rdfs:label xml:lang="en">replaces</rdfs:label>
        <vs:term_status rdf:datatype="http://www.w3.org/2001/XMLSchema#string">proposed</vs:term_status>
    </owl:ObjectProperty>



    <!-- http://data.europa.eu/esco/model#replacesTransitive -->

    <owl:ObjectProperty rdf:about="http://data.europa.eu/esco/model#replacesTransitive">
        <rdfs:domain rdf:resource="http://www.w3.org/2004/02/skos/core#Concept"/>
        <rdfs:range rdf:resource="http://www.w3.org/2004/02/skos/core#Concept"/>
        <terms:issued rdf:datatype="http://www.w3.org/2001/XMLSchema#date">2014-05-30</terms:issued>
        <terms:modified rdf:datatype="http://www.w3.org/2001/XMLSchema#date">2015-04-10</terms:modified>
        <rdfs:comment xml:lang="en">Typical for a chain of deprecated concepts that replaces one or more other concepts over more than one version.</rdfs:comment>
        <rdfs:isDefinedBy rdf:resource="http://data.europa.eu/esco/model"/>
        <rdfs:label xml:lang="en">transitively replaces</rdfs:label>
        <owl:deprecated rdf:datatype="http://www.w3.org/2001/XMLSchema#boolean">true</owl:deprecated>
        <vs:term_status rdf:datatype="http://www.w3.org/2001/XMLSchema#string">rejected</vs:term_status>
    </owl:ObjectProperty>



    <!-- http://data.europa.eu/esco/model#requirementLevel -->

    <owl:ObjectProperty rdf:about="http://data.europa.eu/esco/model#requirementLevel">
        <rdfs:domain rdf:resource="http://data.europa.eu/esco/model#EntryRequirement"/>
        <rdfs:range rdf:resource="http://www.w3.org/2004/02/skos/core#Concept"/>
        <rdfs:comment xml:lang="en">Refers to a skos:Concept that indicates the requirement level of a certain entry requirement. It indicates the necessity of the entry requirement</rdfs:comment>
        <rdfs:isDefinedBy rdf:resource="http://data.europa.eu/esco/model"/>
        <rdfs:label xml:lang="en">requirement level</rdfs:label>
        <rdfs:seeAlso rdf:resource="http://data.europa.eu/esco/model#EntryRequirement"/>
    </owl:ObjectProperty>



    <!-- http://data.europa.eu/esco/model#skillReuseLevel -->

    <owl:ObjectProperty rdf:about="http://data.europa.eu/esco/model#skillReuseLevel">
        <rdfs:subPropertyOf rdf:resource="http://purl.org/dc/terms/subject"/>
        <rdfs:domain rdf:resource="http://data.europa.eu/esco/model#Skill"/>
        <rdfs:range rdf:resource="http://data.europa.eu/esco/model#SkillReuseLevel"/>
        <terms:issued rdf:datatype="http://www.w3.org/2001/XMLSchema#date">2014-06-05</terms:issued>
        <terms:modified rdf:datatype="http://www.w3.org/2001/XMLSchema#date">2016-06-08</terms:modified>
        <rdfs:comment xml:lang="en">Reuseability level of a skill</rdfs:comment>
        <rdfs:isDefinedBy rdf:resource="http://data.europa.eu/esco/model"/>
        <rdfs:label xml:lang="en">skill reuseability level</rdfs:label>
        <owl:deprecated rdf:datatype="http://www.w3.org/2001/XMLSchema#boolean">true</owl:deprecated>
        <vs:term_status>rejected</vs:term_status>
    </owl:ObjectProperty>



    <!-- http://data.europa.eu/esco/model#skillType -->

    <owl:ObjectProperty rdf:about="http://data.europa.eu/esco/model#skillType">
        <rdfs:subPropertyOf rdf:resource="http://purl.org/dc/terms/subject"/>
        <rdfs:domain rdf:resource="http://data.europa.eu/esco/model#Skill"/>
        <rdfs:range rdf:resource="http://data.europa.eu/esco/model#SkillCompetenceType"/>
        <terms:issued rdf:datatype="http://www.w3.org/2001/XMLSchema#date">2013-12-03</terms:issued>
        <terms:modified rdf:datatype="http://www.w3.org/2001/XMLSchema#date">2013-12-03</terms:modified>
        <rdfs:comment xml:lang="en">Type of competence (a tagging concept)</rdfs:comment>
        <rdfs:isDefinedBy rdf:resource="http://data.europa.eu/esco/model"/>
        <rdfs:label xml:lang="en">skill type</rdfs:label>
        <vs:term_status>proposed</vs:term_status>
        <vs:term_status>released</vs:term_status>
    </owl:ObjectProperty>



    <!-- http://data.europa.eu/esco/model#structureFor -->

    <owl:ObjectProperty rdf:about="http://data.europa.eu/esco/model#structureFor">
        <rdfs:subPropertyOf rdf:resource="http://www.w3.org/2002/07/owl#topObjectProperty"/>
        <rdfs:range rdf:resource="http://data.europa.eu/esco/model#ConceptScheme"/>
        <terms:created rdf:datatype="http://www.w3.org/2001/XMLSchema#date">2016-06-21</terms:created>
        <terms:modified rdf:datatype="http://www.w3.org/2001/XMLSchema#date">2016-06-21</terms:modified>
        <rdfs:isDefinedBy rdf:resource="http://data.europa.eu/esco/model"/>
        <rdfs:label>defines structure for</rdfs:label>
        <rdfs:seeAlso rdf:resource="http://data.europa.eu/esco/model#Structure"/>
        <rdfs:seeAlso rdf:resource="http://data.europa.eu/esco/model#codeList"/>
        <vs:term_status>proposed</vs:term_status>
    </owl:ObjectProperty>



    <!-- http://data.europa.eu/esco/model#supplementaryDoc -->

    <owl:ObjectProperty rdf:about="http://data.europa.eu/esco/model#supplementaryDoc">
        <rdfs:subPropertyOf rdf:resource="http://xmlns.com/foaf/0.1/page"/>
        <rdfs:range rdf:resource="http://xmlns.com/foaf/0.1/Document"/>
        <rdfs:comment xml:lang="en"></rdfs:comment>
        <rdfs:isDefinedBy rdf:resource="http://data.europa.eu/esco/model"/>
        <rdfs:label xml:lang="en">supplementary doc</rdfs:label>
    </owl:ObjectProperty>



    <!-- http://data.europa.eu/esco/model#supportedLanguage -->

    <owl:ObjectProperty rdf:about="http://data.europa.eu/esco/model#supportedLanguage">
        <rdfs:domain rdf:resource="http://data.europa.eu/esco/model#ConceptScheme"/>
        <rdfs:range rdf:resource="http://data.europa.eu/esco/model#Language"/>
        <terms:issued rdf:datatype="http://www.w3.org/2001/XMLSchema#date">2013-06-27</terms:issued>
        <terms:modified rdf:datatype="http://www.w3.org/2001/XMLSchema#date">2013-12-03</terms:modified>
        <rdfs:comment xml:lang="en">Denotes a description of the languages supported by the (subject) concept scheme.
Required for ESCO taxonomy or thesauri.</rdfs:comment>
        <rdfs:isDefinedBy rdf:resource="http://data.europa.eu/esco/model"/>
        <rdfs:label xml:lang="en">supported language</rdfs:label>
        <vs:term_status rdf:datatype="http://www.w3.org/2001/XMLSchema#string">released</vs:term_status>
    </owl:ObjectProperty>



    <!-- http://data.europa.eu/esco/model#target -->

    <owl:ObjectProperty rdf:about="http://data.europa.eu/esco/model#target">
        <rdf:type rdf:resource="http://www.w3.org/2002/07/owl#FunctionalProperty"/>
        <rdfs:domain rdf:resource="http://data.europa.eu/esco/model#AssociationObject"/>
        <rdfs:range rdf:resource="http://www.w3.org/2000/01/rdf-schema#Resource"/>
        <rdfs:comment xml:lang="en">The associated resource. Refers to a node (e.g. a skos:Concept) in another established framework (e.g. a skill or occupation from the ESCO classification, a skill or occupation from the national classification system, the qualification level according the national qualification framework,â¦).</rdfs:comment>
        <rdfs:isDefinedBy rdf:resource="http://data.europa.eu/esco/model"/>
        <rdfs:label xml:lang="en">association to</rdfs:label>
        <rdfs:seeAlso rdf:resource="http://data.europa.eu/esco/model#AssociationObject"/>
        <rdfs:seeAlso rdf:resource="http://data.europa.eu/esco/model#targetFramework"/>
    </owl:ObjectProperty>



    <!-- http://data.europa.eu/esco/model#targetFramework -->

    <owl:ObjectProperty rdf:about="http://data.europa.eu/esco/model#targetFramework">
        <rdf:type rdf:resource="http://www.w3.org/2002/07/owl#FunctionalProperty"/>
        <rdfs:domain rdf:resource="http://data.europa.eu/esco/model#AssociationObject"/>
        <rdfs:range rdf:resource="http://purl.org/dc/terms/Standard"/>
        <rdfs:comment xml:lang="en">The framework to which the resource being described is associated. It is the framework that describes the target resource (the associated resource) (e.g. ESCO classification system, national qualification framework system,..). It is recommended that the target framework is denoted by a known resource (e.g. a adms:Asset, a dcat:Dataset, a conceptscheme)</rdfs:comment>
        <rdfs:isDefinedBy rdf:resource="http://data.europa.eu/esco/model"/>
        <rdfs:label xml:lang="en">target framework</rdfs:label>
        <rdfs:seeAlso rdf:resource="http://data.europa.eu/esco/model#AssociationObject"/>
        <rdfs:seeAlso rdf:resource="http://data.europa.eu/esco/model#target"/>
    </owl:ObjectProperty>



    <!-- http://data.europa.eu/esco/model#topMember -->

    <owl:ObjectProperty rdf:about="http://data.europa.eu/esco/model#topMember">
        <rdfs:subPropertyOf rdf:resource="http://www.w3.org/2004/02/skos/core#member"/>
        <terms:issued rdf:datatype="http://www.w3.org/2001/XMLSchema#date">2013-12-03</terms:issued>
        <terms:modified rdf:datatype="http://www.w3.org/2001/XMLSchema#date">2016-06-10</terms:modified>
        <rdfs:comment xml:lang="en">Typically specified in case the subject collection is a concept group having a hierarchical representation (hierarchy based on broader/narrower). The referenced concepts are the hierarchical entry points of the concept group hierarchy.
The top may be concepts as well as collections.</rdfs:comment>
        <rdfs:isDefinedBy rdf:resource="http://data.europa.eu/esco/model"/>
        <rdfs:label xml:lang="en">has top member</rdfs:label>
        <owl:deprecated rdf:datatype="http://www.w3.org/2001/XMLSchema#boolean">true</owl:deprecated>
        <vs:term_status rdf:datatype="http://www.w3.org/2001/XMLSchema#string">rejected</vs:term_status>
    </owl:ObjectProperty>



    <!-- http://data.europa.eu/esco/model#undefined -->

    <owl:ObjectProperty rdf:about="http://data.europa.eu/esco/model#undefined">
        <rdfs:subPropertyOf rdf:resource="http://www.w3.org/2004/02/skos/core#related"/>
        <owl:inverseOf rdf:resource="http://data.europa.eu/esco/model#undefinedOf"/>
        <terms:modified rdf:datatype="http://www.w3.org/2001/XMLSchema#date">2013-12-03</terms:modified>
        <rdfs:comment xml:lang="en">undefined skill is a skill that has no optional, recommended or required property assigned to it.</rdfs:comment>
        <rdfs:isDefinedBy rdf:resource="http://data.europa.eu/esco/model"/>
        <rdfs:label xml:lang="en">undefined</rdfs:label>
        <owl:deprecated rdf:datatype="http://www.w3.org/2001/XMLSchema#boolean">true</owl:deprecated>
        <vs:term_status rdf:datatype="http://www.w3.org/2001/XMLSchema#string">rejected</vs:term_status>
        <skos:changeNote xml:lang="en">ESCOv0 has 102K undefined relations.
These cannot be inherited in v1 as occupations are redefined - maybe after merging a decision needs to be taken:
- make relatedOptionalSkill
- make relatedEssentialSkill
- remove the related:undefined.</skos:changeNote>
        <skos:historyNote xml:lang="en">Deprecated with Model version 1.</skos:historyNote>
    </owl:ObjectProperty>



    <!-- http://data.europa.eu/esco/model#undefinedOf -->

    <owl:ObjectProperty rdf:about="http://data.europa.eu/esco/model#undefinedOf">
        <rdfs:subPropertyOf rdf:resource="http://www.w3.org/2004/02/skos/core#related"/>
        <terms:modified rdf:datatype="http://www.w3.org/2001/XMLSchema#date">2013-12-03</terms:modified>
        <rdfs:isDefinedBy rdf:resouce="http://data.europa.eu/esco/model" />
        <rdfs:label xml:lang="en">undefined skill of</rdfs:label>
        <rdfs:seeAlso rdf:resource="http://data.europa.eu/esco/model#undefined"/>
        <owl:deprecated rdf:datatype="http://www.w3.org/2001/XMLSchema#boolean">true</owl:deprecated>
        <vs:term_status rdf:datatype="http://www.w3.org/2001/XMLSchema#string">rejected</vs:term_status>
        <skos:changeNote xml:lang="en">ESCOv0 has 102K undefined relations.  See http://data.europa.eu/esco/model#undefined.</skos:changeNote>
        <skos:historyNote xml:lang="en">Deprecated with Model version 1.</skos:historyNote>
    </owl:ObjectProperty>



    <!-- http://data.europa.eu/esco/model#waysToAcquire -->

    <owl:ObjectProperty rdf:about="http://data.europa.eu/esco/model#waysToAcquire">
        <rdfs:domain rdf:resource="http://data.europa.eu/esco/model#Qualification"/>
        <rdfs:range rdf:resource="http://www.w3.org/2004/02/skos/core#Concept"/>
        <rdfs:comment xml:lang="en">Refers to a skos:Concept that indicates whether the qualification can be acquired by validation of a formal, non-formal and/or informal learning processes.</rdfs:comment>
        <rdfs:isDefinedBy rdf:resource="http://data.europa.eu/esco/model"/>
        <rdfs:label xml:lang="en">way to acquire</rdfs:label>
    </owl:ObjectProperty>

    <!-- http://purl.org/iso25964/DataSet/Versioning#hasVersionRecord -->

    <owl:ObjectProperty rdf:about="http://purl.org/iso25964/DataSet/Versioning#hasVersionRecord">
        <rdfs:range rdf:resource="http://purl.org/iso25964/DataSet/Versioning#VersionHistoryRecord"/>
        <terms:modified rdf:datatype="http://www.w3.org/2001/XMLSchema#date">2013-10-04</terms:modified>
        <rdfs:comment xml:lang="en">The dataset holds this statement using any applicable form
- the dataset is an RDF dataset: as a plain RDF statement on the main resource of the dataset.
- the dataset is an XML or HTML resource: as an annotation using RDFa, schema.org or any other annotation language.
- the dataset is any proper encoding: as documentation or metadata on the metadata provided with the dataset.</rdfs:comment>
        <rdfs:isDefinedBy rdf:resource="http://purl.org/iso25964/DataSet/Versioning"/>
        <rdfs:label xml:lang="en">has version record</rdfs:label>
        <vs:term_status>proposed</vs:term_status>
    </owl:ObjectProperty>


    <!--
    ///////////////////////////////////////////////////////////////////////////////////////
    //
    // Data properties
    //
    ///////////////////////////////////////////////////////////////////////////////////////
     -->




    <!-- http://data.europa.eu/esco/model#awardingBodyDescription -->

    <owl:DatatypeProperty rdf:about="http://data.europa.eu/esco/model#awardingBodyDescription"/>



    <!-- http://data.europa.eu/esco/model#editorialStatus -->

    <owl:DatatypeProperty rdf:about="http://data.europa.eu/esco/model#editorialStatus">
        <rdfs:domain>
            <owl:Class>
                <owl:unionOf rdf:parseType="Collection">
                    <rdf:Description rdf:about="http://www.w3.org/2004/02/skos/core#Concept"/>
                    <rdf:Description rdf:about="http://www.w3.org/2008/05/skos-xl#Label"/>
                </owl:unionOf>
            </owl:Class>
        </rdfs:domain>
        <rdfs:range rdf:resource="http://data.europa.eu/esco/model#editorialStatusDataType"/>
        <terms:issued rdf:datatype="http://www.w3.org/2001/XMLSchema#date">2014-07-03</terms:issued>
        <terms:modified rdf:datatype="http://www.w3.org/2001/XMLSchema#date">2014-07-03</terms:modified>
        <rdfs:comment xml:lang="en">The business or editorial status of a concept or label</rdfs:comment>
        <rdfs:isDefinedBy rdf:resource="http://data.europa.eu/esco/model"/>
        <rdfs:label xml:lang="en">editorial status</rdfs:label>
        <vs:term_status rdf:datatype="http://www.w3.org/2001/XMLSchema#string">proposed</vs:term_status>
    </owl:DatatypeProperty>



    <!-- http://data.europa.eu/esco/model#expirationPeriod -->

    <owl:DatatypeProperty rdf:about="http://data.europa.eu/esco/model#expirationPeriod">
        <rdfs:domain rdf:resource="http://data.europa.eu/esco/model#Qualification"/>
        <rdfs:range rdf:resource="http://www.w3.org/2001/XMLSchema#duration"/>
        <terms:modified rdf:datatype="http://www.w3.org/2001/XMLSchema#date">2013-06-27</terms:modified>
        <rdfs:comment xml:lang="en">Period how long a qualification is valid.

Example: a qualification for aircraft pilot may be subject to hours flight and/or testing within a specified period in order to pro-long the qualification.</rdfs:comment>
        <rdfs:isDefinedBy rdf:resource="http://data.europa.eu/esco/model"/>
        <rdfs:label xml:lang="en">qualification expiration period</rdfs:label>
        <vs:term_status rdf:datatype="http://www.w3.org/2001/XMLSchema#string">released</vs:term_status>
    </owl:DatatypeProperty>



    <!-- http://data.europa.eu/esco/model#expiryPeriod -->

    <owl:DatatypeProperty rdf:about="http://data.europa.eu/esco/model#expiryPeriod">
        <rdfs:domain rdf:resource="http://data.europa.eu/esco/model#Qualification"/>
        <rdfs:range rdf:resource="http://www.w3.org/2001/XMLSchema#duration"/>
        <rdfs:comment xml:lang="en">The validity period of a qualification. The period for which a  qualification is valid, after it is issued to an individual.</rdfs:comment>
        <rdfs:isDefinedBy rdf:resource="http://data.europa.eu/esco/model"/>
        <rdfs:label xml:lang="en">expiry period</rdfs:label>
    </owl:DatatypeProperty>



    <!-- http://data.europa.eu/esco/model#hasECTSCreditPoints -->

    <owl:DatatypeProperty rdf:about="http://data.europa.eu/esco/model#hasECTSCreditPoints">
        <rdfs:domain rdf:resource="http://data.europa.eu/esco/model#Qualification"/>
        <rdfs:range rdf:resource="http://www.w3.org/2001/XMLSchema#decimal"/>
        <rdfs:comment xml:lang="en">The ECTS credit points assigned to a qualification</rdfs:comment>
        <rdfs:isDefinedBy rdf:resource="http://data.europa.eu/esco/model"/>
        <rdfs:label xml:lang="en">ECTS credit points</rdfs:label>
    </owl:DatatypeProperty>



    <!-- http://data.europa.eu/esco/model#hasPolyHierarchy -->

    <owl:DatatypeProperty rdf:about="http://data.europa.eu/esco/model#hasPolyHierarchy">
        <rdfs:range rdf:resource="http://www.w3.org/2001/XMLSchema#boolean"/>
    </owl:DatatypeProperty>



    <!-- http://data.europa.eu/esco/model#isIndirect -->

    <owl:DatatypeProperty rdf:about="http://data.europa.eu/esco/model#isIndirect">
        <rdfs:range rdf:resource="http://www.w3.org/2001/XMLSchema#boolean"/>
    </owl:DatatypeProperty>



    <!-- http://data.europa.eu/esco/model#isPartialQualification -->

    <owl:DatatypeProperty rdf:about="http://data.europa.eu/esco/model#isPartialQualification">
        <rdfs:domain rdf:resource="http://data.europa.eu/esco/model#Qualification"/>
        <rdfs:range rdf:resource="http://www.w3.org/2001/XMLSchema#boolean"/>
        <rdfs:comment xml:lang="en">Default value is &apos;false&apos;^^xsd:boolean </rdfs:comment>
        <rdfs:comment xml:lang="en">Indicates whether a qualification is a full qualification or part of another qualification. In the latter,  the qualification is only obtained as a formal outcome of a âbroaderâ qualification of which it is part.</rdfs:comment>
        <rdfs:isDefinedBy rdf:resource="http://data.europa.eu/esco/model"/>
        <rdfs:label xml:lang="en">is partial qualification</rdfs:label>
    </owl:DatatypeProperty>



    <!-- http://data.europa.eu/esco/model#isTransversal -->

    <owl:DatatypeProperty rdf:about="http://data.europa.eu/esco/model#isTransversal">
        <rdfs:domain>
            <owl:Class>
                <owl:unionOf rdf:parseType="Collection">
                    <rdf:Description rdf:about="http://data.europa.eu/esco/model#Concept"/>
                    <rdf:Description rdf:about="http://data.europa.eu/esco/model#SkillReuseLevel"/>
                </owl:unionOf>
            </owl:Class>
        </rdfs:domain>
        <rdfs:range rdf:resource="http://www.w3.org/2001/XMLSchema#boolean"/>
        <terms:issued rdf:datatype="http://www.w3.org/2001/XMLSchema#date">2013-12-03</terms:issued>
        <terms:modified rdf:datatype="http://www.w3.org/2001/XMLSchema#date">2013-12-03</terms:modified>
        <rdfs:comment xml:lang="en">Typical to indicate that a concept (like a skill) is not job or sector specific.  It is cross sector.

May also be applied (if unambiguous) to qualifications and occupations.

Assertion (to &apos;true&apos;) is required in case transversality must be affirmed.

Skill re-usability levels can be tagged in case the level implies transversal scope of the skills having the re-usability level.</rdfs:comment>
        <rdfs:label xml:lang="en">is transversal</rdfs:label>
        <owl:deprecated rdf:datatype="http://www.w3.org/2001/XMLSchema#boolean">true</owl:deprecated>
        <vs:term_status rdf:datatype="http://www.w3.org/2001/XMLSchema#string">rejected</vs:term_status>
    </owl:DatatypeProperty>



    <!-- http://data.europa.eu/esco/model#isoCountryCodeA2 -->

    <owl:DatatypeProperty rdf:about="http://data.europa.eu/esco/model#isoCountryCodeA2">
        <rdfs:domain rdf:resource="http://data.europa.eu/esco/model#Country"/>
        <rdfs:range rdf:resource="http://www.w3.org/2001/XMLSchema#NMTOKEN"/>
        <terms:issued rdf:datatype="http://www.w3.org/2001/XMLSchema#date">2013-06-27</terms:issued>
        <terms:modified rdf:datatype="http://www.w3.org/2001/XMLSchema#date">2016-06-10</terms:modified>
        <rdfs:comment xml:lang="en">ISO 3166 country code - A2</rdfs:comment>
        <rdfs:isDefinedBy rdf:resource="http://data.europa.eu/esco/model"/>
        <rdfs:label xml:lang="en">country code (A2)</rdfs:label>
        <owl:deprecated rdf:datatype="http://www.w3.org/2001/XMLSchema#boolean">true</owl:deprecated>
        <vs:term_status rdf:datatype="http://www.w3.org/2001/XMLSchema#string">deprecated</vs:term_status>
    </owl:DatatypeProperty>



    <!-- http://data.europa.eu/esco/model#isoCountryCodeA3 -->

    <owl:DatatypeProperty rdf:about="http://data.europa.eu/esco/model#isoCountryCodeA3">
        <rdfs:domain rdf:resource="http://data.europa.eu/esco/model#Country"/>
        <rdfs:range rdf:resource="http://www.w3.org/2001/XMLSchema#NMTOKEN"/>
        <terms:issued rdf:datatype="http://www.w3.org/2001/XMLSchema#date">2013-06-27</terms:issued>
        <terms:modified rdf:datatype="http://www.w3.org/2001/XMLSchema#date">2016-06-10</terms:modified>
        <rdfs:comment xml:lang="en">ISO 3166 country code - A3</rdfs:comment>
        <rdfs:isDefinedBy rdf:resource="http://data.europa.eu/esco/model"/>
        <rdfs:label xml:lang="en">country code (A3)</rdfs:label>
        <owl:deprecated rdf:datatype="http://www.w3.org/2001/XMLSchema#boolean">true</owl:deprecated>
        <vs:term_status rdf:datatype="http://www.w3.org/2001/XMLSchema#string">deprecated</vs:term_status>
    </owl:DatatypeProperty>



    <!-- http://data.europa.eu/esco/model#language -->

    <owl:DatatypeProperty rdf:about="http://data.europa.eu/esco/model#language">
        <rdfs:range rdf:resource="http://www.w3.org/2001/XMLSchema#language"/>
    </owl:DatatypeProperty>



    <!-- http://data.europa.eu/esco/model#nodeLiteral -->

    <owl:DatatypeProperty rdf:about="http://data.europa.eu/esco/model#nodeLiteral">
        <rdfs:domain rdf:resource="http://data.europa.eu/esco/model#NodeLiteral"/>
        <rdfs:range rdf:resource="http://www.w3.org/2000/01/rdf-schema#Literal"/>
        <rdfs:comment xml:lang="en"></rdfs:comment>
        <rdfs:isDefinedBy rdf:resource="http://data.europa.eu/esco/model"/>
        <rdfs:label xml:lang="en"></rdfs:label>
        <rdfs:seeAlso rdf:resource="http://data.europa.eu/esco/model#NodeLiteral"/>
    </owl:DatatypeProperty>



    <!-- http://data.europa.eu/esco/model#noteLiteral -->

    <owl:DatatypeProperty rdf:about="http://data.europa.eu/esco/model#noteLiteral"/>



    <!-- http://data.europa.eu/esco/model#referenceLanguage -->

    <owl:DatatypeProperty rdf:about="http://data.europa.eu/esco/model#referenceLanguage">
        <rdfs:range rdf:resource="http://www.w3.org/2001/XMLSchema#language"/>
        <terms:issued rdf:datatype="http://www.w3.org/2001/XMLSchema#date">2013-06-27</terms:issued>
        <terms:modified rdf:datatype="http://www.w3.org/2001/XMLSchema#date">2013-06-27</terms:modified>
        <rdfs:comment xml:lang="en">QMS usage: The ISO 639-1 code of the language (2-char language code) in which information about the qualification is provided. This language will be used as the default reference language for the qualification.</rdfs:comment>
        <rdfs:comment xml:lang="en">QMS usage: The range must be a rdfs:Literal typed as xsd:language.</rdfs:comment>
        <rdfs:comment xml:lang="en">Reference language for a concept.

Typically set when the concept is first loaded with PT in (at least) 1 language.  (If multiple but not all languages are provided, the reference language must be uniquely set to one of the loaded languages.)

In case the concept needs to be shown or translated in a new language (not having a PT yet), the label in the reference language is shown.</rdfs:comment>
        <rdfs:isDefinedBy rdf:resource="http://data.europa.eu/esco/model"/>
        <rdfs:label xml:lang="en">Reference language</rdfs:label>
        <rdfs:label xml:lang="en">reference language</rdfs:label>
        <vs:term_status rdf:datatype="http://www.w3.org/2001/XMLSchema#string">released</vs:term_status>
    </owl:DatatypeProperty>



    <!-- http://data.europa.eu/esco/model#relevantURL -->

    <owl:DatatypeProperty rdf:about="http://data.europa.eu/esco/model#relevantURL"/>



    <!-- http://data.europa.eu/esco/model#reviewedAtTime -->

    <owl:DatatypeProperty rdf:about="http://data.europa.eu/esco/model#reviewedAtTime">
        <rdfs:range rdf:resource="http://www.w3.org/2001/XMLSchema#dateTime"/>
        <rdfs:comment xml:lang="en"></rdfs:comment>
        <rdfs:isDefinedBy rdf:resource="http://data.europa.eu/esco/model"/>
        <rdfs:label xml:lang="en">review date</rdfs:label>
        <rdfs:seeAlso rdf:resource="http://data.europa.eu/esco/model#Accreditation"/>
    </owl:DatatypeProperty>



    <!-- http://data.europa.eu/esco/model#targetDescription -->

    <owl:DatatypeProperty rdf:about="http://data.europa.eu/esco/model#targetDescription">
        <rdfs:domain rdf:resource="http://data.europa.eu/esco/model#AssociationObject"/>
        <rdfs:range rdf:resource="http://www.w3.org/2000/01/rdf-schema#Literal"/>
        <rdfs:comment xml:lang="en">A free-text description of a node in another established framework.</rdfs:comment>
        <rdfs:isDefinedBy rdf:resource="http://data.europa.eu/esco/model"/>
        <rdfs:label xml:lang="en"></rdfs:label>
        <rdfs:seeAlso rdf:resource="http://data.europa.eu/esco/model#AssociationObject"/>
        <rdfs:seeAlso rdf:resource="http://data.europa.eu/esco/model#target"/>
        <rdfs:seeAlso rdf:resource="http://data.europa.eu/esco/model#targetFramework"/>
    </owl:DatatypeProperty>



    <!-- http://data.europa.eu/esco/model#targetName -->

    <owl:DatatypeProperty rdf:about="http://data.europa.eu/esco/model#targetName">
        <rdfs:domain rdf:resource="http://data.europa.eu/esco/model#AssociationObject"/>
        <rdfs:range rdf:resource="http://www.w3.org/2000/01/rdf-schema#Literal"/>
        <rdfs:comment xml:lang="en">The name or value of a node in another established framework.</rdfs:comment>
        <rdfs:isDefinedBy rdf:resource="http://data.europa.eu/esco/model"/>
        <rdfs:label xml:lang="en"></rdfs:label>
        <rdfs:seeAlso rdf:resource="http://data.europa.eu/esco/model#AssociationObject"/>
        <rdfs:seeAlso rdf:resource="http://data.europa.eu/esco/model#target"/>
        <rdfs:seeAlso rdf:resource="http://data.europa.eu/esco/model#targetFramework"/>
    </owl:DatatypeProperty>



    <!-- http://data.europa.eu/esco/model#targetNotation -->

    <owl:DatatypeProperty rdf:about="http://data.europa.eu/esco/model#targetNotation">
        <rdfs:domain rdf:resource="http://data.europa.eu/esco/model#AssociationObject"/>
        <rdfs:range rdf:resource="http://www.w3.org/2000/01/rdf-schema#Literal"/>
        <rdfs:comment xml:lang="en"></rdfs:comment>
        <rdfs:isDefinedBy rdf:resource="http://data.europa.eu/esco/model"/>
        <rdfs:label xml:lang="en">target notation</rdfs:label>
        <rdfs:seeAlso rdf:resource="http://data.europa.eu/esco/model#AssociationObject"/>
        <rdfs:seeAlso rdf:resource="http://data.europa.eu/esco/model#target"/>
        <rdfs:seeAlso rdf:resource="http://data.europa.eu/esco/model#targetFramework"/>
    </owl:DatatypeProperty>



    <!-- http://data.europa.eu/esco/model#targetURL -->

    <owl:DatatypeProperty rdf:about="http://data.europa.eu/esco/model#targetURL">
        <rdfs:domain rdf:resource="http://data.europa.eu/esco/model#AssociationObject"/>
        <rdfs:range rdf:resource="http://www.w3.org/2001/XMLSchema#anyURI"/>
        <rdfs:comment xml:lang="en">The URL of a node in another established framework.</rdfs:comment>
        <rdfs:isDefinedBy rdf:resource="http://data.europa.eu/esco/model"/>
        <rdfs:label xml:lang="en"></rdfs:label>
        <rdfs:seeAlso rdf:resource="http://data.europa.eu/esco/model#AssociationObject"/>
        <rdfs:seeAlso rdf:resource="http://data.europa.eu/esco/model#target"/>
        <rdfs:seeAlso rdf:resource="http://data.europa.eu/esco/model#targetFramework"/>
    </owl:DatatypeProperty>



    <!-- http://data.europa.eu/esco/model#volumeOfLearning -->

    <owl:DatatypeProperty rdf:about="http://data.europa.eu/esco/model#volumeOfLearning">
        <rdfs:domain rdf:resource="http://data.europa.eu/esco/model#Qualification"/>
        <rdfs:range rdf:resource="http://www.w3.org/2001/XMLSchema#duration"/>
        <rdfs:comment xml:lang="en">Indicates how many hours of learning effort is needed to acquire a particular qualification (notional learning hours).</rdfs:comment>
        <rdfs:isDefinedBy rdf:resource="http://data.europa.eu/esco/model"/>
        <rdfs:label xml:lang="en">volume of learning</rdfs:label>
    </owl:DatatypeProperty>



    <!-- http://purl.org/iso25964/skos-thes#status -->

    <owl:DatatypeProperty rdf:about="http://purl.org/iso25964/skos-thes#status">
        <rdfs:range rdf:resource="http://data.europa.eu/esco/model#statusDataType"/>
        <vs:term_status>released</vs:term_status>
    </owl:DatatypeProperty>



    <!--
    ///////////////////////////////////////////////////////////////////////////////////////
    //
    // Classes
    //
    ///////////////////////////////////////////////////////////////////////////////////////
     -->




    <!-- http://data.europa.eu/esco/model#Accreditation -->

    <owl:Class rdf:about="http://data.europa.eu/esco/model#Accreditation">
        <rdfs:comment xml:lang="en">Can be used to specify:
	- the agent that was primarily responsible for the accreditation
	- the date the accreditation was formally approved
	- a review date or expiry date
	- related documents with additional information about the accreditation or used standards and procedures in the assessment and quality assurance of the qualification</rdfs:comment>
        <rdfs:comment xml:lang="en">The accreditation class is used to specify information related to the accreditation, monitoring and quality assurance of a qualification and/or awarding body</rdfs:comment>
        <rdfs:isDefinedBy rdf:resource="http://data.europa.eu/esco/model#"/>
        <rdfs:label xml:lang="en">Accreditation</rdfs:label>
        <rdfs:seeAlso rdf:resource="http://data.europa.eu/esco/model#hasAccreditation"/>
    </owl:Class>



    <!-- http://data.europa.eu/esco/model#AssociationObject -->

    <owl:Class rdf:about="http://data.europa.eu/esco/model#AssociationObject">
        <rdfs:subClassOf>
            <owl:Restriction>
                <owl:onProperty rdf:resource="http://data.europa.eu/esco/model#isAssociationFor"/>
                <owl:cardinality rdf:datatype="http://www.w3.org/2001/XMLSchema#nonNegativeInteger">1</owl:cardinality>
            </owl:Restriction>
        </rdfs:subClassOf>
        <rdfs:subClassOf>
            <owl:Restriction>
                <owl:onProperty rdf:resource="http://data.europa.eu/esco/model#targetFramework"/>
                <owl:cardinality rdf:datatype="http://www.w3.org/2001/XMLSchema#nonNegativeInteger">1</owl:cardinality>
            </owl:Restriction>
        </rdfs:subClassOf>
        <rdfs:subClassOf>
            <owl:Restriction>
                <owl:onProperty rdf:resource="http://data.europa.eu/esco/model#target"/>
                <owl:maxCardinality rdf:datatype="http://www.w3.org/2001/XMLSchema#nonNegativeInteger">1</owl:maxCardinality>
            </owl:Restriction>
        </rdfs:subClassOf>
        <rdfs:subClassOf>
            <owl:Restriction>
                <owl:onProperty rdf:resource="http://data.europa.eu/esco/model#targetName"/>
                <owl:minCardinality rdf:datatype="http://www.w3.org/2001/XMLSchema#nonNegativeInteger">0</owl:minCardinality>
            </owl:Restriction>
        </rdfs:subClassOf>
        <rdfs:subClassOf>
            <owl:Restriction>
                <owl:onProperty rdf:resource="http://data.europa.eu/esco/model#targetNotation"/>
                <owl:minCardinality rdf:datatype="http://www.w3.org/2001/XMLSchema#nonNegativeInteger">0</owl:minCardinality>
            </owl:Restriction>
        </rdfs:subClassOf>
        <rdfs:subClassOf>
            <owl:Restriction>
                <owl:onProperty rdf:resource="http://data.europa.eu/esco/model#targetURL"/>
                <owl:maxCardinality rdf:datatype="http://www.w3.org/2001/XMLSchema#nonNegativeInteger">1</owl:maxCardinality>
            </owl:Restriction>
        </rdfs:subClassOf>
        <rdfs:comment xml:lang="en">The generic class of extended directed associative relationships from a resource to a semantic asset.</rdfs:comment>
        <rdfs:comment xml:lang="en">This class relates a qualification to a node from another established framework or classification system. This allows to specify metadata on the association:
	- The relationship type (describing the semantics of the association) is given by the dcterms:type property using a skos:Concept from the controlled vocabulary &lt;http://data.europa.eu/esco/concept-scheme/association-type&gt;.
	- The framework and/or classification system to which the related semantic asset belongs is given by the esco:targetFramework property.
	- The resource being described (the resource the association starts from e.g. a qualification) is given by esco:isAssociationFor and the associated resource by esco:target.&quot;@en;
	rdfs:comment &quot;Used to express a learning outcome of a qualification as a relation from a qualification to an ESCO skill, competence or knowdledge (see &lt;http://data.europa.eu/esco/association-type#learning-outcome&gt;).&quot;@en;
	rdfs:comment &quot;Used to related a qualification to an occupation from an international, national or regional occupation classification system (see &lt;http://data.europa.eu/esco/association-type#related-occupation&gt;).&quot;@en;
	rdfs:comment &quot;Used to link a qualification to a international, national or regional qualification framework level (see &lt;http://data.europa.eu/esco/association-type#qf-level&gt;).&quot;@en;
	rdfs:comment &quot;List of properties:
	- dcterms:type (0..1)
	- dcterms:description (0..n)
	- dcterms:issued (0..1)
	- esco:targetFramework (1..1)
	- esco:isAssociationFor (1..1)
	- esco:target (0..1)
	- esco:targetDescription (0..n)
	- esco:targetNotation(0..n)
	- esco:targetName(0..n)
	- esco:targetURL (0..1)
		</rdfs:comment>
        <rdfs:isDefinedBy rdf:resource="http://data.europa.eu/esco/model"/>
        <rdfs:label xml:lang="en">Association object</rdfs:label>
    </owl:Class>



    <!-- http://data.europa.eu/esco/model#AssociationType -->

    <owl:Class rdf:about="http://data.europa.eu/esco/model#AssociationType">
        <rdfs:subClassOf rdf:resource="http://www.w3.org/2004/02/skos/core#Concept"/>
        <rdfs:comment xml:lang="en">The class of association types used in the metadata schema. The relations from a  qualification  to other semantic assets (nodes from other semantic frameworks and or classification systems) are &apos;typed relations&apos;.
	The different association types and their semantics in the metadata schema are SKOS Concepts that are part of a taxonomy managed by the metadata schema (see &lt;http://data.europa.eu/esco/concept-scheme/association-type&gt;)</rdfs:comment>
        <rdfs:isDefinedBy rdf:resource="http://data.europa.eu/esco/model"/>
        <rdfs:label xml:lang="en">association type</rdfs:label>
        <rdfs:seeAlso rdf:resource="http://data.europa.eu/esco/model#AssociationObject"/>
        <owl:deprecated rdf:datatype="http://www.w3.org/2001/XMLSchema#boolean">true</owl:deprecated>
        <vs:term_status>deprecated</vs:term_status>
    </owl:Class>



    <!-- http://data.europa.eu/esco/model#AwardingActivity -->

    <owl:Class rdf:about="http://data.europa.eu/esco/model#AwardingActivity">
        <rdfs:comment xml:lang="en">An awarding activity represents an activity related to the awarding of a qualification. It is used to specify an awarding body, a country or region where the qualification is awarded and optionally an awarding period.</rdfs:comment>
        <rdfs:isDefinedBy rdf:resource="http://data.europa.eu/esco/model"/>
        <rdfs:label xml:lang="en">Awarding activity</rdfs:label>
        <rdfs:seeAlso rdf:resource="http://data.europa.eu/esco/model#hasAwardingActivity"/>
    </owl:Class>



    <!-- http://data.europa.eu/esco/model#AwardingBody -->

    <owl:Class rdf:about="http://data.europa.eu/esco/model#AwardingBody">
        <rdfs:subClassOf rdf:resource="http://www.w3.org/ns/org#Organization"/>
        <rdfs:comment xml:lang="en">&quot;Additional properties defined by the QMS are:
	    - dcterms:spatial (0..1) main site location</rdfs:comment>
        <rdfs:comment xml:lang="en">An awarding body is an institution, organization or company that is recognised (official or otherwise) for issuing qualifications (certificates, diplomas or titles) and formally recognising the learning outcomes (knowledge, skills and/or competences) of an individual, following an assessment and validation procedure.</rdfs:comment>
        <rdfs:comment xml:lang="en">For the minimal set of properties on an AwardingBody see usage note http://xmlns.com/foaf/0.1/Agent.</rdfs:comment>
        <rdfs:isDefinedBy rdf:resource="http://data.europa.eu/esco/model"/>
        <rdfs:label xml:lang="en">Awarding body</rdfs:label>
        <rdfs:seeAlso rdf:resource="http://www.w3.org/ns/org#Organization"/>
        <rdfs:seeAlso rdf:resource="http://xmlns.com/foaf/0.1/Agent"/>
    </owl:Class>



    <!-- http://data.europa.eu/esco/model#Concept -->

    <owl:Class rdf:about="http://data.europa.eu/esco/model#Concept">
        <rdfs:subClassOf rdf:resource="http://www.w3.org/2004/02/skos/core#Concept"/>
        <rdfs:subClassOf>
            <owl:Restriction>
                <owl:onProperty rdf:resource="http://purl.org/dc/terms/identifier"/>
                <owl:minCardinality rdf:datatype="http://www.w3.org/2001/XMLSchema#nonNegativeInteger">1</owl:minCardinality>
            </owl:Restriction>
        </rdfs:subClassOf>
        <owl:disjointWith rdf:resource="http://data.europa.eu/esco/model#EQFLevel"/>
        <owl:disjointWith rdf:resource="http://data.europa.eu/esco/model#FoETCode"/>
        <owl:disjointWith rdf:resource="http://data.europa.eu/esco/model#Language"/>
        <owl:disjointWith rdf:resource="http://data.europa.eu/esco/model#Location"/>
        <owl:disjointWith rdf:resource="http://data.europa.eu/esco/model#NACECode"/>
        <owl:disjointWith rdf:resource="http://data.europa.eu/esco/model#WorkContext"/>
        <owl:disjointUnionOf rdf:parseType="Collection">
            <rdf:Description rdf:about="http://data.europa.eu/esco/model#FacetedConcept"/>
            <rdf:Description rdf:about="http://data.europa.eu/esco/model#SimpleConcept"/>
        </owl:disjointUnionOf>
        <owl:disjointUnionOf rdf:parseType="Collection">
            <rdf:Description rdf:about="http://data.europa.eu/esco/model#Occupation"/>
            <rdf:Description rdf:about="http://data.europa.eu/esco/model#Qualification"/>
            <rdf:Description rdf:about="http://data.europa.eu/esco/model#Skill"/>
        </owl:disjointUnionOf>
        <terms:issued rdf:datatype="http://www.w3.org/2001/XMLSchema#date">2013-06-27</terms:issued>
        <terms:modified rdf:datatype="http://www.w3.org/2001/XMLSchema#date">2016-06-08</terms:modified>
        <rdfs:comment xml:lang="en">The class of ESCO pillar concepts.

ESCO pillar concepts are divided in tree semantic classes: esco:Occupation, esco:Skill and esco:Qualification, each organized in a dedicated ConceptScheme.

All concepts are specializations of skos:Concept and are structured using the skos semantic relationships.
- skos:mappingRelation is used to relate ESCO concepts to similar concepts in other concept schemes (e.g. ISCO-08 or ROME). The mapping to ISCO has particular business relevance and uses a special mapping sub-property (see http://data.europa.eu/esco/model#Occupation and  http://data.europa.eu/esco/model#memberOfISCOGroup).
- sub-properties of skos:related are used to express special relations among ESCO pillar concepts. (e.g. http://data.europa.eu/esco/model#isEssentialSkillFor)
- sub-properties of the DCMI terms:subject capture codified characteristics of ESCO concepts (e.g. http://data.europa.eu/esco/model#hasNACECode, http://data.europa.eu/esco/model#skillType).

The skos:broader and skos:narrower concepts are the prime concepts organizing hierarchy among ESCO pillar concepts.
The hierarchical structure is modelled according three classes
- esco:GroupConcept (see http://data.europa.eu/esco/model#GroupConcept) - the top level concepts, only used for strucutring. These concepts typically are not relevant for annotating CV or job postings.
- esco:LeafGroupConcept (see http://data.europa.eu/esco/model#LeafGroupConcept) - the lowest top level concept, a special esco:GroupConcept.
- esco:MemberConccept (see http://data.europa.eu/esco/model#MemberConcept) - the concepts used for coding or annotating CV and Job Postings.

The ESCO concepts are also divided according their analytical structure.  There are two sub-classes:
- simple concepts (see http://data.europa.eu/esco/model#SimpleConcept) and
- compound concepts (see http://data.europa.eu/esco/model#FacetedConcept).

A concept specialized by faceted concepts holds the labels of each of the faceted concepts in the property http://data.europa.eu/esco/model#plusUF.  These labels are not synonyms or alternate labels.

Among hierarchical related ESCO pillar concepts the following inheritance rules apply
- the ESCO relationships from any broader transitive concept are inherited with the following restrictions
  in case a relationship with the same skill is typed as well essential as optional, only the essential skill relationship is inherited
  in case a relationship with the same qualification is typed as well required as legally required, only the legally required qualification relationship is inherited
- the occasional tagging of the faceted concept (with NUTS, NACE, FoET, ISCO, SkillType, SkillReuseLevel ... codes) must be equal or more specific (specialized) than the code of any of its broader transitive ESCO concepts.

The ESCO concepts are specializations of skos:Concepts and use skos:note specializations (see http://www.w3.org/2004/02/skos/core#note).
- the skos:definition gives the full description of the ESCO concept.
- the skos:scopeNote is the practical instruction for when to apply the ESCO concept.
- the skos:historyNote gives a system log of significant versioned changes to the ESCO concept.
- the skos:changeNote gives the human provided documentation for ESCO concept version modifications.

Characteristics:
- At the time of publication, the ESCO concepts are available in Icelandic and the official languages of the European Union, except Irish.  Per release, actual languages covered are provided by esco:supportedLanguage.  Some concepts are originally developped in a reference language.  This particular language is indicated by http://data.europa.eu/esco/model#referenceLanguage,
- Any ESCO concept may refer relevant hyperlinked sources of reference or of information. See http://data.europa.eu/esco/model#relevantURL.

Each ESCO pillar concept may hold provenance and audit metadata:
- rightsHolder: the owner (http://purl.org/dc/terms/rightsHolder) - optional
- editorial status (http://data.europa.eu/esco/model#editorialStatus) - required
- publishing status (http://purl.org/iso25964/skos-thes#status) - required
- creator : the author (http://purl.org/dc/terms/creator) - optional
- contributor : modifier (http://purl.org/dc/terms/contributor) - required
- modified : last modification date (http://purl.org/dc/terms/modified) - required</rdfs:comment>
        <rdfs:isDefinedBy rdf:resource="http://data.europa.eu/esco/model" />
        <rdfs:label xml:lang="en">ESCO Concept</rdfs:label>
        <rdfs:seeAlso rdf:resource="http://data.europa.eu/esco/model#FacetedConcept"/>
        <rdfs:seeAlso rdf:resource="http://data.europa.eu/esco/model#GroupConcept"/>
        <rdfs:seeAlso rdf:resource="http://data.europa.eu/esco/model#LeafGroupConcept"/>
        <rdfs:seeAlso rdf:resource="http://data.europa.eu/esco/model#MemberConcept"/>
        <rdfs:seeAlso rdf:resource="http://data.europa.eu/esco/model#SimpleConcept"/>
        <rdfs:seeAlso rdf:resource="http://data.europa.eu/esco/model#editorialStatus"/>
        <rdfs:seeAlso rdf:resource="http://data.europa.eu/esco/model#plusUF"/>
        <rdfs:seeAlso rdf:resource="http://purl.org/dc/terms/contributor"/>
        <rdfs:seeAlso rdf:resource="http://purl.org/dc/terms/creator"/>
        <rdfs:seeAlso rdf:resource="http://purl.org/dc/terms/modified"/>
        <rdfs:seeAlso rdf:resource="http://purl.org/dc/terms/rightsHolder"/>
        <rdfs:seeAlso rdf:resource="http://purl.org/dc/terms/subject"/>
        <rdfs:seeAlso rdf:resource="http://purl.org/iso25964/skos-thes#status"/>
        <owl:deprecated rdf:datatype="http://www.w3.org/2001/XMLSchema#boolean">true</owl:deprecated>
        <vs:term_status rdf:datatype="http://www.w3.org/2001/XMLSchema#string">deprecated</vs:term_status>
    </owl:Class>



    <!-- http://data.europa.eu/esco/model#ConceptScheme -->

    <owl:Class rdf:about="http://data.europa.eu/esco/model#ConceptScheme">
        <rdfs:subClassOf rdf:resource="http://www.w3.org/2004/02/skos/core#ConceptScheme"/>
        <terms:issued rdf:datatype="http://www.w3.org/2001/XMLSchema#date">2013-06-27</terms:issued>
        <terms:modified rdf:datatype="http://www.w3.org/2001/XMLSchema#date">2016-04-01</terms:modified>
        <rdfs:comment xml:lang="en">The ESCO concept schemes (pillars)

The &quot;current&quot; ESCO scheme and historic versions of the ESCO scheme will be instances of this class.  Typically, these support poly-hierarchy.

The ISCO representations that are the backbone of at least one ESCO version (v0) also will be represented by this concept scheme.  Typically these do not have poly-hierarchy.


Provenance information that may be added:
- rightsHolder: the owner (http://purl.org/dc/terms/rightsHolder) - required
- publishing status: (http://purl.org/iso25964/skos-thes#status) - required
- creator : the author (http://purl.org/dc/terms/creator) - required
- contributor : modifier (http://purl.org/dc/terms/contributor) - required
- modified : last modification date (http://purl.org/dc/terms/modified) - required</rdfs:comment>
        <rdfs:isDefinedBy rdf:resource="http://data.europa.eu/esco/model" />
        <rdfs:label xml:lang="en">Concept scheme (ESCO pillar)</rdfs:label>
        <rdfs:seeAlso rdf:resource="http://purl.org/dc/terms/contributor"/>
        <rdfs:seeAlso rdf:resource="http://purl.org/dc/terms/creator"/>
        <rdfs:seeAlso rdf:resource="http://purl.org/dc/terms/modified"/>
        <rdfs:seeAlso rdf:resource="http://purl.org/dc/terms/rightsHolder"/>
        <rdfs:seeAlso rdf:resource="http://purl.org/iso25964/skos-thes#status"/>
        <vs:term_status>released</vs:term_status>
    </owl:Class>



    <!-- http://data.europa.eu/esco/model#Country -->

    <owl:Class rdf:about="http://data.europa.eu/esco/model#Country">
        <rdfs:subClassOf rdf:resource="http://data.europa.eu/esco/model#Location"/>
        <terms:issued rdf:datatype="http://www.w3.org/2001/XMLSchema#date">2013-06-27</terms:issued>
        <terms:modified rdf:datatype="http://www.w3.org/2001/XMLSchema#date">2016-06-10</terms:modified>
        <rdfs:comment xml:lang="en">Relevant standards for country locations are documented under the super class: http://data.europa.eu/esco/model#Location</rdfs:comment>
        <rdfs:isDefinedBy rdf:resource="http://data.europa.eu/esco/model"/>
        <rdfs:label xml:lang="en">Country</rdfs:label>
        <owl:deprecated rdf:datatype="http://www.w3.org/2001/XMLSchema#boolean">true</owl:deprecated>
        <vs:term_status rdf:datatype="http://www.w3.org/2001/XMLSchema#string">deprecated</vs:term_status>
    </owl:Class>



    <!-- http://data.europa.eu/esco/model#EQFLevel -->

    <owl:Class rdf:about="http://data.europa.eu/esco/model#EQFLevel">
        <rdfs:subClassOf rdf:resource="http://www.w3.org/2004/02/skos/core#Concept"/>
        <terms:issued rdf:datatype="http://www.w3.org/2001/XMLSchema#date">2013-06-27</terms:issued>
        <terms:modified rdf:datatype="http://www.w3.org/2001/XMLSchema#date">2017-02-10</terms:modified>
        <rdfs:comment xml:lang="en">The EQF levels have been published as recommendation by the EU Publication office under CELEX number 32008H0506(01)
 See http://publications.europa.eu/resource/celex/32008H0506%2801%29</rdfs:comment>
        <rdfs:isDefinedBy rdf:resource="http://data.europa.eu/esco/model"/>
        <rdfs:label xml:lang="en">Level (European Qualification Framework)</rdfs:label>
        <rdfs:seeAlso rdf:resource="http://publications.europa.eu/resource/celex/32008H0506%2801%29"/>
        <owl:deprecated rdf:datatype="http://www.w3.org/2001/XMLSchema#boolean">true</owl:deprecated>
        <vs:term_status rdf:datatype="http://www.w3.org/2001/XMLSchema#string">rejected</vs:term_status>
        <skos:changeNote xml:lang="en">URI of  ESCO copy of EQF will need to be updated in order to get LOD properly working from ESCO platform.</skos:changeNote>
    </owl:Class>



    <!-- http://data.europa.eu/esco/model#EntryRequirement -->

    <owl:Class rdf:about="http://data.europa.eu/esco/model#EntryRequirement">
        <rdfs:comment xml:lang="en">Entry requirements are structured into categories such as work experience, pre-assessment or a specific qualification.
	- The category of an entry requirement is given by dcterms:type property using a skos:Concept from the controlled vocabulary &lt;http://data.europa.eu/esco/concept-scheme/entryrequirement-category&gt;.
	- The requirement level expresses the necessity. It is given by the esco:requirementLevel property using a skos:Concept from the controlled voabulary &lt;http://data.europa.eu/esco/concept-scheme/entryrequirement-level&gt;. </rdfs:comment>
        <rdfs:comment xml:lang="en">The generic class for entry requirements of a qualification. For example a requirement to enter the programme that leads to a qualification, or to access the examination or certification process, such as a prior (professional) experience or a specific qualification.</rdfs:comment>
        <rdfs:isDefinedBy rdf:resource="http://data.europa.eu/esco/model"/>
        <rdfs:label xml:lang="en">entry requirement</rdfs:label>
        <rdfs:seeAlso rdf:resource="http://data.europa.eu/esco/concept-scheme/entryrequirement-category"/>
        <rdfs:seeAlso rdf:resource="http://data.europa.eu/esco/concept-scheme/entryrequirement-level"/>
    </owl:Class>



    <!-- http://data.europa.eu/esco/model#EscoExtension -->

    <owl:Class rdf:about="http://data.europa.eu/esco/model#EscoExtension">
        <rdfs:subClassOf rdf:resource="http://www.w3.org/2004/02/skos/core#Concept"/>
        <terms:issued rdf:datatype="http://www.w3.org/2001/XMLSchema#date">2016-09-02</terms:issued>
        <rdfs:comment xml:lang="en">This class denotes concepts of non-EU relevance separate from the usual scope of ESCO.</rdfs:comment>
        <rdfs:isDefinedBy rdf:resource="http://data.europa.eu/esco/model"/>
        <rdfs:label xml:lang="en">Esco extension</rdfs:label>
    </owl:Class>



    <!-- http://data.europa.eu/esco/model#FacetConceptGroup -->

    <owl:Class rdf:about="http://data.europa.eu/esco/model#FacetConceptGroup">
        <rdfs:subClassOf rdf:resource="http://www.w3.org/2004/02/skos/core#Collection"/>
        <rdfs:subClassOf>
            <owl:Restriction>
                <owl:onProperty rdf:resource="http://www.w3.org/2004/02/skos/core#inScheme"/>
                <owl:hasValue rdf:resource="http://data.europa.eu/esco/ConceptScheme/FacetConceptGroups"/>
            </owl:Restriction>
        </rdfs:subClassOf>
        <terms:issued rdf:datatype="http://www.w3.org/2001/XMLSchema#date">2013-12-03</terms:issued>
        <terms:modified rdf:datatype="http://www.w3.org/2001/XMLSchema#date">2016-06-08</terms:modified>
        <rdfs:comment xml:lang="en">A Facet concept group (i.e. an instance of the class esco:FacetConceptGroup) is a sub-set of concepts from a facet.
A facet is a supporting taxonomy for ESCO.  Examples are:
- Languages
- Species
- Tools

An (instance of the) esco:FacetConceptGroup is a sub-set of concepts from a facet.
Each esco:FacetConceptGroup is defined by the ESCO concept scheme http://data.europa.eu/esco/ConceptScheme/FacetConceptGroups.
The typical use of an esco:FacetConceptGroup is to specialize one or more ESCO pillar concepts. (see http://data.europa.eu/esco/model#facet).
The specialization creates narrower (or transitive narrower) concepts of the specialized ESCO pillar concept.
Each specialization is a Faceted (or compound) concept (with type http://data.europa.eu/esco/model#FacetedConcept) having as component concepts:
- the ESCO pillar object being specialized and
- one member concept from the facet group.

An ESCO pillar concept is either an esco:SimpleConcept or an esco:FacetedConcept

An ESCO concept can be specialized in different ways using different Facet concept groups

The Facet concept group may be structured:
- members of an esco:FacetConceptGroup can have hierarchical relationships (skos:broader and skos:narrower) among its member concepts.
  If this is the case, the hierarchical structure among the specialized concepts constructed with this facet group will mirror the hierarchy of the facet group.
  See also skos:topMember.
- an esco:FacetConceptGroup can be an oredered collection.
  In this case, the order among the spicialized concepts constructed with this facet group will mirror the order of the facet group.
- an esco:FacetConceptGroup can have different sub-collections (i.e. have skos:member that are a skos:Collection and an iso-thes:ThesaurusArray).
  Collections only serve to organize the constructed faceted concepts such that the faceted concepts
  that are specializations based on the structured Facet concept group are organized by thesaurus arrays
  that each mirror an original thesaurus array of the Facet concept group.

Example: the language FacetConceptGroup can have as members
- the (possibly ordered) collection of spoken languages
  having as members the language concepts
- the (possibly ordered) collection of sign languages
  having as members the sign language concepts

The name of the facet group is given by skos:prefLabel</rdfs:comment>
        <rdfs:isDefinedBy rdf:resource="http://data.europa.eu/esco/model"/>
        <rdfs:label xml:lang="en">Facet concept group</rdfs:label>
        <rdfs:seeAlso rdf:resource="http://data.europa.eu/esco/model#FacetedConcept"/>
        <rdfs:seeAlso rdf:resource="http://data.europa.eu/esco/model#SimpleConcept"/>
        <rdfs:seeAlso rdf:resource="http://data.europa.eu/esco/model#facet"/>
        <rdfs:seeAlso rdf:resource="http://www.w3.org/2004/02/skos/core#prefLabel"/>
        <owl:deprecated rdf:datatype="http://www.w3.org/2001/XMLSchema#boolean">true</owl:deprecated>
        <vs:term_status rdf:datatype="http://www.w3.org/2001/XMLSchema#string">rejected</vs:term_status>
    </owl:Class>



    <!-- http://data.europa.eu/esco/model#FacetedConcept -->

    <owl:Class rdf:about="http://data.europa.eu/esco/model#FacetedConcept">
        <rdfs:subClassOf rdf:resource="http://data.europa.eu/esco/model#Concept"/>
        <rdfs:subClassOf>
            <owl:Restriction>
                <owl:onProperty rdf:resource="http://data.europa.eu/esco/model#hasFacet"/>
                <owl:minQualifiedCardinality rdf:datatype="http://www.w3.org/2001/XMLSchema#nonNegativeInteger">1</owl:minQualifiedCardinality>
                <owl:onClass rdf:resource="http://www.w3.org/2004/02/skos/core#Concept"/>
            </owl:Restriction>
        </rdfs:subClassOf>
        <rdfs:subClassOf>
            <owl:Restriction>
                <owl:onProperty rdf:resource="http://data.europa.eu/esco/model#constructedFrom"/>
                <owl:qualifiedCardinality rdf:datatype="http://www.w3.org/2001/XMLSchema#nonNegativeInteger">1</owl:qualifiedCardinality>
                <owl:onClass rdf:resource="http://data.europa.eu/esco/model#SimpleConcept"/>
            </owl:Restriction>
        </rdfs:subClassOf>
        <owl:disjointWith rdf:resource="http://data.europa.eu/esco/model#SimpleConcept"/>
        <terms:issued rdf:datatype="http://www.w3.org/2001/XMLSchema#date">2014-02-03</terms:issued>
        <terms:modified rdf:datatype="http://www.w3.org/2001/XMLSchema#date">2016-06-08</terms:modified>
        <rdfs:comment xml:lang="en">The class of compound ESCO pillar concepts.
A compound concept is a concept that is broken down in a set of mare basic component concepts  (e.g. a pianist is a &apos;musician&apos; performing on a &apos;piano&apos;)

An ESCO concept is either a faceted concept or a simple concept (see http://data.europa.eu/esco/model#SimpleConcept).

An ESCO faceted (or compound) concept is the specialization of an ESCO concept that identifies one or more specialization facets (see http://data.europa.eu/esco/model#facet).
A specializing facet is a group of concepts with a common characteristic (e.g. the group of music instruments).
The specialization makes a compound of the ESCO concept and of one concept of each of its related specializing  facets.

- During the editorial phase, one or more faceted concepts may be created ad hoc by the ESCO taxonomists.
- During the ESCO publishing phase all possible faceted concepts are generated by the publication process.  The process adds the possible compound conepts that were not created by the (human) taxonomist.
- Each faceted concept is the specialization (i.e. the skos:narrowerTransitive) of an ESCO simple concept (see http://data.europa.eu/esco/model#constructedFrom)
- All facet componets (i.e. the facet values) of the faceted conept are given by the property http://data.europa.eu/esco/model#hasFacet

Uniqueness rule:
Two instances of esco:FacetedConcept are the same if and only if both instances
- refer the same simple ESCO concept using http://data.europa.eu/esco/model#constructedFrom
- refer the same set of components (facet values) using http://data.europa.eu/esco/model#hasFacet

The faceted concept inherits certain characteristics from the Simple Concept it is constructed from:
- the ESCO pillar type (Occupation, Skill or Qualification) of its simple concept it is constructed from (see esco:constructedFrom).
- the memberOfISCOGroup of the occasional Occupation it is constructed from
- the skillType and the skillReuseLevel of the occasional Skill it is constructed from
Further, inheritance rules apply as on ESCO concepts (see http://data.europa.eu/esco/model#Concept).</rdfs:comment>
        <rdfs:isDefinedBy rdf:resource="http://data.europa.eu/esco/model"/>
        <rdfs:label xml:lang="en">Faceted ESCO concept</rdfs:label>
        <owl:deprecated rdf:datatype="http://www.w3.org/2001/XMLSchema#boolean">true</owl:deprecated>
        <vs:term_status rdf:datatype="http://www.w3.org/2001/XMLSchema#string">rejected</vs:term_status>
        <skos:editorialNote xml:lang="en">
The preferred label of a Faceted concept need not be persisted in the editorial system. It may be automatically constructed on publishing as follows:
   {FacetedConcept prefLabel} :=  {SimpleConcept prefLabel} + &apos;: &apos; + {facet prefLabel}  (  &apos; / &apos; + {facet prefLabel} ) *
   where facet prefLabels are ordered alhabetically.
   The (gender related) label roles are inherited from the prefered label of the SimplConcept.
Occasionally the automated pref label will be overruled by a compound label.</skos:editorialNote>
    </owl:Class>



    <!-- http://data.europa.eu/esco/model#FoETCode -->

    <owl:Class rdf:about="http://data.europa.eu/esco/model#FoETCode">
        <rdfs:subClassOf rdf:resource="http://www.w3.org/2004/02/skos/core#Concept"/>
        <terms:issued rdf:datatype="http://www.w3.org/2001/XMLSchema#date">2013-12-03</terms:issued>
        <terms:modified rdf:datatype="http://www.w3.org/2001/XMLSchema#date">2016-06-08</terms:modified>
        <rdfs:comment xml:lang="en">The class of ISCED 2013/FoET classificaton code (International Standard Classification of Education: Fields of Education and Training 2013)

The Fields of Education and Training have been submitted to the UNESCO Conference - session 37 - Paris.
The version submitted for resolution is available from: http://unesdoc.unesco.org/images/0022/002218/221863e.pdf

Other original source references:
- http://www.uis.unesco.org/Education/Documents/isced-37c-fos-review-222729e.pdf
- http://www.uis.unesco.org/EDUCATION/Pages/international-standard-classification-of-education.aspx</rdfs:comment>
        <rdfs:isDefinedBy rdf:resource="http://data.europa.eu/esco/model"/>
        <rdfs:label xml:lang="en">FoET code</rdfs:label>
        <rdfs:seeAlso rdf:resource="http://unesdoc.unesco.org/images/0022/002218/221863e.pdf"/>
        <rdfs:seeAlso rdf:resource="http://www.uis.unesco.org/EDUCATION/Pages/international-standard-classification-of-education.aspx"/>
        <owl:deprecated rdf:datatype="http://www.w3.org/2001/XMLSchema#boolean">true</owl:deprecated>
        <vs:term_status rdf:datatype="http://www.w3.org/2001/XMLSchema#string">rejected</vs:term_status>
    </owl:Class>



    <!-- http://data.europa.eu/esco/model#GroupConcept -->

    <owl:Class rdf:about="http://data.europa.eu/esco/model#GroupConcept">
        <rdfs:subClassOf rdf:resource="http://www.w3.org/2004/02/skos/core#Concept"/>
        <rdfs:subClassOf>
            <owl:Restriction>
                <owl:onProperty rdf:resource="http://www.w3.org/2004/02/skos/core#broader"/>
                <owl:allValuesFrom rdf:resource="http://data.europa.eu/esco/model#GroupConcept"/>
            </owl:Restriction>
        </rdfs:subClassOf>
        <owl:disjointWith rdf:resource="http://data.europa.eu/esco/model#MemberConcept"/>
        <terms:issued rdf:datatype="http://www.w3.org/2001/XMLSchema#date">2013-06-27</terms:issued>
        <terms:modified rdf:datatype="http://www.w3.org/2001/XMLSchema#date">2016-06-08</terms:modified>
        <rdfs:comment xml:lang="en">Concepts
 of this type are aggregations.  The property http://data.europa.eu/esco/model#hasGroupMember gives the members concepts of the group.  The member concepts have type http://data.europa.eu/esco/model#MemberConcept.  These member concepts are skos:narrowerTransitive spcializations of the group concept.  Among GroupConcept, the skos:broader/skos:narrower is like a super-group/sub-group relation meaning that all members of the (narrower) sub-group also are members of the (broader) super-group.

Typically these group concepts are NOT used in CV or job postings, but serve organization, reporting and statiscal purposes.
The member concepts of group concepts are used for coding or annotating CV or job postings.

A Group concept typically will be
- in the upper levels of an ESCO pillar (or concept schema)
- in an external concept schema (e.g. ISCO)</rdfs:comment>
        <rdfs:isDefinedBy rdf:resource="http://data.europa.eu/esco/model"/>
        <rdfs:label xml:lang="en">Group concept</rdfs:label>
        <owl:deprecated rdf:datatype="http://www.w3.org/2001/XMLSchema#boolean">true</owl:deprecated>
        <vs:term_status rdf:datatype="http://www.w3.org/2001/XMLSchema#string">deprecated</vs:term_status>
    </owl:Class>



    <!-- http://data.europa.eu/esco/model#Label -->

    <owl:Class rdf:about="http://data.europa.eu/esco/model#Label">
        <rdfs:subClassOf rdf:resource="http://www.w3.org/2008/05/skos-xl#Label"/>
        <terms:issued rdf:datatype="http://www.w3.org/2001/XMLSchema#date">2013-06-27</terms:issued>
        <terms:modified rdf:datatype="http://www.w3.org/2001/XMLSchema#date">2016-06-08</terms:modified>
        <rdfs:comment xml:lang="en">The class of labels used on esco Concepts.

Characteristics
- An ESCO label may be motivated by relevant original sources.  These sources are referenced uising http://data.europa.eu/esco/model#relevantURL
- An ESCO label typically gets label roles detailing the gender specific characteristics of the label (see http://data.europa.eu/esco/model#hasLabelRole)

Provenance information that may be added:
- rightsHolder: the owner (http://purl.org/dc/terms/rightsHolder) - optional
- editorial status (http://data.europa.eu/esco/model#editorialStatus) - optional
- workflow status (http://data.europa.eu/esco/flow#status) - required
- creator : the author (http://purl.org/dc/terms/creator) - optional
- contributor : modifier (http://purl.org/dc/terms/contributor) - required
- modified : last modification date (http://purl.org/dc/terms/modified) - required</rdfs:comment>
        <rdfs:isDefinedBy rdf:resource="http://data.europa.eu/esco/model" />
        <rdfs:label xml:lang="en">ESCO concept Label</rdfs:label>
        <rdfs:seeAlso rdf:resource="http://data.europa.eu/esco/model#hasLabelRole"/>
        <rdfs:seeAlso rdf:resource="http://purl.org/dc/terms/contributor"/>
        <rdfs:seeAlso rdf:resource="http://purl.org/dc/terms/creator"/>
        <rdfs:seeAlso rdf:resource="http://purl.org/dc/terms/modified"/>
        <rdfs:seeAlso rdf:resource="http://purl.org/dc/terms/rightsHolder"/>
        <rdfs:seeAlso rdf:resource="itm:status"/>
        <owl:deprecated rdf:datatype="http://www.w3.org/2001/XMLSchema#boolean">true</owl:deprecated>
        <vs:term_status rdf:datatype="http://www.w3.org/2001/XMLSchema#string">deprecated</vs:term_status>
    </owl:Class>



    <!-- http://data.europa.eu/esco/model#LabelRole -->

    <owl:Class rdf:about="http://data.europa.eu/esco/model#LabelRole">
        <owl:equivalentClass>
            <owl:Restriction>
                <owl:onProperty rdf:resource="http://www.w3.org/2004/02/skos/core#inScheme"/>
                <owl:hasValue rdf:resource="http://data.europa.eu/esco/ConceptScheme/LabelRole"/>
            </owl:Restriction>
        </owl:equivalentClass>
        <rdfs:subClassOf rdf:resource="http://www.w3.org/2004/02/skos/core#Concept"/>
        <terms:issued rdf:datatype="http://www.w3.org/2001/XMLSchema#date">2013-06-27</terms:issued>
        <terms:modified rdf:datatype="http://www.w3.org/2001/XMLSchema#date">2013-12-03</terms:modified>
        <rdfs:comment xml:lang="en">Allows to capture one or more particular characteristics of a name.

Example usage: Gender related terms.
- ESCO concepts may get a gender neutral term as preferred label.  The gender specific terms are provided as alternate labels.
- Relevant use cases:
  - concept look-up based on gender specific term
  - Job posting generation with gender neutral terms
  - CV generation with gender specific terms</rdfs:comment>
        <rdfs:isDefinedBy rdf:resource="http://data.europa.eu/esco/model" />
        <rdfs:label xml:lang="en">Label role</rdfs:label>
        <vs:term_status rdf:datatype="http://www.w3.org/2001/XMLSchema#string">proposed</vs:term_status>
    </owl:Class>



    <!-- http://data.europa.eu/esco/model#Language -->

    <owl:Class rdf:about="http://data.europa.eu/esco/model#Language">
        <rdfs:subClassOf rdf:resource="http://www.w3.org/2004/02/skos/core#Concept"/>
        <rdfs:subClassOf>
            <owl:Restriction>
                <owl:onProperty rdf:resource="http://data.europa.eu/esco/model#language"/>
                <owl:cardinality rdf:datatype="http://www.w3.org/2001/XMLSchema#nonNegativeInteger">1</owl:cardinality>
            </owl:Restriction>
        </rdfs:subClassOf>
        <terms:issued rdf:datatype="http://www.w3.org/2001/XMLSchema#date">2013-06-27</terms:issued>
        <terms:modified rdf:datatype="http://www.w3.org/2001/XMLSchema#date">2016-06-10</terms:modified>
        <rdfs:comment xml:lang="en">The class of language concepts.
Each language is
- labeled using skos:prefLabel in all of the other languages and
- identified using the ESCO esco:language property (value = ISO 2-char language code).

The class provides the set of languages that can be in use in the thesaurus.
Two ESCO concept schemes provide language concepts:
- http://data.europa.eu/esco/ConceptScheme/ISO639/cs - all languages of ISO 639-1 and ISO 639-2
- http://data.europa.eu/esco/ConceptScheme/ISO639-3/cs - all sign languages listed in ISO 639-3

The esco:ConceptScheme identifies the languages actually used via its property esco:supportedLanguage.</rdfs:comment>
        <rdfs:isDefinedBy rdf:resource="http://data.europa.eu/esco/model" />
        <rdfs:label xml:lang="en">Language</rdfs:label>
        <owl:deprecated rdf:datatype="http://www.w3.org/2001/XMLSchema#boolean">true</owl:deprecated>
        <vs:term_status rdf:datatype="http://www.w3.org/2001/XMLSchema#string">deprecated</vs:term_status>
    </owl:Class>



    <!-- http://data.europa.eu/esco/model#LeafGroupConcept -->

    <owl:Class rdf:about="http://data.europa.eu/esco/model#LeafGroupConcept">
        <rdfs:subClassOf rdf:resource="http://data.europa.eu/esco/model#GroupConcept"/>
        <terms:issued rdf:datatype="http://www.w3.org/2001/XMLSchema#date">2013-06-27</terms:issued>
        <terms:modified rdf:datatype="http://www.w3.org/2001/XMLSchema#date">2016-06-08</terms:modified>
        <rdfs:comment xml:lang="en">A Group (or aggregation) concept, having no sub-groups anymore.

Narrower concepts only can be members (or narrower instances) of the group concept.
The specialization http://data.europa.eu/esco/model#narrowerInstance of skos:narrower is used to identify the top level members of the group.</rdfs:comment>
        <rdfs:isDefinedBy rdf:resource="http://data.europa.eu/esco/model"/>
        <rdfs:label xml:lang="en">Leaf-group concept</rdfs:label>
        <rdfs:seeAlso rdf:resource="http://data.europa.eu/esco/model#MemberConcept"/>
        <owl:deprecated rdf:datatype="http://www.w3.org/2001/XMLSchema#boolean">true</owl:deprecated>
        <vs:term_status rdf:datatype="http://www.w3.org/2001/XMLSchema#string">deprecated</vs:term_status>
    </owl:Class>



    <!-- http://data.europa.eu/esco/model#Location -->

    <owl:Class rdf:about="http://data.europa.eu/esco/model#Location">
        <rdfs:subClassOf rdf:resource="http://www.w3.org/2004/02/skos/core#Concept"/>
        <terms:issued rdf:datatype="http://www.w3.org/2001/XMLSchema#date">2013-06-27</terms:issued>
        <terms:modified rdf:datatype="http://www.w3.org/2001/XMLSchema#date">2016-06-10</terms:modified>
        <rdfs:comment xml:lang="en">A teritorial area like a federation, a country, a region, a jurisdiction area.

Standards useful for locations and regions:
- ISO 3166
- NUTS - http://epp.eurostat.ec.europa.eu/portal/page/portal/nuts_nomenclature/introduction (extends ISO 3166 with sub-regions)
- geonames - http://www.geonames.org/ (includes ISO 3166)
- EU publication Office - http://publications.europa.eu/mdr/authority/country/index.html</rdfs:comment>
        <rdfs:isDefinedBy rdf:resource="http://data.europa.eu/esco/model"/>
        <rdfs:label xml:lang="en">Location</rdfs:label>
        <owl:deprecated rdf:datatype="http://www.w3.org/2001/XMLSchema#boolean">true</owl:deprecated>
        <vs:term_status rdf:datatype="http://www.w3.org/2001/XMLSchema#string">rejected</vs:term_status>
    </owl:Class>



    <!-- http://data.europa.eu/esco/model#MemberConcept -->

    <owl:Class rdf:about="http://data.europa.eu/esco/model#MemberConcept">
        <rdfs:subClassOf rdf:resource="http://www.w3.org/2004/02/skos/core#Concept"/>
        <owl:disjointUnionOf rdf:parseType="Collection">
            <rdf:Description rdf:about="http://data.europa.eu/esco/model#Occupation"/>
            <rdf:Description rdf:about="http://data.europa.eu/esco/model#Qualification"/>
            <rdf:Description rdf:about="http://data.europa.eu/esco/model#Skill"/>
        </owl:disjointUnionOf>
        <terms:issued rdf:datatype="http://www.w3.org/2001/XMLSchema#date">2013-06-27</terms:issued>
        <terms:modified rdf:datatype="http://www.w3.org/2001/XMLSchema#date">2017-02-10</terms:modified>
        <rdfs:comment xml:lang="en">Concepts of this class are specifically used to be referenced in CV or job postings.  Typically these concepts are at the more specialized levels of the hierarchy.
Example: A particular occupation, not a group of occupations.
These concepts in general have
However, some Member concept may be specializations of other ones.  In general these specializations will not comply to (1). General group membership within ESCO pillars is provided by esco:memberOfGroup.</rdfs:comment>
        <rdfs:isDefinedBy rdf:resource="http://data.europa.eu/esco/model"/>
        <rdfs:label>Member concept</rdfs:label>
        <vs:term_status rdf:datatype="http://www.w3.org/2001/XMLSchema#string">released</vs:term_status>
    </owl:Class>



    <!-- http://data.europa.eu/esco/model#NACECode -->

    <owl:Class rdf:about="http://data.europa.eu/esco/model#NACECode">
        <rdfs:subClassOf rdf:resource="http://www.w3.org/2004/02/skos/core#Concept"/>
        <terms:issued rdf:datatype="http://www.w3.org/2001/XMLSchema#date">2013-12-05</terms:issued>
        <terms:modified rdf:datatype="http://www.w3.org/2001/XMLSchema#date">2016-06-08</terms:modified>
        <rdfs:comment xml:lang="en">Industry sector code NACE rev2

The NACE codes are published in http://epp.eurostat.ec.europa.eu/cache/ITY_OFFPUB/KS-RA-07-015/EN/KS-RA-07-015-EN.PDF
The RDF version is available from: http://ec.europa.eu/eurostat/ramon/rdfdata/nace_r2.rdf - Note, this is not SKOS but can be made SKOS compliant.
ESCO keeps a SKOS compliant copy of NACE codes. These are organized in the concept scheme http://data.europa.eu/esco/ConceptScheme/NACErev2/cs</rdfs:comment>
        <rdfs:isDefinedBy rdf:resource="http://data.europa.eu/esco/model"/>
        <rdfs:label xml:lang="en">NACE code</rdfs:label>
        <rdfs:seeAlso rdf:resource="http://ec.europa.eu/eurostat/ramon/rdfdata/nace_r2.rdf"/>
        <rdfs:seeAlso rdf:resource="http://epp.eurostat.ec.europa.eu/cache/ITY_OFFPUB/KS-RA-07-015/EN/KS-RA-07-015-EN.PDF"/>
        <owl:deprecated rdf:datatype="http://www.w3.org/2001/XMLSchema#boolean">true</owl:deprecated>
        <vs:term_status>deprecated</vs:term_status>
    </owl:Class>



    <!-- http://data.europa.eu/esco/model#NodeLiteral -->

    <owl:Class rdf:about="http://data.europa.eu/esco/model#NodeLiteral">
        <rdfs:subClassOf rdf:resource="http://www.w3.org/2004/02/skos/core#Concept"/>
        <rdfs:subClassOf>
            <owl:Restriction>
                <owl:onProperty rdf:resource="http://purl.org/dc/terms/subject"/>
                <owl:minCardinality rdf:datatype="http://www.w3.org/2001/XMLSchema#nonNegativeInteger">0</owl:minCardinality>
            </owl:Restriction>
        </rdfs:subClassOf>
        <rdfs:subClassOf>
            <owl:Restriction>
                <owl:onProperty rdf:resource="http://data.europa.eu/esco/model#language"/>
                <owl:maxCardinality rdf:datatype="http://www.w3.org/2001/XMLSchema#nonNegativeInteger">1</owl:maxCardinality>
            </owl:Restriction>
        </rdfs:subClassOf>
        <rdfs:subClassOf>
            <owl:Restriction>
                <owl:onProperty rdf:resource="http://data.europa.eu/esco/model#nodeLiteral"/>
                <owl:cardinality rdf:datatype="http://www.w3.org/2001/XMLSchema#nonNegativeInteger">1</owl:cardinality>
            </owl:Restriction>
        </rdfs:subClassOf>
        <rdfs:comment xml:lang="en">Free text metadata fields, such as the description, a historical or additional note of a qualification can contain a plain text or a XHTML fragment as literal value. By using a NodeLiteral both the datatype of the literal as the language can be specified.</rdfs:comment>
        <rdfs:comment xml:lang="en">The class used to specify Literals that can have both a datatype and a language tag</rdfs:comment>
        <rdfs:isDefinedBy rdf:resource="http://data.europa.eu/esco/model"/>
        <rdfs:label xml:lang="en">node literal</rdfs:label>
    </owl:Class>



    <!-- http://data.europa.eu/esco/model#Occupation -->

    <owl:Class rdf:about="http://data.europa.eu/esco/model#Occupation">
        <rdfs:subClassOf rdf:resource="http://data.europa.eu/esco/model#MemberConcept"/>
        <rdfs:subClassOf>
            <owl:Restriction>
                <owl:onProperty rdf:resource="http://www.w3.org/2004/02/skos/core#inScheme"/>
                <owl:hasValue rdf:resource="http://data.europa.eu/esco/ConceptScheme/ESCO_Occupations"/>
            </owl:Restriction>
        </rdfs:subClassOf>
        <owl:disjointWith rdf:resource="http://data.europa.eu/esco/model#Qualification"/>
        <owl:disjointWith rdf:resource="http://data.europa.eu/esco/model#Skill"/>
        <terms:issued rdf:datatype="http://www.w3.org/2001/XMLSchema#date">2013-06-27</terms:issued>
        <terms:modified rdf:datatype="http://www.w3.org/2001/XMLSchema#date">2017-02-10</terms:modified>
        <rdfs:comment xml:lang="en">The class of ESCO Occupation concepts. An Occuaption is an ESCO pillar concept (see http://data.europa.eu/esco/model#MemberConcept).


Characteristics of an Occupation:
- The relevant industry sector for an occupation is given by the Eurostat NACE codes (see http://data.europa.eu/esco/model#hasNACECode)
- The different Work context applicable for an occupation (see http://data.europa.eu/esco/model#hasWorkContext).

An occupation may be related to
- esco:Skill (see http://data.europa.eu/esco/model#relatedEssentialSkill and http://data.europa.eu/esco/model#relatedOptionalSkill)
- esco:Qualification (see http://data.europa.eu/esco/model#AssociationObject)

Occupations having a legal or other regulations in a specific region
- must identify these regulations in the occupation definition (and refer the professional DB stating that regulation - e.g. http://ec.europa.eu/internal_market/qualifications/regprof/index.cfm?action=profession&amp;id_profession=12142)
- could identify such a region with the location property (see http://data.europa.eu/esco/model#location)

ESCO Occupations are maintained in the ESCO concept scheme http://data.europa.eu/esco/ConceptScheme/ESCO_Occupations.</rdfs:comment>
        <rdfs:isDefinedBy rdf:resource="http://data.europa.eu/esco/model"/>
        <rdfs:label xml:lang="en">Occupation</rdfs:label>
        <rdfs:seeAlso rdf:resource="http://data.europa.eu/esco/model#Concept"/>
        <rdfs:seeAlso rdf:resource="http://data.europa.eu/esco/model#hasNACECode"/>
        <rdfs:seeAlso rdf:resource="http://data.europa.eu/esco/model#location"/>
        <rdfs:seeAlso rdf:resource="http://data.europa.eu/esco/model#memberOfISCOGroup"/>
        <vs:term_status rdf:datatype="http://www.w3.org/2001/XMLSchema#string">released</vs:term_status>
        <skos:historyNote xml:lang="en">2013-06-27
An Occupation that is a MemberConcept:
- Initially coming from the Occupations listed by the Swedisch PES in tab of file Taxonomy 3 - Taxonomy db DB 20 l-corr.xls.
An Occupation that is a GroupConcept:
- Initially coming from the file ISCO &apos;88 codes 25l.xls</skos:historyNote>
    </owl:Class>



    <!-- http://data.europa.eu/esco/model#OverlappingSkillGroup -->

    <owl:Class rdf:about="http://data.europa.eu/esco/model#OverlappingSkillGroup">
        <rdfs:subClassOf rdf:resource="http://www.w3.org/2004/02/skos/core#Collection"/>
        <rdfs:subClassOf>
            <owl:Restriction>
                <owl:onProperty rdf:resource="http://www.w3.org/2004/02/skos/core#inScheme"/>
                <owl:hasValue rdf:resource="http://data.europa.eu/esco/ConceptScheme/ESCO_Skills"/>
            </owl:Restriction>
        </rdfs:subClassOf>
        <terms:issued rdf:datatype="http://www.w3.org/2001/XMLSchema#date">2014-08-10</terms:issued>
        <terms:modified rdf:datatype="http://www.w3.org/2001/XMLSchema#date">2016-06-08</terms:modified>
        <rdfs:comment xml:lang="en">The class of collections of overlapping esco:Skill concepts. All skills within one collection of overlapping skills have overlapping semantics with each other.

The collection has a name using http://www.w3.org/2004/02/skos/core#prefLabel .

As clarifications about the overlapping emerge, a decision from ESCO editorial team may instruct to merge some or all of the member concepts of this collection or to relate its members in another way.</rdfs:comment>
        <rdfs:isDefinedBy rdf:resource="http://data.europa.eu/esco/model"/>
        <rdfs:label xml:lang="en">Group of overlapping skills</rdfs:label>
        <rdfs:seeAlso rdf:resource="http://www.w3.org/2004/02/skos/core#prefLabel"/>
        <owl:deprecated rdf:datatype="http://www.w3.org/2001/XMLSchema#boolean">true</owl:deprecated>
        <vs:term_status rdf:datatype="http://www.w3.org/2001/XMLSchema#string">rejected</vs:term_status>
    </owl:Class>



    <!-- http://data.europa.eu/esco/model#Qualification -->

    <owl:Class rdf:about="http://data.europa.eu/esco/model#Qualification">
        <rdfs:subClassOf rdf:resource="http://www.w3.org/2004/02/skos/core#Concept"/>
        <rdfs:subClassOf rdf:resource="http://www.w3.org/2004/02/skos/core#MemberConcept"/>
        <rdfs:comment xml:lang="en">A qualification is a formal outcome of an assessment and validation process, which is obtained when a competent body determines that an individual has achieved learning outcomes to given standards.</rdfs:comment>
        <rdfs:comment xml:lang="en">List of properties on a qualification defined by the QMS application profile:
	- adms:identifier (1..n)
	- esco:referenceLanguage (0..n)
	- skos:prefLabel (1..n)
	- skos:altLabel (0..n)
	- skos:definition (0..n)
	- dcterms:description (1..n)
	- esco:hasISCED-FCode (1..n)
	- esco:hasAssociation (0..n)
	- esco:hasECTSCreditPoints (0..1)
	- esco:volumeOfLearning (0..1)
	- esco:isPartialQualification (0..1)
	- esco:waysToAcquire (0..n)
	- esco:expiryPeriod (0..n)
	- esco:hasRecognition (0..n)
	- esco:hasAwardingActivity (0..n)
	- esco:hasAccreditation (0..n)
	- foaf:homepage (0..n)
	- dcat:landingPage (0..n)
	- esco:supplementaryDoc (0..n)
	- dcterms:issued (1..1)
	- dcterms:modified (1..1)
	- skos:changeNote (0..1)
	- skos:historyNote (0..1)
	- esco:additionalNote (0..n)
	- dcterms:replaces  (0..n)
	- dcterms:isReplacedBy  (0..n)
	- iso-thes:status (0..1)
	- dcterms:creator (0..1)
	- dcterms:rightsHolder (0..1)
	- dcterms:publisher (1..1)</rdfs:comment>
        <rdfs:isDefinedBy rdf:resource="http://data.europa.eu/esco/model"/>
        <rdfs:label xml:lang="en">Qualification</rdfs:label>
    </owl:Class>



    <!-- http://data.europa.eu/esco/model#Recognition -->

    <owl:Class rdf:about="http://data.europa.eu/esco/model#Recognition">
        <rdfs:comment xml:lang="en">The recognition class is used to specify information related to the formal recognition of a qualification and/or awarding body. It is used to model a national or regional authority that formally recognises a qualification and/or a certain awarding body</rdfs:comment>
        <rdfs:isDefinedBy rdf:resource="http://data.europa.eu/esco/model"/>
        <rdfs:label xml:lang="en">Recognition</rdfs:label>
        <rdfs:seeAlso rdf:resource="http://data.europa.eu/esco/model#hasRecognition"/>
    </owl:Class>



    <!-- http://data.europa.eu/esco/model#Relationship -->

    <owl:Class rdf:about="http://data.europa.eu/esco/model#Relationship">
        <rdfs:subClassOf>
            <owl:Restriction>
                <owl:onProperty rdf:resource="http://data.europa.eu/esco/model#isRelationshipFor"/>
                <owl:qualifiedCardinality rdf:datatype="http://www.w3.org/2001/XMLSchema#nonNegativeInteger">1</owl:qualifiedCardinality>
                <owl:onClass rdf:resource="http://data.europa.eu/esco/model#Concept"/>
            </owl:Restriction>
        </rdfs:subClassOf>
        <rdfs:subClassOf>
            <owl:Restriction>
                <owl:onProperty rdf:resource="http://data.europa.eu/esco/model#refersConcept"/>
                <owl:qualifiedCardinality rdf:datatype="http://www.w3.org/2001/XMLSchema#nonNegativeInteger">1</owl:qualifiedCardinality>
                <owl:onClass rdf:resource="http://data.europa.eu/esco/model#Concept"/>
            </owl:Restriction>
        </rdfs:subClassOf>
        <owl:deprecated rdf:datatype="http://www.w3.org/2001/XMLSchema#boolean">true</owl:deprecated>
        <vs:term_status rdf:datatype="http://www.w3.org/2001/XMLSchema#string">deprecated</vs:term_status>
        <terms:issued rdf:datatype="http://www.w3.org/2001/XMLSchema#date">2013-12-03</terms:issued>
        <terms:modified rdf:datatype="http://www.w3.org/2001/XMLSchema#date">2017-02-10</terms:modified>
        <rdfs:comment xml:lang="en">The class of directed relationships between two ESCO Pillar concepts (e.g. between an esco:Occupation and an esco:Qualification).

The relationship:
- starts from the ESCO concept identified by http://data.europa.eu/esco/model#isRelationshipFor.
- is detailed using a descriptive text (http://purl.org/dc/terms/description).  This description may contain reference to external sources (see http://data.europa.eu/esco/model#relatedLegallyRequiredQualification)
- ends in the ESCO concept identified by http://data.europa.eu/esco/model#refersConcept.
- is typed by the tagging property http://data.europa.eu/esco/model#hasRelationshipType.
A relationship may be industry sector or location specific. This can be acieved by tagging the relationship using esco:hasNACECode or esco:location respectively.</rdfs:comment>
        <rdfs:isDefinedBy rdf:resource="http://data.europa.eu/esco/model"/>
        <rdfs:label xml:lang="en">ESCO concepts Relationship</rdfs:label>
        <rdfs:seeAlso rdf:resource="http://data.europa.eu/esco/model#hasRelationshipType"/>
        <rdfs:seeAlso rdf:resource="http://data.europa.eu/esco/model#isRelationshipFor"/>
        <rdfs:seeAlso rdf:resource="http://data.europa.eu/esco/model#refersConcept"/>
        <rdfs:seeAlso rdf:resource="http://data.europa.eu/esco/model#relatedLegallyRequiredQualification"/>
    </owl:Class>



    <!-- http://data.europa.eu/esco/model#RelationshipType -->

    <owl:Class rdf:about="http://data.europa.eu/esco/model#RelationshipType">
        <owl:equivalentClass>
            <owl:Restriction>
                <owl:onProperty rdf:resource="http://www.w3.org/2004/02/skos/core#inScheme"/>
                <owl:hasValue rdf:resource="http://data.europa.eu/esco/ConceptScheme/RelationshipType"/>
            </owl:Restriction>
        </owl:equivalentClass>
        <rdfs:subClassOf rdf:resource="http://www.w3.org/2004/02/skos/core#Concept"/>
        <terms:issued rdf:datatype="http://www.w3.org/2001/XMLSchema#date">2014-04-16</terms:issued>
        <terms:modified rdf:datatype="http://www.w3.org/2001/XMLSchema#date">2014-04-16</terms:modified>
        <rdfs:comment xml:lang="en">The class of the types of ESCO relations.
The concepts having this type are managed in the small SKOS taxonomy (see http://data.europa.eu/esco/ConceptScheme/RelationshipType).</rdfs:comment>
        <rdfs:isDefinedBy rdf:resource="http://data.europa.eu/esco/model" />
        <rdfs:label xml:lang="en">ESCO relationship type</rdfs:label>
        <owl:deprecated rdf:datatype="http://www.w3.org/2001/XMLSchema#boolean">true</owl:deprecated>
        <vs:term_status>rejected</vs:term_status>
    </owl:Class>



    <!-- http://data.europa.eu/esco/model#SectorBreakDownConcept -->

    <owl:Class rdf:about="http://data.europa.eu/esco/model#SectorBreakDownConcept">
        <rdfs:subClassOf rdf:resource="http://data.europa.eu/esco/model#Concept"/>
        <terms:issued rdf:datatype="http://www.w3.org/2001/XMLSchema#date">2014-02-03</terms:issued>
        <terms:modified rdf:datatype="http://www.w3.org/2001/XMLSchema#date">2014-02-03</terms:modified>
        <rdfs:comment xml:lang="en">A sector breakdown concept can be used in the Occupation and in the Skill/Competences pillar to organize navigation.  As such, it may be related (or characterize) a group of occupations as well as a group of skills.
It is not an industry sector, but it may be tagged with NACE codes.

This notion is specifically used for organizing the ESCO thesaurus creation (cfr. ESCO v1 methdology and SREF groups).</rdfs:comment>
        <rdfs:isDefinedBy rdf:resource="http://data.europa.eu/esco/model"/>
        <rdfs:label xml:lang="en">ESCO concept used for sector breakdown.</rdfs:label>
        <owl:deprecated rdf:datatype="http://www.w3.org/2001/XMLSchema#boolean">true</owl:deprecated>
        <vs:term_status rdf:datatype="http://www.w3.org/2001/XMLSchema#string">rejected</vs:term_status>
    </owl:Class>



    <!-- http://data.europa.eu/esco/model#SimpleConcept -->

    <owl:Class rdf:about="http://data.europa.eu/esco/model#SimpleConcept">
        <rdfs:subClassOf rdf:resource="http://data.europa.eu/esco/model#Concept"/>
        <terms:issued rdf:datatype="http://www.w3.org/2001/XMLSchema#date">2014-02-03</terms:issued>
        <terms:modified rdf:datatype="http://www.w3.org/2001/XMLSchema#date">2016-06-08</terms:modified>
        <rdfs:comment xml:lang="en">The class of simple ESCO concepts.

A simple ESCO concept is not decomposed into components (for compound ESCO concepts see http://data.europa.eu/esco/model#FacetedConcept).
A simple concept may be further specialized by faceted concepts.  The facets used for this specialization are represented by the property http://data.europa.eu/esco/model#facet.</rdfs:comment>
        <rdfs:isDefinedBy rdf:resource="http://data.europa.eu/esco/model"/>
        <rdfs:label xml:lang="en">Simple ESCO concept</rdfs:label>
        <rdfs:seeAlso rdf:resource="http://data.europa.eu/esco/model#FacetedConcept"/>
        <rdfs:seeAlso rdf:resource="http://data.europa.eu/esco/model#facet"/>
        <owl:deprecated rdf:datatype="http://www.w3.org/2001/XMLSchema#boolean">true</owl:deprecated>
        <vs:term_status rdf:datatype="http://www.w3.org/2001/XMLSchema#string">rejected</vs:term_status>
    </owl:Class>



    <!-- http://data.europa.eu/esco/model#Skill -->

    <owl:Class rdf:about="http://data.europa.eu/esco/model#Skill">
        <rdfs:subClassOf rdf:resource="http://data.europa.eu/esco/model#MemberConcept"/>
        <rdfs:subClassOf>
            <owl:Restriction>
                <owl:onProperty rdf:resource="http://www.w3.org/2004/02/skos/core#inScheme"/>
                <owl:hasValue rdf:resource="http://data.europa.eu/esco/ConceptScheme/ESCO_Skills"/>
            </owl:Restriction>
        </rdfs:subClassOf>
        <terms:issued rdf:datatype="http://www.w3.org/2001/XMLSchema#date">2013-06-27</terms:issued>
        <terms:modified rdf:datatype="http://www.w3.org/2001/XMLSchema#date">2013-12-03</terms:modified>
        <rdfs:comment xml:lang="en">The class of ESCO Skill concepts.

ESCO skills are sub-typed (e.g. to differentiate between knowledge and competence).
This sub-typing is modelled using the concept scheme http://data.europa.eu/esco/ConceptScheme/SkillCompetenceType and its concept class http://data.europa.eu/esco/model#SkillCompetenceType

This organization is modelled using the concept scheme http://data.europa.eu/esco/ConceptScheme/SkillReuseLevel and its concept class http://data.europa.eu/esco/model#SkillReuseLevel
ESCO skills with a different re-use applicability across sectors can be put in a hierarchical relation (skos:broader and skos:narrower) in acordance with the rules detailed by http://data.europa.eu/esco/model#SkillReuseLevel.

Characteristics
- An ESCO skill sub-type is given by http://data.europa.eu/esco/model#skillType
- An ESCO skill re-use level is given by http://data.europa.eu/esco/model#skillReuseLevel

An ESCO Skill may be related to other ESCO concepts.
- Essential related concepts of class esco:Skills are indicated by http://data.europa.eu/esco/model#isEssentialSkillFor and http://data.europa.eu/esco/model#relatedEssentialSkill
- Optional related concepts of class esco:Skills are indicated http://data.europa.eu/esco/model#isOptionalSkillFor and http://data.europa.eu/esco/model#relatedOptionalSkill
- Occupations a skill is essential for are concepts of type esco:Occupation indicated by http://data.europa.eu/esco/model#isEssentialSkillFor
- Occupations a skill is optional for are concepts of type esco:Occupation indicated by http://data.europa.eu/esco/model#isEssentialSkillFor
The property http://data.europa.eu/esco/model#hasRelationship details the relationships (see http://data.europa.eu/esco/model#Relationship)</rdfs:comment>
        <rdfs:isDefinedBy rdf:resource="http://data.europa.eu/esco/model"/>
        <rdfs:label xml:lang="en">Skill</rdfs:label>
        <rdfs:seeAlso rdf:resource="http://data.europa.eu/esco/model#Qualification"/>
        <rdfs:seeAlso rdf:resource="http://data.europa.eu/esco/model#SkillReuseLevel"/>
        <rdfs:seeAlso rdf:resource="http://data.europa.eu/esco/model#skillType"/>
        <vs:term_status rdf:datatype="http://www.w3.org/2001/XMLSchema#string">released</vs:term_status>
        <skos:definition xml:lang="en">A skill may also be an informal recognition of a competence.
The recognition typically is obtained by experience, practice or informal tests.</skos:definition>
        <skos:historyNote xml:lang="en">2013-06-27:
A Skill that is a MemberConcept:
- Initially (i.e. ESCOv0) coming from the Swedisch PES Skills tab in file Taxonomy 3 - Taxonomy db DB 20 l-corr.xls.
- Initially (i.e. ESCOv0) linked as related concepts to leaf occupation groups as described in ISCO_SKILLS.xls.
A Skill that is a GroupConcept:
- Is created by ESCO</skos:historyNote>
    </owl:Class>



    <!-- http://data.europa.eu/esco/model#SkillCompetenceType -->

    <owl:Class rdf:about="http://data.europa.eu/esco/model#SkillCompetenceType">
        <owl:equivalentClass>
            <owl:Restriction>
                <owl:onProperty rdf:resource="http://www.w3.org/2004/02/skos/core#inScheme"/>
                <owl:hasValue rdf:resource="http://data.europa.eu/esco/ConceptScheme/SkillCompetenceType"/>
            </owl:Restriction>
        </owl:equivalentClass>
        <rdfs:subClassOf rdf:resource="http://www.w3.org/2004/02/skos/core#Concept"/>
        <terms:issued rdf:datatype="http://www.w3.org/2001/XMLSchema#date">2013-12-03</terms:issued>
        <terms:modified rdf:datatype="http://www.w3.org/2001/XMLSchema#date">2013-12-03</terms:modified>
        <rdfs:comment xml:lang="en">Sub-Typing of a Skill Concept:
- Skill/Competence
- Knowledge</rdfs:comment>
        <rdfs:isDefinedBy rdf:resource="http://data.europa.eu/esco/model"/>
        <rdfs:label xml:lang="en">Competence sub-type</rdfs:label>
        <vs:term_status>released</vs:term_status>
    </owl:Class>



    <!-- http://data.europa.eu/esco/model#SkillReuseLevel -->

    <owl:Class rdf:about="http://data.europa.eu/esco/model#SkillReuseLevel">
        <owl:equivalentClass>
            <owl:Restriction>
                <owl:onProperty rdf:resource="http://www.w3.org/2004/02/skos/core#inScheme"/>
                <owl:hasValue rdf:resource="http://data.europa.eu/esco/ConceptScheme/SkillReuseLevel"/>
            </owl:Restriction>
        </owl:equivalentClass>
        <rdfs:subClassOf rdf:resource="http://www.w3.org/2004/02/skos/core#Concept"/>
        <terms:issued rdf:datatype="http://www.w3.org/2001/XMLSchema#date">2013-06-05</terms:issued>
        <terms:modified rdf:datatype="http://www.w3.org/2001/XMLSchema#date">2016-06-08</terms:modified>
        <rdfs:comment xml:lang="en">Re-usability level of a Skill or competence.
Details are provided by the ESCOpedia article on Cross-sector skills and competences (see https://ec.europa.eu/esco/escopedia/-/escopedia/Cross-sector_skills_and_competences?resetLanguage=true&amp;newLanguage=en&quot;)

The concept hierarchy in the Skill Reuse Level concept scheme (http://data.europa.eu/esco/ConceptScheme/SkillReuseLevel) must detail the allowed skill hierarchy.
A skill with re-use level A can only be a broader of a skill with reuse level B if either of the following holds:
- reuse level A = reuse level B
- reuse level A is a broader transitive of reuse level B.
A skill can have at most one re-use level (see http://data.europa.eu/esco/model#Skill).</rdfs:comment>
        <rdfs:label xml:lang="en">Skill reuse level</rdfs:label>
        <rdfs:seeAlso rdf:resource="http://data.europa.eu/esco/model#Skill"/>
        <owl:deprecated rdf:datatype="http://www.w3.org/2001/XMLSchema#boolean">true</owl:deprecated>
        <vs:term_status>deprecated</vs:term_status>
    </owl:Class>



    <!-- http://data.europa.eu/esco/model#Structure -->

    <owl:Class rdf:about="http://data.europa.eu/esco/model#Structure">
        <terms:created rdf:datatype="http://www.w3.org/2001/XMLSchema#date">2016-06-10</terms:created>
        <terms:modified rdf:datatype="http://www.w3.org/2001/XMLSchema#date">2016-06-10</terms:modified>
        <rdfs:comment rdf:datatype="http://www.w3.org/2001/XMLSchema#string">A structure defines a tagging relationship between one or more conceptschemes and an ESCO pillar.

The structure identifies the predicate used for the relationship between an esco:MemberConcept and a skos:Concept that is part of the linked conceptscheme(s).
				</rdfs:comment>
        <rdfs:isDefinedBy rdf:resource="http://data.europa.eu/esco/model"/>
        <rdfs:label rdf:datatype="http://www.w3.org/2001/XMLSchema#string">ESCO Structure</rdfs:label>
        <vs:term_status rdf:datatype="http://www.w3.org/2001/XMLSchema#string">proposed</vs:term_status>
    </owl:Class>



    <!-- http://data.europa.eu/esco/model#WorkContext -->

    <owl:Class rdf:about="http://data.europa.eu/esco/model#WorkContext">
        <rdfs:subClassOf rdf:resource="http://www.w3.org/2004/02/skos/core#Concept"/>
        <rdfs:subClassOf>
            <owl:Restriction>
                <owl:onProperty rdf:resource="http://www.w3.org/2004/02/skos/core#inScheme"/>
                <owl:hasValue rdf:resource="http://data.europa.eu/esco/ConceptScheme/WorkContext/cs"/>
            </owl:Restriction>
        </rdfs:subClassOf>
        <terms:issued rdf:datatype="http://www.w3.org/2001/XMLSchema#date">2014-08-10</terms:issued>
        <terms:modified rdf:datatype="http://www.w3.org/2001/XMLSchema#date">2014-08-10</terms:modified>
        <rdfs:comment xml:lang="en">The class of work contexts registered by ESCO
A work context iIdentifies types of business, environmental conditions, types of product, etc.
ESCO manages and organizes work context in the concept scheme: http://data.europa.eu/esco/ConceptScheme/WorkContext/cs
				</rdfs:comment>
        <rdfs:isDefinedBy rdf:resource="http://data.europa.eu/esco/model"/>
        <rdfs:label xml:lang="en">Work context</rdfs:label>
        <vs:term_status rdf:datatype="http://www.w3.org/2001/XMLSchema#string">released</vs:term_status>
    </owl:Class>


    <!-- http://purl.org/iso25964/skos-thes#SplitNonPreferredTerm -->

    <rdf:Description rdf:about="http://purl.org/iso25964/skos-thes#SplitNonPreferredTerm">
        <rdfs:comment xml:lang="en">By ESCO: Captures the compound terms established by the ESCO taxonomists.</rdfs:comment>
        <rdfs:seeAlso rdf:resource="http://data.europa.eu/esco/model#FacetedConcept"/>
        <owl:deprecated rdf:datatype="http://www.w3.org/2001/XMLSchema#boolean">true</owl:deprecated>
    </rdf:Description>




    <!--
    ///////////////////////////////////////////////////////////////////////////////////////
    //
    // Individuals
    //
    ///////////////////////////////////////////////////////////////////////////////////////
     -->




    <!-- http://data.europa.eu/esco/ConceptScheme/ESCO_Occupations -->

    <owl:NamedIndividual rdf:about="http://data.europa.eu/esco/ConceptScheme/ESCO_Occupations"/>



    <!-- http://data.europa.eu/esco/ConceptScheme/ESCO_Qualifications -->

    <owl:NamedIndividual rdf:about="http://data.europa.eu/esco/ConceptScheme/ESCO_Qualifications"/>



    <!-- http://data.europa.eu/esco/ConceptScheme/ESCO_Skills -->

    <owl:NamedIndividual rdf:about="http://data.europa.eu/esco/ConceptScheme/ESCO_Skills"/>



    <!-- http://data.europa.eu/esco/ConceptScheme/FacetConceptGroups -->

    <owl:NamedIndividual rdf:about="http://data.europa.eu/esco/ConceptScheme/FacetConceptGroups"/>



    <!-- http://data.europa.eu/esco/ConceptScheme/LabelRole -->

    <owl:NamedIndividual rdf:about="http://data.europa.eu/esco/ConceptScheme/LabelRole"/>



    <!-- http://data.europa.eu/esco/ConceptScheme/SkillCompetenceType -->

    <owl:NamedIndividual rdf:about="http://data.europa.eu/esco/ConceptScheme/SkillCompetenceType"/>



    <!-- http://data.europa.eu/esco/ConceptScheme/SkillReuseLevel -->

    <owl:NamedIndividual rdf:about="http://data.europa.eu/esco/ConceptScheme/SkillReuseLevel">
        <owl:deprecated rdf:datatype="http://www.w3.org/2001/XMLSchema#boolean">true</owl:deprecated>
    </owl:NamedIndividual>



    <!-- http://data.europa.eu/esco/ConceptScheme/AwardingBodies/cs -->

    <owl:NamedIndividual rdf:about="http://data.europa.eu/esco/ConceptScheme/AwardingBodies/cs"/>



    <!-- http://data.europa.eu/esco/ConceptScheme/WorkContext/cs -->

    <owl:NamedIndividual rdf:about="http://data.europa.eu/esco/ConceptScheme/WorkContext/cs"/>
    <rdf:Description>
        <rdfs:comment xml:lang="en"></rdfs:comment>
    </rdf:Description>
    <rdf:Description>
        <rdfs:comment xml:lang="en"></rdfs:comment>
    </rdf:Description>
    <rdf:Description>
        <rdfs:comment xml:lang="en"></rdfs:comment>
    </rdf:Description>
    <rdf:Description>
        <rdfs:comment xml:lang="en"></rdfs:comment>
    </rdf:Description>
    <rdf:Description>
        <rdfs:comment xml:lang="en"></rdfs:comment>
    </rdf:Description>
    <rdf:Description>
        <rdfs:comment xml:lang="en">The ISO 639-1 code  of the language (2-char language code) associated with the provided literal.</rdfs:comment>
    </rdf:Description>
    <rdf:Description>
        <rdfs:comment xml:lang="en">The literal value. In case it is plain text, no datatype must be specified. In case of an XHTML fragment the datatype rdf:XMLLiteral must be specified</rdfs:comment>
    </rdf:Description>
    <rdf:Description>
        <rdfs:comment xml:lang="en"></rdfs:comment>
    </rdf:Description>
    <rdf:Description>
        <rdfs:comment xml:lang="en">This property is used to point to the information topic that an additional note is about. The different topics are encoded as skos:Concepts in &lt;http://data.europa.eu/esco/concept-scheme/qualification-topics&gt;</rdfs:comment>
    </rdf:Description>



    <!--
    ///////////////////////////////////////////////////////////////////////////////////////
    //
    // Annotations
    //
    ///////////////////////////////////////////////////////////////////////////////////////
     -->

    <rdf:Description rdf:about="http://data.europa.eu/esco/model#awardingBodyDescription">
        <terms:modified rdf:datatype="http://www.w3.org/2001/XMLSchema#date">2013-12-03</terms:modified>
        <rdfs:isDefinedBy rdf:resource="http://data.europa.eu/esco/model"/>
        <terms:issued rdf:datatype="http://www.w3.org/2001/XMLSchema#date">2013-12-03</terms:issued>
        <rdfs:comment xml:lang="en">An awarding body provided using a descriptive text.
A more precise definition of an awarding body known by ESCO can be given using http://data.europa.eu/esco/model#hasAwardingBody</rdfs:comment>
        <vs:term_status rdf:datatype="http://www.w3.org/2001/XMLSchema#string">rejected</vs:term_status>
        <rdfs:label xml:lang="en">awarding body (descriptive)</rdfs:label>
        <owl:deprecated rdf:datatype="http://www.w3.org/2001/XMLSchema#boolean">true</owl:deprecated>
    </rdf:Description>
    <rdf:Description rdf:about="http://data.europa.eu/esco/model#hasPolyHierarchy">
        <terms:modified rdf:datatype="http://www.w3.org/2001/XMLSchema#date">2016-04-01</terms:modified>
        <rdfs:comment xml:lang="en">true: Indicates wether a ESCO thesaurus/taxonomy supports poly-hierarchy. Not present or false indicate mono-hierarchy.</rdfs:comment>
        <rdfs:isDefinedBy rdf:resource="http://data.europa.eu/esco/model"/>
        <rdfs:label xml:lang="en">has poly-hierarchy</rdfs:label>
        <vs:term_status rdf:datatype="http://www.w3.org/2001/XMLSchema#string">released</vs:term_status>
        <terms:issued rdf:datatype="http://www.w3.org/2001/XMLSchema#date">2013-06-27</terms:issued>
    </rdf:Description>
    <rdf:Description rdf:about="http://data.europa.eu/esco/model#isIndirect">
        <terms:modified rdf:datatype="http://www.w3.org/2001/XMLSchema#date">2013-12-03</terms:modified>
        <vs:term_status rdf:datatype="http://www.w3.org/2001/XMLSchema#string">proposed</vs:term_status>
        <rdfs:comment xml:lang="en">True: Indicates the subject concept (like a qualification) is not directly managed by ESCO. instead the concept is loaded into ESCO when it is provided by an external (typical national) body or agent.

Could also be applied (if unambiguous) to skills and occupations.

Assertion (to &apos;true&apos;) is required in case external contribution must be affirmed.</rdfs:comment>
        <terms:issued rdf:datatype="http://www.w3.org/2001/XMLSchema#date">2013-12-03</terms:issued>
        <rdfs:label xml:lang="en">is indirectly included</rdfs:label>
    </rdf:Description>
    <rdf:Description rdf:about="http://data.europa.eu/esco/model#language">
        <rdfs:comment xml:lang="en">The language of the subject resource.</rdfs:comment>
        <rdfs:comment xml:lang="en">The ISO 639-1 code of the language (2-char language code) in which a text is available.</rdfs:comment>
        <rdfs:label xml:lang="en">language</rdfs:label>
        <vs:term_status rdf:datatype="http://www.w3.org/2001/XMLSchema#string">released</vs:term_status>
        <terms:issued rdf:datatype="http://www.w3.org/2001/XMLSchema#date">2013-06-27</terms:issued>
        <rdfs:label xml:lang="en">content language</rdfs:label>
        <skos:changeNote xml:lang="en">ESCO v0 -&gt; ESCO v1 literals having XMLLiteral parsetype are now coded as pllain literal with mark-up escaped.  Hence the standard RDF language tagging of literals can be used.
see http://data.europa.eu/esco/model#noteLiteral</skos:changeNote>
        <rdfs:isDefinedBy rdf:resource="http://data.europa.eu/esco/model"/>
        <rdfs:comment xml:lang="en">QMS usage: The range must be a rdfs:Literal typed as xsd:language.</rdfs:comment>
        <terms:modified rdf:datatype="http://www.w3.org/2001/XMLSchema#date">2013-06-27</terms:modified>
    </rdf:Description>
    <rdf:Description rdf:about="http://data.europa.eu/esco/model#noteLiteral">
        <rdfs:seeAlso rdf:resouce="http://data.europa.eu/esco/model#language" />
        <owl:deprecated rdf:datatype="http://www.w3.org/2001/XMLSchema#boolean">true</owl:deprecated>
        <terms:modified rdf:datatype="http://www.w3.org/2001/XMLSchema#date">2013-06-27</terms:modified>
        <rule rdf:datatype="http://www.w3.org/2001/XMLSchema#string">Embedded hyperlinks need to be parsed and validated on import.
Content needs to be XHTML validated on import.</rule>
        <terms:issued rdf:datatype="http://www.w3.org/2001/XMLSchema#date">2013-06-27</terms:issued>
        <rdfs:isDefinedBy rdf:resource="http://data.europa.eu/esco/model"/>
        <vs:term_status rdf:datatype="http://www.w3.org/2001/XMLSchema#string">rejected</vs:term_status>
        <rdfs:comment xml:lang="en">An xml literal taking a plain text or xhtml.body.type content type.

The property typically allows to validate the content of a SKOS note (or any of its SKOS sub-properties).
Notes are then provided as blank nodes with this property and with the ESCO language property.

The motivations for this complex approach are:
- Provides structure content (XML literal) according a format that can be validated.
- xml:lang and rdf:parseType=&quot;Literal&quot; can not be provided on the same property.</rdfs:comment>
        <rdfs:label xml:lang="en">note text</rdfs:label>
    </rdf:Description>
    <rdf:Description rdf:about="http://data.europa.eu/esco/model#relevantURL">
        <terms:modified rdf:datatype="http://www.w3.org/2001/XMLSchema#date">2013-06-27</terms:modified>
        <rdfs:isDefinedBy rdf:resource="http://data.europa.eu/esco/model"/>
        <terms:issued rdf:datatype="http://www.w3.org/2001/XMLSchema#date">2013-06-27</terms:issued>
        <rdfs:label xml:lang="en">relevant URL</rdfs:label>
        <vs:term_status rdf:datatype="http://www.w3.org/2001/XMLSchema#string">released</vs:term_status>
        <rdfs:comment xml:lang="en">A web site that is relevant for the subject (any modelled class, including an ESCO concept or term).

Such URL may be part literal content value of a description, a definition or a scope note.
A relevant URI may be language specific (hence the range is literal).</rdfs:comment>
    </rdf:Description>
    <rdf:Description rdf:about="http://purl.org/iso25964/skos-thes#ConceptGroup">
        <owl:deprecated rdf:datatype="http://www.w3.org/2001/XMLSchema#boolean">true</owl:deprecated>
    </rdf:Description>
    <rdf:Description rdf:about="http://purl.org/iso25964/skos-thes#PreferredTerm">
        <rdfs:comment xml:lang="en">By ESCO: Not directly set by ESCO applications, but inferred from the range of skos-xl:pref:Label or iso-thes:plusUse.</rdfs:comment>
        <vs:term_status>released</vs:term_status>
    </rdf:Description>
    <rdf:Description rdf:about="http://purl.org/iso25964/skos-thes#SimpleNonPreferredTerm">
        <owl:deprecated rdf:datatype="http://www.w3.org/2001/XMLSchema#boolean">true</owl:deprecated>
        <rdfs:comment xml:lang="en">By ESCO: Not directly set by ESCO applications, but inferred from the range of skos-xl:alt:Label.</rdfs:comment>
    </rdf:Description>
    <rdf:Description rdf:about="http://purl.org/iso25964/skos-thes#plusUF">
        <owl:deprecated rdf:datatype="http://www.w3.org/2001/XMLSchema#boolean">true</owl:deprecated>
    </rdf:Description>
    <rdf:Description rdf:about="http://purl.org/iso25964/skos-thes#plusUse">
        <owl:deprecated rdf:datatype="http://www.w3.org/2001/XMLSchema#boolean">true</owl:deprecated>
    </rdf:Description>
</rdf:RDF>



<!-- Generated by the OWL API (version 4.2.1.20160306-0033) https://github.com/owlcs/owlapi -->
