<?xml version="1.0"?>
<rdf:RDF xmlns="http://linkeddata.center/kees/v1#"
     xml:base="http://linkeddata.center/kees/v1"
     xmlns:void="http://rdfs.org/ns/void#"
     xmlns:owl="http://www.w3.org/2002/07/owl#"
     xmlns:xsd="http://www.w3.org/2001/XMLSchema#"
     xmlns:rdfs="http://www.w3.org/2000/01/rdf-schema#"
     xmlns:llo="http://lodlaundromat.org/ontology/"
     xmlns:sd="http://www.w3.org/ns/sparql-service-description#"
     xmlns:rdf="http://www.w3.org/1999/02/22-rdf-syntax-ns#"
     xmlns:xml="http://www.w3.org/XML/1998/namespace"
     xmlns:dcterms="http://purl.org/dc/terms/"
     xmlns:v1="http://linkeddata.center/kees/v1#"
     xmlns:prov="http://www.w3.org/ns/prov#"
     xmlns:foaf="http://xmlns.com/foaf/0.1/"
     xmlns:dc="http://purl.org/dc/elements/1.1/"
     xmlns:wv="http://vocab.org/waiver/terms/norms">
    <owl:Ontology rdf:about="http://linkeddata.center/kees/v1">
        <dc:creator xml:lang="en">Enrico Fagnoni</dc:creator>
        <dcterms:license rdf:resource="http://creativecommons.org/licenses/by/4.0/"/>
        <foaf:homepage rdf:resource="http://linkeddata.center/kees/"/>
        <dc:description xml:lang="en">KEES ontology Defines few new terms used in KEES Language Application as defined in http://linkeddata.center/kees</dc:description>
        <dc:description rdf:resource="https://raw.githubusercontent.com/linkeddatacenter/kees/master/v1/images/uml.png"/>
        <owl:versionInfo>V 1.2.3 Release 2019-01-22</owl:versionInfo>
        <rdfs:label xml:lang="en">KEES Ontology</rdfs:label>
        <dc:rights xml:lang="en">The KEES ontology is available under the Creative Commons Attribution 4.0 Unported license; see http://creativecommons.org/licenses/by/4.0/. In a nutshell, you are free to copy, distribute and transmit the work; to remix/adapt the work (e.g. to import the ontology and create specializations of its elements), as long as you attribute the work in the manner specified by the author or licensor (but not in any way that suggests that they endorse you or your use of the work). Proper Attribution: Simply include the statement &quot;This work is based on the KEES ontology, developed by Enrico Fagnoni&quot; and link back to http:/linkeddata.center/kees/v1</dc:rights>
        <dc:title xml:lang="en">The KEES Vocabulary</dc:title>
    </owl:Ontology>
    


    <!-- 
    ///////////////////////////////////////////////////////////////////////////////////////
    //
    // Annotation properties
    //
    ///////////////////////////////////////////////////////////////////////////////////////
     -->

    


    <!-- http://purl.org/dc/elements/1.1/contributor -->

    <owl:AnnotationProperty rdf:about="http://purl.org/dc/elements/1.1/contributor"/>
    


    <!-- http://purl.org/dc/elements/1.1/creator -->

    <owl:AnnotationProperty rdf:about="http://purl.org/dc/elements/1.1/creator"/>
    


    <!-- http://purl.org/dc/elements/1.1/description -->

    <owl:AnnotationProperty rdf:about="http://purl.org/dc/elements/1.1/description"/>
    


    <!-- http://purl.org/dc/elements/1.1/modifed -->

    <owl:AnnotationProperty rdf:about="http://purl.org/dc/elements/1.1/modifed"/>
    


    <!-- http://purl.org/dc/elements/1.1/rights -->

    <owl:AnnotationProperty rdf:about="http://purl.org/dc/elements/1.1/rights"/>
    


    <!-- http://purl.org/dc/elements/1.1/subject -->

    <owl:AnnotationProperty rdf:about="http://purl.org/dc/elements/1.1/subject"/>
    


    <!-- http://purl.org/dc/elements/1.1/title -->

    <owl:AnnotationProperty rdf:about="http://purl.org/dc/elements/1.1/title"/>
    


    <!-- http://purl.org/dc/terms/license -->

    <owl:AnnotationProperty rdf:about="http://purl.org/dc/terms/license"/>
    


    <!-- http://www.w3.org/2002/07/owl#deprecated -->

    <owl:AnnotationProperty rdf:about="http://www.w3.org/2002/07/owl#deprecated"/>
    


    <!-- http://xmlns.com/foaf/0.1/homepage -->

    <owl:AnnotationProperty rdf:about="http://xmlns.com/foaf/0.1/homepage"/>
    


    <!-- 
    ///////////////////////////////////////////////////////////////////////////////////////
    //
    // Datatypes
    //
    ///////////////////////////////////////////////////////////////////////////////////////
     -->

    


    <!-- http://linkeddata.center/kees/v1#sparqlQueryAskOperation -->

    <rdfs:Datatype rdf:about="http://linkeddata.center/kees/v1#sparqlQueryAskOperation">
        <rdfs:comment xml:lang="en">States the datatype of a literal string containing a sparql query ASK operation.</rdfs:comment>
        <rdfs:label xml:lang="en">SPARQL  query ask operation</rdfs:label>
    </rdfs:Datatype>
    


    <!-- http://linkeddata.center/kees/v1#sparqlQueryConstructOperation -->

    <rdfs:Datatype rdf:about="http://linkeddata.center/kees/v1#sparqlQueryConstructOperation">
        <rdfs:comment xml:lang="en">States the datatype of a literal string containing a sparql query CONSTRUCT operation.</rdfs:comment>
        <rdfs:label xml:lang="en">SPARQL query construct operation</rdfs:label>
    </rdfs:Datatype>
    


    <!-- http://linkeddata.center/kees/v1#sparqlQueryDescribeOperation -->

    <rdfs:Datatype rdf:about="http://linkeddata.center/kees/v1#sparqlQueryDescribeOperation">
        <rdfs:comment xml:lang="en">States the datatype of a literal string containing a sparql query DESCRIBE operation</rdfs:comment>
        <rdfs:label xml:lang="en">SPARQL query describe operation</rdfs:label>
    </rdfs:Datatype>
    


    <!-- http://linkeddata.center/kees/v1#sparqlQuerySelectOperation -->

    <rdfs:Datatype rdf:about="http://linkeddata.center/kees/v1#sparqlQuerySelectOperation">
        <rdfs:comment xml:lang="en">States the datatype of a literal string containing a sparql query SELECT operation.</rdfs:comment>
        <rdfs:label xml:lang="en">SPARQL query select operation</rdfs:label>
    </rdfs:Datatype>
    


    <!-- http://linkeddata.center/kees/v1#sparqlUpdateScript -->

    <rdfs:Datatype rdf:about="http://linkeddata.center/kees/v1#sparqlUpdateScript">
        <rdfs:comment xml:lang="en">States the datatype of a literal string containing a sparql update scrirpt.</rdfs:comment>
        <rdfs:label xml:lang="en">SPARQL update script</rdfs:label>
    </rdfs:Datatype>
    


    <!-- 
    ///////////////////////////////////////////////////////////////////////////////////////
    //
    // Object Properties
    //
    ///////////////////////////////////////////////////////////////////////////////////////
     -->

    


    <!-- http://linkeddata.center/kees/v1#accrualPolicy -->

    <owl:ObjectProperty rdf:about="http://linkeddata.center/kees/v1#accrualPolicy">
        <rdf:type rdf:resource="http://www.w3.org/2002/07/owl#FunctionalProperty"/>
        <rdfs:domain rdf:resource="http://linkeddata.center/kees/v1#Plan"/>
        <rdfs:range rdf:resource="http://linkeddata.center/kees/v1#AccrualPolicy"/>
        <rdfs:comment xml:lang="en">The policy governing the addition of items to a collection.</rdfs:comment>
        <rdfs:label xml:lang="en">accrualPolicy</rdfs:label>
    </owl:ObjectProperty>
    


    <!-- http://linkeddata.center/kees/v1#answerMethod -->

    <owl:ObjectProperty rdf:about="http://linkeddata.center/kees/v1#answerMethod">
        <rdfs:comment xml:lang="en">The method used to answer a question</rdfs:comment>
        <rdfs:label xml:lang="en">answerMethod</rdfs:label>
    </owl:ObjectProperty>
    


    <!-- http://linkeddata.center/kees/v1#answers -->

    <owl:ObjectProperty rdf:about="http://linkeddata.center/kees/v1#answers">
        <rdf:type rdf:resource="http://www.w3.org/2002/07/owl#FunctionalProperty"/>
        <rdfs:domain rdf:resource="http://linkeddata.center/kees/v1#KnowledgeBase"/>
        <rdfs:range rdf:resource="http://linkeddata.center/kees/v1#Question"/>
        <rdfs:comment xml:lang="en">answer a question</rdfs:comment>
        <rdfs:label xml:lang="en">answers</rdfs:label>
    </owl:ObjectProperty>
    


    <!-- http://linkeddata.center/kees/v1#asserts -->

    <owl:ObjectProperty rdf:about="http://linkeddata.center/kees/v1#asserts">
        <rdf:type rdf:resource="http://www.w3.org/2002/07/owl#FunctionalProperty"/>
        <rdfs:domain rdf:resource="http://linkeddata.center/kees/v1#Plan"/>
        <rdfs:comment xml:lang="en">a reasoning that mus eval to true.</rdfs:comment>
        <rdfs:label xml:lang="en">asserts</rdfs:label>
    </owl:ObjectProperty>
    


    <!-- http://linkeddata.center/kees/v1#builds -->

    <owl:ObjectProperty rdf:about="http://linkeddata.center/kees/v1#builds">
        <rdfs:subPropertyOf rdf:resource="http://www.w3.org/2002/07/owl#topObjectProperty"/>
        <rdf:type rdf:resource="http://www.w3.org/2002/07/owl#FunctionalProperty"/>
        <rdf:type rdf:resource="http://www.w3.org/2002/07/owl#InverseFunctionalProperty"/>
        <rdfs:domain rdf:resource="http://linkeddata.center/kees/v1#Plan"/>
        <rdfs:comment xml:lang="en">Relates to the target graph name. That contains metadata and data derived from a KEES agent activities.</rdfs:comment>
        <rdfs:label xml:lang="en">builds</rdfs:label>
    </owl:ObjectProperty>
    


    <!-- http://linkeddata.center/kees/v1#changes -->

    <owl:ObjectProperty rdf:about="http://linkeddata.center/kees/v1#changes">
        <rdf:type rdf:resource="http://www.w3.org/2002/07/owl#FunctionalProperty"/>
        <rdfs:domain rdf:resource="http://linkeddata.center/kees/v1#Plan"/>
        <rdfs:comment xml:lang="en">Specifies that the referenced URI is changed by the KEES Plan execution. 
URI MUST be a graph name. The resource referenced by keees:builds property must always referenced also by this property.</rdfs:comment>
        <rdfs:label xml:lang="en">changes</rdfs:label>
    </owl:ObjectProperty>
    


    <!-- http://linkeddata.center/kees/v1#destructor -->

    <owl:ObjectProperty rdf:about="http://linkeddata.center/kees/v1#destructor">
        <rdfs:comment xml:lang="en">Specifies a resource (normally a SPIN Update resource) that destroies all resouces created by constructor. If not specified by default, to destroy all resources  generated by constructod just drop all changed named graph referred from kees:changes property.</rdfs:comment>
        <rdfs:label xml:lang="en">destructor</rdfs:label>
    </owl:ObjectProperty>
    


    <!-- http://linkeddata.center/kees/v1#from -->

    <owl:ObjectProperty rdf:about="http://linkeddata.center/kees/v1#from">
        <rdf:type rdf:resource="http://www.w3.org/2002/07/owl#FunctionalProperty"/>
        <rdfs:domain rdf:resource="http://linkeddata.center/kees/v1#Plan"/>
        <rdfs:comment xml:lang="en">Specify the constructor of a plan. A constructor can be a  data source or any resource that a KEES agent can understand (.e.g. a SPIN Construct ou Insert resource)</rdfs:comment>
        <rdfs:comment xml:lang="en">from</rdfs:comment>
    </owl:ObjectProperty>
    


    <!-- http://linkeddata.center/kees/v1#planSequence -->

    <owl:ObjectProperty rdf:about="http://linkeddata.center/kees/v1#planSequence">
        <rdf:type rdf:resource="http://www.w3.org/2002/07/owl#FunctionalProperty"/>
        <rdfs:domain rdf:resource="http://linkeddata.center/kees/v1#KnowledgeBase"/>
        <rdfs:comment xml:lang="en">It is a shortcut to specify plan dependencies. 
For example:

ex:kb kees:workflow ( ex:plan1 ex:plan2)`
means that 
ex:plan2 kees:requires ex:plan1</rdfs:comment>
        <rdfs:label xml:lang="en">workflow</rdfs:label>
    </owl:ObjectProperty>
    


    <!-- http://linkeddata.center/kees/v1#requires -->

    <owl:ObjectProperty rdf:about="http://linkeddata.center/kees/v1#requires">
        <rdf:type rdf:resource="http://www.w3.org/2002/07/owl#FunctionalProperty"/>
        <rdfs:domain rdf:resource="http://linkeddata.center/kees/v1#Plan"/>
        <rdfs:comment xml:lang="en">The referenced object must be interpreted as the :name of a named graph (  to be created or to be update). At least one kees:required named graph imust be  newer tha the target graph.</rdfs:comment>
        <rdfs:label xml:lang="en">requires</rdfs:label>
    </owl:ObjectProperty>
    


    <!-- http://linkeddata.center/kees/v1#workflow -->

    <owl:ObjectProperty rdf:about="http://linkeddata.center/kees/v1#workflow">
        <rdf:type rdf:resource="http://www.w3.org/2002/07/owl#FunctionalProperty"/>
        <rdfs:domain rdf:resource="http://linkeddata.center/kees/v1#KnowledgeBase"/>
        <rdfs:comment xml:lang="en">relates to a RDF list of kees:Plan.  The list order determine the
plan execution.</rdfs:comment>
        <rdfs:label xml:lang="en">workflow</rdfs:label>
    </owl:ObjectProperty>
    


    <!-- http://linkeddata.center/kees/v1#accrual:accrualPeriodicity -->

    <owl:ObjectProperty rdf:about="http://linkeddata.center/kees/v1#accrual:accrualPeriodicity">
        <rdf:type rdf:resource="http://www.w3.org/2002/07/owl#FunctionalProperty"/>
        <rdfs:domain rdf:resource="http://linkeddata.center/kees/v1#Plan"/>
        <rdfs:comment xml:lang="en">The frequency with which data are added to a knowledge base.</rdfs:comment>
        <rdfs:label xml:lang="en">accrualPeriodicity</rdfs:label>
    </owl:ObjectProperty>
    


    <!-- 
    ///////////////////////////////////////////////////////////////////////////////////////
    //
    // Classes
    //
    ///////////////////////////////////////////////////////////////////////////////////////
     -->

    


    <!-- http://linkeddata.center/kees/v1#AccrualPolicy -->

    <owl:Class rdf:about="http://linkeddata.center/kees/v1#AccrualPolicy">
        <rdfs:comment xml:lang="en">A KEES agent MUST recognize kees:modify and kees:create individuals as valid object for dct:accrualPolicy property in a kees:Plan. In case of inconsistencies or if no dct:accrualPolicy property is specified, the agent MUST choose kees:create.

If the accrual policy is kees:create, the named graph and all related metadata MUST be deleted and recreated BEFORE to execute accrual policies.</rdfs:comment>
        <rdfs:label xml:lang="en">AccrualPolicy</rdfs:label>
    </owl:Class>
    


    <!-- http://linkeddata.center/kees/v1#KnowledgeBase -->

    <owl:Class rdf:about="http://linkeddata.center/kees/v1#KnowledgeBase">
        <rdfs:comment xml:lang="en">A container of linked data with a purpose, that is a related set information that can be composed to provide answer to some questions.</rdfs:comment>
        <rdfs:label xml:lang="en">KnowledgeBase</rdfs:label>
    </owl:Class>
    


    <!-- http://linkeddata.center/kees/v1#KnowledgeBaseDescription -->

    <owl:Class rdf:about="http://linkeddata.center/kees/v1#KnowledgeBaseDescription">
        <rdfs:comment xml:lang="en">A document describing a knowledge base configuration. A KEES Agent should be able to rebuild the whole knowlege graph just looking to the KEES configuration.</rdfs:comment>
        <rdfs:label xml:lang="en">KnowledgeBaseDescription</rdfs:label>
    </owl:Class>
    


    <!-- http://linkeddata.center/kees/v1#Plan -->

    <owl:Class rdf:about="http://linkeddata.center/kees/v1#Plan">
        <rdfs:subClassOf>
            <owl:Restriction>
                <owl:onProperty rdf:resource="http://linkeddata.center/kees/v1#changes"/>
                <owl:someValuesFrom rdf:resource="http://www.w3.org/2002/07/owl#Thing"/>
            </owl:Restriction>
        </rdfs:subClassOf>
        <rdfs:subClassOf>
            <owl:Restriction>
                <owl:onProperty rdf:resource="http://linkeddata.center/kees/v1#accrualPolicy"/>
                <owl:qualifiedCardinality rdf:datatype="http://www.w3.org/2001/XMLSchema#nonNegativeInteger">1</owl:qualifiedCardinality>
                <owl:onClass rdf:resource="http://linkeddata.center/kees/v1#AccrualPolicy"/>
            </owl:Restriction>
        </rdfs:subClassOf>
        <rdfs:subClassOf>
            <owl:Restriction>
                <owl:onProperty rdf:resource="http://linkeddata.center/kees/v1#builds"/>
                <owl:cardinality rdf:datatype="http://www.w3.org/2001/XMLSchema#nonNegativeInteger">1</owl:cardinality>
            </owl:Restriction>
        </rdfs:subClassOf>
        <rdfs:comment xml:lang="en">A subclass of a prov:Plan. States a named graph accual activity plan</rdfs:comment>
        <rdfs:label xml:lang="en">Plan</rdfs:label>
    </owl:Class>
    


    <!-- http://linkeddata.center/kees/v1#Question -->

    <owl:Class rdf:about="http://linkeddata.center/kees/v1#Question">
        <rdfs:comment xml:lang="en">The Question represents the reason for the the knowledge base existence. In other words, the knoledge base exists to answer to questions. Question are natural language expressions that can be expressed as parametric SPARQL queries on a populated knowledge graph. The answer to a question can be a table of data, a structured document, a boolean or a translation of these in a natural language sentences.</rdfs:comment>
        <rdfs:label xml:lang="en">Question</rdfs:label>
    </owl:Class>
    


    <!-- 
    ///////////////////////////////////////////////////////////////////////////////////////
    //
    // Individuals
    //
    ///////////////////////////////////////////////////////////////////////////////////////
     -->

    


    <!-- http://linkeddata.center/kees/v1#append -->

    <owl:NamedIndividual rdf:about="http://linkeddata.center/kees/v1#append">
        <rdf:type rdf:resource="http://linkeddata.center/kees/v1#AccrualPolicy"/>
        <rdfs:comment xml:lang="en">An accrual policy where the data ar appended to existing named graphs</rdfs:comment>
        <rdfs:label xml:lang="en">update</rdfs:label>
    </owl:NamedIndividual>
    


    <!-- http://linkeddata.center/kees/v1#guard -->

    <owl:NamedIndividual rdf:about="http://linkeddata.center/kees/v1#guard">
        <rdfs:comment xml:lang="en">A SPARQL service description feature that states that the RDF store supports KEES guard specifications</rdfs:comment>
        <rdfs:label xml:lang="en">guard</rdfs:label>
    </owl:NamedIndividual>
    


    <!-- http://linkeddata.center/kees/v1#replace -->

    <owl:NamedIndividual rdf:about="http://linkeddata.center/kees/v1#replace">
        <rdf:type rdf:resource="http://linkeddata.center/kees/v1#AccrualPolicy"/>
        <rdfs:comment xml:lang="en">An accrual policy where the named graph is re-created on data change</rdfs:comment>
        <rdfs:isDefinedBy rdf:resource="http://linkeddata.center/kees/:"/>
        <rdfs:label xml:lang="en">create</rdfs:label>
    </owl:NamedIndividual>
    


    <!-- http://linkeddata.center/kees/v1#sharableKnowledge -->

    <owl:NamedIndividual rdf:about="http://linkeddata.center/kees/v1#sharableKnowledge">
        <rdf:type rdf:resource="http://linkeddata.center/kees/v1#KnowledgeBase"/>
        <rdfs:comment xml:lang="en">The default name for all  shared knowledge bases</rdfs:comment>
        <rdfs:label xml:lang="en">sharableKnowledge</rdfs:label>
    </owl:NamedIndividual>
    


    <!-- http://linkeddata.center/kees/v1#trustGraphMetric -->

    <owl:NamedIndividual rdf:about="http://linkeddata.center/kees/v1#trustGraphMetric">
        <rdfs:comment xml:lang="en">defines a metric that evaluate a trust value for a graph with a specific name. All can be used in graph quality observations.</rdfs:comment>
        <rdfs:label xml:lang="en">trustGraphMetric</rdfs:label>
    </owl:NamedIndividual>
    


    <!-- 
    ///////////////////////////////////////////////////////////////////////////////////////
    //
    // Annotations
    //
    ///////////////////////////////////////////////////////////////////////////////////////
     -->

    <rdf:Description rdf:about="http://www.w3.org/2001/XMLSchema#success">
        <rdfs:label xml:lang="en">has input</rdfs:label>
        <owl:priorVersion xml:lang="en">task  processor input as a json structure.</owl:priorVersion>
    </rdf:Description>
    


    <!-- 
    ///////////////////////////////////////////////////////////////////////////////////////
    //
    // General axioms
    //
    ///////////////////////////////////////////////////////////////////////////////////////
     -->

    <rdf:Description>
        <rdf:type rdf:resource="http://www.w3.org/2002/07/owl#AllDifferent"/>
        <owl:distinctMembers rdf:parseType="Collection">
            <rdf:Description rdf:about="http://linkeddata.center/kees/v1#append"/>
            <rdf:Description rdf:about="http://linkeddata.center/kees/v1#replace"/>
        </owl:distinctMembers>
    </rdf:Description>
</rdf:RDF>



<!-- Generated by the OWL API (version 4.2.8.20170104-2310) https://github.com/owlcs/owlapi -->

